{
    "@context": {
        "iudx": "https://iudx.org.in/voc/",
        "owl": "http://www.w3.org/2002/07/owl#",
        "rdf": "http://www.w3.org/1999/02/22-rdf-syntax-ns#",
        "rdfs": "http://www.w3.org/2000/01/rdf-schema#"
    },
    "@graph": [
        {
            "@id": "iudx:AuthServerInfoValue",
            "@type": [
                "owl:Class",
                "rdfs:Class"
            ],
            "rdfs:label": "AuthServerInfoValue",
            "rdfs:comment": "Describes information about the IUDX Authorization Server for a given resource.",
            "rdfs:isDefinedBy": {
                "@id": "iudx:"
            },
            "rdfs:subClassOf": {
                "@id": "iudx:StructuredValue"
            }
        },
        {
            "@id": "iudx:authServerURL",
            "@type": [
                "rdf:Property",
                "iudx:Relationship"
            ],
            "rdfs:comment": "URL of the IUDX authorization server used for a given resource.",
            "rdfs:label": "authServerURL",
            "iudx:domainIncludes": [
                {
                    "@id": "iudx:AuthServerInfoValue"
                }
            ],
            "iudx:rangeIncludes": [
                {
                    "@id": "xsd:string",
                    "@type": "@id"
                },
                {
                    "@id": "iudx:RelationshipValue"
                }
            ]
        },
        {
            "@id": "iudx:authType",
            "@type": [
                "rdf:Property",
                "iudx:TextProperty"
            ],
            "rdfs:comment": "Identification of the auth scheme used for a given resource.",
            "rdfs:label": "authType",
            "iudx:domainIncludes": [
                {
                    "@id": "iudx:AuthServerInfoValue"
                }
            ],
            "iudx:rangeIncludes": [
                {
                    "@id": "xsd:string"
                }
            ]
        }
    ]
}