{
    "@context": {
        "rdfs": "http://www.w3.org/2000/01/rdf-schema#",
        "rdf": "http://www.w3.org/1999/02/22-rdf-syntax-ns#",
        "owl": "http://www.w3.org/2002/07/owl#",
        "iudx": "https://iudx.org.in/voc/"
    },
    "@graph": [
        {
            "@id": "iudx:ResourceGroup",
            "@type": [
                "owl:Class",
                "rdfs:Class"
            ],
            "rdfs:comment": "Describes the Resource Group entry in the IUDX catalogue.",
            "rdfs:label": "ResourceGroup",
            "rdfs:isDefinedBy": {
                "@id": "iudx:"
            },
            "rdfs:subClassOf": {
                "@id": "iudx:IUDXEntity"
            },
            "iudx:requiredProperties": [
                "iudx:name",
                "iudx:tags",
                "iudx:resourceServer",
                "iudx:description",
                "iudx:dataModel",
                "iudx:provider",
                "iudx:authServerInfo",
                "iudx:iudxResourceAPIs",
                "iudx:resourceType"
            ]
        },
        {
            "@id": "iudx:resourceType",
            "@type": [
                "iudx:TextProperty"
            ],
            "rdfs:comment": "Type of resource. ENUM: [messageStream, message, dataset-table, dataset-file, mediaStream].",
            "rdfs:label": "resourceType",
            "iudx:domainIncludes": [
                {
                    "@id": "iudx:ResourceGroup"
                }
            ],
            "iudx:rangeIncludes": [
                {
                    "@id": "iudx:Text"
                }
            ],
            "rdfs:isDefinedBy": {
                "@id": "iudx:"
            }
        },
        {
            "@id": "iudx:geoCovers",
            "@type": [
                "iudx:GeoProperty"
            ],
            "rdfs:comment": "Represents the coverage relationship between two geometries/places.",
            "rdfs:label": "geoCovers",
            "iudx:domainIncludes": [
                {
                    "@id": "iudx:Place"
                },
                {
                    "@id": "iudx:Resource"
                },
                {
                    "@id": "iudx:ResourceGroup"
                },
                {
                    "@id": "iudx:ResourceServer"
                }
            ],
            "iudx:rangeIncludes": [
                {
                    "@id": "iudx:GeoJSONGeometry"
                },
                {
                    "@id": "iudx:Place"
                }
            ],
            "rdfs:isDefinedBy": {
                "@id": "iudx:"
            }
        },
        {
            "@id": "iudx:accessObjectInfo",
            "@type": [
                "iudx:StructuredProperty"
            ],
            "rdfs:comment": "Link to the access object. For example, an open API object.",
            "rdfs:label": "accessObjectInfo",
            "iudx:domainIncludes": [
                {
                    "@id": "iudx:ResourceGroup"
                }
            ],
            "iudx:rangeIncludes": [
                {
                    "@id": "iudx:AccessObjectInfoValue"
                }
            ]
        },
        {
            "@id": "iudx:authServerInfo",
            "@type": [
                "iudx:StructuredProperty"
            ],
            "rdfs:comment": "Information about the Authorization Server used for a given resource.",
            "rdfs:label": "authServerInfo",
            "iudx:domainIncludes": [
                {
                    "@id": "iudx:ResourceGroup"
                }
            ],
            "iudx:rangeIncludes": [
                {
                    "@id": "iudx:AuthServerInfoValue"
                }
            ]
        },
        {
            "@id": "iudx:location",
            "@type": [
                "iudx:GeoProperty"
            ],
            "rdfs:comment": "Location associated with a resource Item (a spatial point), a group of resource items (a spatial region) or even an observation in case of a mobile sensor.",
            "rdfs:label": "location",
            "iudx:domainIncludes": [
                {
                    "@id": "iudx:Resource"
                },
                {
                    "@id": "iudx:ResourceGroup"
                },
                {
                    "@id": "iudx:Provider"
                },
                {
                    "@id": "iudx:ResourceServer"
                },
                {
                    "@id": "iudx:EnvAQM"
                }
            ],
            "iudx:rangeIncludes": [
                {
                    "@id": "iudx:Place"
                },
                {
                    "@id": "iudx:Text"
                }
            ],
            "skos:exactMatch": {
                "@id": "schema:location"
            },
            "rdfs:isDefinedBy": {
                "@id": "iudx:"
            }
        },
        {
            "@id": "iudx:geoJSON",
            "@type": [
                "iudx:GeoProperty"
            ],
            "rdfs:comment": "Geo-coordinates of a place specified in GeoJSON format.",
            "rdfs:label": "geoJSON",
            "iudx:domainIncludes": [
                {
                    "@id": "iudx:Place"
                },
                {
                    "@id": "iudx:Resource"
                },
                {
                    "@id": "iudx:ResourceGroup"
                }
            ],
            "iudx:rangeIncludes": [
                {
                    "@id": "iudx:GeoJSONGeometry"
                }
            ],
            "rdfs:isDefinedBy": {
                "@id": "iudx:"
            }
        },
        {
            "iudx:domainIncludes": [
                {
                    "@id": "iudx:ResourceGroup"
                }
            ],
            "iudx:rangeIncludes": [
                {
                    "@type": "@id",
                    "@id": "xsd:string"
                },
                {
                    "@id": "iudx:RelationshipValue"
                }
            ],
            "@id": "iudx:hasDataDescriptor",
            "rdfs:comment": "URI pointing to the data-descriptor entity",
            "rdfs:label": "hasDataDescriptor",
            "@type": "iudx:Relationship"
        },
        {
            "@id": "iudx:listOfDataFields",
            "@type": [
                "iudx:TextProperty"
            ],
            "rdfs:comment": "List of properties/fields/attributes contained in the data available from the resources associated with a given resource Group. The meta-information related to the individual fields/attributes are further defined in data-model item referred to by the resource Group item.",
            "rdfs:label": "listOfDataFields",
            "iudx:domainIncludes": [
                {
                    "@id": "iudx:ResourceGroup"
                }
            ],
            "iudx:rangeIncludes": [
                {
                    "@id": "iudx:DataFieldListValue"
                }
            ]
        },
        {
            "@id": "iudx:tags",
            "@type": [
                "iudx:TextProperty"
            ],
            "rdfs:comment": "Discovery tags associated with items (resource item, resource Group item, data models) in IUDX catalogue",
            "rdfs:label": "tags",
            "iudx:domainIncludes": [
                {
                    "@id": "iudx:Resource"
                },
                {
                    "@id": "iudx:ResourceGroup"
                }
            ],
            "iudx:rangeIncludes": [
                {
                    "@id": "iudx:Text",
                    "@container": "@set"
                }
            ]
        },
        {
            "@id": "iudx:resourceAuthControlLevel",
            "@type": [
                "iudx:TextProperty"
            ],
            "rdfs:comment": "Authorizataion Control Level for resouces associated with a given resource-group. ENUM: [individual, group]. Individual authorization control level indicates that access control is available per resource, i.e., authorization can be granted/not-granted on a per resource basis for the resources. Group authorization control level indicates that the authorization is available on group level only, i.e., authorization will be granted/not-granted for all the resources associated with the given resource group.",
            "rdfs:label": "resourceAuthControlLevel",
            "iudx:domainIncludes": [
                {
                    "@id": "iudx:ResourceGroup"
                }
            ],
            "iudx:rangeIncludes": [
                {
                    "@id": "iudx:Text"
                }
            ],
            "rdfs:isDefinedBy": {
                "@id": "iudx:"
            }
        },
        {
            "@id": "iudx:dataModel",
            "@type": [
                "iudx:Relationship"
            ],
            "rdfs:comment": "IRI pointing to the data-model object for a given Resource or ResourceGroup.",
            "rdfs:label": "dataModel",
            "iudx:domainIncludes": [
                {
                    "@id": "iudx:ResourceGroup"
                },
                {
                    "@id": "iudx:Resource"
                }
            ],
            "iudx:rangeIncludes": [
                {
                    "@id": "iudx:Text",
                    "@type": "@id"
                },
                {
                    "@id": "iudx:RelationshipValue"
                }
            ]
        },
        {
            "@id": "iudx:provider",
            "@type": [
                "iudx:Relationship"
            ],
            "rdfs:comment": "URN pointing to the provider entity associated with the given catalogue item",
            "rdfs:label": "provider",
            "iudx:domainIncludes": [
                {
                    "@id": "iudx:Resource"
                },
                {
                    "@id": "iudx:ResourceGroup"
                }
            ],
            "iudx:rangeIncludes": [
                {
                    "@id": "iudx:Text",
                    "@type": "@id"
                },
                {
                    "@id": "iudx:RelationshipValue"
                }
            ]
        },
        {
            "@id": "iudx:iudxResourceAPIs",
            "@type": [
                "iudx:TextProperty"
            ],
            "rdfs:comment": "The set of IUDX resource APIs supported by a given resource. Array of multiple strings with values from the set: [TEMPORAL, SPATIAL, ATTR, TEXT]",
            "rdfs:label": "iudxResourceAPIs",
            "iudx:domainIncludes": [
                {
                    "@id": "iudx:ResourceGroup"
                }
            ],
            "iudx:rangeIncludes": [
                {
                    "@id": "iudx:Text",
                    "@container": "@set"
                }
            ],
            "rdfs:isDefinedBy": {
                "@id": "iudx:"
            }
        },
        {
            "@id": "iudx:name",
            "@type": [
                "iudx:TextProperty"
            ],
            "rdfs:comment": "Name of the entity.",
            "rdfs:label": "name",
            "iudx:domainIncludes": [
                {
                    "@id": "iudx:Place"
                },
                {
                    "@id": "iudx:Organization"
                },
                {
                    "@id": "iudx:ResourceServer"
                },
                {
                    "@id": "iudx:ResourceGroup"
                },
                {
                    "@id": "iudx:Provider"
                },
                {
                    "@id": "iudx:FunctionDescription"
                }
            ],
            "iudx:rangeIncludes": [
                {
                    "@id": "iudx:Text"
                }
            ],
            "skos:exactMatch": {
                "@id": "schema:name"
            },
            "rdfs:isDefinedBy": {
                "@id": "iudx:"
            }
        },
        {
            "@id": "iudx:resourceServer",
            "@type": [
                "iudx:Relationship"
            ],
            "rdfs:comment": "IRI pointing to the ResourceServer entity for a given Resource or ResourceGroup.",
            "rdfs:label": "resourceServer",
            "iudx:domainIncludes": [
                {
                    "@id": "iudx:Resource"
                },
                {
                    "@id": "iudx:ResourceGroup"
                }
            ],
            "iudx:rangeIncludes": [
                {
                    "@id": "iudx:Text",
                    "@type": "@id"
                },
                {
                    "@id": "iudx:RelationshipValue"
                }
            ]
        }
    ]
}