{
    "@context": {
        "iudx": "https://iudx.org.in/voc/",
        "owl": "http://www.w3.org/2002/07/owl#",
        "rdf": "http://www.w3.org/1999/02/22-rdf-syntax-ns#",
        "rdfs": "http://www.w3.org/2000/01/rdf-schema#"
    },
    "@graph": [
        {
            "@id": "iudx:Property",
            "@type": "rdfs:Class",
            "owl:equivalentClass": {
                "@id": "rdf:Property"
            },
            "rdfs:comment": "Class of all generic properties of IUDX. In general, the values are strings.",
            "rdfs:label": "Property",
            "rdfs:subClassOf": {
                "@id": "rdf:Property"
            }
        },
        {
            "@id": "iudx:rangeIncludes",
            "@type": "rdf:Property",
            "rdfs:comment": "Relates a property to a class that constitutes (one of) the expected type(s) for values of the property.",
            "rdfs:label": "rangeIncludes",
            "iudx:domainIncludes": {
                "@id": "iudx:Property"
            },
            "schema:isPartOf": {
                "@id": "http://iudx.org.in/voc/meta"
            },
            "schema:rangeIncludes": {
                "@id": "iudx:Class"
            }
        },
        {
            "@id": "iudx:domainIncludes",
            "@type": "rdf:Property",
            "rdfs:comment": "Relates a property to a class that is (one of) the type(s) the property is expected to be used on.",
            "rdfs:label": "domainIncludes",
            "iudx:domainIncludes": {
                "@id": "iudx:Property"
            },
            "iudx:isPartOf": {
                "@id": "https://iudx.org.in/voc/meta"
            },
            "iudx:rangeIncludes": {
                "@id": "iudx:Class"
            }
        }
    ]
}