{
    "@graph": [
        {
            "@id": "iudx:EnvAQM",
            "@type": [
                "owl:Class",
                "rdfs:Class"
            ],
            "rdfs:comment": "Air Quality Monitoring (AQM) Data Model.",
            "rdfs:label": "EnvAQM",
            "rdfs:isDefinedBy": {
                "@id": "iudx:"
            },
            "rdfs:subClassOf": {
                "@id": "iudx:Environment"
            }
        },
        {
            "@id": "iudx:DataModel",
            "@type": [
                "owl:Class",
                "rdfs:Class"
            ],
            "rdfs:comment": "Class of all Data Models.",
            "rdfs:label": "DataModel",
            "rdfs:isDefinedBy": {
                "@id": "iudx:"
            },
            "rdfs:subClassOf": {
                "@id": "iudx:Thing"
            }
        },
        {
            "@id": "iudx:Environment",
            "@type": [
                "owl:Class",
                "rdfs:Class"
            ],
            "rdfs:comment": "Data models that pertain to the environment domain",
            "rdfs:label": "Environment",
            "rdfs:isDefinedBy": {
                "@id": "iudx:"
            },
            "rdfs:subClassOf": {
                "@id": "iudx:DataModel"
            }
        },
        {
            "@id": "iudx:Thing",
            "@type": [
                "owl:Class",
                "rdfs:Class"
            ],
            "rdfs:comment": "Most generic IUDX object.",
            "rdfs:label": "Thing",
            "rdfs:isDefinedBy": {
                "@id": "iudx:"
            },
            "skos:exactMatch": {
                "@id": "schema:Thing"
            }
        },
        {
            "@id": "iudx:airQualityIndex",
            "@type": [
                "iudx:QuantitativeProperty"
            ],
            "rdfs:comment": "Overall Air Quality Index (AQI) for the observed air quality.",
            "rdfs:label": "airQualityIndex",
            "iudx:domainIncludes": [
                {
                    "@id": "iudx:EnvWeather"
                },
                {
                    "@id": "iudx:EnvAQM"
                },
                {
                    "@id": "iudx:AirQuality"
                }
            ],
            "iudx:rangeIncludes": [
                {
                    "@id": "iudx:Number"
                },
                {
                    "@id": "iudx:ValueDescriptor"
                }
            ],
            "rdfs:isDefinedBy": {
                "@id": "iudx:"
            }
        },
        {
            "@id": "iudx:airQualityLevel",
            "@type": [
                "iudx:TextProperty"
            ],
            "rdfs:comment": "Air Quality Category Indication. Qualitative level defined according to the local health agencies. For example, 'GOOD', 'MODERATE', 'POOR', 'UNHEALTHY', 'SEVERE', 'HAZARDOUS' etc.",
            "rdfs:label": "airQualityLevel",
            "iudx:domainIncludes": [
                {
                    "@id": "iudx:EnvAQM"
                },
                {
                    "@id": "iudx:AirQuality"
                }
            ],
            "iudx:rangeIncludes": [
                {
                    "@id": "iudx:Text"
                },
                {
                    "@id": "iudx:ValueDescriptor"
                }
            ],
            "rdfs:isDefinedBy": {
                "@id": "iudx:"
            },
            "skos:exactMatch": {
                "@id": "Fiware:airQualityLevel"
            }
        },
        {
            "@id": "iudx:airTemperature",
            "@type": [
                "iudx:QuantitativeProperty"
            ],
            "rdfs:comment": "Observed value of air temperature. Value is an object containing attributes representing statistical aggregates derived from past data.",
            "rdfs:label": "airTemperature",
            "iudx:domainIncludes": [
                {
                    "@id": "iudx:EnvWeather"
                },
                {
                    "@id": "iudx:EnvAQM"
                },
                {
                    "@id": "iudx:MosquitoDensity"
                },
                {
                    "@id": "iudx:SolarEnergy"
                },
                {
                    "@id": "iudx:AirConditioner"
                },
                {
                    "@id": "iudx:RoomOccupancy"
                },
                {
                    "@id": "iudx:AirQuality"
                }
            ],
            "iudx:rangeIncludes": [
                {
                    "@id": "iudx:TimeSeriesAggregation"
                }
            ],
            "rdfs:isDefinedBy": {
                "@id": "iudx:"
            },
            "skos:exactMatch": {
                "@id": "Fiware:temperature"
            }
        },
        {
            "@id": "iudx:ambientNoise",
            "@type": [
                "iudx:QuantitativeProperty"
            ],
            "rdfs:comment": "Observed value of ambient noise levels. Value is an object containing attributes representing statistical aggregates derived from past data.",
            "rdfs:label": "ambientNoise",
            "iudx:domainIncludes": [
                {
                    "@id": "iudx:EnvAQM"
                },
                {
                    "@id": "iudx:AirQuality"
                }
            ],
            "iudx:rangeIncludes": [
                {
                    "@id": "iudx:TimeSeriesAggregation"
                }
            ],
            "rdfs:isDefinedBy": {
                "@id": "iudx:"
            }
        },
        {
            "@id": "iudx:aqiMajorPollutant",
            "@type": [
                "iudx:TextProperty"
            ],
            "rdfs:comment": "Major pollutant in the Air Quality Index (AQI).",
            "rdfs:label": "aqiMajorPollutant",
            "iudx:domainIncludes": [
                {
                    "@id": "iudx:EnvWeather"
                },
                {
                    "@id": "iudx:EnvAQM"
                },
                {
                    "@id": "iudx:AirQuality"
                }
            ],
            "iudx:rangeIncludes": [
                {
                    "@id": "iudx:Text"
                },
                {
                    "@id": "iudx:ValueDescriptor"
                }
            ],
            "rdfs:isDefinedBy": {
                "@id": "iudx:"
            }
        },
        {
            "@id": "iudx:arsenic",
            "@type": [
                "iudx:QuantitativeProperty"
            ],
            "rdfs:comment": "Observed value of environmental pollutant Arsenic (As). Value is an object containing attributes representing statistical aggregates derived from past data.",
            "rdfs:label": "arsenic",
            "iudx:domainIncludes": [
                {
                    "@id": "iudx:EnvAQM"
                },
                {
                    "@id": "iudx:AirQuality"
                }
            ],
            "iudx:rangeIncludes": [
                {
                    "@id": "iudx:TimeSeriesAggregation"
                }
            ],
            "rdfs:isDefinedBy": {
                "@id": "iudx:"
            }
        },
        {
            "@id": "iudx:atmosphericPressure",
            "@type": [
                "iudx:QuantitativeProperty"
            ],
            "rdfs:comment": "Observed air (atmospheric or barometric) pressure.",
            "rdfs:label": "atmosphericPressure",
            "iudx:domainIncludes": [
                {
                    "@id": "iudx:EnvWeather"
                },
                {
                    "@id": "iudx:EnvAQM"
                },
                {
                    "@id": "iudx:AirQuality"
                }
            ],
            "iudx:rangeIncludes": [
                {
                    "@id": "iudx:Number"
                },
                {
                    "@id": "iudx:ValueDescriptor"
                }
            ],
            "rdfs:isDefinedBy": {
                "@id": "iudx:"
            },
            "skos:exactMatch": {
                "@id": "Fiware:atmosphericPressure"
            }
        },
        {
            "@id": "iudx:bap",
            "@type": [
                "iudx:QuantitativeProperty"
            ],
            "rdfs:comment": "Observed value of environmental pollutant Benzo[a]pyrene (BaP). Value is an object containing attributes representing statistical aggregates derived from past data.",
            "rdfs:label": "bap",
            "iudx:domainIncludes": [
                {
                    "@id": "iudx:EnvAQM"
                },
                {
                    "@id": "iudx:AirQuality"
                }
            ],
            "iudx:rangeIncludes": [
                {
                    "@id": "iudx:TimeSeriesAggregation"
                }
            ],
            "rdfs:isDefinedBy": {
                "@id": "iudx:"
            }
        },
        {
            "@id": "iudx:benzene",
            "@type": [
                "iudx:QuantitativeProperty"
            ],
            "rdfs:comment": "Observed value of environmental pollutant Benzene (C6H6). Value is an object containing attributes representing statistical aggregates derived from past data.",
            "rdfs:label": "benzene",
            "iudx:domainIncludes": [
                {
                    "@id": "iudx:EnvAQM"
                },
                {
                    "@id": "iudx:AirQuality"
                }
            ],
            "iudx:rangeIncludes": [
                {
                    "@id": "iudx:TimeSeriesAggregation"
                }
            ],
            "rdfs:isDefinedBy": {
                "@id": "iudx:"
            }
        },
        {
            "@id": "iudx:co",
            "@type": [
                "iudx:QuantitativeProperty"
            ],
            "rdfs:comment": "Observed value of environmental pollutant Carbon Monoxide (CO). Value is an object containing attributes representing statistical aggregates derived from past data.",
            "rdfs:label": "co",
            "iudx:domainIncludes": [
                {
                    "@id": "iudx:EnvAQM"
                },
                {
                    "@id": "iudx:AirQuality"
                }
            ],
            "iudx:rangeIncludes": [
                {
                    "@id": "iudx:TimeSeriesAggregation"
                }
            ],
            "rdfs:isDefinedBy": {
                "@id": "iudx:"
            }
        },
        {
            "@id": "iudx:co2",
            "@type": [
                "iudx:QuantitativeProperty"
            ],
            "rdfs:comment": "Observed value of environmental pollutant Carbon Dioxide (CO2). Value is an object containing attributes representing statistical aggregates derived from past data.",
            "rdfs:label": "co2",
            "iudx:domainIncludes": [
                {
                    "@id": "iudx:EnvAQM"
                },
                {
                    "@id": "iudx:AirQuality"
                }
            ],
            "iudx:rangeIncludes": [
                {
                    "@id": "iudx:TimeSeriesAggregation"
                }
            ],
            "rdfs:isDefinedBy": {
                "@id": "iudx:"
            }
        },
        {
            "@id": "iudx:dataDescriptor",
            "@type": [
                "iudx:Relationship"
            ],
            "rdfs:comment": "URI pointing to the data-descriptor entity",
            "rdfs:label": "dataDescriptor",
            "iudx:domainIncludes": [
                {
                    "@id": "iudx:ResourceGroup"
                },
                {
                    "@id": "iudx:Resource"
                }
            ],
            "iudx:rangeIncludes": [
                {
                    "@type": "@id",
                    "@id": "iudx:Text"
                },
                {
                    "@id": "iudx:RelationshipValue"
                },
                {
                    "@id": "iudx:DataModel"
                }
            ]
        },
        {
            "@id": "iudx:description",
            "@type": [
                "iudx:TextProperty"
            ],
            "rdfs:comment": "Description for an IUDX thing.",
            "rdfs:label": "description",
            "iudx:domainIncludes": [
                {
                    "@id": "iudx:Thing"
                }
            ],
            "iudx:rangeIncludes": [
                {
                    "@id": "iudx:Text"
                }
            ],
            "rdfs:isDefinedBy": {
                "@id": "iudx:"
            }
        },
        {
            "@id": "iudx:deviceInfo",
            "@type": [
                "iudx:StructuredProperty"
            ],
            "rdfs:comment": "Information about the device associated with the observations.",
            "rdfs:label": "deviceInfo",
            "iudx:domainIncludes": [
                {
                    "@id": "iudx:EnvAQM"
                },
                {
                    "@id": "iudx:EnvFlood"
                },
                {
                    "@id": "iudx:TransitManagement"
                },
                {
                    "@id": "iudx:StreetLightFeeder"
                },
                {
                    "@id": "iudx:Streetlight"
                },
                {
                    "@id": "iudx:WaterDistributionNetwork"
                },
                {
                    "@id": "iudx:PointOfInterest"
                },
                {
                    "@id": "iudx:EnergyMeter"
                },
                {
                    "@id": "iudx:MosquitoDensity"
                },
                {
                    "@id": "iudx:WmgmtVehicle"
                },
                {
                    "@id": "iudx:WmgmtBin"
                },
                {
                    "@id": "iudx:EmergencyVehicle"
                },
                {
                    "@id": "iudx:RoomOccupancy"
                },
                {
                    "@id": "iudx:Resource"
                },
                {
                    "@id": "iudx:ResourceGroup"
                },
                {
                    "@id": "iudx:AirQuality"
                }
            ],
            "iudx:rangeIncludes": [
                {
                    "@id": "iudx:Device"
                }
            ],
            "rdfs:isDefinedBy": {
                "@id": "iudx:"
            }
        },
        {
            "@id": "iudx:deviceStatus",
            "@type": [
                "iudx:TextProperty"
            ],
            "rdfs:comment": "Indicates the status of physical device or devices.",
            "rdfs:label": "deviceStatus",
            "iudx:domainIncludes": [
                {
                    "@id": "iudx:EnvAQM"
                },
                {
                    "@id": "iudx:EnvFlood"
                },
                {
                    "@id": "iudx:Streetlight"
                },
                {
                    "@id": "iudx:AirQuality"
                }
            ],
            "iudx:rangeIncludes": [
                {
                    "@id": "iudx:Text"
                },
                {
                    "@id": "iudx:ValueDescriptor"
                }
            ],
            "rdfs:isDefinedBy": {
                "@id": "iudx:"
            }
        },
        {
            "@id": "iudx:illuminance",
            "@type": [
                "iudx:QuantitativeProperty"
            ],
            "rdfs:comment": "Observed instantaneous ambient light intensity.",
            "rdfs:label": "illuminance",
            "iudx:domainIncludes": [
                {
                    "@id": "iudx:EnvWeather"
                },
                {
                    "@id": "iudx:EnvAQM"
                },
                {
                    "@id": "iudx:AirQuality"
                }
            ],
            "iudx:rangeIncludes": [
                {
                    "@id": "iudx:Number"
                },
                {
                    "@id": "iudx:ValueDescriptor"
                },
                {
                    "@id": "iudx:TimeSeriesAggregation"
                }
            ],
            "rdfs:isDefinedBy": {
                "@id": "iudx:"
            },
            "skos:exactMatch": {
                "@id": "Fiware:illuminance"
            }
        },
        {
            "@id": "iudx:location",
            "@type": [
                "iudx:GeoProperty"
            ],
            "rdfs:comment": "Location associated with a resource Item (a spatial point), a group of resource items (a spatial region) or even an observation in case of a mobile sensor.",
            "rdfs:label": "location",
            "iudx:domainIncludes": [
                {
                    "@id": "iudx:Resource"
                },
                {
                    "@id": "iudx:ResourceGroup"
                },
                {
                    "@id": "iudx:Provider"
                },
                {
                    "@id": "iudx:ResourceServer"
                },
                {
                    "@id": "iudx:Organization"
                },
                {
                    "@id": "iudx:EnvAQM"
                },
                {
                    "@id": "iudx:EnvFlood"
                },
                {
                    "@id": "iudx:StreetLightFeeder"
                },
                {
                    "@id": "iudx:WmgmtBin"
                },
                {
                    "@id": "iudx:TransitManagement"
                },
                {
                    "@id": "iudx:PointOfInterest"
                },
                {
                    "@id": "iudx:SafetiPin"
                },
                {
                    "@id": "iudx:IssueReporting"
                },
                {
                    "@id": "iudx:TrafficViolations"
                },
                {
                    "@id": "iudx:Streetlight"
                },
                {
                    "@id": "iudx:BikeDockingStation"
                },
                {
                    "@id": "iudx:WaterDistributionNetwork"
                },
                {
                    "@id": "iudx:Camera"
                },
                {
                    "@id": "iudx:WasteWaterMgmt"
                },
                {
                    "@id": "iudx:SmartParking"
                },
                {
                    "@id": "iudx:EmergencyVehicle"
                },
                {
                    "@id": "iudx:SolarEnergy"
                },
                {
                    "@id": "iudx:LaneDesc"
                },
                {
                    "@id": "iudx:EVChargingStation"
                },
                {
                    "@id": "iudx:MosquitoDensity"
                },
                {
                    "@id": "iudx:WmgmtVehicle"
                },
                {
                    "@id": "iudx:TouristDestination"
                },
                {
                    "@id": "iudx:AirQuality"
                }
            ],
            "iudx:rangeIncludes": [
                {
                    "@id": "iudx:Point"
                },
                {
                    "@id": "iudx:GeoJSONGeometry"
                },
                {
                    "@id": "iudx:Place"
                },
                {
                    "@id": "iudx:Text"
                },
                {
                    "@id": "iudx:ValueDescriptor"
                },
                {
                    "@id": "iudx:Geojsongeometry"
                }
            ],
            "rdfs:isDefinedBy": {
                "@id": "iudx:"
            },
            "skos:exactMatch": {
                "@id": "schema:location"
            }
        },
        {
            "@id": "iudx:nh3",
            "@type": [
                "iudx:QuantitativeProperty"
            ],
            "rdfs:comment": "Observed value of environmental pollutant Ammonia (NH3). Value is an object containing attributes representing statistical aggregates derived from past data.",
            "rdfs:label": "nh3",
            "iudx:domainIncludes": [
                {
                    "@id": "iudx:EnvAQM"
                },
                {
                    "@id": "iudx:AirQuality"
                }
            ],
            "iudx:rangeIncludes": [
                {
                    "@id": "iudx:TimeSeriesAggregation"
                }
            ],
            "rdfs:isDefinedBy": {
                "@id": "iudx:"
            }
        },
        {
            "@id": "iudx:nickel",
            "@type": [
                "iudx:QuantitativeProperty"
            ],
            "rdfs:comment": "Observed value of environmental pollutant Nickel (Ni). Value is an object containing attributes representing statistical aggregates derived from past data.",
            "rdfs:label": "nickel",
            "iudx:domainIncludes": [
                {
                    "@id": "iudx:EnvAQM"
                },
                {
                    "@id": "iudx:AirQuality"
                }
            ],
            "iudx:rangeIncludes": [
                {
                    "@id": "iudx:TimeSeriesAggregation"
                }
            ],
            "rdfs:isDefinedBy": {
                "@id": "iudx:"
            }
        },
        {
            "@id": "iudx:no",
            "@type": [
                "iudx:QuantitativeProperty"
            ],
            "rdfs:comment": "Observed value of environmental pollutant Nitrogen Monoxide (NO). Value is an object containing attributes representing statistical aggregates derived from past data.",
            "rdfs:label": "no",
            "iudx:domainIncludes": [
                {
                    "@id": "iudx:EnvAQM"
                },
                {
                    "@id": "iudx:AirQuality"
                }
            ],
            "iudx:rangeIncludes": [
                {
                    "@id": "iudx:TimeSeriesAggregation"
                }
            ],
            "rdfs:isDefinedBy": {
                "@id": "iudx:"
            }
        },
        {
            "@id": "iudx:no2",
            "@type": [
                "iudx:QuantitativeProperty"
            ],
            "rdfs:comment": "Observed value of environmental pollutant Nitrogen Dioxide (NO2). Value is an object containing attributes representing statistical aggregates derived from past data.",
            "rdfs:label": "no2",
            "iudx:domainIncludes": [
                {
                    "@id": "iudx:EnvAQM"
                },
                {
                    "@id": "iudx:AirQuality"
                }
            ],
            "iudx:rangeIncludes": [
                {
                    "@id": "iudx:TimeSeriesAggregation"
                }
            ],
            "rdfs:isDefinedBy": {
                "@id": "iudx:"
            }
        },
        {
            "@id": "iudx:o2",
            "@type": [
                "iudx:QuantitativeProperty"
            ],
            "rdfs:comment": "Observed value of Oxygen (O2). Value is an object containing attributes representing statistical aggregates derived from past data.",
            "rdfs:label": "o2",
            "iudx:domainIncludes": [
                {
                    "@id": "iudx:EnvAQM"
                },
                {
                    "@id": "iudx:AirQuality"
                }
            ],
            "iudx:rangeIncludes": [
                {
                    "@id": "iudx:TimeSeriesAggregation"
                }
            ],
            "rdfs:isDefinedBy": {
                "@id": "iudx:"
            }
        },
        {
            "@id": "iudx:o3",
            "@type": [
                "iudx:QuantitativeProperty"
            ],
            "rdfs:comment": "Observed value of environmental pollutant Ozone (O3). Value is an object containing attributes representing statistical aggregates derived from past data.",
            "rdfs:label": "o3",
            "iudx:domainIncludes": [
                {
                    "@id": "iudx:EnvAQM"
                },
                {
                    "@id": "iudx:AirQuality"
                }
            ],
            "iudx:rangeIncludes": [
                {
                    "@id": "iudx:TimeSeriesAggregation"
                }
            ],
            "rdfs:isDefinedBy": {
                "@id": "iudx:"
            }
        },
        {
            "@id": "iudx:observationDateTime",
            "@type": [
                "iudx:TimeProperty"
            ],
            "rdfs:comment": "Last reported time of observation.",
            "rdfs:label": "observationDateTime",
            "iudx:domainIncludes": [
                {
                    "@id": "iudx:EnvAQM"
                },
                {
                    "@id": "iudx:EnvFlood"
                },
                {
                    "@id": "iudx:EnvWeather"
                },
                {
                    "@id": "iudx:TransitManagement"
                },
                {
                    "@id": "iudx:StreetLightFeeder"
                },
                {
                    "@id": "iudx:WmgmtVehicle"
                },
                {
                    "@id": "iudx:SafetiPin"
                },
                {
                    "@id": "iudx:IssueReporting"
                },
                {
                    "@id": "iudx:FareCollectionSystem"
                },
                {
                    "@id": "iudx:EmployeeDetails"
                },
                {
                    "@id": "iudx:TrafficViolations"
                },
                {
                    "@id": "iudx:Streetlight"
                },
                {
                    "@id": "iudx:BikeDockingStation"
                },
                {
                    "@id": "iudx:WaterDistributionNetwork"
                },
                {
                    "@id": "iudx:WasteWaterMgmt"
                },
                {
                    "@id": "iudx:SmartParking"
                },
                {
                    "@id": "iudx:EmergencyVehicle"
                },
                {
                    "@id": "iudx:GISData"
                },
                {
                    "@id": "iudx:SolarEnergy"
                },
                {
                    "@id": "iudx:EnergyMeter"
                },
                {
                    "@id": "iudx:EVChargingStation"
                },
                {
                    "@id": "iudx:MosquitoDensity"
                },
                {
                    "@id": "iudx:RoomOccupancy"
                },
                {
                    "@id": "iudx:TouristDestination"
                },
                {
                    "@id": "iudx:RoadSegment"
                },
                {
                    "@id": "iudx:AirQuality"
                }
            ],
            "iudx:rangeIncludes": [
                {
                    "@id": "iudx:DateTime"
                },
                {
                    "@id": "iudx:ValueDescriptor"
                },
                {
                    "@id": "iudx:Datetime"
                }
            ],
            "rdfs:isDefinedBy": {
                "@id": "iudx:"
            }
        },
        {
            "@id": "iudx:pb",
            "@type": [
                "iudx:QuantitativeProperty"
            ],
            "rdfs:comment": "Observed value of environmental pollutant Lead (Pb). Value is an object containing attributes representing statistical aggregates derived from past data.",
            "rdfs:label": "pb",
            "iudx:domainIncludes": [
                {
                    "@id": "iudx:EnvAQM"
                },
                {
                    "@id": "iudx:AirQuality"
                }
            ],
            "iudx:rangeIncludes": [
                {
                    "@id": "iudx:TimeSeriesAggregation"
                }
            ],
            "rdfs:isDefinedBy": {
                "@id": "iudx:"
            }
        },
        {
            "@id": "iudx:pm10",
            "@type": [
                "iudx:QuantitativeProperty"
            ],
            "rdfs:comment": "Observed value of environmental pollutant  Particulate Matter 10 (PM10). Value is an object containing attributes representing statistical aggregates derived from past data.",
            "rdfs:label": "pm10",
            "iudx:domainIncludes": [
                {
                    "@id": "iudx:EnvAQM"
                },
                {
                    "@id": "iudx:AirQuality"
                }
            ],
            "iudx:rangeIncludes": [
                {
                    "@id": "iudx:TimeSeriesAggregation"
                }
            ],
            "rdfs:isDefinedBy": {
                "@id": "iudx:"
            }
        },
        {
            "@id": "iudx:pm2p5",
            "@type": [
                "iudx:QuantitativeProperty"
            ],
            "rdfs:comment": "Observed value of environmental pollutant Particulate Matter 2.5 (PM2.5). Value is an object containing attributes representing statistical aggregates derived from past data.",
            "rdfs:label": "pm2p5",
            "iudx:domainIncludes": [
                {
                    "@id": "iudx:EnvAQM"
                },
                {
                    "@id": "iudx:AirQuality"
                }
            ],
            "iudx:rangeIncludes": [
                {
                    "@id": "iudx:TimeSeriesAggregation"
                }
            ],
            "rdfs:isDefinedBy": {
                "@id": "iudx:"
            }
        },
        {
            "@id": "iudx:precipitation",
            "@type": [
                "iudx:QuantitativeProperty"
            ],
            "rdfs:comment": "Observed precipitation/rainfall level over a given duration.",
            "rdfs:label": "precipitation",
            "iudx:domainIncludes": [
                {
                    "@id": "iudx:EnvWeather"
                },
                {
                    "@id": "iudx:EnvAQM"
                },
                {
                    "@id": "iudx:MosquitoDensity"
                },
                {
                    "@id": "iudx:AirQuality"
                }
            ],
            "iudx:rangeIncludes": [
                {
                    "@id": "iudx:Number"
                },
                {
                    "@id": "iudx:ValueDescriptor"
                }
            ],
            "rdfs:isDefinedBy": {
                "@id": "iudx:"
            },
            "skos:exactMatch": {
                "@id": "Fiware:precipitation"
            }
        },
        {
            "@id": "iudx:relativeHumidity",
            "@type": [
                "iudx:QuantitativeProperty"
            ],
            "rdfs:comment": "Observed instantaneous relative humidity (water vapour in air).",
            "rdfs:label": "relativeHumidity",
            "iudx:domainIncludes": [
                {
                    "@id": "iudx:EnvWeather"
                },
                {
                    "@id": "iudx:EnvAQM"
                },
                {
                    "@id": "iudx:SolarEnergy"
                },
                {
                    "@id": "iudx:RoomOccupancy"
                },
                {
                    "@id": "iudx:AirQuality"
                }
            ],
            "iudx:rangeIncludes": [
                {
                    "@id": "iudx:TimeSeriesAggregation"
                }
            ],
            "rdfs:isDefinedBy": {
                "@id": "iudx:"
            },
            "skos:exactMatch": {
                "@id": "Fiware:relativeHumidity"
            }
        },
        {
            "@id": "iudx:so2",
            "@type": [
                "iudx:QuantitativeProperty"
            ],
            "rdfs:comment": "Observed value of environmental pollutant Sulphur Dioxide (SO2). Value is an object containing attributes representing statistical aggregates derived from past data.",
            "rdfs:label": "so2",
            "iudx:domainIncludes": [
                {
                    "@id": "iudx:EnvAQM"
                },
                {
                    "@id": "iudx:AirQuality"
                }
            ],
            "iudx:rangeIncludes": [
                {
                    "@id": "iudx:TimeSeriesAggregation"
                }
            ],
            "rdfs:isDefinedBy": {
                "@id": "iudx:"
            }
        },
        {
            "@id": "iudx:solarRadiation",
            "@type": [
                "iudx:QuantitativeProperty"
            ],
            "rdfs:comment": "The number of photons that are being emitted by the sun.",
            "rdfs:label": "solarRadiation",
            "iudx:domainIncludes": [
                {
                    "@id": "iudx:EnvWeather"
                },
                {
                    "@id": "iudx:EnvAQM"
                },
                {
                    "@id": "iudx:SolarEnergy"
                },
                {
                    "@id": "iudx:AirQuality"
                }
            ],
            "iudx:rangeIncludes": [
                {
                    "@id": "iudx:Number"
                },
                {
                    "@id": "iudx:ValueDescriptor"
                }
            ],
            "rdfs:isDefinedBy": {
                "@id": "iudx:"
            },
            "skos:exactMatch": {
                "@id": "Fiware:solarRadiation"
            }
        },
        {
            "@id": "iudx:uv",
            "@type": [
                "iudx:QuantitativeProperty"
            ],
            "rdfs:comment": "Observed levels of UV radiation. Value is an object containing attributes representing statistical aggregates derived from past data.",
            "rdfs:label": "uv",
            "iudx:domainIncludes": [
                {
                    "@id": "iudx:EnvWeather"
                },
                {
                    "@id": "iudx:EnvAQM"
                },
                {
                    "@id": "iudx:AirQuality"
                }
            ],
            "iudx:rangeIncludes": [
                {
                    "@id": "iudx:TimeSeriesAggregation"
                }
            ],
            "rdfs:isDefinedBy": {
                "@id": "iudx:"
            }
        },
        {
            "@id": "iudx:versionInfo",
            "@type": [
                "iudx:StructuredProperty"
            ],
            "rdfs:comment": "Version information corresponding to this observation.",
            "rdfs:label": "versionInfo",
            "iudx:domainIncludes": [
                {
                    "@id": "iudx:EnvAQM"
                },
                {
                    "@id": "iudx:SolarEnergy"
                },
                {
                    "@id": "iudx:EnergyMeter"
                },
                {
                    "@id": "iudx:Streetlight"
                },
                {
                    "@id": "iudx:RoomOccupancy"
                },
                {
                    "@id": "iudx:AirQuality"
                }
            ],
            "iudx:rangeIncludes": [
                {
                    "@id": "iudx:Version"
                },
                {
                    "@container": "@list",
                    "@id": "iudx:Version"
                }
            ],
            "rdfs:isDefinedBy": {
                "@id": "iudx:"
            }
        },
        {
            "@id": "iudx:vocRaw",
            "@type": [
                "iudx:QuantitativeProperty"
            ],
            "rdfs:comment": "Observed value of the natural form of volatile organic compounds in the environment corresponding to this observation.",
            "rdfs:label": "vocRaw",
            "iudx:domainIncludes": [
                {
                    "@id": "iudx:EnvAQM"
                },
                {
                    "@id": "iudx:AirQuality"
                }
            ],
            "iudx:rangeIncludes": [
                {
                    "@id": "iudx:Number"
                },
                {
                    "@id": "iudx:ValueDescriptor"
                }
            ],
            "rdfs:isDefinedBy": {
                "@id": "iudx:"
            },
            "skos:exactMatch": {
                "@id": "Fiware:volatileOrganicCompoundsTotal"
            }
        },
        {
            "@id": "iudx:vocTotal",
            "@type": [
                "iudx:QuantitativeProperty"
            ],
            "rdfs:comment": "Observed value of volatile organic compounds present in the environment corresponding to this observation. It could be industrial solvents, chemical by-products etc.",
            "rdfs:label": "vocTotal",
            "iudx:domainIncludes": [
                {
                    "@id": "iudx:EnvAQM"
                },
                {
                    "@id": "iudx:AirQuality"
                }
            ],
            "iudx:rangeIncludes": [
                {
                    "@id": "iudx:Number"
                },
                {
                    "@id": "iudx:ValueDescriptor"
                }
            ],
            "rdfs:isDefinedBy": {
                "@id": "iudx:"
            }
        },
        {
            "@id": "iudx:weatherType",
            "@type": [
                "iudx:TextProperty"
            ],
            "rdfs:comment": "Observed weather type or status. Represented by a comma separated list of weather types, e.g., cloudy, sunny etc.",
            "rdfs:label": "weatherType",
            "iudx:domainIncludes": [
                {
                    "@id": "iudx:EnvWeather"
                },
                {
                    "@id": "iudx:EnvAQM"
                },
                {
                    "@id": "iudx:AirQuality"
                }
            ],
            "iudx:rangeIncludes": [
                {
                    "@id": "iudx:Text"
                },
                {
                    "@id": "iudx:ValueDescriptor"
                }
            ],
            "rdfs:isDefinedBy": {
                "@id": "iudx:"
            },
            "skos:exactMatch": {
                "@id": "Fiware:weatherType"
            }
        }
    ],
    "@context": {
        "rdfs": "http://www.w3.org/2000/01/rdf-schema#",
        "iudx": "https://voc.iudx.org.in/",
        "rdf": "http://www.w3.org/1999/02/22-rdf-syntax-ns#",
        "owl": "http://www.w3.org/2002/07/owl#",
        "schema": "http://schema.org/",
        "skos": "http://www.w3.org/2004/02/skos/core#",
        "geojson": "https://purl.org/geojson/vocab#",
        "xsd": "http://www.w3.org/2001/XMLSchema#"
    }
}