{
    "@graph": [
        {
            "@id": "iudx:Object",
            "@type": [
                "rdfs:Class"
            ],
            "rdfs:comment": "Data type: literals containing key/value pairs, with each key/value pair being separated by a comma.",
            "rdfs:label": "Object"
        },
        {
            "@id": "iudx:vehicleTypeCount",
            "@type": [
                "iudx:StructuredProperty"
            ],
            "rdfs:comment": "Provides the count of vehicles for each vehicle type corresponding to this observation.",
            "rdfs:label": "vehicleTypeCount",
            "rdfs:isDefinedBy": {
                "@id": "iudx:"
            },
            "iudx:domainIncludes": [
                {
                    "@id": "iudx:RoadSegment"
                }
            ],
            "iudx:rangeIncludes": [
                {
                    "@id": "iudx:Object"
                },
                {
                    "@id": "iudx:ValueDescriptor"
                }
            ]
        },
        {
            "@id": "iudx:versionSpec",
            "@type": [
                "iudx:StructuredProperty"
            ],
            "rdfs:comment": "Version specifications or information corresponding to the version in this observation.",
            "rdfs:label": "versionSpec",
            "iudx:domainIncludes": [
                {
                    "@id": "iudx:Version"
                }
            ],
            "iudx:rangeIncludes": [
                {
                    "@id": "iudx:Text"
                },
                {
                    "@id": "iudx:Object"
                },
                {
                    "@id": "iudx:ValueDescriptor"
                }
            ]
        }
    ],
    "@context": {
        "iudx": "https://voc.iudx.org.in/",
        "owl": "http://www.w3.org/2002/07/owl#",
        "rdf": "http://www.w3.org/1999/02/22-rdf-syntax-ns#",
        "skos": "http://www.w3.org/2004/02/skos/core#",
        "schema": "http://schema.org/",
        "rdfs": "http://www.w3.org/2000/01/rdf-schema#",
        "xsd": "http://www.w3.org/2001/XMLSchema#",
        "geojson": "https://purl.org/geojson/vocab#"
    }
}