{
    "@graph": [
        {
            "@id": "iudx:Position",
            "@type": [
                "owl:Class",
                "rdfs:Class"
            ],
            "rdfs:comment": "A Data Model for realtime aspects of vehicle like speed, bearing etc.",
            "rdfs:label": "Position",
            "rdfs:isDefinedBy": {
                "@id": "iudx:"
            }
        },
        {
            "@id": "iudx:bearing",
            "@type": [
                "iudx:QuantitativeProperty"
            ],
            "rdfs:comment": "Gives the vehicle GPS angle measured in a clockwise direction from the True North. SameAs 'bearing' field from GTFS Realtime message-Position(https://developers.google.com/transit/gtfs-realtime/reference#message-position)",
            "rdfs:label": "bearing",
            "rdfs:isDefinedBy": {
                "@id": "iudx:"
            },
            "iudx:domainIncludes": [
                {
                    "@id": "iudx:Position"
                },
                {
                    "@id": "iudx:WmgmtVehicle"
                },
                {
                    "@id": "iudx:EmergencyVehicle"
                }
            ],
            "iudx:rangeIncludes": [
                {
                    "@id": "iudx:Number"
                },
                {
                    "@id": "iudx:ValueDescriptor"
                }
            ],
            "skos:exactMatch": {
                "@id": "GTFS: bearing"
            }
        },
        {
            "@id": "iudx:odometer",
            "@type": [
                "iudx:QuantitativeProperty"
            ],
            "rdfs:comment": "Odometer value.",
            "rdfs:label": "odometer",
            "rdfs:isDefinedBy": {
                "@id": "iudx:"
            },
            "iudx:domainIncludes": [
                {
                    "@id": "iudx:Position"
                }
            ],
            "iudx:rangeIncludes": [
                {
                    "@id": "iudx:Number"
                },
                {
                    "@id": "iudx:ValueDescriptor"
                }
            ],
            "skos:exactMatch": {
                "@id": "GTFS: odometer"
            }
        },
        {
            "@id": "iudx:positionInfo",
            "@type": [
                "iudx:StructuredProperty"
            ],
            "rdfs:comment": "Describes the current position of the vehicle corresponding to this observation. SameAs:'position' field from GTFS Realtime message-VehiclePosition(https://developers.google.com/transit/gtfs-realtime/reference#message-vehicleposition)",
            "rdfs:label": "positionInfo",
            "rdfs:isDefinedBy": {
                "@id": "iudx:"
            },
            "iudx:domainIncludes": [
                {
                    "@id": "iudx:TransitManagement"
                }
            ],
            "iudx:rangeIncludes": [
                {
                    "@id": "iudx:Position"
                }
            ]
        },
        {
            "@id": "iudx:speed",
            "@type": [
                "iudx:QuantitativeProperty"
            ],
            "rdfs:comment": "Momentary speed measured by the vehicle.",
            "rdfs:label": "speed",
            "rdfs:isDefinedBy": {
                "@id": "iudx:"
            },
            "iudx:domainIncludes": [
                {
                    "@id": "iudx:Position"
                },
                {
                    "@id": "iudx:WmgmtVehicle"
                },
                {
                    "@id": "iudx:EmergencyVehicle"
                }
            ],
            "iudx:rangeIncludes": [
                {
                    "@id": "iudx:Number"
                },
                {
                    "@id": "iudx:ValueDescriptor"
                }
            ],
            "skos:exactMatch": {
                "@id": "GTFS: speed"
            }
        }
    ],
    "@context": {
        "rdfs": "http://www.w3.org/2000/01/rdf-schema#",
        "iudx": "https://voc.iudx.org.in/",
        "rdf": "http://www.w3.org/1999/02/22-rdf-syntax-ns#",
        "owl": "http://www.w3.org/2002/07/owl#",
        "schema": "http://schema.org/",
        "geojson": "https://purl.org/geojson/vocab#",
        "skos": "http://www.w3.org/2004/02/skos/core#",
        "xsd": "http://www.w3.org/2001/XMLSchema#"
    }
}