{
    "@graph": [
        {
            "@id": "iudx:ShapesDesc",
            "@type": [
                "owl:Class",
                "rdfs:Class"
            ],
            "rdfs:comment": "A Data Model describing the path that a vehicle travels along a route alignment.",
            "rdfs:label": "ShapesDesc",
            "rdfs:isDefinedBy": {
                "@id": "iudx:"
            }
        },
        {
            "@id": "iudx:shapeInfo",
            "@type": [
                "iudx:StructuredProperty"
            ],
            "rdfs:comment": "Information about the path the vehicle corresponding to this observation travels along.",
            "rdfs:label": "shapeInfo",
            "rdfs:isDefinedBy": {
                "@id": "iudx:"
            },
            "iudx:domainIncludes": [
                {
                    "@id": "iudx:TransitManagement"
                }
            ],
            "iudx:rangeIncludes": [
                {
                    "@id": "iudx:ShapesDesc"
                }
            ]
        },
        {
            "@id": "iudx:shape_dist_traveled",
            "@type": [
                "iudx:QuantitativeProperty"
            ],
            "rdfs:comment": "Actual distance traveled along the shape from the first shape point to the point specified in this record. Used by trip planners to show the correct portion of the shape on a map. Values must increase along with shape_pt_sequence; they cannot be used to show reverse travel along a route. Distance units must be consistent with those used in stop_times.txt.\n\nExample: If a bus travels along the three points defined above for A_shp, the additional shape_dist_traveled values (shown here in kilometers) would look like this:\nshape_id,shape_pt_lat,shape_pt_lon,shape_pt_sequence,shape_dist_traveled\nA_shp,37.61956,-122.48161,0,0\nA_shp,37.64430,-122.41070,6,6.8310\nA_shp,37.65863,-122.30839,11,15.8765",
            "rdfs:label": "shape_dist_traveled",
            "rdfs:isDefinedBy": {
                "@id": "iudx:"
            },
            "iudx:domainIncludes": [
                {
                    "@id": "iudx:ShapesDesc"
                }
            ],
            "iudx:rangeIncludes": [
                {
                    "@id": "iudx:Number"
                },
                {
                    "@id": "iudx:ValueDescriptor"
                }
            ],
            "skos:exactMatch": {
                "@id": "GTFS: shape_dist_traveled"
            }
        },
        {
            "@id": "iudx:shape_id",
            "@type": [
                "iudx:TextProperty"
            ],
            "rdfs:comment": "Identifies a shape.",
            "rdfs:label": "shape_id",
            "rdfs:isDefinedBy": {
                "@id": "iudx:"
            },
            "iudx:domainIncludes": [
                {
                    "@id": "iudx:ShapesDesc"
                }
            ],
            "iudx:rangeIncludes": [
                {
                    "@id": "iudx:Text"
                },
                {
                    "@id": "iudx:ValueDescriptor"
                }
            ],
            "skos:exactMatch": {
                "@id": "GTFS: shape_id"
            }
        },
        {
            "@id": "iudx:shape_pt_sequence",
            "@type": [
                "iudx:QuantitativeProperty"
            ],
            "rdfs:comment": "Sequence in which the shape points connect to form the shape. Values must increase along the trip but do not need to be consecutive.\n\nExample: If the shape \"A_shp\" has three points in its definition, the shapes.txt file might contain these records to define the shape:\nshape_id,shape_pt_lat,shape_pt_lon,shape_pt_sequence\nA_shp,37.61956,-122.48161,0\nA_shp,37.64430,-122.41070,6\nA_shp,37.65863,-122.30839,11",
            "rdfs:label": "shape_pt_sequence",
            "rdfs:isDefinedBy": {
                "@id": "iudx:"
            },
            "iudx:domainIncludes": [
                {
                    "@id": "iudx:ShapesDesc"
                }
            ],
            "iudx:rangeIncludes": [
                {
                    "@id": "iudx:Number"
                },
                {
                    "@id": "iudx:ValueDescriptor"
                }
            ],
            "skos:exactMatch": {
                "@id": "GTFS: shape_pt_sequence"
            }
        }
    ],
    "@context": {
        "rdfs": "http://www.w3.org/2000/01/rdf-schema#",
        "iudx": "https://voc.iudx.org.in/",
        "rdf": "http://www.w3.org/1999/02/22-rdf-syntax-ns#",
        "owl": "http://www.w3.org/2002/07/owl#",
        "schema": "http://schema.org/",
        "geojson": "https://purl.org/geojson/vocab#",
        "skos": "http://www.w3.org/2004/02/skos/core#",
        "xsd": "http://www.w3.org/2001/XMLSchema#"
    }
}