{
    "@graph": [
        {
            "@id": "iudx:StopTimeUpdate",
            "@type": [
                "owl:Class",
                "rdfs:Class"
            ],
            "rdfs:comment": "A Data Model for realtime update of events for a given stop on a trip.",
            "rdfs:label": "StopTimeUpdate",
            "rdfs:isDefinedBy": {
                "@id": "iudx:"
            }
        },
        {
            "@id": "iudx:stopScheduleRelationship",
            "@type": [
                "iudx:TextProperty"
            ],
            "rdfs:comment": "Describes the relationship between the static schedule and the stop. SameAs: 'schedule_relationship' field from GTFS Realtime message-StopTimeUpdate ENUM[SCHEDULED, SKIPPED, NO_DATA] (https://developers.google.com/transit/gtfs-realtime/reference#message-stoptimeupdate)",
            "rdfs:label": "stopScheduleRelationship",
            "rdfs:isDefinedBy": {
                "@id": "iudx:"
            },
            "iudx:domainIncludes": [
                {
                    "@id": "iudx:StopTimeUpdate"
                }
            ],
            "iudx:rangeIncludes": [
                {
                    "@id": "iudx:Text"
                },
                {
                    "@id": "iudx:ValueDescriptor"
                }
            ],
            "skos:exactMatch": {
                "@id": "GTFS: schedule_relationship"
            }
        },
        {
            "@id": "iudx:stopTimeUpdateInfo",
            "@type": [
                "iudx:StructuredProperty"
            ],
            "rdfs:comment": "Updated sorted stop sequence for the trip made by the vehicle corresponding to this observation, not to be considered if schedule_realtionship is \"CANCELED\". SameAs: 'stop_time_update' field from GTFS Realtime message-TripUpdate (https://developers.google.com/transit/gtfs-realtime/reference#message-tripupdate)",
            "rdfs:label": "stopTimeUpdateInfo",
            "rdfs:isDefinedBy": {
                "@id": "iudx:"
            },
            "iudx:domainIncludes": [
                {
                    "@id": "iudx:TransitManagement"
                }
            ],
            "iudx:rangeIncludes": [
                {
                    "@id": "iudx:StopTimeUpdate"
                }
            ]
        },
        {
            "@id": "iudx:stop_id",
            "@type": [
                "iudx:TextProperty"
            ],
            "rdfs:comment": "Unique ID assigned to the stop corresponding to this observation.",
            "rdfs:label": "stop_id",
            "rdfs:isDefinedBy": {
                "@id": "iudx:"
            },
            "iudx:domainIncludes": [
                {
                    "@id": "iudx:GtfsCommons"
                },
                {
                    "@id": "iudx:VehiclePosition"
                },
                {
                    "@id": "iudx:StopTimeUpdate"
                },
                {
                    "@id": "iudx:StopsDesc"
                },
                {
                    "@id": "iudx:StopTimesDesc"
                }
            ],
            "iudx:rangeIncludes": [
                {
                    "@id": "iudx:Text"
                },
                {
                    "@id": "iudx:ValueDescriptor"
                }
            ],
            "skos:exactMatch": {
                "@id": "GTFS: stop_id"
            }
        },
        {
            "@id": "iudx:stop_sequence",
            "@type": [
                "iudx:QuantitativeProperty"
            ],
            "rdfs:comment": "This field identifies the order of the stops for a particular trip. The values for stop_sequence must be non-negative integers, and they must increase along the trip. For example, the first stop on the trip could have a stop_sequence of 1, the second stop on the trip could have a stop_sequence of 23, the third stop could have a stop_sequence of 40, and so on.",
            "rdfs:label": "stop_sequence",
            "rdfs:isDefinedBy": {
                "@id": "iudx:"
            },
            "iudx:domainIncludes": [
                {
                    "@id": "iudx:GtfsCommons"
                },
                {
                    "@id": "iudx:StopTimeUpdate"
                },
                {
                    "@id": "iudx:StopTimesDesc"
                }
            ],
            "iudx:rangeIncludes": [
                {
                    "@id": "iudx:Number"
                },
                {
                    "@id": "iudx:ValueDescriptor"
                }
            ],
            "skos:exactMatch": {
                "@id": "GTFS: stop_sequence"
            }
        }
    ],
    "@context": {
        "rdfs": "http://www.w3.org/2000/01/rdf-schema#",
        "iudx": "https://voc.iudx.org.in/",
        "rdf": "http://www.w3.org/1999/02/22-rdf-syntax-ns#",
        "owl": "http://www.w3.org/2002/07/owl#",
        "schema": "http://schema.org/",
        "geojson": "https://purl.org/geojson/vocab#",
        "skos": "http://www.w3.org/2004/02/skos/core#",
        "xsd": "http://www.w3.org/2001/XMLSchema#"
    }
}