{
    "@graph": [
        {
            "@id": "iudx:Text",
            "@type": [
                "rdfs:Class"
            ],
            "rdfs:comment": "Data type: Text for string values",
            "rdfs:label": "Text",
            "skos:exactMatch": {
                "@id": "schema:Text"
            }
        },
        {
            "@id": "iudx:acAvailable",
            "@type": [
                "iudx:TextProperty"
            ],
            "rdfs:comment": "Describes the presence of air conditioning option in the vehicle corresponding to this observation.",
            "rdfs:label": "acAvailable",
            "rdfs:isDefinedBy": {
                "@id": "iudx:"
            },
            "iudx:domainIncludes": [
                {
                    "@id": "iudx:TransitManagement"
                }
            ],
            "iudx:rangeIncludes": [
                {
                    "@id": "iudx:Text"
                },
                {
                    "@id": "iudx:ValueDescriptor"
                }
            ]
        },
        {
            "@id": "iudx:acMode",
            "@type": [
                "iudx:TextProperty"
            ],
            "rdfs:comment": "Describes the mode of operation of the air conditioning system.",
            "rdfs:label": "acMode",
            "rdfs:isDefinedBy": {
                "@id": "iudx:"
            },
            "iudx:domainIncludes": [
                {
                    "@id": "iudx:AirConditioner"
                }
            ],
            "iudx:rangeIncludes": [
                {
                    "@id": "iudx:Text"
                },
                {
                    "@id": "iudx:ValueDescriptor"
                }
            ]
        },
        {
            "@id": "iudx:accessObject",
            "@type": [
                "iudx:Relationship"
            ],
            "rdfs:comment": "Link to the access object. For example, an open API object.",
            "rdfs:label": "accessObject",
            "iudx:domainIncludes": [
                {
                    "@id": "iudx:AccessObjectInfoValue"
                }
            ],
            "iudx:rangeIncludes": [
                {
                    "@id": "iudx:Text",
                    "@type": "@id"
                },
                {
                    "@id": "iudx:RelationshipValue"
                }
            ]
        },
        {
            "@id": "iudx:accessObjectType",
            "@type": [
                "iudx:TextProperty"
            ],
            "rdfs:comment": "Type of access object. ENUM: [OpenAPI, AsyncAPI]",
            "rdfs:label": "accessObjectType",
            "iudx:domainIncludes": [
                {
                    "@id": "iudx:AccessObjectInfoValue"
                }
            ],
            "iudx:rangeIncludes": [
                {
                    "@id": "iudx:Text"
                }
            ]
        },
        {
            "@id": "iudx:accessPolicy",
            "@type": [
                "iudx:TextProperty"
            ],
            "rdfs:comment": "Defines the access policy for resources belonging to ResourceGroup or an individual Resource. In case of ResourceGroup item, it can take values: [OPEN, SECURE, MIXED]. OPEN implies all Resources in the group are open (and need no authorization token for data access). SECURE implies that all Resources are secured and will need authorization token for access. MIXED implies that some of Resource items may be open. In case of accessPolicy being set to MIXED in the resource group, the individual resource items will further qualify the access policy using this field. In case of Resource item, it will take values from: [OPEN, SECURE].",
            "rdfs:label": "accessPolicy",
            "iudx:domainIncludes": [
                {
                    "@id": "iudx:ResourceGroup"
                },
                {
                    "@id": "iudx:Resource"
                }
            ],
            "iudx:rangeIncludes": [
                {
                    "@id": "iudx:Text"
                }
            ],
            "rdfs:isDefinedBy": {
                "@id": "iudx:"
            }
        },
        {
            "@id": "iudx:accessURL",
            "@type": [
                "iudx:TextProperty"
            ],
            "rdfs:comment": "The IRI pointing to the domain from which data can be accessed.",
            "rdfs:label": "accessURL",
            "iudx:domainIncludes": [
                {
                    "@id": "iudx:HTTPAccess"
                },
                {
                    "@id": "iudx:FileAccess"
                },
                {
                    "@id": "iudx:StreamingAccess"
                }
            ],
            "iudx:rangeIncludes": [
                {
                    "@id": "iudx:Text"
                },
                {
                    "@id": "iudx:ValueDescriptor"
                }
            ],
            "rdfs:isDefinedBy": {
                "@id": "iudx:"
            }
        },
        {
            "@id": "iudx:additionalInfoURL",
            "@type": [
                "iudx:Relationship"
            ],
            "rdfs:comment": "URL from which additional information of the subject can be obtained",
            "rdfs:label": "additionalInfoURL",
            "iudx:domainIncludes": [
                {
                    "@id": "iudx:AccessObjectInfoValue"
                },
                {
                    "@id": "iudx:Organization"
                },
                {
                    "@id": "iudx:PointOfInterest"
                }
            ],
            "iudx:rangeIncludes": [
                {
                    "@id": "iudx:Text",
                    "@type": "@id"
                },
                {
                    "@id": "iudx:RelationshipValue"
                }
            ]
        },
        {
            "@id": "iudx:address",
            "@type": [
                "iudx:GeoProperty"
            ],
            "rdfs:comment": "Physical address of a place.",
            "rdfs:label": "address",
            "iudx:domainIncludes": [
                {
                    "@id": "iudx:Place"
                },
                {
                    "@id": "iudx:PointOfInterest"
                },
                {
                    "@id": "iudx:IssueReporting"
                },
                {
                    "@id": "iudx:Streetlight"
                },
                {
                    "@id": "iudx:BikeDockingStation"
                },
                {
                    "@id": "iudx:WaterDistributionNetwork"
                },
                {
                    "@id": "iudx:RevenueCollection"
                },
                {
                    "@id": "iudx:EmergencyVehicle"
                },
                {
                    "@id": "iudx:EVChargingStation"
                },
                {
                    "@id": "iudx:MosquitoDensity"
                },
                {
                    "@id": "iudx:TouristDestination"
                },
                {
                    "@id": "iudx:WmgmtVehicle"
                }
            ],
            "iudx:rangeIncludes": [
                {
                    "@id": "iudx:Text"
                },
                {
                    "@id": "iudx:ValueDescriptor"
                }
            ],
            "rdfs:isDefinedBy": {
                "@id": "iudx:"
            },
            "skos:exactMatch": {
                "@id": "schema:address"
            }
        },
        {
            "@id": "iudx:agency_email",
            "@type": [
                "iudx:TextProperty"
            ],
            "rdfs:comment": "Email address actively monitored by the agency\u2019s customer service department. SameAs: 'agency_email' field from GTFS Static Field Definition - agency.txt (https://developers.google.com/transit/gtfs/reference#agencytxt)",
            "rdfs:label": "agency_email",
            "rdfs:isDefinedBy": {
                "@id": "iudx:"
            },
            "iudx:domainIncludes": [
                {
                    "@id": "iudx:AgencyDesc"
                }
            ],
            "iudx:rangeIncludes": [
                {
                    "@id": "iudx:Text"
                },
                {
                    "@id": "iudx:ValueDescriptor"
                }
            ],
            "skos:exactMatch": {
                "@id": "GTFS: agency_email"
            }
        },
        {
            "@id": "iudx:agency_fare_url",
            "@type": [
                "iudx:TextProperty"
            ],
            "rdfs:comment": "URL of a web page that contains the details of the fares and also could allow to purchase tickets for that agency online. SameAs: 'agency_fare_url' field from GTFS Static Field Definition - agency.txt (https://developers.google.com/transit/gtfs/reference#agencytxt)",
            "rdfs:label": "agency_fare_url",
            "rdfs:isDefinedBy": {
                "@id": "iudx:"
            },
            "iudx:domainIncludes": [
                {
                    "@id": "iudx:AgencyDesc"
                }
            ],
            "iudx:rangeIncludes": [
                {
                    "@id": "iudx:Text"
                },
                {
                    "@id": "iudx:ValueDescriptor"
                }
            ],
            "skos:exactMatch": {
                "@id": "GTFS: agency_fare_url"
            }
        },
        {
            "@id": "iudx:agency_id",
            "@type": [
                "iudx:TextProperty"
            ],
            "rdfs:comment": "ID that uniquely identifies a transit agency. A transit feed may represent data from more than one agency. The agency_id is dataset unique. This field is optional for transit feeds that only contain data for a single agency. SameAs: 'agency_id' field from GTFS Static Field Definition - agency.txt (https://developers.google.com/transit/gtfs/reference#agencytxt)",
            "rdfs:label": "agency_id",
            "rdfs:isDefinedBy": {
                "@id": "iudx:"
            },
            "iudx:domainIncludes": [
                {
                    "@id": "iudx:AgencyDesc"
                }
            ],
            "iudx:rangeIncludes": [
                {
                    "@id": "iudx:Text"
                },
                {
                    "@id": "iudx:ValueDescriptor"
                }
            ],
            "skos:exactMatch": {
                "@id": "GTFS: agency_id"
            }
        },
        {
            "@id": "iudx:agency_lang",
            "@type": [
                "iudx:TextProperty"
            ],
            "rdfs:comment": "Contains a two-letter ISO 639-1 code for the primary language used by this transit agency. The language code is case-insensitive (both en and EN are accepted). SameAs: 'agency_lang' field from GTFS Static Field Definition - agency.txt (https://developers.google.com/transit/gtfs/reference#agencytxt)",
            "rdfs:label": "agency_lang",
            "rdfs:isDefinedBy": {
                "@id": "iudx:"
            },
            "iudx:domainIncludes": [
                {
                    "@id": "iudx:AgencyDesc"
                }
            ],
            "iudx:rangeIncludes": [
                {
                    "@id": "iudx:Text"
                },
                {
                    "@id": "iudx:ValueDescriptor"
                }
            ],
            "skos:exactMatch": {
                "@id": "GTFS: agency_lang"
            }
        },
        {
            "@id": "iudx:agency_name",
            "@type": [
                "iudx:TextProperty"
            ],
            "rdfs:comment": "The agency_name field contains the full name of the transit agency. SameAs: 'agency_name' field from GTFS Static Field Definition - agency.txt (https://developers.google.com/transit/gtfs/reference#agencytxt)",
            "rdfs:label": "agency_name",
            "rdfs:isDefinedBy": {
                "@id": "iudx:"
            },
            "iudx:domainIncludes": [
                {
                    "@id": "iudx:AgencyDesc"
                }
            ],
            "iudx:rangeIncludes": [
                {
                    "@id": "iudx:Text"
                },
                {
                    "@id": "iudx:ValueDescriptor"
                }
            ],
            "skos:exactMatch": {
                "@id": "GTFS: agency_name"
            }
        },
        {
            "@id": "iudx:agency_phone",
            "@type": [
                "iudx:TextProperty"
            ],
            "rdfs:comment": "A voice telephone number for the specified agency.SameAs: 'agency_phone' field from GTFS Static Field Definition - agency.txt (https://developers.google.com/transit/gtfs/reference#agencytxt)",
            "rdfs:label": "agency_phone",
            "rdfs:isDefinedBy": {
                "@id": "iudx:"
            },
            "iudx:domainIncludes": [
                {
                    "@id": "iudx:AgencyDesc"
                }
            ],
            "iudx:rangeIncludes": [
                {
                    "@id": "iudx:Text"
                },
                {
                    "@id": "iudx:ValueDescriptor"
                }
            ],
            "skos:exactMatch": {
                "@id": "GTFS: agency_phone"
            }
        },
        {
            "@id": "iudx:agency_timezone",
            "@type": [
                "iudx:TextProperty"
            ],
            "rdfs:comment": "Timezone field contains the timezone where the transit agency is located. SameAs: 'agency_timezone' field from GTFS Static Field Definition - agency.txt (https://developers.google.com/transit/gtfs/reference#agencytxt)",
            "rdfs:label": "agency_timezone",
            "rdfs:isDefinedBy": {
                "@id": "iudx:"
            },
            "iudx:domainIncludes": [
                {
                    "@id": "iudx:AgencyDesc"
                }
            ],
            "iudx:rangeIncludes": [
                {
                    "@id": "iudx:Text"
                },
                {
                    "@id": "iudx:ValueDescriptor"
                }
            ],
            "skos:exactMatch": {
                "@id": "GTFS:agency_timezone"
            }
        },
        {
            "@id": "iudx:agency_url",
            "@type": [
                "iudx:TextProperty"
            ],
            "rdfs:comment": "The agency_url field contains the URL of the transit agency. SameAs: 'agency_url' field from GTFS Static Field Definition - agency.txt (https://developers.google.com/transit/gtfs/reference#agencytxt)",
            "rdfs:label": "agency_url",
            "iudx:domainIncludes": [
                {
                    "@id": "iudx:AgencyDesc"
                },
                {
                    "@id": "iudx:TouristDestination"
                }
            ],
            "iudx:rangeIncludes": [
                {
                    "@id": "iudx:Text"
                },
                {
                    "@id": "iudx:ValueDescriptor"
                }
            ],
            "rdfs:isDefinedBy": {
                "@id": "iudx:"
            },
            "skos:exactMatch": {
                "@id": "GTFS: agency_url"
            }
        },
        {
            "@id": "iudx:airFlowRate",
            "@type": [
                "iudx:TextProperty"
            ],
            "rdfs:comment": "Describes the rate of air flow corresponding to this observation.",
            "rdfs:label": "airFlowRate",
            "rdfs:isDefinedBy": {
                "@id": "iudx:"
            },
            "iudx:domainIncludes": [
                {
                    "@id": "iudx:AirConditioner"
                }
            ],
            "iudx:rangeIncludes": [
                {
                    "@id": "iudx:Text"
                },
                {
                    "@id": "iudx:ValueDescriptor"
                }
            ]
        },
        {
            "@id": "iudx:airQualityLevel",
            "@type": [
                "iudx:TextProperty"
            ],
            "rdfs:comment": "Air Quality Category Indication. Qualitative level defined according to the local health agencies. For example, 'GOOD', 'MODERATE', 'POOR', 'UNHEALTHY', 'SEVERE', 'HAZARDOUS' etc.",
            "rdfs:label": "airQualityLevel",
            "iudx:domainIncludes": [
                {
                    "@id": "iudx:EnvAQM"
                },
                {
                    "@id": "iudx:AirQuality"
                }
            ],
            "iudx:rangeIncludes": [
                {
                    "@id": "iudx:Text"
                },
                {
                    "@id": "iudx:ValueDescriptor"
                }
            ],
            "rdfs:isDefinedBy": {
                "@id": "iudx:"
            },
            "skos:exactMatch": {
                "@id": "Fiware:airQualityLevel"
            }
        },
        {
            "@id": "iudx:allowedVehicleType",
            "@type": [
                "iudx:TextProperty"
            ],
            "rdfs:comment": "Represents the vehicle type(s) allowed to ply on the road segment corresponding to this observation.",
            "rdfs:label": "allowedVehicleType",
            "rdfs:isDefinedBy": {
                "@id": "iudx:"
            },
            "iudx:domainIncludes": [
                {
                    "@id": "iudx:RoadSegment"
                }
            ],
            "iudx:rangeIncludes": [
                {
                    "@id": "iudx:Text"
                },
                {
                    "@id": "iudx:ValueDescriptor"
                }
            ],
            "skos:exactMatch": {
                "@id": "Fiware: allowedVehicleType"
            }
        },
        {
            "@id": "iudx:altitude",
            "@type": [
                "iudx:GeoProperty"
            ],
            "rdfs:comment": "Altitude of a place. Specified in WGS 84 CRS (https://en.wikipedia.org/wiki/World_Geodetic_System)",
            "rdfs:label": "altitude",
            "iudx:domainIncludes": [
                {
                    "@id": "iudx:GeoCoordinates"
                },
                {
                    "@id": "iudx:Place"
                }
            ],
            "iudx:rangeIncludes": [
                {
                    "@id": "iudx:Number"
                },
                {
                    "@id": "iudx:Text"
                }
            ],
            "skos:exactMatch": {
                "@id": "schema:elevation"
            },
            "rdfs:isDefinedBy": {
                "@id": "iudx:"
            }
        },
        {
            "@id": "iudx:annotatedMap",
            "@type": [
                "iudx:TextProperty"
            ],
            "rdfs:comment": "Annotated map view indicating the orientations for the camera corresponding to this observation",
            "rdfs:label": "annotatedMap",
            "rdfs:isDefinedBy": {
                "@id": "iudx:"
            },
            "iudx:domainIncludes": [
                {
                    "@id": "iudx:Orientation"
                }
            ],
            "iudx:rangeIncludes": [
                {
                    "@id": "iudx:Text"
                },
                {
                    "@id": "iudx:ValueDescriptor"
                }
            ]
        },
        {
            "@id": "iudx:apdURL",
            "@type": [
                "iudx:TextProperty"
            ],
            "rdfs:comment": "URL pointing to the Access Policy Decision (APD) for an individual Resource.",
            "rdfs:label": "apdURL",
            "iudx:domainIncludes": [
                {
                    "@id": "iudx:Resource"
                }
            ],
            "iudx:rangeIncludes": [
                {
                    "@id": "iudx:Text"
                }
            ],
            "rdfs:isDefinedBy": {
                "@id": "iudx:"
            }
        },
        {
            "@id": "iudx:aqiMajorPollutant",
            "@type": [
                "iudx:TextProperty"
            ],
            "rdfs:comment": "Major pollutant in the Air Quality Index (AQI).",
            "rdfs:label": "aqiMajorPollutant",
            "iudx:domainIncludes": [
                {
                    "@id": "iudx:EnvWeather"
                },
                {
                    "@id": "iudx:EnvAQM"
                },
                {
                    "@id": "iudx:AirQuality"
                }
            ],
            "iudx:rangeIncludes": [
                {
                    "@id": "iudx:Text"
                },
                {
                    "@id": "iudx:ValueDescriptor"
                }
            ],
            "rdfs:isDefinedBy": {
                "@id": "iudx:"
            }
        },
        {
            "@id": "iudx:aqiMajorPollutantForecast",
            "@type": [
                "iudx:TextProperty"
            ],
            "rdfs:comment": "Forecasted major air pollutant in the Air Quality Index (AQI) over a certain duration in future.",
            "rdfs:label": "aqiMajorPollutantForecast",
            "rdfs:isDefinedBy": {
                "@id": "iudx:"
            },
            "iudx:domainIncludes": [
                {
                    "@id": "iudx:EnvWeather"
                }
            ],
            "iudx:rangeIncludes": [
                {
                    "@id": "iudx:Text"
                },
                {
                    "@id": "iudx:ValueDescriptor"
                }
            ]
        },
        {
            "@id": "iudx:areaServed",
            "@type": [
                "iudx:GeoProperty"
            ],
            "rdfs:comment": "Area served by the entity or a service.",
            "rdfs:label": "areaServed",
            "rdfs:isDefinedBy": {
                "@id": "iudx:"
            },
            "iudx:domainIncludes": [
                {
                    "@id": "iudx:ModelInfo"
                },
                {
                    "@id": "iudx:StreetLightFeeder"
                }
            ],
            "iudx:rangeIncludes": [
                {
                    "@id": "iudx:Text"
                }
            ]
        },
        {
            "@id": "iudx:arrival_time",
            "@type": [
                "iudx:TimeProperty"
            ],
            "rdfs:comment": "Specifies the arrival time at a specific stop for a specific trip on a route. Times must be eight digits in HH:MM:SS format (HH:MM:SS is also accepted, if the hour begins with 0). Note: Trips that span multiple dates will have stop times greater than 24:00:00. For example, if a trip begins at 10:30:00 p.m. and ends at 2:15:00 a.m. on the following day, the stop times would be 22:30:00 and 26:15:00. Entering those stop times as 22:30:00 and 02:15:00 would not produce the desired results. SameAs: 'arrival_time' field from GTFS Static Field definitions-stop_times.txt (https://developers.google.com/transit/gtfs/reference#stop_timestxt)",
            "rdfs:label": "arrival_time",
            "rdfs:isDefinedBy": {
                "@id": "iudx:"
            },
            "iudx:domainIncludes": [
                {
                    "@id": "iudx:StopTimesDesc"
                }
            ],
            "iudx:rangeIncludes": [
                {
                    "@id": "iudx:Text"
                },
                {
                    "@id": "iudx:ValueDescriptor"
                }
            ],
            "skos:exactMatch": {
                "@id": "GTFS: arrival_time"
            }
        },
        {
            "@id": "iudx:associatedEntity",
            "@type": [
                "iudx:Relationship"
            ],
            "rdfs:comment": "ID of the associated entity.",
            "rdfs:label": "associatedEntity",
            "iudx:domainIncludes": [
                {
                    "@id": "iudx:IUDXEntity"
                }
            ],
            "iudx:rangeIncludes": [
                {
                    "@id": "iudx:Text"
                },
                {
                    "@id": "iudx:RelationshipValue"
                }
            ],
            "rdfs:isDefinedBy": {
                "@id": "iudx:"
            }
        },
        {
            "@id": "iudx:authControlLevel",
            "@type": [
                "iudx:TextProperty"
            ],
            "rdfs:comment": "Authorizataion Control Level for resouces associated with a given resource-group.  Individual authorization control level indicates that access control is available per resource, i.e., authorization can be granted/not-granted on a per resource basis for the resources. Group authorization control level indicates that the authorization is available on group level only, i.e., authorization will be granted/not-granted for all the resources associated with the given resource group. ENUM: [GROUP, INDIVIDUAL]. Default value is set to GROUP. This field is applicable only for non-open data, i.e., when the accessPolicy field is set to value other than OPEN.",
            "rdfs:label": "authControlLevel",
            "iudx:domainIncludes": [
                {
                    "@id": "iudx:ResourceGroup"
                }
            ],
            "iudx:rangeIncludes": [
                {
                    "@id": "iudx:Text"
                }
            ],
            "rdfs:isDefinedBy": {
                "@id": "iudx:"
            }
        },
        {
            "@id": "iudx:authServerURL",
            "@type": [
                "iudx:Relationship"
            ],
            "rdfs:comment": "URL of the IUDX authorization server used for a given resource.",
            "rdfs:label": "authServerURL",
            "iudx:domainIncludes": [
                {
                    "@id": "iudx:AuthServerInfoValue"
                }
            ],
            "iudx:rangeIncludes": [
                {
                    "@id": "iudx:Text",
                    "@type": "@id"
                },
                {
                    "@id": "iudx:RelationshipValue"
                }
            ]
        },
        {
            "@id": "iudx:authType",
            "@type": [
                "iudx:TextProperty"
            ],
            "rdfs:comment": "Identification of the auth scheme used for a given resource.  ENUM: [IUDXAUTH].",
            "rdfs:label": "authType",
            "iudx:domainIncludes": [
                {
                    "@id": "iudx:AuthServerInfoValue"
                }
            ],
            "iudx:rangeIncludes": [
                {
                    "@id": "iudx:Text"
                }
            ]
        },
        {
            "@id": "iudx:bikeType",
            "@type": [
                "iudx:TextProperty"
            ],
            "rdfs:comment": "Type of the bike corresponding to this observation. ENUM: [ELECTRIC BIKE, BICYCLE, STANDARD BIKE, GEARLESS BIKE, ELECTRIC BICYCLE, HYBRID BIKE, MOPED BIKE, MOPED BICYCLE, SPECIALITY BIKE].",
            "rdfs:label": "bikeType",
            "rdfs:isDefinedBy": {
                "@id": "iudx:"
            },
            "iudx:domainIncludes": [
                {
                    "@id": "iudx:BikeDockingStation"
                }
            ],
            "iudx:rangeIncludes": [
                {
                    "@id": "iudx:Text"
                },
                {
                    "@id": "iudx:ValueDescriptor"
                }
            ]
        },
        {
            "@id": "iudx:binCategory",
            "@type": [
                "iudx:TextProperty"
            ],
            "rdfs:comment": "Category/type of the waste container bin. It can be a household bin or a dumpster or any other pre-defined category/type.",
            "rdfs:label": "binCategory",
            "rdfs:isDefinedBy": {
                "@id": "iudx:"
            },
            "iudx:domainIncludes": [
                {
                    "@id": "iudx:WmgmtBin"
                },
                {
                    "@id": "iudx:WasteBinModel"
                }
            ],
            "iudx:rangeIncludes": [
                {
                    "@id": "iudx:Text"
                },
                {
                    "@id": "iudx:ValueDescriptor"
                }
            ]
        },
        {
            "@id": "iudx:binColor",
            "@type": [
                "iudx:TextProperty"
            ],
            "rdfs:comment": "Color of the bin. Could be used for indicating the type of waste. The color coding should follow the conventions applicable to the geographical area the bins are located.",
            "rdfs:label": "binColor",
            "rdfs:isDefinedBy": {
                "@id": "iudx:"
            },
            "iudx:domainIncludes": [
                {
                    "@id": "iudx:WmgmtBin"
                },
                {
                    "@id": "iudx:WasteBinModel"
                }
            ],
            "iudx:rangeIncludes": [
                {
                    "@id": "iudx:Text"
                },
                {
                    "@id": "iudx:ValueDescriptor"
                }
            ],
            "skos:exactMatch": {
                "@id": "fiware:color"
            }
        },
        {
            "@id": "iudx:binID",
            "@type": [
                "iudx:TextProperty"
            ],
            "rdfs:comment": "ID of the waste carrying bin",
            "rdfs:label": "binID",
            "rdfs:isDefinedBy": {
                "@id": "iudx:"
            },
            "iudx:domainIncludes": [
                {
                    "@id": "iudx:WmgmtBin"
                }
            ],
            "iudx:rangeIncludes": [
                {
                    "@id": "iudx:Text"
                },
                {
                    "@id": "iudx:ValueDescriptor"
                }
            ]
        },
        {
            "@id": "iudx:brandName",
            "@type": [
                "iudx:TextProperty"
            ],
            "rdfs:comment": "Name of the brand associated with an entity, e.g., sensor, device etc.",
            "rdfs:label": "brandName",
            "rdfs:isDefinedBy": {
                "@id": "iudx:"
            },
            "iudx:domainIncludes": [
                {
                    "@id": "iudx:ModelInfo"
                }
            ],
            "iudx:rangeIncludes": [
                {
                    "@id": "iudx:Text"
                }
            ],
            "skos:exactMatch": {
                "@id": "Fiware:brandName"
            }
        },
        {
            "@id": "iudx:cameraName",
            "@type": [
                "iudx:TextProperty"
            ],
            "rdfs:comment": "Name of the camera corresponding to this observation",
            "rdfs:label": "cameraName",
            "rdfs:isDefinedBy": {
                "@id": "iudx:"
            },
            "iudx:domainIncludes": [
                {
                    "@id": "iudx:Camera"
                }
            ],
            "iudx:rangeIncludes": [
                {
                    "@id": "iudx:Text"
                },
                {
                    "@id": "iudx:ValueDescriptor"
                }
            ]
        },
        {
            "@id": "iudx:cameraType",
            "@type": [
                "iudx:TextProperty"
            ],
            "rdfs:comment": "Type of the camera corresponding to this observation. ENUM: [FIXED, PTZ, DOME, DAY/NIGHT, C-MOUNT, BULLET].",
            "rdfs:label": "cameraType",
            "rdfs:isDefinedBy": {
                "@id": "iudx:"
            },
            "iudx:domainIncludes": [
                {
                    "@id": "iudx:Camera"
                }
            ],
            "iudx:rangeIncludes": [
                {
                    "@id": "iudx:Text"
                },
                {
                    "@id": "iudx:ValueDescriptor"
                }
            ]
        },
        {
            "@id": "iudx:cameraUsage",
            "@type": [
                "iudx:TextProperty"
            ],
            "rdfs:comment": "Purpose of the camera corresponding to this observation. ENUM: [SURVEILLANCE, RLVD, ANPR/LPR].",
            "rdfs:label": "cameraUsage",
            "rdfs:isDefinedBy": {
                "@id": "iudx:"
            },
            "iudx:domainIncludes": [
                {
                    "@id": "iudx:Camera"
                }
            ],
            "iudx:rangeIncludes": [
                {
                    "@id": "iudx:Text"
                },
                {
                    "@id": "iudx:ValueDescriptor"
                }
            ]
        },
        {
            "@id": "iudx:cardID",
            "@type": [
                "iudx:TextProperty"
            ],
            "rdfs:comment": "Unique ticket ID of the transaction or ID of the smart card used in the transaction.",
            "rdfs:label": "cardID",
            "rdfs:isDefinedBy": {
                "@id": "iudx:"
            },
            "iudx:domainIncludes": [
                {
                    "@id": "iudx:FareCollectionSystem"
                }
            ],
            "iudx:rangeIncludes": [
                {
                    "@id": "iudx:Text"
                },
                {
                    "@id": "iudx:ValueDescriptor"
                }
            ]
        },
        {
            "@id": "iudx:category",
            "@type": [
                "iudx:TextProperty"
            ],
            "rdfs:comment": "The category name corresponding to the issue that has been reported.",
            "rdfs:label": "category",
            "iudx:domainIncludes": [
                {
                    "@id": "iudx:IssueReporting"
                },
                {
                    "@id": "iudx:TouristDestination"
                }
            ],
            "iudx:rangeIncludes": [
                {
                    "@id": "iudx:Text"
                },
                {
                    "@id": "iudx:ValueDescriptor"
                }
            ],
            "rdfs:isDefinedBy": {
                "@id": "iudx:"
            },
            "skos:exactMatch": {
                "@id": "open311:group"
            }
        },
        {
            "@id": "iudx:categoryCode",
            "@type": [
                "iudx:TextProperty"
            ],
            "rdfs:comment": "Unique identifier for the category corresponding to the issue reported.",
            "rdfs:label": "categoryCode",
            "rdfs:isDefinedBy": {
                "@id": "iudx:"
            },
            "iudx:domainIncludes": [
                {
                    "@id": "iudx:IssueReporting"
                }
            ],
            "iudx:rangeIncludes": [
                {
                    "@id": "iudx:Text"
                },
                {
                    "@id": "iudx:ValueDescriptor"
                }
            ]
        },
        {
            "@id": "iudx:chargingUnitID",
            "@type": [
                "iudx:TextProperty"
            ],
            "rdfs:comment": "The ID of the charging point in the EV charging station corresponding to this observation.",
            "rdfs:label": "chargingUnitID",
            "rdfs:isDefinedBy": {
                "@id": "iudx:"
            },
            "iudx:domainIncludes": [
                {
                    "@id": "iudx:EVChargingStation"
                }
            ],
            "iudx:rangeIncludes": [
                {
                    "@id": "iudx:Text"
                },
                {
                    "@id": "iudx:ValueDescriptor"
                }
            ]
        },
        {
            "@id": "iudx:cityID",
            "@type": [
                "iudx:TextProperty"
            ],
            "rdfs:comment": "City ID corresponding to this observation.",
            "rdfs:label": "cityID",
            "rdfs:isDefinedBy": {
                "@id": "iudx:"
            },
            "iudx:domainIncludes": [
                {
                    "@id": "iudx:MunicipalityDesc"
                }
            ],
            "iudx:rangeIncludes": [
                {
                    "@id": "iudx:Text"
                },
                {
                    "@id": "iudx:ValueDescriptor"
                }
            ]
        },
        {
            "@id": "iudx:cityName",
            "@type": [
                "iudx:TextProperty"
            ],
            "rdfs:comment": "City name corresponding to this observation.",
            "rdfs:label": "cityName",
            "rdfs:isDefinedBy": {
                "@id": "iudx:"
            },
            "iudx:domainIncludes": [
                {
                    "@id": "iudx:MunicipalityDesc"
                }
            ],
            "iudx:rangeIncludes": [
                {
                    "@id": "iudx:Text"
                },
                {
                    "@id": "iudx:ValueDescriptor"
                }
            ]
        },
        {
            "@id": "iudx:comments",
            "@type": [
                "iudx:TextProperty"
            ],
            "rdfs:comment": "User comments corresponding to this observation.",
            "rdfs:label": "comments",
            "rdfs:isDefinedBy": {
                "@id": "iudx:"
            },
            "iudx:domainIncludes": [
                {
                    "@id": "iudx:SafetiPin"
                },
                {
                    "@id": "iudx:IssueReporting"
                },
                {
                    "@id": "iudx:Version"
                },
                {
                    "@id": "iudx:Orientation"
                },
                {
                    "@id": "iudx:BikeDockingStation"
                }
            ],
            "iudx:rangeIncludes": [
                {
                    "@container": "@list",
                    "@id": "iudx:Text"
                },
                {
                    "@id": "iudx:Text"
                },
                {
                    "@id": "iudx:ValueDescriptor"
                }
            ]
        },
        {
            "@id": "iudx:congestion_level",
            "@type": [
                "iudx:TextProperty"
            ],
            "rdfs:comment": "Describes the congestion level that is affecting this vehicle. ENUM [UNKNOWN_CONGESTION_LEVEL, RUNNING_SMOOTHLY, STOP_AND_GO, CONGESTION, SEVERE_CONGESTION]",
            "rdfs:label": "congestion_level",
            "rdfs:isDefinedBy": {
                "@id": "iudx:"
            },
            "iudx:domainIncludes": [
                {
                    "@id": "iudx:VehiclePosition"
                }
            ],
            "iudx:rangeIncludes": [
                {
                    "@id": "iudx:Text"
                },
                {
                    "@id": "iudx:ValueDescriptor"
                }
            ],
            "skos:exactMatch": {
                "@id": "GTFS: congestion_level"
            }
        },
        {
            "@id": "iudx:cos",
            "@type": [
                "iudx:Relationship"
            ],
            "rdfs:comment": "UUID of the COS(City Operations System) entity associated with the given catalogue item .",
            "rdfs:label": "cos",
            "iudx:domainIncludes": [
                {
                    "@id": "iudx:ResourceServer",
                    "iudx:requiredProperty": true
                }
            ],
            "iudx:rangeIncludes": [
                {
                    "@id": "iudx:Text",
                    "@type": "@id"
                },
                {
                    "@id": "iudx:RelationshipValue"
                }
            ]
        },
        {
            "@id": "iudx:cosUI",
            "@type": [
                "iudx:Relationship"
            ],
            "rdfs:comment": "URL pointing to the user interface/ catalogue which consists of information about the resources stored in the City Operations System(COS) corresponding to this observation.",
            "rdfs:label": "cosUI",
            "iudx:domainIncludes": [
                {
                    "@id": "iudx:COS"
                }
            ],
            "iudx:rangeIncludes": [
                {
                    "@id": "iudx:Text",
                    "@type": "@id"
                },
                {
                    "@id": "iudx:RelationshipValue"
                }
            ]
        },
        {
            "@id": "iudx:cosURL",
            "@type": [
                "iudx:Relationship"
            ],
            "rdfs:comment": "The URL(s) of the server(s) corresponding to the City Operations System(COS) in consideration. For eg., it may be include the domain links of the data resource server, the file system server, etc.",
            "rdfs:label": "cosURL",
            "iudx:domainIncludes": [
                {
                    "@id": "iudx:COS"
                }
            ],
            "iudx:rangeIncludes": [
                {
                    "@id": "iudx:Text",
                    "@type": "@id"
                },
                {
                    "@id": "iudx:RelationshipValue"
                }
            ]
        },
        {
            "@id": "iudx:current_status",
            "@type": [
                "iudx:TextProperty"
            ],
            "rdfs:comment": "Describes the status of the vehicle w.r.t the stop corresponding to this observation ENUM: [INCOMING_AT, STOPPED_AT, IN_TRANSIT_TO]. SameAs:'current_status' field from GTFS Realtime message-VehiclePosition(https://developers.google.com/transit/gtfs-realtime/reference#message-vehicleposition)",
            "rdfs:label": "current_status",
            "rdfs:isDefinedBy": {
                "@id": "iudx:"
            },
            "iudx:domainIncludes": [
                {
                    "@id": "iudx:VehiclePosition"
                }
            ],
            "iudx:rangeIncludes": [
                {
                    "@id": "iudx:Text"
                },
                {
                    "@id": "iudx:ValueDescriptor"
                }
            ],
            "skos:exactMatch": {
                "@id": "GTFS: current_status"
            }
        },
        {
            "@id": "iudx:cyclePathMaterial",
            "@type": [
                "iudx:TextProperty"
            ],
            "rdfs:comment": "Construction material used for laying the cycle path on the sides of the road corresponding to this observation.",
            "rdfs:label": "cyclePathMaterial",
            "rdfs:isDefinedBy": {
                "@id": "iudx:"
            },
            "iudx:domainIncludes": [
                {
                    "@id": "iudx:RoadSegment"
                }
            ],
            "iudx:rangeIncludes": [
                {
                    "@id": "iudx:Text"
                },
                {
                    "@id": "iudx:ValueDescriptor"
                }
            ]
        },
        {
            "@id": "iudx:cyclePathPlacement",
            "@type": [
                "iudx:TextProperty"
            ],
            "rdfs:comment": "Describes the placement of cycle track along the road segment corresponding to this observation. ENUM: [RIGHT, LEFT, BOTH, NOT_AVAILABLE]",
            "rdfs:label": "cyclePathPlacement",
            "rdfs:isDefinedBy": {
                "@id": "iudx:"
            },
            "iudx:domainIncludes": [
                {
                    "@id": "iudx:RoadSegment"
                }
            ],
            "iudx:rangeIncludes": [
                {
                    "@id": "iudx:Text"
                },
                {
                    "@id": "iudx:ValueDescriptor"
                }
            ]
        },
        {
            "@id": "iudx:dataDescriptor",
            "@type": [
                "iudx:Relationship"
            ],
            "rdfs:comment": "URI pointing to the data-descriptor entity",
            "rdfs:label": "dataDescriptor",
            "iudx:domainIncludes": [
                {
                    "@id": "iudx:ResourceGroup"
                },
                {
                    "@id": "iudx:Resource"
                }
            ],
            "iudx:rangeIncludes": [
                {
                    "@type": "@id",
                    "@id": "iudx:Text"
                },
                {
                    "@id": "iudx:RelationshipValue"
                },
                {
                    "@id": "iudx:DataModel"
                }
            ]
        },
        {
            "@id": "iudx:dataDescriptorLabel",
            "@type": [
                "iudx:TextProperty"
            ],
            "rdfs:comment": "Human readable label for an entity",
            "rdfs:label": "dataDescriptorLabel",
            "iudx:domainIncludes": [
                {
                    "@id": "iudx:DataDescriptor"
                }
            ],
            "iudx:rangeIncludes": [
                {
                    "@id": "iudx:Text"
                }
            ],
            "rdfs:isDefinedBy": {
                "@id": "iudx:"
            }
        },
        {
            "@id": "iudx:dataDescriptorName",
            "@type": [
                "iudx:TextProperty"
            ],
            "rdfs:comment": "Name of the entity.",
            "rdfs:label": "dataDescriptorName",
            "iudx:domainIncludes": [
                {
                    "@id": "iudx:DataDescriptor"
                }
            ],
            "iudx:rangeIncludes": [
                {
                    "@id": "iudx:Text"
                }
            ],
            "skos:exactMatch": {
                "@id": "schema:name"
            },
            "rdfs:isDefinedBy": {
                "@id": "iudx:"
            }
        },
        {
            "@id": "iudx:dataQualityFile",
            "@type": [
                "iudx:Relationship"
            ],
            "rdfs:comment": " Data Quality file download link for the resource",
            "rdfs:label": "dataQualityFile",
            "iudx:domainIncludes": [
                {
                    "@id": "iudx:ResourceGroup"
                },
                {
                    "@id": "iudx:Resource"
                }
            ],
            "iudx:rangeIncludes": [
                {
                    "@container": "@list",
                    "@id": "iudx:Text"
                },
                {
                    "@container": "@list",
                    "@id": "iudx:RelationshipValue"
                }
            ],
            "rdfs:isDefinedBy": {
                "@id": "iudx:"
            }
        },
        {
            "@id": "iudx:dataSample",
            "@type": [
                "iudx:TextProperty"
            ],
            "rdfs:comment": "Stringified sample object of the resource",
            "rdfs:label": "dataSample",
            "iudx:domainIncludes": [
                {
                    "@id": "iudx:ResourceGroup"
                },
                {
                    "@id": "iudx:Resource"
                }
            ],
            "iudx:rangeIncludes": [
                {
                    "@id": "iudx:Text"
                }
            ],
            "rdfs:isDefinedBy": {
                "@id": "iudx:"
            }
        },
        {
            "@id": "iudx:dataSampleFile",
            "@type": [
                "iudx:Relationship"
            ],
            "rdfs:comment": "Sample file download link for the resource",
            "rdfs:label": "dataSampleFile",
            "iudx:domainIncludes": [
                {
                    "@id": "iudx:ResourceGroup"
                },
                {
                    "@id": "iudx:Resource"
                }
            ],
            "iudx:rangeIncludes": [
                {
                    "@container": "@list",
                    "@id": "iudx:Text"
                },
                {
                    "@container": "@list",
                    "@id": "iudx:RelationshipValue"
                }
            ],
            "rdfs:isDefinedBy": {
                "@id": "iudx:"
            }
        },
        {
            "@id": "iudx:dataSchema",
            "@type": [
                "iudx:TextProperty"
            ],
            "rdfs:comment": "Associated data schema. Specified as an URI (linking it to one of the known data type vocabulary, e.g., xsd)",
            "rdfs:label": "dataSchema",
            "iudx:domainIncludes": [
                {
                    "@id": "iudx:ValueDescriptor"
                }
            ],
            "iudx:rangeIncludes": [
                {
                    "@id": "iudx:Text",
                    "@type": "@id"
                }
            ],
            "rdfs:isDefinedBy": {
                "@id": "iudx:"
            }
        },
        {
            "@id": "iudx:date",
            "@type": [
                "iudx:TextProperty"
            ],
            "rdfs:comment": "Date corresponding to this observation and is described in YYYY-MM-DD format, for eg. '2020-11-01'.",
            "rdfs:label": "date",
            "iudx:domainIncludes": [
                {
                    "@id": "iudx:RevenueCollection"
                },
                {
                    "@id": "iudx:EmployeeDetails"
                }
            ],
            "iudx:rangeIncludes": [
                {
                    "@id": "iudx:Text"
                },
                {
                    "@id": "iudx:ValueDescriptor"
                }
            ],
            "rdfs:isDefinedBy": {
                "@id": "iudx:"
            }
        },
        {
            "@id": "iudx:daysOff",
            "@type": [
                "iudx:TextProperty"
            ],
            "rdfs:comment": "The days on which the public site or tourist destination is closed.",
            "rdfs:label": "daysOff",
            "rdfs:isDefinedBy": {
                "@id": "iudx:"
            },
            "iudx:domainIncludes": [
                {
                    "@id": "iudx:TouristDestination"
                }
            ],
            "iudx:rangeIncludes": [
                {
                    "@id": "iudx:Text"
                },
                {
                    "@id": "iudx:ValueDescriptor"
                }
            ]
        },
        {
            "@id": "iudx:department",
            "@type": [
                "iudx:TextProperty"
            ],
            "rdfs:comment": "Division or section of the organization corresponding to this observation. Eg. Health, Transport.",
            "rdfs:label": "department",
            "iudx:domainIncludes": [
                {
                    "@id": "iudx:EmployeeDetails"
                },
                {
                    "@id": "iudx:IssueReporting"
                },
                {
                    "@id": "iudx:EnergyMeter"
                },
                {
                    "@id": "iudx:PublicSchemes"
                }
            ],
            "iudx:rangeIncludes": [
                {
                    "@id": "iudx:Text"
                },
                {
                    "@id": "iudx:ValueDescriptor"
                }
            ],
            "rdfs:isDefinedBy": {
                "@id": "iudx:"
            },
            "skos:exactMatch": {
                "@id": "schema:department"
            }
        },
        {
            "@id": "iudx:departmentID",
            "@type": [
                "iudx:TextProperty"
            ],
            "rdfs:comment": "Unique ID or code associated with the department which is associated with the service or the issue corresponding to this observation.",
            "rdfs:label": "departmentID",
            "iudx:domainIncludes": [
                {
                    "@id": "iudx:IssueReporting"
                },
                {
                    "@id": "iudx:EmployeeDetails"
                },
                {
                    "@id": "iudx:PublicSchemes"
                }
            ],
            "iudx:rangeIncludes": [
                {
                    "@id": "iudx:Text"
                },
                {
                    "@id": "iudx:ValueDescriptor"
                }
            ],
            "rdfs:isDefinedBy": {
                "@id": "iudx:"
            }
        },
        {
            "@id": "iudx:departure_time",
            "@type": [
                "iudx:TimeProperty"
            ],
            "rdfs:comment": "Specifies the departure time from a specific stop for a specific trip on a route. Times must be eight digits in HH:MM:SS format (HH:MM:SS is also accepted, if the hour begins with 0). Note: Trips that span multiple dates will have stop times greater than 24:00:00. For example, if a trip begins at 10:30:00 p.m. and ends at 2:15:00 a.m. on the following day, the stop times would be 22:30:00 and 26:15:00. Entering those stop times as 22:30:00 and 02:15:00 would not produce the desired results. SameAs: 'departure_time' field from GTFS Static Field definitions-stop_times.txt (https://developers.google.com/transit/gtfs/reference#stop_timestxt)",
            "rdfs:label": "departure_time",
            "rdfs:isDefinedBy": {
                "@id": "iudx:"
            },
            "iudx:domainIncludes": [
                {
                    "@id": "iudx:StopTimesDesc"
                }
            ],
            "iudx:rangeIncludes": [
                {
                    "@id": "iudx:Text"
                },
                {
                    "@id": "iudx:ValueDescriptor"
                }
            ],
            "skos:exactMatch": {
                "@id": "GTFS: departure_time"
            }
        },
        {
            "@id": "iudx:depotID",
            "@type": [
                "iudx:TextProperty"
            ],
            "rdfs:comment": "Describes the unique id of the bus depot corresponding to this observation.",
            "rdfs:label": "depotID",
            "rdfs:isDefinedBy": {
                "@id": "iudx:"
            },
            "iudx:domainIncludes": [
                {
                    "@id": "iudx:TransitManagement"
                }
            ],
            "iudx:rangeIncludes": [
                {
                    "@id": "iudx:Text"
                },
                {
                    "@id": "iudx:ValueDescriptor"
                }
            ]
        },
        {
            "@id": "iudx:depotName",
            "@type": [
                "iudx:TextProperty"
            ],
            "rdfs:comment": "Describes the depot name of the bus depot corresponding to this observation.",
            "rdfs:label": "depotName",
            "rdfs:isDefinedBy": {
                "@id": "iudx:"
            },
            "iudx:domainIncludes": [
                {
                    "@id": "iudx:TransitManagement"
                }
            ],
            "iudx:rangeIncludes": [
                {
                    "@id": "iudx:Text"
                },
                {
                    "@id": "iudx:ValueDescriptor"
                }
            ]
        },
        {
            "@id": "iudx:description",
            "@type": [
                "iudx:TextProperty"
            ],
            "rdfs:comment": "Description for an IUDX thing.",
            "rdfs:label": "description",
            "iudx:domainIncludes": [
                {
                    "@id": "iudx:Thing"
                }
            ],
            "iudx:rangeIncludes": [
                {
                    "@id": "iudx:Text"
                }
            ],
            "rdfs:isDefinedBy": {
                "@id": "iudx:"
            }
        },
        {
            "@id": "iudx:destinationStopCategory",
            "@type": [
                "iudx:TextProperty"
            ],
            "rdfs:comment": "Type of the destination bus stop corresponding to this observation.",
            "rdfs:label": "destinationStopCategory",
            "rdfs:isDefinedBy": {
                "@id": "iudx:"
            },
            "iudx:domainIncludes": [
                {
                    "@id": "iudx:FareCollectionSystem"
                }
            ],
            "iudx:rangeIncludes": [
                {
                    "@id": "iudx:Text"
                },
                {
                    "@id": "iudx:ValueDescriptor"
                }
            ]
        },
        {
            "@id": "iudx:destinationStopID",
            "@type": [
                "iudx:TextProperty"
            ],
            "rdfs:comment": "Unique ID of the bus stop at which the passenger deboards from the bus corresponding to this observation.",
            "rdfs:label": "destinationStopID",
            "rdfs:isDefinedBy": {
                "@id": "iudx:"
            },
            "iudx:domainIncludes": [
                {
                    "@id": "iudx:FareCollectionSystem"
                }
            ],
            "iudx:rangeIncludes": [
                {
                    "@id": "iudx:Text"
                },
                {
                    "@id": "iudx:ValueDescriptor"
                }
            ]
        },
        {
            "@id": "iudx:destinationStopName",
            "@type": [
                "iudx:TextProperty"
            ],
            "rdfs:comment": "The name of the destination bus stop corresponding to this observation.",
            "rdfs:label": "destinationStopName",
            "rdfs:isDefinedBy": {
                "@id": "iudx:"
            },
            "iudx:domainIncludes": [
                {
                    "@id": "iudx:FareCollectionSystem"
                }
            ],
            "iudx:rangeIncludes": [
                {
                    "@id": "iudx:Text"
                },
                {
                    "@id": "iudx:ValueDescriptor"
                }
            ]
        },
        {
            "@id": "iudx:destinationType",
            "@type": [
                "iudx:TextProperty"
            ],
            "rdfs:comment": "The type of public site or tourist destination corresponding to this observation. Example Historic Monuments, Religious sites, etc.",
            "rdfs:label": "destinationType",
            "rdfs:isDefinedBy": {
                "@id": "iudx:"
            },
            "iudx:domainIncludes": [
                {
                    "@id": "iudx:TouristDestination"
                }
            ],
            "iudx:rangeIncludes": [
                {
                    "@id": "iudx:Text"
                },
                {
                    "@id": "iudx:ValueDescriptor"
                }
            ]
        },
        {
            "@id": "iudx:deviceBatteryStatus",
            "@type": [
                "iudx:TextProperty"
            ],
            "rdfs:comment": "Gives the Battery charging status of the reporting device. ENUM: [Connected, Disconnected].",
            "rdfs:label": "deviceBatteryStatus",
            "rdfs:isDefinedBy": {
                "@id": "iudx:"
            },
            "iudx:domainIncludes": [
                {
                    "@id": "iudx:Device"
                }
            ],
            "iudx:rangeIncludes": [
                {
                    "@id": "iudx:Text"
                },
                {
                    "@id": "iudx:ValueDescriptor"
                }
            ]
        },
        {
            "@id": "iudx:deviceID",
            "@type": [
                "iudx:TextProperty"
            ],
            "rdfs:comment": "Device ID of the physical sensor/ measurement station corresponding to this observation.",
            "rdfs:label": "deviceID",
            "rdfs:isDefinedBy": {
                "@id": "iudx:"
            },
            "iudx:domainIncludes": [
                {
                    "@id": "iudx:Device"
                }
            ],
            "iudx:rangeIncludes": [
                {
                    "@id": "iudx:Text"
                },
                {
                    "@id": "iudx:ValueDescriptor"
                }
            ]
        },
        {
            "@id": "iudx:deviceName",
            "@type": [
                "iudx:TextProperty"
            ],
            "rdfs:comment": "Device Name or Station name of the sensor device/station corresponding to this observation.",
            "rdfs:label": "deviceName",
            "rdfs:isDefinedBy": {
                "@id": "iudx:"
            },
            "iudx:domainIncludes": [
                {
                    "@id": "iudx:Device"
                }
            ],
            "iudx:rangeIncludes": [
                {
                    "@id": "iudx:Text"
                },
                {
                    "@id": "iudx:ValueDescriptor"
                }
            ]
        },
        {
            "@id": "iudx:deviceSimNumber",
            "@type": [
                "iudx:TextProperty"
            ],
            "rdfs:comment": "Gives the sim number of the tracker device in the vehicle.",
            "rdfs:label": "deviceSimNumber",
            "rdfs:isDefinedBy": {
                "@id": "iudx:"
            },
            "iudx:domainIncludes": [
                {
                    "@id": "iudx:Device"
                }
            ],
            "iudx:rangeIncludes": [
                {
                    "@id": "iudx:Text"
                },
                {
                    "@id": "iudx:ValueDescriptor"
                }
            ]
        },
        {
            "@id": "iudx:deviceStatus",
            "@type": [
                "iudx:TextProperty"
            ],
            "rdfs:comment": "Indicates the status of physical device or devices.",
            "rdfs:label": "deviceStatus",
            "iudx:domainIncludes": [
                {
                    "@id": "iudx:EnvAQM"
                },
                {
                    "@id": "iudx:EnvFlood"
                },
                {
                    "@id": "iudx:Streetlight"
                },
                {
                    "@id": "iudx:AirQuality"
                }
            ],
            "iudx:rangeIncludes": [
                {
                    "@id": "iudx:Text"
                },
                {
                    "@id": "iudx:ValueDescriptor"
                }
            ],
            "rdfs:isDefinedBy": {
                "@id": "iudx:"
            }
        },
        {
            "@id": "iudx:district",
            "@type": [
                "iudx:TextProperty"
            ],
            "rdfs:comment": "District name corresponding to this observation.",
            "rdfs:label": "district",
            "iudx:domainIncludes": [
                {
                    "@id": "iudx:Headquarters"
                },
                {
                    "@id": "iudx:District"
                },
                {
                    "@id": "iudx:Headquarters"
                }
            ],
            "iudx:rangeIncludes": [
                {
                    "@id": "iudx:Text"
                },
                {
                    "@id": "iudx:ValueDescriptor"
                }
            ],
            "rdfs:isDefinedBy": {
                "@id": "iudx:"
            }
        },
        {
            "@id": "iudx:district_l",
            "@type": [
                "iudx:TextProperty"
            ],
            "rdfs:comment": "Name of district I corresponding to this observation",
            "rdfs:label": "district_l",
            "rdfs:isDefinedBy": {
                "@id": "iudx:"
            },
            "iudx:domainIncludes": [
                {
                    "@id": "iudx:District"
                }
            ],
            "iudx:rangeIncludes": [
                {
                    "@id": "iudx:Text"
                },
                {
                    "@id": "iudx:ValueDescriptor"
                }
            ]
        },
        {
            "@id": "iudx:downloadURL",
            "@type": [
                "iudx:Relationship"
            ],
            "rdfs:comment": "A download URL specifying the protocol, for e.g s3:// or https://, etc.",
            "rdfs:label": "downloadURL",
            "rdfs:isDefinedBy": {
                "@id": "iudx:"
            },
            "iudx:domainIncludes": [],
            "iudx:rangeIncludes": [
                {
                    "@id": "iudx:Text",
                    "@type": "@id"
                },
                {
                    "@id": "iudx:RelationshipValue"
                }
            ]
        },
        {
            "@id": "iudx:drop_off_type",
            "@type": [
                "iudx:TextProperty"
            ],
            "rdfs:comment": "Indicates drop off method. SameAs: 'drop_off_type' field from GTFS Static Field definitions-stop_times.txt (https://developers.google.com/transit/gtfs/reference#stop_timestxt)",
            "rdfs:label": "drop_off_type",
            "rdfs:isDefinedBy": {
                "@id": "iudx:"
            },
            "iudx:domainIncludes": [
                {
                    "@id": "iudx:StopTimesDesc"
                }
            ],
            "iudx:rangeIncludes": [
                {
                    "@id": "iudx:Text"
                },
                {
                    "@id": "iudx:ValueDescriptor"
                }
            ],
            "skos:exactMatch": {
                "@id": "GTFS: drop_off_type"
            }
        },
        {
            "@id": "iudx:eligibleBeneficiaries",
            "@type": [
                "iudx:TextProperty"
            ],
            "rdfs:comment": "Represents the group(s) or category(ies) of people who can avail the benefits of the scheme corresponding to this observation.",
            "rdfs:label": "eligibleBeneficiaries",
            "rdfs:isDefinedBy": {
                "@id": "iudx:"
            },
            "iudx:domainIncludes": [
                {
                    "@id": "iudx:PublicSchemes"
                }
            ],
            "iudx:rangeIncludes": [
                {
                    "@container": "@list",
                    "@id": "iudx:Text"
                },
                {
                    "@id": "iudx:ValueDescriptor"
                }
            ]
        },
        {
            "@id": "iudx:emergencyVehicleType",
            "@type": [
                "iudx:TextProperty"
            ],
            "rdfs:comment": "Type of emergency vehicle corresponding to this observation. ENUM: [POLICE CAR, POLICE MOTORCYCLE, POLICE VAN, POLICE S.W.A.T, FIRE ENGINE, WATER TENDER, AIR AMBULANCE, AMBULANCE, MOTORCYCLE AMBULANCE, RESCUE VEHICLE, HAZARDOUS MATERIALS APPARATUS, TOW TRUCK]",
            "rdfs:label": "emergencyVehicleType",
            "rdfs:isDefinedBy": {
                "@id": "iudx:"
            },
            "iudx:domainIncludes": [
                {
                    "@id": "iudx:EmergencyVehicle"
                }
            ],
            "iudx:rangeIncludes": [
                {
                    "@id": "iudx:Text"
                },
                {
                    "@id": "iudx:ValueDescriptor"
                }
            ]
        },
        {
            "@id": "iudx:employeeDesignation",
            "@type": [
                "iudx:TextProperty"
            ],
            "rdfs:comment": "Title assigned to the employee corresponding to this observation. Eg. Sweeper, Driver, Helper, Supervisor, Safai Meth, Cleaner, Bhisti. etc.",
            "rdfs:label": "employeeDesignation",
            "rdfs:isDefinedBy": {
                "@id": "iudx:"
            },
            "iudx:domainIncludes": [
                {
                    "@id": "iudx:EmployeeDetails"
                }
            ],
            "iudx:rangeIncludes": [
                {
                    "@id": "iudx:Text"
                },
                {
                    "@id": "iudx:ValueDescriptor"
                }
            ],
            "skos:exactMatch": {
                "@id": "schema:jobTitle"
            }
        },
        {
            "@id": "iudx:employeeID",
            "@type": [
                "iudx:TextProperty"
            ],
            "rdfs:comment": "Unique ID of the employee corresponding to this observation",
            "rdfs:label": "employeeID",
            "rdfs:isDefinedBy": {
                "@id": "iudx:"
            },
            "iudx:domainIncludes": [
                {
                    "@id": "iudx:EmployeeDetails"
                }
            ],
            "iudx:rangeIncludes": [
                {
                    "@id": "iudx:Text"
                },
                {
                    "@id": "iudx:ValueDescriptor"
                }
            ]
        },
        {
            "@id": "iudx:employmentType",
            "@type": [
                "iudx:TextProperty"
            ],
            "rdfs:comment": "Type of employment. ENUM: [Contractual New, Contractual Old, Regular, Outsourcing]",
            "rdfs:label": "employmentType",
            "rdfs:isDefinedBy": {
                "@id": "iudx:"
            },
            "iudx:domainIncludes": [
                {
                    "@id": "iudx:EmployeeDetails"
                }
            ],
            "iudx:rangeIncludes": [
                {
                    "@id": "iudx:Text"
                },
                {
                    "@id": "iudx:ValueDescriptor"
                }
            ],
            "skos:exactMatch": {
                "@id": "schema:employmentType"
            }
        },
        {
            "@id": "iudx:employmentUnit",
            "@type": [
                "iudx:TextProperty"
            ],
            "rdfs:comment": "Unit and/or facility where the employee reports and/or in which the job is to be performed.\nENUM: [Sweeping, Drainage, Vehicle Driver, Vehicle Helper, Workshop, Door to Door, Supervisor, Office Work]",
            "rdfs:label": "employmentUnit",
            "rdfs:isDefinedBy": {
                "@id": "iudx:"
            },
            "iudx:domainIncludes": [
                {
                    "@id": "iudx:EmployeeDetails"
                }
            ],
            "iudx:rangeIncludes": [
                {
                    "@id": "iudx:Text"
                },
                {
                    "@id": "iudx:ValueDescriptor"
                }
            ],
            "skos:exactMatch": {
                "@id": "schema:employmentUnit"
            }
        },
        {
            "@id": "iudx:entity_id",
            "@type": [
                "iudx:TextProperty"
            ],
            "rdfs:comment": "Feed unique ID for the entity corresponding to this observation.SameAs:'entity_id' field from GTFS Realtime message-FeedEntity(https://developers.google.com/transit/gtfs-realtime/reference#message-feedentity)",
            "rdfs:label": "entity_id",
            "rdfs:isDefinedBy": {
                "@id": "iudx:"
            },
            "iudx:domainIncludes": [
                {
                    "@id": "iudx:TransitManagement"
                }
            ],
            "iudx:rangeIncludes": [
                {
                    "@id": "iudx:Text"
                },
                {
                    "@id": "iudx:ValueDescriptor"
                }
            ]
        },
        {
            "@id": "iudx:entryAreaCode",
            "@type": [
                "iudx:TextProperty"
            ],
            "rdfs:comment": "Area code of the passenger boarding stop (used by the fare collection agency). For example, whether the stop is city-bus-service stop or brts stop or other service type stop etc.",
            "rdfs:label": "entryAreaCode",
            "rdfs:isDefinedBy": {
                "@id": "iudx:"
            },
            "iudx:domainIncludes": [
                {
                    "@id": "iudx:FareCollectionSystem"
                }
            ],
            "iudx:rangeIncludes": [
                {
                    "@id": "iudx:Text"
                },
                {
                    "@id": "iudx:ValueDescriptor"
                }
            ]
        },
        {
            "@id": "iudx:entryFee",
            "@type": [
                "iudx:TextProperty"
            ],
            "rdfs:comment": "The amount to be paid to enter the  public site or tourist destination.",
            "rdfs:label": "entryFee",
            "rdfs:isDefinedBy": {
                "@id": "iudx:"
            },
            "iudx:domainIncludes": [
                {
                    "@id": "iudx:TouristDestination"
                }
            ],
            "iudx:rangeIncludes": [
                {
                    "@id": "iudx:Text"
                },
                {
                    "@id": "iudx:ValueDescriptor"
                }
            ]
        },
        {
            "@id": "iudx:equipmentCompanyCode",
            "@type": [
                "iudx:TextProperty"
            ],
            "rdfs:comment": "Company/Agency code for the transaction equipment (used by fare collection agency). For example, 103 - CBS (city bus service),102 -  BRTS etc.",
            "rdfs:label": "equipmentCompanyCode",
            "rdfs:isDefinedBy": {
                "@id": "iudx:"
            },
            "iudx:domainIncludes": [
                {
                    "@id": "iudx:FareCollectionSystem"
                }
            ],
            "iudx:rangeIncludes": [
                {
                    "@id": "iudx:Text"
                },
                {
                    "@id": "iudx:ValueDescriptor"
                }
            ]
        },
        {
            "@id": "iudx:equipmentID",
            "@type": [
                "iudx:TextProperty"
            ],
            "rdfs:comment": "Unique ID of the equipment corresponding to this observation.",
            "rdfs:label": "equipmentID",
            "rdfs:isDefinedBy": {
                "@id": "iudx:"
            },
            "iudx:domainIncludes": [
                {
                    "@id": "iudx:FareCollectionSystem"
                },
                {
                    "@id": "iudx:TrafficViolations"
                }
            ],
            "iudx:rangeIncludes": [
                {
                    "@id": "iudx:Text"
                },
                {
                    "@id": "iudx:ValueDescriptor"
                }
            ]
        },
        {
            "@id": "iudx:equipmentStopID",
            "@type": [
                "iudx:TextProperty"
            ],
            "rdfs:comment": "Stop ID (BRTS) at which the equipment corresponding to this transaction is installed.",
            "rdfs:label": "equipmentStopID",
            "rdfs:isDefinedBy": {
                "@id": "iudx:"
            },
            "iudx:domainIncludes": [
                {
                    "@id": "iudx:FareCollectionSystem"
                }
            ],
            "iudx:rangeIncludes": [
                {
                    "@id": "iudx:Text"
                },
                {
                    "@id": "iudx:ValueDescriptor"
                }
            ]
        },
        {
            "@id": "iudx:equipmentType",
            "@type": [
                "iudx:TextProperty"
            ],
            "rdfs:comment": "Type of equipment or the name of the equipment corresponding to this observation.",
            "rdfs:label": "equipmentType",
            "rdfs:isDefinedBy": {
                "@id": "iudx:"
            },
            "iudx:domainIncludes": [
                {
                    "@id": "iudx:FareCollectionSystem"
                },
                {
                    "@id": "iudx:TrafficViolations"
                }
            ],
            "iudx:rangeIncludes": [
                {
                    "@id": "iudx:Text"
                },
                {
                    "@id": "iudx:ValueDescriptor"
                }
            ]
        },
        {
            "@id": "iudx:equipmentTypeCode",
            "@type": [
                "iudx:TextProperty"
            ],
            "rdfs:comment": "Unique code indicating the type of equipment used in the transaction (used by fare collection agency).ENUM [1B, 42, 02, 08, 41]\n1B - POS, 42 - HTT, 02- Mobile, 08- Fare Gate, 41- Pole Validator",
            "rdfs:label": "equipmentTypeCode",
            "rdfs:isDefinedBy": {
                "@id": "iudx:"
            },
            "iudx:domainIncludes": [
                {
                    "@id": "iudx:FareCollectionSystem"
                }
            ],
            "iudx:rangeIncludes": [
                {
                    "@id": "iudx:Text"
                },
                {
                    "@id": "iudx:ValueDescriptor"
                }
            ]
        },
        {
            "@id": "iudx:establishmentType",
            "@type": [
                "iudx:TextProperty"
            ],
            "rdfs:comment": "Type of public service or business or facility set up for public welfare or governance. For eg., the establishment can be a business under an individual as a sole proprietor(or a company) or smart public installments such as lavatories etc.",
            "rdfs:label": "establishmentType",
            "rdfs:isDefinedBy": {
                "@id": "iudx:"
            },
            "iudx:domainIncludes": [
                {
                    "@id": "iudx:RevenueCollection"
                }
            ],
            "iudx:rangeIncludes": [
                {
                    "@id": "iudx:Text"
                },
                {
                    "@id": "iudx:ValueDescriptor"
                }
            ]
        },
        {
            "@id": "iudx:exitAreaCode",
            "@type": [
                "iudx:TextProperty"
            ],
            "rdfs:comment": "Area code of the passenger alighting stop (used by the fare collection agency). For example, whether the stop is city-bus-service stop or brts stop or other service type stop etc.",
            "rdfs:label": "exitAreaCode",
            "rdfs:isDefinedBy": {
                "@id": "iudx:"
            },
            "iudx:domainIncludes": [
                {
                    "@id": "iudx:FareCollectionSystem"
                }
            ],
            "iudx:rangeIncludes": [
                {
                    "@id": "iudx:Text"
                },
                {
                    "@id": "iudx:ValueDescriptor"
                }
            ]
        },
        {
            "@id": "iudx:f_name",
            "@type": [
                "iudx:TextProperty"
            ],
            "rdfs:comment": "Name of the feature corresponding this observation",
            "rdfs:label": "f_name",
            "rdfs:isDefinedBy": {
                "@id": "iudx:"
            },
            "iudx:domainIncludes": [
                {
                    "@id": "iudx:FeaturesOfInterest"
                }
            ],
            "iudx:rangeIncludes": [
                {
                    "@id": "iudx:Text"
                },
                {
                    "@id": "iudx:ValueDescriptor"
                }
            ]
        },
        {
            "@id": "iudx:faultTitle",
            "@type": [
                "iudx:TextProperty"
            ],
            "rdfs:comment": "The brief discription of the fault or issues of the product based on the experience of user.",
            "rdfs:label": "faultTitle",
            "rdfs:isDefinedBy": {
                "@id": "iudx:"
            },
            "iudx:domainIncludes": [
                {
                    "@id": "iudx:BikeDockingStation"
                }
            ],
            "iudx:rangeIncludes": [
                {
                    "@id": "iudx:Text"
                },
                {
                    "@id": "iudx:ValueDescriptor"
                }
            ],
            "skos:exactMatch": {
                "@id": "Fiware:faultLog"
            }
        },
        {
            "@id": "iudx:feederConnectivity",
            "@type": [
                "iudx:TextProperty"
            ],
            "rdfs:comment": "Describes the connectivity status of the streetlight feeder panel associated with the streetlight corresponding to this observation. ENUM: [connected, disconnected]",
            "rdfs:label": "feederConnectivity",
            "rdfs:isDefinedBy": {
                "@id": "iudx:"
            },
            "iudx:domainIncludes": [
                {
                    "@id": "iudx:Streetlight"
                }
            ],
            "iudx:rangeIncludes": [
                {
                    "@id": "iudx:Text"
                },
                {
                    "@id": "iudx:ValueDescriptor"
                }
            ]
        },
        {
            "@id": "iudx:feederID",
            "@type": [
                "iudx:Relationship"
            ],
            "rdfs:comment": "Unique ID of the streetlight feeder panel associated with the streetlight corresponding to this observation.",
            "rdfs:label": "feederID",
            "iudx:domainIncludes": [
                {
                    "@id": "iudx:Streetlight"
                }
            ],
            "iudx:rangeIncludes": [
                {
                    "@id": "iudx:Text"
                },
                {
                    "@id": "iudx:Text",
                    "@type": "@id"
                },
                {
                    "@id": "iudx:RelationshipValue"
                }
            ],
            "rdfs:isDefinedBy": {
                "@id": "iudx:"
            }
        },
        {
            "@id": "iudx:feederPillarNum",
            "@type": [
                "iudx:TextProperty"
            ],
            "rdfs:comment": "Streetlight feeder pillar information associated with the streetlight corresponding to this observation.",
            "rdfs:label": "feederPillarNum",
            "rdfs:isDefinedBy": {
                "@id": "iudx:"
            },
            "iudx:domainIncludes": [
                {
                    "@id": "iudx:Streetlight"
                }
            ],
            "iudx:rangeIncludes": [
                {
                    "@id": "iudx:Text"
                },
                {
                    "@id": "iudx:ValueDescriptor"
                }
            ]
        },
        {
            "@id": "iudx:floodLevelStatus",
            "@type": [
                "iudx:TextProperty"
            ],
            "rdfs:comment": "Flood level status indication given by the flood sensing device. The status is marked Danger if the current level is higher than the danger level threshold value.",
            "rdfs:label": "floodLevelStatus",
            "rdfs:isDefinedBy": {
                "@id": "iudx:"
            },
            "iudx:domainIncludes": [
                {
                    "@id": "iudx:EnvFlood"
                }
            ],
            "iudx:rangeIncludes": [
                {
                    "@id": "iudx:Text"
                },
                {
                    "@id": "iudx:ValueDescriptor"
                }
            ]
        },
        {
            "@id": "iudx:fuelType",
            "@type": [
                "iudx:TextProperty"
            ],
            "rdfs:comment": "The type of fuel suitable for the engine or engines of the vehicle corresponding to this observation.",
            "rdfs:label": "fuelType",
            "rdfs:isDefinedBy": {
                "@id": "iudx:"
            },
            "iudx:domainIncludes": [
                {
                    "@id": "iudx:WmgmtVehicle"
                },
                {
                    "@id": "iudx:EmergencyVehicle"
                }
            ],
            "iudx:rangeIncludes": [
                {
                    "@id": "iudx:Text"
                },
                {
                    "@id": "iudx:ValueDescriptor"
                }
            ],
            "skos:exactMatch": {
                "@id": "schema:fuelType"
            }
        },
        {
            "@id": "iudx:functionParameters",
            "@type": [
                "iudx:TextProperty"
            ],
            "rdfs:comment": "List of parameters associated with a function.",
            "rdfs:label": "functionParameters",
            "iudx:domainIncludes": [
                {
                    "@id": "iudx:FunctionDescription"
                }
            ],
            "iudx:rangeIncludes": [
                {
                    "@id": "iudx:Text",
                    "@container": "@list"
                }
            ]
        },
        {
            "@id": "iudx:gender",
            "@type": [
                "iudx:TextProperty"
            ],
            "rdfs:comment": "Gender of the employee or person corresponding to this observation.",
            "rdfs:label": "gender",
            "rdfs:isDefinedBy": {
                "@id": "iudx:"
            },
            "iudx:domainIncludes": [
                {
                    "@id": "iudx:EmployeeDetails"
                }
            ],
            "iudx:rangeIncludes": [
                {
                    "@id": "iudx:Text"
                },
                {
                    "@id": "iudx:ValueDescriptor"
                }
            ],
            "skos:exactMatch": {
                "@id": "schema:gender"
            }
        },
        {
            "@id": "iudx:gisAccessToken",
            "@type": [
                "iudx:TextProperty"
            ],
            "rdfs:comment": "A string of encrypted information that contains the user's name, the token expiration time, and some proprietary information, which is used to access the secured GIS services from the GIS Server.",
            "rdfs:label": "gisAccessToken",
            "rdfs:isDefinedBy": {
                "@id": "iudx:"
            },
            "iudx:domainIncludes": [
                {
                    "@id": "iudx:GISData"
                }
            ],
            "iudx:rangeIncludes": [
                {
                    "@id": "iudx:Text"
                },
                {
                    "@id": "iudx:ValueDescriptor"
                }
            ]
        },
        {
            "@id": "iudx:gisLayers",
            "@type": [
                "iudx:TextProperty"
            ],
            "rdfs:comment": "The GIS data layers stored in the GIS Server corresponding to this observation.",
            "rdfs:label": "gisLayers",
            "rdfs:isDefinedBy": {
                "@id": "iudx:"
            },
            "iudx:domainIncludes": [
                {
                    "@id": "iudx:GISData"
                }
            ],
            "iudx:rangeIncludes": [
                {
                    "@container": "@list",
                    "@id": "iudx:Text"
                }
            ]
        },
        {
            "@id": "iudx:gisServerURL",
            "@type": [
                "iudx:TextProperty"
            ],
            "rdfs:comment": "The Geographic Information System (GIS) Server's URL, used\u00a0for capturing, storing, and displaying data on positions on the earth's surface.",
            "rdfs:label": "gisServerURL",
            "rdfs:isDefinedBy": {
                "@id": "iudx:"
            },
            "iudx:domainIncludes": [
                {
                    "@id": "iudx:GISData"
                }
            ],
            "iudx:rangeIncludes": [
                {
                    "@id": "iudx:Text"
                },
                {
                    "@id": "iudx:ValueDescriptor"
                }
            ]
        },
        {
            "@id": "iudx:hasObject",
            "@type": [
                "iudx:TextProperty"
            ],
            "rdfs:comment": "Value associated with RelationshipValue class. Contains IRI(s) that specify the relationship object(s).",
            "rdfs:label": "hasObject",
            "iudx:domainIncludes": [
                {
                    "@id": "iudx:RelationshipValue"
                }
            ],
            "iudx:rangeIncludes": [
                {
                    "@id": "iudx:Text",
                    "@type": "@id"
                },
                {
                    "@id": "iudx:Text",
                    "@type": "@id",
                    "@container": "@set"
                },
                {
                    "@id": "iudx:ValueDescriptor"
                }
            ]
        },
        {
            "@id": "iudx:hq",
            "@type": [
                "iudx:TextProperty"
            ],
            "rdfs:comment": "Name of the headquarters corresponding to this observation.",
            "rdfs:label": "hq",
            "rdfs:isDefinedBy": {
                "@id": "iudx:"
            },
            "iudx:domainIncludes": [
                {
                    "@id": "iudx:Headquarters"
                }
            ],
            "iudx:rangeIncludes": [
                {
                    "@id": "iudx:Text"
                },
                {
                    "@id": "iudx:ValueDescriptor"
                }
            ]
        },
        {
            "@id": "iudx:id",
            "@type": [
                "iudx:TextProperty"
            ],
            "rdfs:comment": "ID of the entity.",
            "rdfs:label": "id",
            "iudx:domainIncludes": [
                {
                    "@id": "iudx:IUDXEntity",
                    "iudx:requiredProperty": true
                }
            ],
            "iudx:rangeIncludes": [
                {
                    "@id": "iudx:Text"
                }
            ],
            "rdfs:isDefinedBy": {
                "@id": "iudx:"
            }
        },
        {
            "@id": "iudx:ignitionStatus",
            "@type": [
                "iudx:TextProperty"
            ],
            "rdfs:comment": "Gives the ignition status of the vehicle.ENUM: [Y, N]",
            "rdfs:label": "ignitionStatus",
            "rdfs:isDefinedBy": {
                "@id": "iudx:"
            },
            "iudx:domainIncludes": [
                {
                    "@id": "iudx:WmgmtVehicle"
                },
                {
                    "@id": "iudx:EmergencyVehicle"
                }
            ],
            "iudx:rangeIncludes": [
                {
                    "@id": "iudx:Text"
                },
                {
                    "@id": "iudx:ValueDescriptor"
                }
            ]
        },
        {
            "@id": "iudx:imageFormat",
            "@type": [
                "iudx:TextProperty"
            ],
            "rdfs:comment": "The format of the image corresponding this observation. It can take up values like png, jpg, etc",
            "rdfs:label": "imageFormat",
            "rdfs:isDefinedBy": {
                "@id": "iudx:"
            },
            "iudx:domainIncludes": [
                {
                    "@id": "iudx:MapTiles"
                }
            ],
            "iudx:rangeIncludes": [
                {
                    "@id": "iudx:Text"
                },
                {
                    "@id": "iudx:ValueDescriptor"
                }
            ]
        },
        {
            "@id": "iudx:imageSnapshot",
            "@type": [
                "iudx:TextProperty"
            ],
            "rdfs:comment": "Camera feed snapshot download link for the camera corresponding to this observation",
            "rdfs:label": "imageSnapshot",
            "rdfs:isDefinedBy": {
                "@id": "iudx:"
            },
            "iudx:domainIncludes": [
                {
                    "@id": "iudx:Camera"
                }
            ],
            "iudx:rangeIncludes": [
                {
                    "@id": "iudx:Text"
                },
                {
                    "@id": "iudx:ValueDescriptor"
                }
            ]
        },
        {
            "@id": "iudx:isRelatedTo",
            "@type": [
                "iudx:TextProperty"
            ],
            "rdfs:comment": "Value associated with RelationshipValue class. Contains IRI(s) that specify the relationship object(s).",
            "rdfs:label": "isRelatedTo",
            "iudx:domainIncludes": [
                {
                    "@id": "iudx:RelationshipValue"
                }
            ],
            "iudx:rangeIncludes": [
                {
                    "@id": "iudx:Text",
                    "@type": "@id"
                },
                {
                    "@id": "iudx:Text",
                    "@type": "@id",
                    "@container": "@set"
                },
                {
                    "@id": "iudx:ValueDescriptor"
                }
            ]
        },
        {
            "@id": "iudx:itemStatus",
            "@type": [
                "iudx:TextProperty"
            ],
            "rdfs:comment": "Status of a catalouge item. ENUM: [ACTIVE, DEPRECATED].",
            "rdfs:label": "itemStatus",
            "iudx:domainIncludes": [
                {
                    "@id": "iudx:IUDXEntity"
                }
            ],
            "iudx:rangeIncludes": [
                {
                    "@id": "iudx:Text"
                }
            ],
            "rdfs:isDefinedBy": {
                "@id": "iudx:"
            }
        },
        {
            "@id": "iudx:iudxResourceAPIs",
            "@type": [
                "iudx:TextProperty"
            ],
            "rdfs:comment": "The set of IUDX resource APIs supported by a given ResourceGroup. ENUM: [TEMPORAL, SPATIAL, ATTR, TEXT]",
            "rdfs:label": "iudxResourceAPIs",
            "iudx:domainIncludes": [
                {
                    "@id": "iudx:ResourceGroup",
                    "iudx:requiredProperty": true
                },
                {
                    "@id": "iudx:Resource"
                }
            ],
            "iudx:rangeIncludes": [
                {
                    "@id": "iudx:Text",
                    "@container": "@set"
                }
            ],
            "rdfs:isDefinedBy": {
                "@id": "iudx:"
            }
        },
        {
            "@id": "iudx:junctionID",
            "@type": [
                "iudx:TextProperty"
            ],
            "rdfs:comment": "Unique representation of the junction corresponding to this observation.",
            "rdfs:label": "junctionID",
            "rdfs:isDefinedBy": {
                "@id": "iudx:"
            },
            "iudx:domainIncludes": [
                {
                    "@id": "iudx:RoadSegment"
                }
            ],
            "iudx:rangeIncludes": [
                {
                    "@id": "iudx:Text"
                },
                {
                    "@id": "iudx:ValueDescriptor"
                }
            ]
        },
        {
            "@id": "iudx:junctionMode",
            "@type": [
                "iudx:TextProperty"
            ],
            "rdfs:comment": "The mode of operation of the traffic junction corresponding to this observation. For eg, Blinker, Flash, ATCS, etc.",
            "rdfs:label": "junctionMode",
            "rdfs:isDefinedBy": {
                "@id": "iudx:"
            },
            "iudx:domainIncludes": [
                {
                    "@id": "iudx:RoadSegment"
                }
            ],
            "iudx:rangeIncludes": [
                {
                    "@id": "iudx:Text"
                },
                {
                    "@id": "iudx:ValueDescriptor"
                }
            ]
        },
        {
            "@id": "iudx:junctionName",
            "@type": [
                "iudx:TextProperty"
            ],
            "rdfs:comment": "The name of the road junction corresponding to this observation",
            "rdfs:label": "junctionName",
            "rdfs:isDefinedBy": {
                "@id": "iudx:"
            },
            "iudx:domainIncludes": [
                {
                    "@id": "iudx:RoadSegment"
                }
            ],
            "iudx:rangeIncludes": [
                {
                    "@id": "iudx:Text"
                },
                {
                    "@id": "iudx:ValueDescriptor"
                }
            ]
        },
        {
            "@id": "iudx:label",
            "@type": [
                "iudx:TextProperty"
            ],
            "rdfs:comment": "Human readable label for an entity",
            "rdfs:label": "label",
            "iudx:domainIncludes": [
                {
                    "@id": "iudx:IUDXEntity"
                }
            ],
            "iudx:rangeIncludes": [
                {
                    "@id": "iudx:Text"
                }
            ],
            "rdfs:isDefinedBy": {
                "@id": "iudx:"
            }
        },
        {
            "@id": "iudx:landfillSite",
            "@type": [
                "iudx:TextProperty"
            ],
            "rdfs:comment": "The name of the landfill site or dump yard or dumping station corresponding this observation.",
            "rdfs:label": "landfillSite",
            "rdfs:isDefinedBy": {
                "@id": "iudx:"
            },
            "iudx:domainIncludes": [
                {
                    "@id": "iudx:WmgmtVehicle"
                }
            ],
            "iudx:rangeIncludes": [
                {
                    "@id": "iudx:Text"
                },
                {
                    "@id": "iudx:ValueDescriptor"
                }
            ]
        },
        {
            "@id": "iudx:landmark",
            "@type": [
                "iudx:GeoProperty"
            ],
            "rdfs:comment": "A physical distinguishing feature on land that marks a locality or a place.",
            "rdfs:label": "landmark",
            "iudx:domainIncludes": [
                {
                    "@id": "iudx:IssueReporting"
                }
            ],
            "iudx:rangeIncludes": [
                {
                    "@id": "iudx:Text"
                },
                {
                    "@id": "iudx:ValueDescriptor"
                }
            ],
            "rdfs:isDefinedBy": {
                "@id": "iudx:"
            }
        },
        {
            "@id": "iudx:laneDirection",
            "@type": [
                "iudx:TextProperty"
            ],
            "rdfs:comment": "Describes the direction in which vehicles are plying on the lane corresponding to this observation. ENUM [FORWARD, BACKWARD, INBOUND, OUTBOUND, RIGHT, LEFT]",
            "rdfs:label": "laneDirection",
            "rdfs:isDefinedBy": {
                "@id": "iudx:"
            },
            "iudx:domainIncludes": [
                {
                    "@id": "iudx:LaneDesc"
                }
            ],
            "iudx:rangeIncludes": [
                {
                    "@id": "iudx:Text"
                },
                {
                    "@id": "iudx:ValueDescriptor"
                }
            ],
            "skos:exactMatch": {
                "@id": "Fiware:laneDirection"
            }
        },
        {
            "@id": "iudx:last_stop_arrival_time",
            "@type": [
                "iudx:TimeProperty"
            ],
            "rdfs:comment": "Specifies the arrival time at the previous stop for a specific trip on a route. Times must be eight digits in HH:MM:SS format (H:MM:SS is also accepted, if the hour begins with 0). \nNote: Trips that span multiple dates will have stop times greater than 24:00:00. For example, if a trip begins at 10:30:00 p.m. and ends at 2:15:00 a.m. on the following day, the stop times would be 22:30:00 and 26:15:00. Entering those stop times as 22:30:00 and 02:15:00 would not produce the desired results. This is SameAs: absolute 'time'(StopTimeEvent) in the 'arrival' field of the stop_time_update (StopTimeUpdate) message of the GTFS Realtime message-TripUpdate (https://developers.google.com/transit/gtfs-realtime/reference#message-tripupdate)",
            "rdfs:label": "last_stop_arrival_time",
            "rdfs:isDefinedBy": {
                "@id": "iudx:"
            },
            "iudx:domainIncludes": [
                {
                    "@id": "iudx:TransitManagement"
                }
            ],
            "iudx:rangeIncludes": [
                {
                    "@id": "iudx:Text"
                },
                {
                    "@id": "iudx:ValueDescriptor"
                }
            ]
        },
        {
            "@id": "iudx:last_stop_departure_time",
            "@type": [
                "iudx:TimeProperty"
            ],
            "rdfs:comment": "Specifies the departure time from the previous stop for a specific trip on a route. Times must be eight digits in HH:MM:SS format (H:MM:SS is also accepted, if the hour begins with 0). \nNote: Trips that span multiple dates will have stop times greater than 24:00:00. For example, if a trip begins at 10:30:00 p.m. and ends at 2:15:00 a.m. on the following day, the stop times would be 22:30:00 and 26:15:00. Entering those stop times as 22:30:00 and 02:15:00 would not produce the desired results. This is SameAs: absolute 'time'(StopTimeEvent) in the 'departure' field of the stop_time_update (StopTimeUpdate) message of the GTFS Realtime message-TripUpdate (https://developers.google.com/transit/gtfs-realtime/reference#message-tripupdate)",
            "rdfs:label": "last_stop_departure_time",
            "rdfs:isDefinedBy": {
                "@id": "iudx:"
            },
            "iudx:domainIncludes": [
                {
                    "@id": "iudx:TransitManagement"
                }
            ],
            "iudx:rangeIncludes": [
                {
                    "@id": "iudx:Text"
                },
                {
                    "@id": "iudx:ValueDescriptor"
                }
            ]
        },
        {
            "@id": "iudx:last_stop_id",
            "@type": [
                "iudx:TextProperty"
            ],
            "rdfs:comment": "Stop ID/Stop name of the previous bus stop corresponding to the bus in this observation. SameAs: 'stop_id' field from GTFS Realtime message-VehiclePosition (https://developers.google.com/transit/gtfs-realtime/reference#message-vehicleposition)",
            "rdfs:label": "last_stop_id",
            "rdfs:isDefinedBy": {
                "@id": "iudx:"
            },
            "iudx:domainIncludes": [
                {
                    "@id": "iudx:TransitManagement"
                }
            ],
            "iudx:rangeIncludes": [
                {
                    "@id": "iudx:Text"
                },
                {
                    "@id": "iudx:ValueDescriptor"
                }
            ]
        },
        {
            "@id": "iudx:latitude",
            "@type": [
                "iudx:GeoProperty"
            ],
            "rdfs:comment": "Latitude of a place. Specified in WGS 84 CRS (https://en.wikipedia.org/wiki/World_Geodetic_System)",
            "rdfs:label": "latitude",
            "iudx:domainIncludes": [
                {
                    "@id": "iudx:GeoCoordinates"
                },
                {
                    "@id": "iudx:Place"
                }
            ],
            "iudx:rangeIncludes": [
                {
                    "@id": "iudx:Number"
                },
                {
                    "@id": "iudx:Text"
                }
            ],
            "skos:exactMatch": {
                "@id": "schema:latitude"
            },
            "rdfs:isDefinedBy": {
                "@id": "iudx:"
            }
        },
        {
            "@id": "iudx:licenseExpiryDate",
            "@type": [
                "iudx:TimeProperty"
            ],
            "rdfs:comment": "License number expiry date for the business establishment corresponding to this observation.",
            "rdfs:label": "licenseExpiryDate",
            "rdfs:isDefinedBy": {
                "@id": "iudx:"
            },
            "iudx:domainIncludes": [
                {
                    "@id": "iudx:RevenueCollection"
                }
            ],
            "iudx:rangeIncludes": [
                {
                    "@id": "iudx:Text"
                },
                {
                    "@id": "iudx:ValueDescriptor"
                }
            ]
        },
        {
            "@id": "iudx:licenseIssualDate",
            "@type": [
                "iudx:TimeProperty"
            ],
            "rdfs:comment": "Date of issual of license for the entity or service corresponding to this observation.",
            "rdfs:label": "licenseIssualDate",
            "rdfs:isDefinedBy": {
                "@id": "iudx:"
            },
            "iudx:domainIncludes": [
                {
                    "@id": "iudx:RevenueCollection"
                }
            ],
            "iudx:rangeIncludes": [
                {
                    "@id": "iudx:Text"
                },
                {
                    "@id": "iudx:ValueDescriptor"
                }
            ]
        },
        {
            "@id": "iudx:license_plate",
            "@type": [
                "iudx:TextProperty"
            ],
            "rdfs:comment": "Gives the License Plate number of the vehice. SameAs: 'license_plate' field from GTFS Realtime message-VehicleDescriptor (https://developers.google.com/transit/gtfs-realtime/reference#message-vehicledescriptor)",
            "rdfs:label": "license_plate",
            "rdfs:isDefinedBy": {
                "@id": "iudx:"
            },
            "iudx:domainIncludes": [
                {
                    "@id": "iudx:WmgmtBin"
                },
                {
                    "@id": "iudx:WmgmtVehicle"
                },
                {
                    "@id": "iudx:VehicleDescriptor"
                },
                {
                    "@id": "iudx:EmergencyVehicle"
                }
            ],
            "iudx:rangeIncludes": [
                {
                    "@id": "iudx:Text"
                },
                {
                    "@id": "iudx:ValueDescriptor"
                }
            ],
            "skos:exactMatch": {
                "@id": "GTFS: license_plate"
            }
        },
        {
            "@id": "iudx:location",
            "@type": [
                "iudx:GeoProperty"
            ],
            "rdfs:comment": "Location associated with a resource Item (a spatial point), a group of resource items (a spatial region) or even an observation in case of a mobile sensor.",
            "rdfs:label": "location",
            "iudx:domainIncludes": [
                {
                    "@id": "iudx:Resource"
                },
                {
                    "@id": "iudx:ResourceGroup"
                },
                {
                    "@id": "iudx:Provider"
                },
                {
                    "@id": "iudx:ResourceServer"
                },
                {
                    "@id": "iudx:Organization"
                },
                {
                    "@id": "iudx:EnvAQM"
                },
                {
                    "@id": "iudx:EnvFlood"
                },
                {
                    "@id": "iudx:StreetLightFeeder"
                },
                {
                    "@id": "iudx:WmgmtBin"
                },
                {
                    "@id": "iudx:TransitManagement"
                },
                {
                    "@id": "iudx:PointOfInterest"
                },
                {
                    "@id": "iudx:SafetiPin"
                },
                {
                    "@id": "iudx:IssueReporting"
                },
                {
                    "@id": "iudx:TrafficViolations"
                },
                {
                    "@id": "iudx:Streetlight"
                },
                {
                    "@id": "iudx:BikeDockingStation"
                },
                {
                    "@id": "iudx:WaterDistributionNetwork"
                },
                {
                    "@id": "iudx:Camera"
                },
                {
                    "@id": "iudx:WasteWaterMgmt"
                },
                {
                    "@id": "iudx:SmartParking"
                },
                {
                    "@id": "iudx:EmergencyVehicle"
                },
                {
                    "@id": "iudx:SolarEnergy"
                },
                {
                    "@id": "iudx:LaneDesc"
                },
                {
                    "@id": "iudx:EVChargingStation"
                },
                {
                    "@id": "iudx:MosquitoDensity"
                },
                {
                    "@id": "iudx:WmgmtVehicle"
                },
                {
                    "@id": "iudx:TouristDestination"
                },
                {
                    "@id": "iudx:AirQuality"
                }
            ],
            "iudx:rangeIncludes": [
                {
                    "@id": "iudx:Point"
                },
                {
                    "@id": "iudx:GeoJSONGeometry"
                },
                {
                    "@id": "iudx:Place"
                },
                {
                    "@id": "iudx:Text"
                },
                {
                    "@id": "iudx:ValueDescriptor"
                },
                {
                    "@id": "iudx:Geojsongeometry"
                }
            ],
            "rdfs:isDefinedBy": {
                "@id": "iudx:"
            },
            "skos:exactMatch": {
                "@id": "schema:location"
            }
        },
        {
            "@id": "iudx:longitude",
            "@type": [
                "iudx:GeoProperty"
            ],
            "rdfs:comment": "Longitude of a place. Specified in WGS 84 CRS (https://en.wikipedia.org/wiki/World_Geodetic_System)",
            "rdfs:label": "longitude",
            "iudx:domainIncludes": [
                {
                    "@id": "iudx:GeoCoordinates"
                },
                {
                    "@id": "iudx:Place"
                }
            ],
            "iudx:rangeIncludes": [
                {
                    "@id": "iudx:Number"
                },
                {
                    "@id": "iudx:Text"
                }
            ],
            "skos:exactMatch": {
                "@id": "schema:longitude"
            },
            "rdfs:isDefinedBy": {
                "@id": "iudx:"
            }
        },
        {
            "@id": "iudx:macAddress",
            "@type": [
                "iudx:TextProperty"
            ],
            "rdfs:comment": "The Media Access Control address which is a 12-digit hexadecimal number assigned to each device connected to the network",
            "rdfs:label": "macAddress",
            "rdfs:isDefinedBy": {
                "@id": "iudx:"
            },
            "iudx:domainIncludes": [
                {
                    "@id": "iudx:WirelessNetwork"
                }
            ],
            "iudx:rangeIncludes": [
                {
                    "@id": "iudx:Text"
                },
                {
                    "@id": "iudx:ValueDescriptor"
                }
            ]
        },
        {
            "@id": "iudx:malfunctionCode",
            "@type": [
                "iudx:TextProperty"
            ],
            "rdfs:comment": "Describes the error code/ malfunction code of the air conditioning system.",
            "rdfs:label": "malfunctionCode",
            "rdfs:isDefinedBy": {
                "@id": "iudx:"
            },
            "iudx:domainIncludes": [
                {
                    "@id": "iudx:AirConditioner"
                }
            ],
            "iudx:rangeIncludes": [
                {
                    "@id": "iudx:Text"
                },
                {
                    "@id": "iudx:ValueDescriptor"
                }
            ]
        },
        {
            "@id": "iudx:manufacturerName",
            "@type": [
                "iudx:TextProperty"
            ],
            "rdfs:comment": "Name of the manufacturer associated with an entity, e.g., sensor, device etc.",
            "rdfs:label": "manufacturerName",
            "rdfs:isDefinedBy": {
                "@id": "iudx:"
            },
            "iudx:domainIncludes": [
                {
                    "@id": "iudx:ModelInfo"
                }
            ],
            "iudx:rangeIncludes": [
                {
                    "@id": "iudx:Text"
                }
            ],
            "skos:exactMatch": {
                "@id": "Fiware:manufacturerName"
            }
        },
        {
            "@id": "iudx:measAccuracy",
            "@type": [
                "iudx:TextProperty"
            ],
            "rdfs:comment": "Accuracy of a measurement. Maximum difference that can exist between the actual value and the measured value. It can be specified in relative as well as absolute terms.",
            "rdfs:label": "measAccuracy",
            "iudx:domainIncludes": [
                {
                    "@id": "iudx:ValueDescriptor"
                }
            ],
            "iudx:rangeIncludes": [
                {
                    "@id": "iudx:Text"
                },
                {
                    "@id": "iudx:ValueDescriptor"
                }
            ],
            "rdfs:isDefinedBy": {
                "@id": "iudx:"
            }
        },
        {
            "@id": "iudx:measurand",
            "@type": [
                "iudx:TextProperty"
            ],
            "rdfs:comment": "Property/properties sensed/observed/measured by the device.",
            "rdfs:label": "measurand",
            "rdfs:isDefinedBy": {
                "@id": "iudx:"
            },
            "iudx:domainIncludes": [
                {
                    "@id": "iudx:Device"
                }
            ],
            "iudx:rangeIncludes": [
                {
                    "@id": "iudx:Text"
                }
            ]
        },
        {
            "@id": "iudx:mediaURL",
            "@type": [
                "iudx:TextProperty"
            ],
            "rdfs:comment": "URL providing further information of any image(s) or media of the complaint or place.",
            "rdfs:label": "mediaURL",
            "iudx:domainIncludes": [
                {
                    "@id": "iudx:SafetiPin"
                },
                {
                    "@id": "iudx:IssueReporting"
                },
                {
                    "@id": "iudx:TrafficViolations"
                },
                {
                    "@id": "iudx:BikeDockingStation"
                },
                {
                    "@id": "iudx:Camera"
                },
                {
                    "@id": "iudx:TouristDestination"
                }
            ],
            "iudx:rangeIncludes": [
                {
                    "@container": "@list",
                    "@id": "iudx:Text"
                },
                {
                    "@id": "iudx:ValueDescriptor"
                }
            ],
            "rdfs:isDefinedBy": {
                "@id": "iudx:"
            },
            "skos:exactMatch": {
                "@id": "open311:media_url"
            }
        },
        {
            "@id": "iudx:modelName",
            "@type": [
                "iudx:TextProperty"
            ],
            "rdfs:comment": "Name of a specific model associated with an entity, e.g., sensor, device etc.",
            "rdfs:label": "modelName",
            "rdfs:isDefinedBy": {
                "@id": "iudx:"
            },
            "iudx:domainIncludes": [
                {
                    "@id": "iudx:ModelInfo"
                },
                {
                    "@id": "iudx:WmgmtVehicle"
                }
            ],
            "iudx:rangeIncludes": [
                {
                    "@id": "iudx:Text"
                }
            ],
            "skos:exactMatch": {
                "@id": "Fiware:modelName"
            }
        },
        {
            "@id": "iudx:modelURL",
            "@type": [
                "iudx:TextProperty"
            ],
            "rdfs:comment": "URL providing further information of a specific model associated with an entity, e.g., sensor, device etc.",
            "rdfs:label": "modelURL",
            "rdfs:isDefinedBy": {
                "@id": "iudx:"
            },
            "iudx:domainIncludes": [
                {
                    "@id": "iudx:ModelInfo"
                }
            ],
            "iudx:rangeIncludes": [
                {
                    "@id": "iudx:Text"
                }
            ]
        },
        {
            "@id": "iudx:name",
            "@type": [
                "iudx:TextProperty"
            ],
            "rdfs:comment": "Name of the entity.",
            "rdfs:label": "name",
            "iudx:domainIncludes": [
                {
                    "@id": "iudx:Place"
                },
                {
                    "@id": "iudx:Organization"
                },
                {
                    "@id": "iudx:RelationshipValue"
                },
                {
                    "@id": "iudx:IUDXEntity",
                    "iudx:requiredProperty": true
                },
                {
                    "@id": "iudx:PointOfInterest"
                },
                {
                    "@id": "iudx:BikeDockingStation"
                },
                {
                    "@id": "iudx:TouristDestination"
                }
            ],
            "iudx:rangeIncludes": [
                {
                    "@id": "iudx:Text"
                },
                {
                    "@id": "iudx:ValueDescriptor"
                }
            ],
            "skos:exactMatch": {
                "@id": "schema:name"
            },
            "rdfs:isDefinedBy": {
                "@id": "iudx:"
            }
        },
        {
            "@id": "iudx:name_of_town",
            "@type": [
                "iudx:TextProperty"
            ],
            "rdfs:comment": "Name of the town corresponding to this observation.",
            "rdfs:label": "name_of_town",
            "rdfs:isDefinedBy": {
                "@id": "iudx:"
            },
            "iudx:domainIncludes": [
                {
                    "@id": "iudx:MajorTowns"
                }
            ],
            "iudx:rangeIncludes": [
                {
                    "@id": "iudx:Text"
                },
                {
                    "@id": "iudx:ValueDescriptor"
                }
            ]
        },
        {
            "@id": "iudx:occupancyLevel",
            "@type": [
                "iudx:TextProperty"
            ],
            "rdfs:comment": "Occupancy level in the public transit bus corresponding to this observation. 'Red' indicates the congestion level in the bus is HIGH, 'Yellow' indicates the congestion level in the bus is MODERATE and 'Green' indicates the congestion level in the bus is LOW.",
            "rdfs:label": "occupancyLevel",
            "rdfs:isDefinedBy": {
                "@id": "iudx:"
            },
            "iudx:domainIncludes": [
                {
                    "@id": "iudx:FareCollectionSystem"
                }
            ],
            "iudx:rangeIncludes": [
                {
                    "@id": "iudx:Text"
                },
                {
                    "@id": "iudx:ValueDescriptor"
                }
            ]
        },
        {
            "@id": "iudx:occupancy_status",
            "@type": [
                "iudx:TextProperty"
            ],
            "rdfs:comment": "The degree of passenger occupancy for the vehicle. ENUM [EMPTY,  MANY_SEATS_AVAILABLE, FEW_SEATS_AVAILABLE, STANDING_ROOM_ONLY, CRUSHED_STANDING_ROOM_ONLY, FULL,  NOT_ACCEPTING_PASSENGERS, NO_DATA_AVAILABLE, NOT_BOARDABLE]",
            "rdfs:label": "occupancy_status",
            "rdfs:isDefinedBy": {
                "@id": "iudx:"
            },
            "iudx:domainIncludes": [
                {
                    "@id": "iudx:VehiclePosition"
                }
            ],
            "iudx:rangeIncludes": [
                {
                    "@id": "iudx:Text"
                },
                {
                    "@id": "iudx:ValueDescriptor"
                }
            ],
            "skos:exactMatch": {
                "@id": "GTFS: occupancy_status"
            }
        },
        {
            "@id": "iudx:openDataFields",
            "@type": [
                "iudx:TextProperty"
            ],
            "rdfs:comment": "List of properties/fields/attributes contained in the data available from the resources associated with a given resource Group which are open, i.e., no authorization is required to access these fields for a given resource.",
            "rdfs:label": "openDataFields",
            "iudx:domainIncludes": [
                {
                    "@id": "iudx:DataFieldListValue"
                }
            ],
            "iudx:rangeIncludes": [
                {
                    "@id": "iudx:Text",
                    "@container": "@set"
                }
            ]
        },
        {
            "@id": "iudx:openHours",
            "@type": [
                "iudx:TextProperty"
            ],
            "rdfs:comment": "The time period or hours between which the entity or service is open or operational.",
            "rdfs:label": "openHours",
            "iudx:domainIncludes": [
                {
                    "@id": "iudx:PointOfInterest"
                },
                {
                    "@id": "iudx:TouristDestination"
                }
            ],
            "iudx:rangeIncludes": [
                {
                    "@id": "iudx:Text"
                },
                {
                    "@id": "iudx:ValueDescriptor"
                }
            ],
            "skos:exactMatch": {
                "@id": "Fiware:Building.openingHours"
            },
            "rdfs:isDefinedBy": {
                "@id": "iudx:"
            }
        },
        {
            "@id": "iudx:originDestinationCode",
            "@type": [
                "iudx:TextProperty"
            ],
            "rdfs:comment": "The code for the origin and destination stops corresponding to this observation.",
            "rdfs:label": "originDestinationCode",
            "rdfs:isDefinedBy": {
                "@id": "iudx:"
            },
            "iudx:domainIncludes": [
                {
                    "@id": "iudx:FareCollectionSystem"
                }
            ],
            "iudx:rangeIncludes": [
                {
                    "@id": "iudx:Text"
                },
                {
                    "@id": "iudx:ValueDescriptor"
                }
            ]
        },
        {
            "@id": "iudx:originStopCategory",
            "@type": [
                "iudx:TextProperty"
            ],
            "rdfs:comment": "Type of the origin bus stop corresponding to this observation.",
            "rdfs:label": "originStopCategory",
            "rdfs:isDefinedBy": {
                "@id": "iudx:"
            },
            "iudx:domainIncludes": [
                {
                    "@id": "iudx:FareCollectionSystem"
                }
            ],
            "iudx:rangeIncludes": [
                {
                    "@id": "iudx:Text"
                },
                {
                    "@id": "iudx:ValueDescriptor"
                }
            ]
        },
        {
            "@id": "iudx:originStopID",
            "@type": [
                "iudx:TextProperty"
            ],
            "rdfs:comment": "Unique ID of the bus stop at which the passenger boards into the bus corresponding to this observation.",
            "rdfs:label": "originStopID",
            "rdfs:isDefinedBy": {
                "@id": "iudx:"
            },
            "iudx:domainIncludes": [
                {
                    "@id": "iudx:FareCollectionSystem"
                }
            ],
            "iudx:rangeIncludes": [
                {
                    "@id": "iudx:Text"
                },
                {
                    "@id": "iudx:ValueDescriptor"
                }
            ]
        },
        {
            "@id": "iudx:originStopName",
            "@type": [
                "iudx:TextProperty"
            ],
            "rdfs:comment": "The name of the origin bus stop corresponding to this observation.",
            "rdfs:label": "originStopName",
            "rdfs:isDefinedBy": {
                "@id": "iudx:"
            },
            "iudx:domainIncludes": [
                {
                    "@id": "iudx:FareCollectionSystem"
                }
            ],
            "iudx:rangeIncludes": [
                {
                    "@id": "iudx:Text"
                },
                {
                    "@id": "iudx:ValueDescriptor"
                }
            ]
        },
        {
            "@id": "iudx:owner",
            "@type": [
                "iudx:Relationship"
            ],
            "rdfs:comment": "UUID of owner entity associated with the given catalogue item.",
            "rdfs:label": "owner",
            "iudx:domainIncludes": [
                {
                    "@id": "iudx:ResourceServer",
                    "iudx:requiredProperty": true
                },
                {
                    "@id": "iudx:COS",
                    "iudx:requiredProperty": true
                }
            ],
            "iudx:rangeIncludes": [
                {
                    "@id": "iudx:Text",
                    "@type": "@id"
                },
                {
                    "@id": "iudx:RelationshipValue"
                }
            ]
        },
        {
            "@id": "iudx:parkingMode",
            "@type": [
                "iudx:TextProperty"
            ],
            "rdfs:comment": "Parking mode followed in the parking site corresponding to this observation.  ENUM [PARALLEL_PARKING, PERPENDICULAR_PARKING, ANGLE_PARKING].",
            "rdfs:label": "parkingMode",
            "rdfs:isDefinedBy": {
                "@id": "iudx:"
            },
            "iudx:domainIncludes": [
                {
                    "@id": "iudx:SmartParking"
                }
            ],
            "iudx:rangeIncludes": [
                {
                    "@id": "iudx:Text"
                },
                {
                    "@id": "iudx:ValueDescriptor"
                }
            ],
            "skos:exactMatch": {
                "@id": "Fiware: OffStreetParking.parkingMode"
            }
        },
        {
            "@id": "iudx:parkingSiteID",
            "@type": [
                "iudx:TextProperty"
            ],
            "rdfs:comment": "The unique ID of the parking site or parking lot corresponding to this observation.",
            "rdfs:label": "parkingSiteID",
            "rdfs:isDefinedBy": {
                "@id": "iudx:"
            },
            "iudx:domainIncludes": [
                {
                    "@id": "iudx:SmartParking"
                }
            ],
            "iudx:rangeIncludes": [
                {
                    "@id": "iudx:Text"
                },
                {
                    "@id": "iudx:ValueDescriptor"
                }
            ]
        },
        {
            "@id": "iudx:parkingSiteName",
            "@type": [
                "iudx:TextProperty"
            ],
            "rdfs:comment": "Name of the parking site or parking lot corresponding to this observation.",
            "rdfs:label": "parkingSiteName",
            "rdfs:isDefinedBy": {
                "@id": "iudx:"
            },
            "iudx:domainIncludes": [
                {
                    "@id": "iudx:SmartParking"
                }
            ],
            "iudx:rangeIncludes": [
                {
                    "@id": "iudx:Text"
                },
                {
                    "@id": "iudx:ValueDescriptor"
                }
            ]
        },
        {
            "@id": "iudx:paymentStatus",
            "@type": [
                "iudx:TextProperty"
            ],
            "rdfs:comment": "The payment status of the fine or violation or challan corresponding to this observation. ENUM[\"Paid\", \"Unpaid\"].",
            "rdfs:label": "paymentStatus",
            "rdfs:isDefinedBy": {
                "@id": "iudx:"
            },
            "iudx:domainIncludes": [
                {
                    "@id": "iudx:TrafficViolations"
                }
            ],
            "iudx:rangeIncludes": [
                {
                    "@id": "iudx:Text"
                },
                {
                    "@id": "iudx:ValueDescriptor"
                }
            ]
        },
        {
            "@id": "iudx:pedestrianPathMaterial",
            "@type": [
                "iudx:TextProperty"
            ],
            "rdfs:comment": "Construction material used for laying the walkway / footpath on the sides of the road corresponding to this observation.",
            "rdfs:label": "pedestrianPathMaterial",
            "rdfs:isDefinedBy": {
                "@id": "iudx:"
            },
            "iudx:domainIncludes": [
                {
                    "@id": "iudx:RoadSegment"
                }
            ],
            "iudx:rangeIncludes": [
                {
                    "@id": "iudx:Text"
                },
                {
                    "@id": "iudx:ValueDescriptor"
                }
            ]
        },
        {
            "@id": "iudx:pedestrianPathPlacement",
            "@type": [
                "iudx:TextProperty"
            ],
            "rdfs:comment": "Describes the presence and placement of pedestrian along the road segment corresponding to this observation. ENUM: [RIGHT, LEFT, BOTH, NOT_AVAILABLE]",
            "rdfs:label": "pedestrianPathPlacement",
            "rdfs:isDefinedBy": {
                "@id": "iudx:"
            },
            "iudx:domainIncludes": [
                {
                    "@id": "iudx:RoadSegment"
                }
            ],
            "iudx:rangeIncludes": [
                {
                    "@id": "iudx:Text"
                },
                {
                    "@id": "iudx:ValueDescriptor"
                }
            ]
        },
        {
            "@id": "iudx:pickup_type",
            "@type": [
                "iudx:TextProperty"
            ],
            "rdfs:comment": "Indicates pickup method.SameAs: 'pickup_type' field from GTFS Static Field definitions-stop_times.txt (https://developers.google.com/transit/gtfs/reference#stop_timestxt)",
            "rdfs:label": "pickup_type",
            "rdfs:isDefinedBy": {
                "@id": "iudx:"
            },
            "iudx:domainIncludes": [
                {
                    "@id": "iudx:StopTimesDesc"
                }
            ],
            "iudx:rangeIncludes": [
                {
                    "@id": "iudx:Text"
                },
                {
                    "@id": "iudx:ValueDescriptor"
                }
            ],
            "skos:exactMatch": {
                "@id": "GTFS: pickup_type"
            }
        },
        {
            "@id": "iudx:poiID",
            "@type": [
                "iudx:TextProperty"
            ],
            "rdfs:comment": "The ID of the waste collection region, which can be an aisle comprising of waste bin(s) or a larger dump yard.",
            "rdfs:label": "poiID",
            "rdfs:isDefinedBy": {
                "@id": "iudx:"
            },
            "iudx:domainIncludes": [
                {
                    "@id": "iudx:WmgmtVehicle"
                }
            ],
            "iudx:rangeIncludes": [
                {
                    "@id": "iudx:Text"
                },
                {
                    "@id": "iudx:ValueDescriptor"
                }
            ]
        },
        {
            "@id": "iudx:poiName",
            "@type": [
                "iudx:TextProperty"
            ],
            "rdfs:comment": "The name identifying the waste collection region, which can be an aisle comprising of waste bin(s) or a larger dump yard.",
            "rdfs:label": "poiName",
            "rdfs:isDefinedBy": {
                "@id": "iudx:"
            },
            "iudx:domainIncludes": [
                {
                    "@id": "iudx:WmgmtVehicle"
                }
            ],
            "iudx:rangeIncludes": [
                {
                    "@id": "iudx:Text"
                },
                {
                    "@id": "iudx:ValueDescriptor"
                }
            ]
        },
        {
            "@id": "iudx:poiType",
            "@type": [
                "iudx:TextProperty"
            ],
            "rdfs:comment": "The type of the waste collection point of interest corresponding to this observation. For eg., landfill, dumpyard, household etc.",
            "rdfs:label": "poiType",
            "rdfs:isDefinedBy": {
                "@id": "iudx:"
            },
            "iudx:domainIncludes": [
                {
                    "@id": "iudx:WmgmtVehicle"
                }
            ],
            "iudx:rangeIncludes": [
                {
                    "@id": "iudx:Text"
                },
                {
                    "@id": "iudx:ValueDescriptor"
                }
            ]
        },
        {
            "@id": "iudx:powerState",
            "@type": [
                "iudx:TextProperty"
            ],
            "rdfs:comment": "Indicates the current power status of the entity corresponding to this observation.",
            "rdfs:label": "powerState",
            "rdfs:isDefinedBy": {
                "@id": "iudx:"
            },
            "iudx:domainIncludes": [
                {
                    "@id": "iudx:StreetLightFeeder"
                },
                {
                    "@id": "iudx:Streetlight"
                }
            ],
            "iudx:rangeIncludes": [
                {
                    "@id": "iudx:Text"
                },
                {
                    "@id": "iudx:ValueDescriptor"
                }
            ],
            "skos:exactMatch": {
                "@id": "Fiware:powerState"
            }
        },
        {
            "@id": "iudx:protocol",
            "@type": [
                "iudx:TextProperty"
            ],
            "rdfs:comment": "The name of the network protocol used for data communication.",
            "rdfs:label": "protocol",
            "iudx:domainIncludes": [
                {
                    "@id": "iudx:HTTPAccess"
                },
                {
                    "@id": "iudx:FileAccess"
                },
                {
                    "@id": "iudx:StreamingAccess"
                }
            ],
            "iudx:rangeIncludes": [
                {
                    "@id": "iudx:Text"
                },
                {
                    "@id": "iudx:ValueDescriptor"
                }
            ],
            "rdfs:isDefinedBy": {
                "@id": "iudx:"
            }
        },
        {
            "@id": "iudx:provider",
            "@type": [
                "iudx:Relationship"
            ],
            "rdfs:comment": "UUID of the IRI pointing to the provider entity associated with the given catalogue item",
            "rdfs:label": "provider",
            "iudx:domainIncludes": [
                {
                    "@id": "iudx:Resource"
                },
                {
                    "@id": "iudx:ResourceGroup",
                    "iudx:requiredProperty": true
                }
            ],
            "iudx:rangeIncludes": [
                {
                    "@id": "iudx:Text",
                    "@type": "@id"
                },
                {
                    "@id": "iudx:RelationshipValue"
                }
            ]
        },
        {
            "@id": "iudx:relatedEntity",
            "@type": [
                "iudx:Relationship"
            ],
            "rdfs:comment": "ID of the associated entity.",
            "rdfs:label": "relatedEntity",
            "iudx:domainIncludes": [
                {
                    "@id": "iudx:IUDXEntity"
                }
            ],
            "iudx:rangeIncludes": [
                {
                    "@id": "iudx:Text"
                },
                {
                    "@id": "iudx:RelationshipValue"
                }
            ],
            "rdfs:isDefinedBy": {
                "@id": "iudx:"
            }
        },
        {
            "@id": "iudx:relationType",
            "@type": [
                "iudx:TextProperty"
            ],
            "rdfs:comment": "Type of relation. ENUM: [REL_MESSAGESTREAM, REL_FILE, REL_DATASET, REL_THING].",
            "rdfs:label": "relationType",
            "iudx:domainIncludes": [
                {
                    "@id": "iudx:RelationshipValue",
                    "iudx:requiredProperty": true
                }
            ],
            "iudx:rangeIncludes": [
                {
                    "@id": "iudx:Text"
                },
                {
                    "@id": "iudx:ValueDescriptor"
                }
            ],
            "rdfs:isDefinedBy": {
                "@id": "iudx:"
            }
        },
        {
            "@id": "iudx:remarks",
            "@type": [
                "iudx:TextProperty"
            ],
            "rdfs:comment": "Remarks or additional information of the entity corresponding to this observation",
            "rdfs:label": "remarks",
            "rdfs:isDefinedBy": {
                "@id": "iudx:"
            },
            "iudx:domainIncludes": [
                {
                    "@id": "iudx:District"
                }
            ],
            "iudx:rangeIncludes": [
                {
                    "@id": "iudx:Text"
                },
                {
                    "@id": "iudx:ValueDescriptor"
                }
            ]
        },
        {
            "@id": "iudx:reportID",
            "@type": [
                "iudx:TextProperty"
            ],
            "rdfs:comment": "Unique ID assigned for the issue or report or feedback or transaction corresponding to this observation.",
            "rdfs:label": "reportID",
            "rdfs:isDefinedBy": {
                "@id": "iudx:"
            },
            "iudx:domainIncludes": [
                {
                    "@id": "iudx:IssueReporting"
                },
                {
                    "@id": "iudx:SafetiPin"
                },
                {
                    "@id": "iudx:TrafficViolations"
                },
                {
                    "@id": "iudx:WmgmtVehicle"
                }
            ],
            "iudx:rangeIncludes": [
                {
                    "@id": "iudx:Text"
                },
                {
                    "@id": "iudx:ValueDescriptor"
                }
            ],
            "skos:exactMatch": {
                "@id": "open311:servicecode"
            }
        },
        {
            "@id": "iudx:reportingMode",
            "@type": [
                "iudx:TextProperty"
            ],
            "rdfs:comment": "The communication channel or medium used to convey the issue or report or feedback or transaction corresponding to this observation. For eg., Email, SMS, Telephone etc.",
            "rdfs:label": "reportingMode",
            "rdfs:isDefinedBy": {
                "@id": "iudx:"
            },
            "iudx:domainIncludes": [
                {
                    "@id": "iudx:IssueReporting"
                }
            ],
            "iudx:rangeIncludes": [
                {
                    "@id": "iudx:Text"
                },
                {
                    "@id": "iudx:ValueDescriptor"
                }
            ]
        },
        {
            "@id": "iudx:repositoryURL",
            "@type": [
                "iudx:Relationship"
            ],
            "rdfs:comment": "A URL pointing to a repository containing additional resources or code pertaining to this entity.",
            "rdfs:label": "repositoryURL",
            "rdfs:isDefinedBy": {
                "@id": "iudx:"
            },
            "iudx:domainIncludes": [],
            "iudx:rangeIncludes": [
                {
                    "@id": "iudx:Text",
                    "@type": "@id"
                },
                {
                    "@id": "iudx:RelationshipValue"
                }
            ]
        },
        {
            "@id": "iudx:resolutionStatus",
            "@type": [
                "iudx:TextProperty"
            ],
            "rdfs:comment": "Status of the issue that was reported in terms of resolution or the actions taken on it. Could be Open, Assigned, InProgress, Unassigned, Resolved, Closed, Reopened.",
            "rdfs:label": "resolutionStatus",
            "rdfs:isDefinedBy": {
                "@id": "iudx:"
            },
            "iudx:domainIncludes": [
                {
                    "@id": "iudx:IssueReporting"
                }
            ],
            "iudx:rangeIncludes": [
                {
                    "@id": "iudx:Text"
                },
                {
                    "@id": "iudx:ValueDescriptor"
                }
            ]
        },
        {
            "@id": "iudx:resourceGroup",
            "@type": [
                "iudx:Relationship"
            ],
            "rdfs:comment": "UUID of the IRI pointing to the resourceGroup entity associated with the resource.",
            "rdfs:label": "resourceGroup",
            "iudx:domainIncludes": [
                {
                    "@id": "iudx:Resource",
                    "iudx:requiredProperty": true
                }
            ],
            "iudx:rangeIncludes": [
                {
                    "@id": "iudx:Text",
                    "@type": "@id"
                },
                {
                    "@id": "iudx:RelationshipValue"
                }
            ]
        },
        {
            "@id": "iudx:resourceServer",
            "@type": [
                "iudx:Relationship"
            ],
            "rdfs:comment": "IRI pointing to the ResourceServer entity for a given Resource or ResourceGroup.",
            "rdfs:label": "resourceServer",
            "iudx:domainIncludes": [
                {
                    "@id": "iudx:Resource",
                    "iudx:requiredProperty": true
                },
                {
                    "@id": "iudx:ResourceGroup"
                },
                {
                    "@id": "adex:Provider"
                }
            ],
            "iudx:rangeIncludes": [
                {
                    "@id": "iudx:Text",
                    "@type": "@id"
                },
                {
                    "@id": "iudx:RelationshipValue"
                }
            ]
        },
        {
            "@id": "iudx:resourceServerRegURL",
            "@type": [
                "iudx:Relationship"
            ],
            "rdfs:comment": "The registered URL for the Resource Server.",
            "rdfs:label": "resourceServerRegURL",
            "iudx:domainIncludes": [
                {
                    "@id": "iudx:ResourceServer",
                    "iudx:requiredProperty": true
                }
            ],
            "iudx:rangeIncludes": [
                {
                    "@id": "iudx:Text",
                    "@type": "@id"
                }
            ]
        },
        {
            "@id": "iudx:resourceType",
            "@type": [
                "iudx:TextProperty"
            ],
            "rdfs:comment": "Type of resource. ENUM: [MESSAGESTREAM, DATASET, FILE, GSLAYER, MEDIASTREAM].",
            "rdfs:label": "resourceType",
            "iudx:domainIncludes": [
                {
                    "@id": "iudx:ResourceGroup",
                    "iudx:requiredProperty": true
                },
                {
                    "@id": "iudx:Resource"
                }
            ],
            "iudx:rangeIncludes": [
                {
                    "@id": "iudx:Text"
                }
            ],
            "rdfs:isDefinedBy": {
                "@id": "iudx:"
            }
        },
        {
            "@id": "iudx:revenueCollectionType",
            "@type": [
                "iudx:TextProperty"
            ],
            "rdfs:comment": "Type of source from which the city administration collects the revenue, could be property tax, vehicle registration, party hall booking, community hall booking, auditorium booking etc.",
            "rdfs:label": "revenueCollectionType",
            "rdfs:isDefinedBy": {
                "@id": "iudx:"
            },
            "iudx:domainIncludes": [
                {
                    "@id": "iudx:RevenueCollection"
                }
            ],
            "iudx:rangeIncludes": [
                {
                    "@id": "iudx:Text"
                },
                {
                    "@id": "iudx:ValueDescriptor"
                }
            ]
        },
        {
            "@id": "iudx:revenueLicense",
            "@type": [
                "iudx:TextProperty"
            ],
            "rdfs:comment": "License number of the business establishment under which an individual as a sole proprietor or a company chooses to do business.",
            "rdfs:label": "revenueLicense",
            "rdfs:isDefinedBy": {
                "@id": "iudx:"
            },
            "iudx:domainIncludes": [
                {
                    "@id": "iudx:RevenueCollection"
                }
            ],
            "iudx:rangeIncludes": [
                {
                    "@id": "iudx:Text"
                },
                {
                    "@id": "iudx:ValueDescriptor"
                }
            ]
        },
        {
            "@id": "iudx:revenueLicenseStatus",
            "@type": [
                "iudx:TextProperty"
            ],
            "rdfs:comment": "Status of the license number of the business establishment under which an individual as a sole proprietor or a company chooses to do business.",
            "rdfs:label": "revenueLicenseStatus",
            "rdfs:isDefinedBy": {
                "@id": "iudx:"
            },
            "iudx:domainIncludes": [
                {
                    "@id": "iudx:RevenueCollection"
                }
            ],
            "iudx:rangeIncludes": [
                {
                    "@id": "iudx:Text"
                },
                {
                    "@id": "iudx:ValueDescriptor"
                }
            ]
        },
        {
            "@id": "iudx:rfID",
            "@type": [
                "iudx:TextProperty"
            ],
            "rdfs:comment": "Gives the ID of the RFID reader.",
            "rdfs:label": "rfID",
            "rdfs:isDefinedBy": {
                "@id": "iudx:"
            },
            "iudx:domainIncludes": [
                {
                    "@id": "iudx:Device"
                },
                {
                    "@id": "iudx:WmgmtBin"
                }
            ],
            "iudx:rangeIncludes": [
                {
                    "@id": "iudx:Text"
                },
                {
                    "@id": "iudx:ValueDescriptor"
                }
            ]
        },
        {
            "@id": "iudx:roadClass",
            "@type": [
                "iudx:TextProperty"
            ],
            "rdfs:comment": "The type of road corresponding to this observation. ENUM: [OTHER_PUBLIC_ROAD, PRIVATE_ROAD, MINOR_CITY_ROAD, MAJOR_DISTRICT_ROAD, MAJOR_CITY_ROAD, NATIONAL_HIGHWAY, SERVICE_ROAD, STATE_HIGHWAY, OTHER_DISTRICT_ROAD, PORT_ROAD].",
            "rdfs:label": "roadClass",
            "rdfs:isDefinedBy": {
                "@id": "iudx:"
            },
            "iudx:domainIncludes": [
                {
                    "@id": "iudx:RoadSegment"
                }
            ],
            "iudx:rangeIncludes": [
                {
                    "@id": "iudx:Text"
                },
                {
                    "@id": "iudx:ValueDescriptor"
                }
            ],
            "skos:exactMatch": {
                "@id": "Fiware: roadClass"
            }
        },
        {
            "@id": "iudx:roadDirection",
            "@type": [
                "iudx:TextProperty"
            ],
            "rdfs:comment": "Represents the direction the road is heading to. ENUM: [N, S, E, W]. The values N,S,E,W represent North,South,East,West respectively.",
            "rdfs:label": "roadDirection",
            "rdfs:isDefinedBy": {
                "@id": "iudx:"
            },
            "iudx:domainIncludes": [
                {
                    "@id": "iudx:RoadSegment"
                }
            ],
            "iudx:rangeIncludes": [
                {
                    "@id": "iudx:Text"
                },
                {
                    "@id": "iudx:ValueDescriptor"
                }
            ]
        },
        {
            "@id": "iudx:roadID",
            "@type": [
                "iudx:TextProperty"
            ],
            "rdfs:comment": "Unique representation of the road corresponding to this observation",
            "rdfs:label": "roadID",
            "rdfs:isDefinedBy": {
                "@id": "iudx:"
            },
            "iudx:domainIncludes": [
                {
                    "@id": "iudx:RoadSegment"
                }
            ],
            "iudx:rangeIncludes": [
                {
                    "@id": "iudx:Text"
                },
                {
                    "@id": "iudx:ValueDescriptor"
                }
            ]
        },
        {
            "@id": "iudx:roadMaterial",
            "@type": [
                "iudx:TextProperty"
            ],
            "rdfs:comment": "The construction material used for laying the carriageway corresponding to this observation. For eg. concrete, earthen, tar etc.",
            "rdfs:label": "roadMaterial",
            "rdfs:isDefinedBy": {
                "@id": "iudx:"
            },
            "iudx:domainIncludes": [
                {
                    "@id": "iudx:RoadSegment"
                }
            ],
            "iudx:rangeIncludes": [
                {
                    "@id": "iudx:Text"
                },
                {
                    "@id": "iudx:ValueDescriptor"
                }
            ]
        },
        {
            "@id": "iudx:roadName",
            "@type": [
                "iudx:TextProperty"
            ],
            "rdfs:comment": "The name of the road corresponding to this observation",
            "rdfs:label": "roadName",
            "rdfs:isDefinedBy": {
                "@id": "iudx:"
            },
            "iudx:domainIncludes": [
                {
                    "@id": "iudx:RoadSegment"
                }
            ],
            "iudx:rangeIncludes": [
                {
                    "@id": "iudx:Text"
                },
                {
                    "@id": "iudx:ValueDescriptor"
                }
            ]
        },
        {
            "@id": "iudx:roadWork",
            "@type": [
                "iudx:TextProperty"
            ],
            "rdfs:comment": "Reasons for the road work in case of urgent intervention. A combination of these values. ENUM: [COLLAPSE, DERAILMENT, FIRE, FLOOD, GASLEAK, LANDSLIDE, OTHER, POWERCUT, ROCKFALL, SAGGING, WATERLEAK]",
            "rdfs:label": "roadWork",
            "rdfs:isDefinedBy": {
                "@id": "iudx:"
            },
            "iudx:domainIncludes": [
                {
                    "@id": "iudx:RoadSegment"
                }
            ],
            "iudx:rangeIncludes": [
                {
                    "@id": "iudx:Text"
                },
                {
                    "@id": "iudx:ValueDescriptor"
                }
            ]
        },
        {
            "@id": "iudx:routeStopSequence",
            "@type": [
                "iudx:TextProperty"
            ],
            "rdfs:comment": "Gives the stop ids/stop codes or station ids/station codes in the right sequence for the route/line/trip corresponding to this observation.",
            "rdfs:label": "routeStopSequence",
            "rdfs:isDefinedBy": {
                "@id": "iudx:"
            },
            "iudx:domainIncludes": [
                {
                    "@id": "iudx:TransitManagement"
                },
                {
                    "@id": "iudx:WmgmtVehicle"
                }
            ],
            "iudx:rangeIncludes": [
                {
                    "@id": "iudx:Text",
                    "@container": "@list"
                },
                {
                    "@id": "iudx:ValueDescriptor"
                }
            ]
        },
        {
            "@id": "iudx:route_color",
            "@type": [
                "iudx:TextProperty"
            ],
            "rdfs:comment": "If assigned, this field defines a color that corresponds to a route. The color must be provided as a six-character hexadecimal number, for example, 00FFFF. If no color is specified, the default route color is white (FFFFFF). SameAs: 'route_color' field from GTFS Static Field definitions-routes.txt (https://developers.google.com/transit/gtfs/reference#routestxt)",
            "rdfs:label": "route_color",
            "rdfs:isDefinedBy": {
                "@id": "iudx:"
            },
            "iudx:domainIncludes": [
                {
                    "@id": "iudx:RoutesDesc"
                }
            ],
            "iudx:rangeIncludes": [
                {
                    "@id": "iudx:Text"
                },
                {
                    "@id": "iudx:ValueDescriptor"
                }
            ],
            "skos:exactMatch": {
                "@id": "GTFS: route_color"
            }
        },
        {
            "@id": "iudx:route_desc",
            "@type": [
                "iudx:TextProperty"
            ],
            "rdfs:comment": "Description of the route. This can include the entire route details including to and from destination and timing information in a text description form. SameAs: 'route_desc' field from GTFS Static Field definitions-routes.txt (https://developers.google.com/transit/gtfs/reference#routestxt)",
            "rdfs:label": "route_desc",
            "rdfs:isDefinedBy": {
                "@id": "iudx:"
            },
            "iudx:domainIncludes": [
                {
                    "@id": "iudx:RoutesDesc"
                }
            ],
            "iudx:rangeIncludes": [
                {
                    "@id": "iudx:Text"
                },
                {
                    "@id": "iudx:ValueDescriptor"
                }
            ],
            "skos:exactMatch": {
                "@id": "GTFS: route_desc"
            }
        },
        {
            "@id": "iudx:route_id",
            "@type": [
                "iudx:TextProperty"
            ],
            "rdfs:comment": "Route ID assigned to the route on which the bus/vehicle corresponding to the bus in this observation is currently plying on.",
            "rdfs:label": "route_id",
            "iudx:domainIncludes": [
                {
                    "@id": "iudx:GtfsCommons"
                },
                {
                    "@id": "iudx:TripDescriptor"
                },
                {
                    "@id": "iudx:FareCollectionSystem"
                },
                {
                    "@id": "iudx:RoutesDesc"
                },
                {
                    "@id": "iudx:TransitManagement"
                }
            ],
            "iudx:rangeIncludes": [
                {
                    "@id": "iudx:Text"
                },
                {
                    "@id": "iudx:ValueDescriptor"
                }
            ],
            "rdfs:isDefinedBy": {
                "@id": "iudx:"
            },
            "skos:exactMatch": {
                "@id": "GTFS: route_id"
            }
        },
        {
            "@id": "iudx:route_long_name",
            "@type": [
                "iudx:TextProperty"
            ],
            "rdfs:comment": "Full name of a route. This name is more descriptive than the routeShortName and often includes the route's destination or stop. This mostly includes the to and from destination names of the route. SameAs: 'route_long_name' field from GTFS Static Field definitions-routes.txt (https://developers.google.com/transit/gtfs/reference#routestxt)",
            "rdfs:label": "route_long_name",
            "rdfs:isDefinedBy": {
                "@id": "iudx:"
            },
            "iudx:domainIncludes": [
                {
                    "@id": "iudx:RoutesDesc"
                }
            ],
            "iudx:rangeIncludes": [
                {
                    "@id": "iudx:Text"
                },
                {
                    "@id": "iudx:ValueDescriptor"
                }
            ],
            "skos:exactMatch": {
                "@id": "GTFS: route_long_name"
            }
        },
        {
            "@id": "iudx:route_short_name",
            "@type": [
                "iudx:TextProperty"
            ],
            "rdfs:comment": "Short name of a route. This will often be the transit vehicle's board name like \"402D\",  or \"Green\" that riders use to identify a route. SameAs: 'route_short_name' field from GTFS Static Field definitions-routes.txt (https://developers.google.com/transit/gtfs/reference#routestxt)",
            "rdfs:label": "route_short_name",
            "rdfs:isDefinedBy": {
                "@id": "iudx:"
            },
            "iudx:domainIncludes": [
                {
                    "@id": "iudx:RoutesDesc"
                }
            ],
            "iudx:rangeIncludes": [
                {
                    "@id": "iudx:Text"
                },
                {
                    "@id": "iudx:ValueDescriptor"
                }
            ],
            "skos:exactMatch": {
                "@id": "GTFS: route_short_name"
            }
        },
        {
            "@id": "iudx:route_text_color",
            "@type": [
                "iudx:TextProperty"
            ],
            "rdfs:comment": "This field can be used to specify a legible color to use for text drawn against a background of route_color. The color must be provided as a six-character hexadecimal number, for example, FFD700. If no color is specified, the default text color is black (000000). SameAs: 'route_text_color' field from GTFS Static Field definitions-routes.txt (https://developers.google.com/transit/gtfs/reference#routestxt)",
            "rdfs:label": "route_text_color",
            "rdfs:isDefinedBy": {
                "@id": "iudx:"
            },
            "iudx:domainIncludes": [
                {
                    "@id": "iudx:RoutesDesc"
                }
            ],
            "iudx:rangeIncludes": [
                {
                    "@id": "iudx:Text"
                },
                {
                    "@id": "iudx:ValueDescriptor"
                }
            ],
            "skos:exactMatch": {
                "@id": "GTFS: route_text_color"
            }
        },
        {
            "@id": "iudx:route_url",
            "@type": [
                "iudx:TextProperty"
            ],
            "rdfs:comment": "Contains the URL of a web page about that particular route and is different from the agency_url. SameAs: 'route_url' field from GTFS Static Field definitions-routes.txt (https://developers.google.com/transit/gtfs/reference#routestxt)",
            "rdfs:label": "route_url",
            "rdfs:isDefinedBy": {
                "@id": "iudx:"
            },
            "iudx:domainIncludes": [
                {
                    "@id": "iudx:RoutesDesc"
                }
            ],
            "iudx:rangeIncludes": [
                {
                    "@id": "iudx:Text"
                },
                {
                    "@id": "iudx:ValueDescriptor"
                }
            ],
            "skos:exactMatch": {
                "@id": "GTFS: route_url"
            }
        },
        {
            "@id": "iudx:sameAs",
            "@type": [
                "iudx:TextProperty"
            ],
            "rdfs:comment": "URL reference to another thing/entity that identifies the given thing/entity. This may be used to provide references to another data models where a property is described or say a reference to Wiki pages for a given thing etc.",
            "rdfs:label": "sameAs",
            "iudx:domainIncludes": [
                {
                    "@id": "iudx:ValueDescriptor"
                }
            ],
            "iudx:rangeIncludes": [
                {
                    "@id": "iudx:Text",
                    "@type": "@id"
                }
            ],
            "skos:exactMatch": {
                "@id": "schema:sameAs"
            },
            "rdfs:isDefinedBy": {
                "@id": "iudx:"
            }
        },
        {
            "@id": "iudx:schedule_relationship",
            "@type": [
                "iudx:TextProperty"
            ],
            "rdfs:comment": "Describes if the Route/Trip has been scheduled. SameAs: 'schedule_relationship' field from GTFS Realtime message-TripDescriptor ENUM[SCHEDULED, ADDED, UNSCHEDULED, CANCELED] (https://developers.google.com/transit/gtfs-realtime/reference#message-tripdescriptor)",
            "rdfs:label": "schedule_relationship",
            "rdfs:isDefinedBy": {
                "@id": "iudx:"
            },
            "iudx:domainIncludes": [
                {
                    "@id": "iudx:TripDescriptor"
                }
            ],
            "iudx:rangeIncludes": [
                {
                    "@id": "iudx:Text"
                },
                {
                    "@id": "iudx:ValueDescriptor"
                }
            ],
            "skos:exactMatch": {
                "@id": "GTFS: schedule_relationship"
            }
        },
        {
            "@id": "iudx:schemeID",
            "@type": [
                "iudx:TextProperty"
            ],
            "rdfs:comment": "The unique ID representing the scheme corresponding to this observation.",
            "rdfs:label": "schemeID",
            "rdfs:isDefinedBy": {
                "@id": "iudx:"
            },
            "iudx:domainIncludes": [
                {
                    "@id": "iudx:PublicSchemes"
                }
            ],
            "iudx:rangeIncludes": [
                {
                    "@id": "iudx:Text"
                },
                {
                    "@id": "iudx:ValueDescriptor"
                }
            ]
        },
        {
            "@id": "iudx:schemeName",
            "@type": [
                "iudx:TextProperty"
            ],
            "rdfs:comment": "The name of the scheme or programme introduced by the government for public welfare and development.",
            "rdfs:label": "schemeName",
            "rdfs:isDefinedBy": {
                "@id": "iudx:"
            },
            "iudx:domainIncludes": [
                {
                    "@id": "iudx:PublicSchemes"
                }
            ],
            "iudx:rangeIncludes": [
                {
                    "@id": "iudx:Text"
                },
                {
                    "@id": "iudx:ValueDescriptor"
                }
            ]
        },
        {
            "@id": "iudx:secureDataFields",
            "@type": [
                "iudx:TextProperty"
            ],
            "rdfs:comment": "List of properties/fields/attributes contained in the data available from the resources associated with a given resource Group which are secure, i.e., need authorization from the auth server to access these fields for a given resource.",
            "rdfs:label": "secureDataFields",
            "iudx:domainIncludes": [
                {
                    "@id": "iudx:DataFieldListValue"
                }
            ],
            "iudx:rangeIncludes": [
                {
                    "@id": "iudx:Text",
                    "@container": "@set"
                }
            ]
        },
        {
            "@id": "iudx:serviceCompany",
            "@type": [
                "iudx:TextProperty"
            ],
            "rdfs:comment": "Service agency or company corresponding to this observation",
            "rdfs:label": "serviceCompany",
            "rdfs:isDefinedBy": {
                "@id": "iudx:"
            },
            "iudx:domainIncludes": [
                {
                    "@id": "iudx:EmployeeDetails"
                }
            ],
            "iudx:rangeIncludes": [
                {
                    "@id": "iudx:Text"
                },
                {
                    "@id": "iudx:ValueDescriptor"
                }
            ]
        },
        {
            "@id": "iudx:serviceOnDuty",
            "@type": [
                "iudx:TextProperty"
            ],
            "rdfs:comment": "Nature of service provided by emergency vehicle corresponding to this observation. ENUM: [YES, NO]. YES indicates the emergency vehicle corresponding to this observation is attending to/ servicing to an emergency call of duty and is NO otherwise.",
            "rdfs:label": "serviceOnDuty",
            "rdfs:isDefinedBy": {
                "@id": "iudx:"
            },
            "iudx:domainIncludes": [
                {
                    "@id": "iudx:EmergencyVehicle"
                }
            ],
            "iudx:rangeIncludes": [
                {
                    "@id": "iudx:Text"
                },
                {
                    "@id": "iudx:ValueDescriptor"
                }
            ]
        },
        {
            "@id": "iudx:shape_id",
            "@type": [
                "iudx:TextProperty"
            ],
            "rdfs:comment": "Identifies a shape.",
            "rdfs:label": "shape_id",
            "rdfs:isDefinedBy": {
                "@id": "iudx:"
            },
            "iudx:domainIncludes": [
                {
                    "@id": "iudx:ShapesDesc"
                }
            ],
            "iudx:rangeIncludes": [
                {
                    "@id": "iudx:Text"
                },
                {
                    "@id": "iudx:ValueDescriptor"
                }
            ],
            "skos:exactMatch": {
                "@id": "GTFS: shape_id"
            }
        },
        {
            "@id": "iudx:shiftOfOperation",
            "@type": [
                "iudx:TextProperty"
            ],
            "rdfs:comment": "Shift of operation of the public transit vehicle operated by the fare collection agency/ public transit agency or the employee corresponding to this observation. Indiacted as '1' when the vehicle operates in the first shift, '2' when the vehicle operates in the second shift and '3' when the vehilce operates in the third shift.",
            "rdfs:label": "shiftOfOperation",
            "rdfs:isDefinedBy": {
                "@id": "iudx:"
            },
            "iudx:domainIncludes": [
                {
                    "@id": "iudx:FareCollectionSystem"
                },
                {
                    "@id": "iudx:EmployeeDetails"
                }
            ],
            "iudx:rangeIncludes": [
                {
                    "@id": "iudx:Text"
                },
                {
                    "@id": "iudx:ValueDescriptor"
                }
            ]
        },
        {
            "@id": "iudx:siteCode",
            "@type": [
                "iudx:TextProperty"
            ],
            "rdfs:comment": "Unique ID of the public site or tourist destination.",
            "rdfs:label": "siteCode",
            "rdfs:isDefinedBy": {
                "@id": "iudx:"
            },
            "iudx:domainIncludes": [
                {
                    "@id": "iudx:TouristDestination"
                }
            ],
            "iudx:rangeIncludes": [
                {
                    "@id": "iudx:Text"
                },
                {
                    "@id": "iudx:ValueDescriptor"
                }
            ]
        },
        {
            "@id": "iudx:siteDescription",
            "@type": [
                "iudx:TextProperty"
            ],
            "rdfs:comment": "The detailed description about a public site or tourist destination corresponding to this observation.",
            "rdfs:label": "siteDescription",
            "rdfs:isDefinedBy": {
                "@id": "iudx:"
            },
            "iudx:domainIncludes": [
                {
                    "@id": "iudx:TouristDestination"
                }
            ],
            "iudx:rangeIncludes": [
                {
                    "@id": "iudx:Text"
                },
                {
                    "@id": "iudx:ValueDescriptor"
                }
            ]
        },
        {
            "@id": "iudx:siteName",
            "@type": [
                "iudx:TextProperty"
            ],
            "rdfs:comment": "Name of the public site or tourist destination.",
            "rdfs:label": "siteName",
            "rdfs:isDefinedBy": {
                "@id": "iudx:"
            },
            "iudx:domainIncludes": [
                {
                    "@id": "iudx:TouristDestination"
                }
            ],
            "iudx:rangeIncludes": [
                {
                    "@id": "iudx:Text"
                },
                {
                    "@id": "iudx:ValueDescriptor"
                }
            ]
        },
        {
            "@id": "iudx:slogan",
            "@type": [
                "iudx:TextProperty"
            ],
            "rdfs:comment": "A slogan or motto associated with the public site or tourist destination.",
            "rdfs:label": "slogan",
            "rdfs:isDefinedBy": {
                "@id": "iudx:"
            },
            "iudx:domainIncludes": [
                {
                    "@id": "iudx:TouristDestination"
                }
            ],
            "iudx:rangeIncludes": [
                {
                    "@id": "iudx:Text"
                },
                {
                    "@id": "iudx:ValueDescriptor"
                }
            ],
            "skos:exactMatch": {
                "@id": "schema:slogan"
            }
        },
        {
            "@id": "iudx:sludgeLevel",
            "@type": [
                "iudx:QuantitativeProperty"
            ],
            "rdfs:comment": "Level of Sludge measured in the waste-water treatment plant's tank or the manhole sensor corresponding to this observation.",
            "rdfs:label": "sludgeLevel",
            "rdfs:isDefinedBy": {
                "@id": "iudx:"
            },
            "iudx:domainIncludes": [
                {
                    "@id": "iudx:WasteWaterMgmt"
                }
            ],
            "iudx:rangeIncludes": [
                {
                    "@id": "iudx:Number"
                },
                {
                    "@id": "iudx:Text"
                },
                {
                    "@id": "iudx:ValueDescriptor"
                }
            ],
            "skos:exactMatch": {
                "@id": "fiware:sludgeLevel"
            }
        },
        {
            "@id": "iudx:socketType",
            "@type": [
                "iudx:TextProperty"
            ],
            "rdfs:comment": "The type of charging socket offered by the EV charging station.",
            "rdfs:label": "socketType",
            "rdfs:isDefinedBy": {
                "@id": "iudx:"
            },
            "iudx:domainIncludes": [
                {
                    "@id": "iudx:EVChargingStation"
                }
            ],
            "iudx:rangeIncludes": [
                {
                    "@id": "iudx:Text"
                },
                {
                    "@id": "iudx:ValueDescriptor"
                }
            ]
        },
        {
            "@id": "iudx:specialRestrictions",
            "@type": [
                "iudx:TextProperty"
            ],
            "rdfs:comment": "The restrictions or considerations at the premises to maintain the sanctity and tradition.",
            "rdfs:label": "specialRestrictions",
            "rdfs:isDefinedBy": {
                "@id": "iudx:"
            },
            "iudx:domainIncludes": [
                {
                    "@id": "iudx:TouristDestination"
                }
            ],
            "iudx:rangeIncludes": [
                {
                    "@id": "iudx:Text"
                },
                {
                    "@id": "iudx:ValueDescriptor"
                }
            ],
            "skos:exactMatch": {
                "@id": "Fiware:specialRestrictions"
            }
        },
        {
            "@id": "iudx:speciesName",
            "@type": [
                "iudx:TextProperty"
            ],
            "rdfs:comment": "The binomial/ zoological nomenclature of the species as identified by the device.",
            "rdfs:label": "speciesName",
            "rdfs:isDefinedBy": {
                "@id": "iudx:"
            },
            "iudx:domainIncludes": [
                {
                    "@id": "iudx:MosquitoDensity"
                }
            ],
            "iudx:rangeIncludes": [
                {
                    "@id": "iudx:Text"
                },
                {
                    "@id": "iudx:ValueDescriptor"
                }
            ]
        },
        {
            "@id": "iudx:start_date",
            "@type": [
                "iudx:TextProperty"
            ],
            "rdfs:comment": "Describes the initial scheduled date of the trip corresponding to the vehicle this observation. An example format for this field - YYYYMMDD. SameAs: 'start_date' field from GTFS Realtime message-TripDescriptor (https://developers.google.com/transit/gtfs-realtime/reference#message-tripdescriptor)",
            "rdfs:label": "start_date",
            "rdfs:isDefinedBy": {
                "@id": "iudx:"
            },
            "iudx:domainIncludes": [
                {
                    "@id": "iudx:TripDescriptor"
                }
            ],
            "iudx:rangeIncludes": [
                {
                    "@id": "iudx:Text"
                },
                {
                    "@id": "iudx:ValueDescriptor"
                }
            ],
            "skos:exactMatch": {
                "@id": "GTFS: start_date"
            }
        },
        {
            "@id": "iudx:start_time",
            "@type": [
                "iudx:TimeProperty"
            ],
            "rdfs:comment": "Describes the initial scheduled start time of the trip corresponding to the vehicle this observation. An example format for this field - 11:15:35 or 25:15:35. SameAs: 'start_time' field from GTFS Realtime message-TripDescriptor (https://developers.google.com/transit/gtfs-realtime/reference#message-tripdescriptor)",
            "rdfs:label": "start_time",
            "rdfs:isDefinedBy": {
                "@id": "iudx:"
            },
            "iudx:domainIncludes": [
                {
                    "@id": "iudx:TripDescriptor"
                }
            ],
            "iudx:rangeIncludes": [
                {
                    "@id": "iudx:Text"
                },
                {
                    "@id": "iudx:ValueDescriptor"
                }
            ],
            "skos:exactMatch": {
                "@id": "GTFS: start_time"
            }
        },
        {
            "@id": "iudx:state",
            "@type": [
                "iudx:TextProperty"
            ],
            "rdfs:comment": "Name of the state corresponding to this observation.",
            "rdfs:label": "state",
            "iudx:domainIncludes": [
                {
                    "@id": "iudx:Headquarters"
                },
                {
                    "@id": "iudx:District"
                },
                {
                    "@id": "iudx:States"
                }
            ],
            "iudx:rangeIncludes": [
                {
                    "@id": "iudx:Text"
                },
                {
                    "@id": "iudx:ValueDescriptor"
                }
            ],
            "rdfs:isDefinedBy": {
                "@id": "iudx:"
            }
        },
        {
            "@id": "iudx:stateName",
            "@type": [
                "iudx:TextProperty"
            ],
            "rdfs:comment": "Name of the state corresponding to this observation.",
            "rdfs:label": "stateName",
            "rdfs:isDefinedBy": {
                "@id": "iudx:"
            },
            "iudx:domainIncludes": [
                {
                    "@id": "iudx:MunicipalityDesc"
                }
            ],
            "iudx:rangeIncludes": [
                {
                    "@id": "iudx:Text"
                },
                {
                    "@id": "iudx:ValueDescriptor"
                }
            ]
        },
        {
            "@id": "iudx:stationCode",
            "@type": [
                "iudx:TextProperty"
            ],
            "rdfs:comment": "The station number or station code of the bike hire docking station corresponding to the observation.",
            "rdfs:label": "stationCode",
            "rdfs:isDefinedBy": {
                "@id": "iudx:"
            },
            "iudx:domainIncludes": [
                {
                    "@id": "iudx:BikeDockingStation"
                }
            ],
            "iudx:rangeIncludes": [
                {
                    "@id": "iudx:Text"
                },
                {
                    "@id": "iudx:ValueDescriptor"
                }
            ]
        },
        {
            "@id": "iudx:stationName",
            "@type": [
                "iudx:TextProperty"
            ],
            "rdfs:comment": "The name station corresponding to this observation. It can be the name of bike docking station, charging station, etc.",
            "rdfs:label": "stationName",
            "rdfs:isDefinedBy": {
                "@id": "iudx:"
            },
            "iudx:domainIncludes": [
                {
                    "@id": "iudx:BikeDockingStation"
                },
                {
                    "@id": "iudx:EVChargingStation"
                }
            ],
            "iudx:rangeIncludes": [
                {
                    "@id": "iudx:Text"
                },
                {
                    "@id": "iudx:ValueDescriptor"
                }
            ]
        },
        {
            "@id": "iudx:stopScheduleRelationship",
            "@type": [
                "iudx:TextProperty"
            ],
            "rdfs:comment": "Describes the relationship between the static schedule and the stop. SameAs: 'schedule_relationship' field from GTFS Realtime message-StopTimeUpdate ENUM[SCHEDULED, SKIPPED, NO_DATA] (https://developers.google.com/transit/gtfs-realtime/reference#message-stoptimeupdate)",
            "rdfs:label": "stopScheduleRelationship",
            "rdfs:isDefinedBy": {
                "@id": "iudx:"
            },
            "iudx:domainIncludes": [
                {
                    "@id": "iudx:StopTimeUpdate"
                }
            ],
            "iudx:rangeIncludes": [
                {
                    "@id": "iudx:Text"
                },
                {
                    "@id": "iudx:ValueDescriptor"
                }
            ],
            "skos:exactMatch": {
                "@id": "GTFS: schedule_relationship"
            }
        },
        {
            "@id": "iudx:stop_code",
            "@type": [
                "iudx:TextProperty"
            ],
            "rdfs:comment": "This field contains short text or a number that uniquely identifies the stop for passengers. Can be same as stop_id if it is for public. SameAs: 'stop_code' field from GTFS Static Field definitions-stops.txt (https://developers.google.com/transit/gtfs/reference#stopstxt)",
            "rdfs:label": "stop_code",
            "rdfs:isDefinedBy": {
                "@id": "iudx:"
            },
            "iudx:domainIncludes": [
                {
                    "@id": "iudx:StopsDesc"
                }
            ],
            "iudx:rangeIncludes": [
                {
                    "@id": "iudx:Text"
                },
                {
                    "@id": "iudx:ValueDescriptor"
                }
            ],
            "skos:exactMatch": {
                "@id": "GTFS: stop_code"
            }
        },
        {
            "@id": "iudx:stop_desc",
            "@type": [
                "iudx:TextProperty"
            ],
            "rdfs:comment": "This field contains a description of a stop. SameAs: 'stop_desc' field from GTFS Static Field definitions-stops.txt (https://developers.google.com/transit/gtfs/reference#stopstxt)",
            "rdfs:label": "stop_desc",
            "rdfs:isDefinedBy": {
                "@id": "iudx:"
            },
            "iudx:domainIncludes": [
                {
                    "@id": "iudx:StopsDesc"
                }
            ],
            "iudx:rangeIncludes": [
                {
                    "@id": "iudx:Text"
                },
                {
                    "@id": "iudx:ValueDescriptor"
                }
            ],
            "skos:exactMatch": {
                "@id": "GTFS: stop_desc"
            }
        },
        {
            "@id": "iudx:stop_headsign",
            "@type": [
                "iudx:TextProperty"
            ],
            "rdfs:comment": "This field contains the text that appears on a sign that identifies the trip\u2019s destination to passengers. SameAs: 'stop_headsign' field from GTFS Static Field definitions-stop_times.txt (https://developers.google.com/transit/gtfs/reference#stop_timestxt)",
            "rdfs:label": "stop_headsign",
            "rdfs:isDefinedBy": {
                "@id": "iudx:"
            },
            "iudx:domainIncludes": [
                {
                    "@id": "iudx:StopTimesDesc"
                }
            ],
            "iudx:rangeIncludes": [
                {
                    "@id": "iudx:Text"
                },
                {
                    "@id": "iudx:ValueDescriptor"
                }
            ],
            "skos:exactMatch": {
                "@id": "GTFS: stop_headsign"
            }
        },
        {
            "@id": "iudx:stop_id",
            "@type": [
                "iudx:TextProperty"
            ],
            "rdfs:comment": "Unique ID assigned to the stop corresponding to this observation.",
            "rdfs:label": "stop_id",
            "rdfs:isDefinedBy": {
                "@id": "iudx:"
            },
            "iudx:domainIncludes": [
                {
                    "@id": "iudx:GtfsCommons"
                },
                {
                    "@id": "iudx:VehiclePosition"
                },
                {
                    "@id": "iudx:StopTimeUpdate"
                },
                {
                    "@id": "iudx:StopsDesc"
                },
                {
                    "@id": "iudx:StopTimesDesc"
                }
            ],
            "iudx:rangeIncludes": [
                {
                    "@id": "iudx:Text"
                },
                {
                    "@id": "iudx:ValueDescriptor"
                }
            ],
            "skos:exactMatch": {
                "@id": "GTFS: stop_id"
            }
        },
        {
            "@id": "iudx:stop_name",
            "@type": [
                "iudx:TextProperty"
            ],
            "rdfs:comment": "Describes the name of a stop or station. SameAs: 'stop_name' field from GTFS Static Field definitions-stops.txt (https://developers.google.com/transit/gtfs/reference#stopstxt)",
            "rdfs:label": "stop_name",
            "rdfs:isDefinedBy": {
                "@id": "iudx:"
            },
            "iudx:domainIncludes": [
                {
                    "@id": "iudx:StopsDesc"
                }
            ],
            "iudx:rangeIncludes": [
                {
                    "@id": "iudx:Text"
                },
                {
                    "@id": "iudx:ValueDescriptor"
                }
            ],
            "skos:exactMatch": {
                "@id": "GTFS: stop_name"
            }
        },
        {
            "@id": "iudx:stop_url",
            "@type": [
                "iudx:TextProperty"
            ],
            "rdfs:comment": "This field contains the URL of a web page about a particular stop and is different from the agency_url and the route_url fields. SameAs: 'stop_url' field from GTFS Static Field definitions-stops.txt (https://developers.google.com/transit/gtfs/reference#stopstxt)",
            "rdfs:label": "stop_url",
            "rdfs:isDefinedBy": {
                "@id": "iudx:"
            },
            "iudx:domainIncludes": [
                {
                    "@id": "iudx:StopsDesc"
                }
            ],
            "iudx:rangeIncludes": [
                {
                    "@id": "iudx:Text"
                },
                {
                    "@id": "iudx:ValueDescriptor"
                }
            ],
            "skos:exactMatch": {
                "@id": "GTFS: stop_url"
            }
        },
        {
            "@id": "iudx:streamName",
            "@type": [
                "iudx:TextProperty"
            ],
            "rdfs:comment": "Name of the video stream from the camera corresponding to this observation",
            "rdfs:label": "streamName",
            "rdfs:isDefinedBy": {
                "@id": "iudx:"
            },
            "iudx:domainIncludes": [
                {
                    "@id": "iudx:Camera"
                }
            ],
            "iudx:rangeIncludes": [
                {
                    "@id": "iudx:Text"
                },
                {
                    "@id": "iudx:ValueDescriptor"
                }
            ]
        },
        {
            "@id": "iudx:streamURL",
            "@type": [
                "iudx:TextProperty"
            ],
            "rdfs:comment": "URL providing video streaming information for the camera corresponding to this observation",
            "rdfs:label": "streamURL",
            "rdfs:isDefinedBy": {
                "@id": "iudx:"
            },
            "iudx:domainIncludes": [
                {
                    "@id": "iudx:Camera"
                }
            ],
            "iudx:rangeIncludes": [
                {
                    "@id": "iudx:Text"
                },
                {
                    "@id": "iudx:ValueDescriptor"
                }
            ]
        },
        {
            "@id": "iudx:streetPoleNum",
            "@type": [
                "iudx:TextProperty"
            ],
            "rdfs:comment": "Street pole information associated with the streetlight corresponding to this observation.",
            "rdfs:label": "streetPoleNum",
            "rdfs:isDefinedBy": {
                "@id": "iudx:"
            },
            "iudx:domainIncludes": [
                {
                    "@id": "iudx:Streetlight"
                }
            ],
            "iudx:rangeIncludes": [
                {
                    "@id": "iudx:Text"
                },
                {
                    "@id": "iudx:ValueDescriptor"
                }
            ]
        },
        {
            "@id": "iudx:subCategory",
            "@type": [
                "iudx:TextProperty"
            ],
            "rdfs:comment": "The sub-category name corresponding to the issue that has been reported.",
            "rdfs:label": "subCategory",
            "rdfs:isDefinedBy": {
                "@id": "iudx:"
            },
            "iudx:domainIncludes": [
                {
                    "@id": "iudx:IssueReporting"
                }
            ],
            "iudx:rangeIncludes": [
                {
                    "@id": "iudx:Text"
                },
                {
                    "@id": "iudx:ValueDescriptor"
                }
            ]
        },
        {
            "@id": "iudx:subCategoryCode",
            "@type": [
                "iudx:TextProperty"
            ],
            "rdfs:comment": "Unique identifier for the sub-category corresponding to the issue reported.",
            "rdfs:label": "subCategoryCode",
            "rdfs:isDefinedBy": {
                "@id": "iudx:"
            },
            "iudx:domainIncludes": [
                {
                    "@id": "iudx:IssueReporting"
                }
            ],
            "iudx:rangeIncludes": [
                {
                    "@id": "iudx:Text"
                },
                {
                    "@id": "iudx:ValueDescriptor"
                }
            ]
        },
        {
            "@id": "iudx:subdistrict",
            "@type": [
                "iudx:TextProperty"
            ],
            "rdfs:comment": "Name of the subdistrict corresponding to this observation.",
            "rdfs:label": "subdistrict",
            "rdfs:isDefinedBy": {
                "@id": "iudx:"
            },
            "iudx:domainIncludes": [
                {
                    "@id": "iudx:District"
                }
            ],
            "iudx:rangeIncludes": [
                {
                    "@id": "iudx:Text"
                },
                {
                    "@id": "iudx:ValueDescriptor"
                }
            ]
        },
        {
            "@id": "iudx:tags",
            "@type": [
                "iudx:TextProperty"
            ],
            "rdfs:comment": "Comma separated discovery tags associated with an IUDXEntity (resource , resource Group)",
            "rdfs:label": "tags",
            "iudx:domainIncludes": [
                {
                    "@id": "iudx:Resource",
                    "iudx:requiredProperty": true
                },
                {
                    "@id": "iudx:ResourceGroup",
                    "iudx:requiredProperty": true
                },
                {
                    "@id": "iudx:ResourceServer",
                    "iudx:requiredProperty": true
                }
            ],
            "iudx:rangeIncludes": [
                {
                    "@container": "@list",
                    "@id": "iudx:Text"
                }
            ]
        },
        {
            "@id": "iudx:taluk",
            "@type": [
                "iudx:TextProperty"
            ],
            "rdfs:comment": "Name of the taluk corresponding to this observation.",
            "rdfs:label": "taluk",
            "rdfs:isDefinedBy": {
                "@id": "iudx:"
            },
            "iudx:domainIncludes": [
                {
                    "@id": "iudx:Headquarters"
                }
            ],
            "iudx:rangeIncludes": [
                {
                    "@id": "iudx:Text"
                },
                {
                    "@id": "iudx:ValueDescriptor"
                }
            ]
        },
        {
            "@id": "iudx:tankName",
            "@type": [
                "iudx:TextProperty"
            ],
            "rdfs:comment": "Name of the water storage tank corresponding to this observation.",
            "rdfs:label": "tankName",
            "rdfs:isDefinedBy": {
                "@id": "iudx:"
            },
            "iudx:domainIncludes": [
                {
                    "@id": "iudx:WaterDistributionNetwork"
                }
            ],
            "iudx:rangeIncludes": [
                {
                    "@id": "iudx:Text"
                },
                {
                    "@id": "iudx:ValueDescriptor"
                }
            ]
        },
        {
            "@id": "iudx:tankShape",
            "@type": [
                "iudx:TextProperty"
            ],
            "rdfs:comment": "Physical shape of the water storage tank corresponding to this observation. ENUM: [Cylindrical, Conical, Cuboid, Spherical]",
            "rdfs:label": "tankShape",
            "rdfs:isDefinedBy": {
                "@id": "iudx:"
            },
            "iudx:domainIncludes": [
                {
                    "@id": "iudx:WaterDistributionNetwork"
                }
            ],
            "iudx:rangeIncludes": [
                {
                    "@id": "iudx:Text"
                },
                {
                    "@id": "iudx:ValueDescriptor"
                }
            ]
        },
        {
            "@id": "iudx:tehsil",
            "@type": [
                "iudx:TextProperty"
            ],
            "rdfs:comment": "Name of the tehsil corresponding to this observation.",
            "rdfs:label": "tehsil",
            "rdfs:isDefinedBy": {
                "@id": "iudx:"
            },
            "iudx:domainIncludes": [
                {
                    "@id": "iudx:District"
                }
            ],
            "iudx:rangeIncludes": [
                {
                    "@id": "iudx:Text"
                },
                {
                    "@id": "iudx:ValueDescriptor"
                }
            ]
        },
        {
            "@id": "iudx:ticketTypeCode",
            "@type": [
                "iudx:TextProperty"
            ],
            "rdfs:comment": "Unique ticket type code of the corresponding trip.",
            "rdfs:label": "ticketTypeCode",
            "rdfs:isDefinedBy": {
                "@id": "iudx:"
            },
            "iudx:domainIncludes": [
                {
                    "@id": "iudx:FareCollectionSystem"
                }
            ],
            "iudx:rangeIncludes": [
                {
                    "@id": "iudx:Text"
                },
                {
                    "@id": "iudx:ValueDescriptor"
                }
            ]
        },
        {
            "@id": "iudx:title",
            "@type": [
                "iudx:TextProperty"
            ],
            "rdfs:comment": "The title assigned to the issue, report or feedback corresponding to this observation.",
            "rdfs:label": "title",
            "rdfs:isDefinedBy": {
                "@id": "iudx:"
            },
            "iudx:domainIncludes": [
                {
                    "@id": "iudx:IssueReporting"
                }
            ],
            "iudx:rangeIncludes": [
                {
                    "@id": "iudx:Text"
                },
                {
                    "@id": "iudx:ValueDescriptor"
                }
            ],
            "skos:exactMatch": {
                "@id": "open311:description"
            }
        },
        {
            "@id": "iudx:titleCode",
            "@type": [
                "iudx:TextProperty"
            ],
            "rdfs:comment": "The code assigned to the title corresponding to this observation.",
            "rdfs:label": "titleCode",
            "rdfs:isDefinedBy": {
                "@id": "iudx:"
            },
            "iudx:domainIncludes": [
                {
                    "@id": "iudx:IssueReporting"
                },
                {
                    "@id": "iudx:TrafficViolations"
                }
            ],
            "iudx:rangeIncludes": [
                {
                    "@id": "iudx:Text"
                },
                {
                    "@id": "iudx:ValueDescriptor"
                }
            ]
        },
        {
            "@id": "iudx:topoSheetNo",
            "@type": [
                "iudx:TextProperty"
            ],
            "rdfs:comment": "The unique number assigned to the toposheet corresponding to this observation.",
            "rdfs:label": "topoSheetNo",
            "rdfs:isDefinedBy": {
                "@id": "iudx:"
            },
            "iudx:domainIncludes": [
                {
                    "@id": "iudx:DigitalElevationModel"
                }
            ],
            "iudx:rangeIncludes": [
                {
                    "@id": "iudx:Text"
                },
                {
                    "@id": "iudx:ValueDescriptor"
                }
            ]
        },
        {
            "@id": "iudx:town",
            "@type": [
                "iudx:TextProperty"
            ],
            "rdfs:comment": "Name of the town corresponding to this observation.",
            "rdfs:label": "town",
            "rdfs:isDefinedBy": {
                "@id": "iudx:"
            },
            "iudx:domainIncludes": [
                {
                    "@id": "iudx:Headquarters"
                }
            ],
            "iudx:rangeIncludes": [
                {
                    "@id": "iudx:Text"
                },
                {
                    "@id": "iudx:ValueDescriptor"
                }
            ]
        },
        {
            "@id": "iudx:tradeName",
            "@type": [
                "iudx:TextProperty"
            ],
            "rdfs:comment": "The official name under which an individual as a sole proprietor or a company chooses to do business.",
            "rdfs:label": "tradeName",
            "rdfs:isDefinedBy": {
                "@id": "iudx:"
            },
            "iudx:domainIncludes": [
                {
                    "@id": "iudx:RevenueCollection"
                }
            ],
            "iudx:rangeIncludes": [
                {
                    "@id": "iudx:Text"
                },
                {
                    "@id": "iudx:ValueDescriptor"
                }
            ]
        },
        {
            "@id": "iudx:transactionID",
            "@type": [
                "iudx:TextProperty"
            ],
            "rdfs:comment": "Unique transaction ID of the entity corresponding to this observation.",
            "rdfs:label": "transactionID",
            "rdfs:isDefinedBy": {
                "@id": "iudx:"
            },
            "iudx:domainIncludes": [
                {
                    "@id": "iudx:FareCollectionSystem"
                },
                {
                    "@id": "iudx:EVChargingStation"
                }
            ],
            "iudx:rangeIncludes": [
                {
                    "@id": "iudx:Text"
                },
                {
                    "@id": "iudx:ValueDescriptor"
                }
            ]
        },
        {
            "@id": "iudx:transactionType",
            "@type": [
                "iudx:TextProperty"
            ],
            "rdfs:comment": "Type of the transaction based on the mode of payment (For eg. mobile/UPI, card, etc) or mode of service (For eg. Issue, ReIssue, Entry, Exit etc.) corresponding to this observation.",
            "rdfs:label": "transactionType",
            "rdfs:isDefinedBy": {
                "@id": "iudx:"
            },
            "iudx:domainIncludes": [
                {
                    "@id": "iudx:FareCollectionSystem"
                },
                {
                    "@id": "iudx:EVChargingStation"
                }
            ],
            "iudx:rangeIncludes": [
                {
                    "@id": "iudx:Text"
                },
                {
                    "@id": "iudx:ValueDescriptor"
                }
            ]
        },
        {
            "@id": "iudx:transactionTypeDescription",
            "@type": [
                "iudx:TextProperty"
            ],
            "rdfs:comment": "Description of the transaction type. Explanation of various transanctionTypeID codes used in the data.",
            "rdfs:label": "transactionTypeDescription",
            "rdfs:isDefinedBy": {
                "@id": "iudx:"
            },
            "iudx:domainIncludes": [
                {
                    "@id": "iudx:FareCollectionSystem"
                }
            ],
            "iudx:rangeIncludes": [
                {
                    "@id": "iudx:Text"
                },
                {
                    "@id": "iudx:ValueDescriptor"
                }
            ]
        },
        {
            "@id": "iudx:transactionTypeID",
            "@type": [
                "iudx:TextProperty"
            ],
            "rdfs:comment": "ID for the transactionType corresponding to this observation. 2401 - QR sale, C201- smart card entry , C202 - smart card exit etc.",
            "rdfs:label": "transactionTypeID",
            "rdfs:isDefinedBy": {
                "@id": "iudx:"
            },
            "iudx:domainIncludes": [
                {
                    "@id": "iudx:FareCollectionSystem"
                }
            ],
            "iudx:rangeIncludes": [
                {
                    "@id": "iudx:Text"
                },
                {
                    "@id": "iudx:ValueDescriptor"
                }
            ]
        },
        {
            "@id": "iudx:travelTime",
            "@type": [
                "iudx:TimeProperty"
            ],
            "rdfs:comment": "The time taken to travel between the origin location and the destination location corresponding to this observation in HH:MM:SS format(HH:MM:SS is also accepted, if the hour begins with 0).",
            "rdfs:label": "travelTime",
            "rdfs:isDefinedBy": {
                "@id": "iudx:"
            },
            "iudx:domainIncludes": [
                {
                    "@id": "iudx:TransitManagement"
                }
            ],
            "iudx:rangeIncludes": [
                {
                    "@id": "iudx:Text"
                },
                {
                    "@id": "iudx:ValueDescriptor"
                }
            ]
        },
        {
            "@id": "iudx:treatmentPlantCode",
            "@type": [
                "iudx:TextProperty"
            ],
            "rdfs:comment": "Unique code for the waste-water treatment plant corresponding to this observation.",
            "rdfs:label": "treatmentPlantCode",
            "rdfs:isDefinedBy": {
                "@id": "iudx:"
            },
            "iudx:domainIncludes": [
                {
                    "@id": "iudx:WasteWaterMgmt"
                }
            ],
            "iudx:rangeIncludes": [
                {
                    "@id": "iudx:Text"
                }
            ]
        },
        {
            "@id": "iudx:treatmentPlantName",
            "@type": [
                "iudx:TextProperty"
            ],
            "rdfs:comment": "Name of the waste-water treatment plant corresponding to this observation.",
            "rdfs:label": "treatmentPlantName",
            "rdfs:isDefinedBy": {
                "@id": "iudx:"
            },
            "iudx:domainIncludes": [
                {
                    "@id": "iudx:WasteWaterMgmt"
                }
            ],
            "iudx:rangeIncludes": [
                {
                    "@id": "iudx:Text"
                },
                {
                    "@id": "iudx:ValueDescriptor"
                }
            ]
        },
        {
            "@id": "iudx:tripStatus",
            "@type": [
                "iudx:TextProperty"
            ],
            "rdfs:comment": "Current status of the ride corresponding to this observation. ENUM: [ACCEPTED, ONGOING, COMPLETED, CANCELLED, TERMINATED]",
            "rdfs:label": "tripStatus",
            "rdfs:isDefinedBy": {
                "@id": "iudx:"
            },
            "iudx:domainIncludes": [
                {
                    "@id": "iudx:BikeDockingStation"
                },
                {
                    "@id": "iudx:WmgmtVehicle"
                }
            ],
            "iudx:rangeIncludes": [
                {
                    "@id": "iudx:Text"
                },
                {
                    "@id": "iudx:ValueDescriptor"
                }
            ]
        },
        {
            "@id": "iudx:trip_direction",
            "@type": [
                "iudx:TextProperty"
            ],
            "rdfs:comment": "Indicates the direction of travel of the vehicle corresponding to this observation, can be referenced from the GTFS static feed trips.txt. SameAs: 'direction_id' field from GTFS Realtime message-TripDescriptor (https://developers.google.com/transit/gtfs-realtime/reference#message-tripdescriptor)",
            "rdfs:label": "trip_direction",
            "rdfs:isDefinedBy": {
                "@id": "iudx:"
            },
            "iudx:domainIncludes": [
                {
                    "@id": "iudx:TransitManagement"
                },
                {
                    "@id": "iudx:FareCollectionSystem"
                }
            ],
            "iudx:rangeIncludes": [
                {
                    "@id": "iudx:Text"
                },
                {
                    "@id": "iudx:ValueDescriptor"
                }
            ],
            "skos:exactMatch": {
                "@id": "GTFS: direction_id"
            }
        },
        {
            "@id": "iudx:trip_id",
            "@type": [
                "iudx:TextProperty"
            ],
            "rdfs:comment": "Trip ID/Trip name allotted to the bus corresponding to this observation, in consideration to the time of the day and the direction of the trip on the given routeId.",
            "rdfs:label": "trip_id",
            "rdfs:isDefinedBy": {
                "@id": "iudx:"
            },
            "iudx:domainIncludes": [
                {
                    "@id": "iudx:GtfsCommons"
                },
                {
                    "@id": "iudx:TripDescriptor"
                },
                {
                    "@id": "iudx:FareCollectionSystem"
                },
                {
                    "@id": "iudx:StopTimesDesc"
                },
                {
                    "@id": "iudx:WmgmtVehicle"
                }
            ],
            "iudx:rangeIncludes": [
                {
                    "@id": "iudx:Text"
                },
                {
                    "@id": "iudx:ValueDescriptor"
                }
            ],
            "skos:exactMatch": {
                "@id": "GTFS: trip_id"
            }
        },
        {
            "@id": "iudx:ulbName",
            "@type": [
                "iudx:TextProperty"
            ],
            "rdfs:comment": "Name of the Urban Local Body corresponding to this observation.",
            "rdfs:label": "ulbName",
            "rdfs:isDefinedBy": {
                "@id": "iudx:"
            },
            "iudx:domainIncludes": [
                {
                    "@id": "iudx:MunicipalityDesc"
                }
            ],
            "iudx:rangeIncludes": [
                {
                    "@id": "iudx:Text"
                },
                {
                    "@id": "iudx:ValueDescriptor"
                }
            ]
        },
        {
            "@id": "iudx:unitCode",
            "@type": [
                "iudx:TextProperty"
            ],
            "rdfs:comment": "The unit of measurement given using the UN/CEFACT Common Code (3 characters) or a URL. Other codes/unit vocabularies may be used with a prefix",
            "rdfs:label": "unitCode",
            "iudx:domainIncludes": [
                {
                    "@id": "iudx:ValueDescriptor"
                }
            ],
            "iudx:rangeIncludes": [
                {
                    "@id": "iudx:Text"
                },
                {
                    "@id": "iudx:Text",
                    "@type": "@id"
                }
            ],
            "skos:exactMatch": {
                "@id": "schema:unitCode"
            },
            "rdfs:isDefinedBy": {
                "@id": "iudx:"
            }
        },
        {
            "@id": "iudx:unitText",
            "@type": [
                "iudx:TextProperty"
            ],
            "rdfs:comment": "Describes the unit of measurement. Useful if unitCode is not available.",
            "rdfs:label": "unitText",
            "iudx:domainIncludes": [
                {
                    "@id": "iudx:ValueDescriptor"
                }
            ],
            "iudx:rangeIncludes": [
                {
                    "@id": "iudx:Text"
                }
            ],
            "skos:exactMatch": {
                "@id": "schema:unitText"
            },
            "rdfs:isDefinedBy": {
                "@id": "iudx:"
            }
        },
        {
            "@id": "iudx:value",
            "@type": [
                "iudx:QuantitativeProperty"
            ],
            "rdfs:comment": "Value of the quantity being described in the ValueDescriptor object.",
            "rdfs:label": "value",
            "iudx:domainIncludes": [
                {
                    "@id": "iudx:ValueDescriptor"
                }
            ],
            "iudx:rangeIncludes": [
                {
                    "@id": "iudx:Number"
                },
                {
                    "@id": "iudx:Text"
                },
                {
                    "@id": "iudx:Boolean"
                },
                {
                    "@id": "iudx:NumericArray"
                },
                {
                    "@id": "iudx:StructuredValue"
                }
            ],
            "rdfs:isDefinedBy": {
                "@id": "iudx:"
            }
        },
        {
            "@id": "iudx:vehicleID",
            "@type": [
                "iudx:TextProperty"
            ],
            "rdfs:comment": "Unique ID(s) assigned to the vehicle(s) corresponding to this observation, used in internal system identification. SameAs: 'id' field from GTFS Realtime message-VehicleDescriptor (https://developers.google.com/transit/gtfs-realtime/reference#message-vehicledescriptor)",
            "rdfs:label": "vehicleID",
            "rdfs:isDefinedBy": {
                "@id": "iudx:"
            },
            "iudx:domainIncludes": [
                {
                    "@id": "iudx:VehicleDescriptor"
                },
                {
                    "@id": "iudx:BikeDockingStation"
                }
            ],
            "iudx:rangeIncludes": [
                {
                    "@container": "@list",
                    "@id": "iudx:Text"
                },
                {
                    "@id": "iudx:ValueDescriptor"
                }
            ],
            "skos:exactMatch": {
                "@id": "GTFS: id"
            }
        },
        {
            "@id": "iudx:vehicleRunningStatus",
            "@type": [
                "iudx:TextProperty"
            ],
            "rdfs:comment": "Moving status of the vehicle. For eg., running, idle, etc.",
            "rdfs:label": "vehicleRunningStatus",
            "rdfs:isDefinedBy": {
                "@id": "iudx:"
            },
            "iudx:domainIncludes": [
                {
                    "@id": "iudx:WmgmtVehicle"
                },
                {
                    "@id": "iudx:EmergencyVehicle"
                }
            ],
            "iudx:rangeIncludes": [
                {
                    "@id": "iudx:Text"
                },
                {
                    "@id": "iudx:ValueDescriptor"
                }
            ]
        },
        {
            "@id": "iudx:vehicleSupportType",
            "@type": [
                "iudx:TextProperty"
            ],
            "rdfs:comment": "Support capability being provided by the vehicle corresponding to this observation. ENUM[ALS,BLS]. \nALS refers to Advance Life Support and BLS refers to Basic life support",
            "rdfs:label": "vehicleSupportType",
            "rdfs:isDefinedBy": {
                "@id": "iudx:"
            },
            "iudx:domainIncludes": [
                {
                    "@id": "iudx:EmergencyVehicle"
                }
            ],
            "iudx:rangeIncludes": [
                {
                    "@id": "iudx:Text"
                },
                {
                    "@id": "iudx:ValueDescriptor"
                }
            ]
        },
        {
            "@id": "iudx:vehicleTrackerDevice",
            "@type": [
                "iudx:TextProperty"
            ],
            "rdfs:comment": "Installation status of the GPS device or the tracking device fitted to the vehicle corresponding to this observation.",
            "rdfs:label": "vehicleTrackerDevice",
            "rdfs:isDefinedBy": {
                "@id": "iudx:"
            },
            "iudx:domainIncludes": [
                {
                    "@id": "iudx:WmgmtVehicle"
                },
                {
                    "@id": "iudx:EmergencyVehicle"
                }
            ],
            "iudx:rangeIncludes": [
                {
                    "@id": "iudx:Text"
                },
                {
                    "@id": "iudx:ValueDescriptor"
                }
            ]
        },
        {
            "@id": "iudx:vehicleType",
            "@type": [
                "iudx:TextProperty"
            ],
            "rdfs:comment": "Describes the type of vehicle corresponding to this observation, could be hopper, compactor, tipper, dumper in case of solid waste management vehicles, BRT mini bus, BRT bus, city bus in case of ITMS vehicles, Ambulance, Fire tender, Police van etc, in case of emergency vehicles and Moped/Scooter, Motor Cycle,  Autorickshaw, Private car/ Jeep car, Tempo, Bus, E-Moped/E-Scooter/E-Motor Cycle, Public motor in case of vehicle registration.",
            "rdfs:label": "vehicleType",
            "iudx:domainIncludes": [
                {
                    "@id": "iudx:WmgmtVehicle"
                },
                {
                    "@id": "iudx:TransitManagement"
                },
                {
                    "@id": "iudx:RevenueCollection"
                },
                {
                    "@id": "iudx:EmergencyVehicle"
                },
                {
                    "@id": "iudx:EVChargingStation"
                }
            ],
            "iudx:rangeIncludes": [
                {
                    "@id": "iudx:Text"
                },
                {
                    "@id": "iudx:ValueDescriptor"
                }
            ],
            "rdfs:isDefinedBy": {
                "@id": "iudx:"
            }
        },
        {
            "@id": "iudx:vehicleTypeCode",
            "@type": [
                "iudx:TextProperty"
            ],
            "rdfs:comment": "The code for vehicleType corresponding to this observation. For eg.- '1' - MOPED/SCOOTER, '2' - MOTOR CYCLE, '4' - PRIVATE MOTOR CAR/JEEP CAR, '21' - TEMPO, '26' - BUS, etc.",
            "rdfs:label": "vehicleTypeCode",
            "rdfs:isDefinedBy": {
                "@id": "iudx:"
            },
            "iudx:domainIncludes": [
                {
                    "@id": "iudx:RevenueCollection"
                }
            ],
            "iudx:rangeIncludes": [
                {
                    "@id": "iudx:Text"
                },
                {
                    "@id": "iudx:ValueDescriptor"
                }
            ]
        },
        {
            "@id": "iudx:vehicle_label",
            "@type": [
                "iudx:TextProperty"
            ],
            "rdfs:comment": "User visible label, i.e., something that must be shown to the passenger to help identify the correct vehicle. SameAs: 'label' field from GTFS Realtime message-VehicleDescriptor (https://developers.google.com/transit/gtfs-realtime/reference#message-vehicledescriptor)",
            "rdfs:label": "vehicle_label",
            "rdfs:isDefinedBy": {
                "@id": "iudx:"
            },
            "iudx:domainIncludes": [
                {
                    "@id": "iudx:VehicleDescriptor"
                },
                {
                    "@id": "iudx:FareCollectionSystem"
                }
            ],
            "iudx:rangeIncludes": [
                {
                    "@id": "iudx:Text"
                },
                {
                    "@id": "iudx:ValueDescriptor"
                }
            ],
            "skos:exactMatch": {
                "@id": "GTFS: label"
            }
        },
        {
            "@id": "iudx:versionName",
            "@type": [
                "iudx:TextProperty"
            ],
            "rdfs:comment": "Version name corresponding to this observation",
            "rdfs:label": "versionName",
            "rdfs:isDefinedBy": {
                "@id": "iudx:"
            },
            "iudx:domainIncludes": [
                {
                    "@id": "iudx:Version"
                }
            ],
            "iudx:rangeIncludes": [
                {
                    "@id": "iudx:Text"
                },
                {
                    "@id": "iudx:ValueDescriptor"
                }
            ]
        },
        {
            "@id": "iudx:versionSpec",
            "@type": [
                "iudx:StructuredProperty"
            ],
            "rdfs:comment": "Version specifications or information corresponding to the version in this observation.",
            "rdfs:label": "versionSpec",
            "iudx:domainIncludes": [
                {
                    "@id": "iudx:Version"
                }
            ],
            "iudx:rangeIncludes": [
                {
                    "@id": "iudx:Text"
                },
                {
                    "@id": "iudx:Object"
                },
                {
                    "@id": "iudx:ValueDescriptor"
                }
            ]
        },
        {
            "@id": "iudx:visitDuration",
            "@type": [
                "iudx:TextProperty"
            ],
            "rdfs:comment": "The approximate amount of time required to explore the tourist site corresponding to this observation.",
            "rdfs:label": "visitDuration",
            "rdfs:isDefinedBy": {
                "@id": "iudx:"
            },
            "iudx:domainIncludes": [
                {
                    "@id": "iudx:TouristDestination"
                }
            ],
            "iudx:rangeIncludes": [
                {
                    "@id": "iudx:Text"
                },
                {
                    "@id": "iudx:ValueDescriptor"
                }
            ]
        },
        {
            "@id": "iudx:wardID",
            "@type": [
                "iudx:TextProperty"
            ],
            "rdfs:comment": "Ward ID corresponding to this observation.",
            "rdfs:label": "wardID",
            "rdfs:isDefinedBy": {
                "@id": "iudx:"
            },
            "iudx:domainIncludes": [
                {
                    "@id": "iudx:MunicipalityDesc"
                }
            ],
            "iudx:rangeIncludes": [
                {
                    "@id": "iudx:Text"
                },
                {
                    "@id": "iudx:ValueDescriptor"
                }
            ]
        },
        {
            "@id": "iudx:wardName",
            "@type": [
                "iudx:TextProperty"
            ],
            "rdfs:comment": "Ward name corresponding to this observation.",
            "rdfs:label": "wardName",
            "rdfs:isDefinedBy": {
                "@id": "iudx:"
            },
            "iudx:domainIncludes": [
                {
                    "@id": "iudx:MunicipalityDesc"
                }
            ],
            "iudx:rangeIncludes": [
                {
                    "@id": "iudx:Text"
                },
                {
                    "@id": "iudx:ValueDescriptor"
                }
            ]
        },
        {
            "@id": "iudx:wasteCollectionStatus",
            "@type": [
                "iudx:TextProperty"
            ],
            "rdfs:comment": "The status of the waste collection corresponding to this observation",
            "rdfs:label": "wasteCollectionStatus",
            "rdfs:isDefinedBy": {
                "@id": "iudx:"
            },
            "iudx:domainIncludes": [
                {
                    "@id": "iudx:WmgmtVehicle"
                }
            ],
            "iudx:rangeIncludes": [
                {
                    "@id": "iudx:Text"
                },
                {
                    "@id": "iudx:ValueDescriptor"
                }
            ]
        },
        {
            "@id": "iudx:wasteType",
            "@type": [
                "iudx:TextProperty"
            ],
            "rdfs:comment": "The type of waste corresponding this observation.",
            "rdfs:label": "wasteType",
            "rdfs:isDefinedBy": {
                "@id": "iudx:"
            },
            "iudx:domainIncludes": [
                {
                    "@id": "iudx:WmgmtVehicle"
                }
            ],
            "iudx:rangeIncludes": [
                {
                    "@id": "iudx:Text"
                },
                {
                    "@id": "iudx:ValueDescriptor"
                }
            ]
        },
        {
            "@id": "iudx:weatherType",
            "@type": [
                "iudx:TextProperty"
            ],
            "rdfs:comment": "Observed weather type or status. Represented by a comma separated list of weather types, e.g., cloudy, sunny etc.",
            "rdfs:label": "weatherType",
            "iudx:domainIncludes": [
                {
                    "@id": "iudx:EnvWeather"
                },
                {
                    "@id": "iudx:EnvAQM"
                },
                {
                    "@id": "iudx:AirQuality"
                }
            ],
            "iudx:rangeIncludes": [
                {
                    "@id": "iudx:Text"
                },
                {
                    "@id": "iudx:ValueDescriptor"
                }
            ],
            "rdfs:isDefinedBy": {
                "@id": "iudx:"
            },
            "skos:exactMatch": {
                "@id": "Fiware:weatherType"
            }
        },
        {
            "@id": "iudx:zoneID",
            "@type": [
                "iudx:TextProperty"
            ],
            "rdfs:comment": "Zone ID corresponding to this observation.",
            "rdfs:label": "zoneID",
            "rdfs:isDefinedBy": {
                "@id": "iudx:"
            },
            "iudx:domainIncludes": [
                {
                    "@id": "iudx:MunicipalityDesc"
                },
                {
                    "@id": "iudx:RoadSegment"
                }
            ],
            "iudx:rangeIncludes": [
                {
                    "@id": "iudx:Text"
                },
                {
                    "@id": "iudx:ValueDescriptor"
                }
            ]
        },
        {
            "@id": "iudx:zoneName",
            "@type": [
                "iudx:TextProperty"
            ],
            "rdfs:comment": "Zone name corresponding to this observation.",
            "rdfs:label": "zoneName",
            "rdfs:isDefinedBy": {
                "@id": "iudx:"
            },
            "iudx:domainIncludes": [
                {
                    "@id": "iudx:MunicipalityDesc"
                }
            ],
            "iudx:rangeIncludes": [
                {
                    "@id": "iudx:Text"
                },
                {
                    "@id": "iudx:ValueDescriptor"
                }
            ]
        }
    ],
    "@context": {
        "iudx": "https://voc.iudx.org.in/",
        "owl": "http://www.w3.org/2002/07/owl#",
        "rdf": "http://www.w3.org/1999/02/22-rdf-syntax-ns#",
        "skos": "http://www.w3.org/2004/02/skos/core#",
        "schema": "http://schema.org/",
        "rdfs": "http://www.w3.org/2000/01/rdf-schema#",
        "geojson": "https://purl.org/geojson/vocab#",
        "xsd": "http://www.w3.org/2001/XMLSchema#",
        "qudt": "http://qudt.org/vocab/unit/"
    }
}