{
    "@graph": [
        {
            "@id": "iudx:Intangible",
            "@type": [
                "owl:Class",
                "rdfs:Class"
            ],
            "rdfs:comment": "Class of all intangible things like Structured valued objects etc.",
            "rdfs:label": "Intangible",
            "rdfs:isDefinedBy": {
                "@id": "iudx:"
            },
            "rdfs:subClassOf": {
                "@id": "iudx:Thing"
            }
        },
        {
            "@id": "iudx:Thing",
            "@type": [
                "owl:Class",
                "rdfs:Class"
            ],
            "rdfs:comment": "Most generic IUDX object.",
            "rdfs:label": "Thing",
            "rdfs:isDefinedBy": {
                "@id": "iudx:"
            },
            "skos:exactMatch": {
                "@id": "schema:Thing"
            }
        },
        {
            "@id": "iudx:ValueDescriptor",
            "@type": [
                "owl:Class",
                "rdfs:Class"
            ],
            "rdfs:comment": "Value descriptors are JSON objects that describes the value object for a given property.",
            "rdfs:label": "ValueDescriptor",
            "rdfs:isDefinedBy": {
                "@id": "iudx:"
            },
            "rdfs:subClassOf": {
                "@id": "iudx:Intangible"
            }
        },
        {
            "@id": "iudx:acAvailable",
            "@type": [
                "iudx:TextProperty"
            ],
            "rdfs:comment": "Describes the presence of air conditioning option in the vehicle corresponding to this observation.",
            "rdfs:label": "acAvailable",
            "rdfs:isDefinedBy": {
                "@id": "iudx:"
            },
            "iudx:domainIncludes": [
                {
                    "@id": "iudx:TransitManagement"
                }
            ],
            "iudx:rangeIncludes": [
                {
                    "@id": "iudx:Text"
                },
                {
                    "@id": "iudx:ValueDescriptor"
                }
            ]
        },
        {
            "@id": "iudx:acMode",
            "@type": [
                "iudx:TextProperty"
            ],
            "rdfs:comment": "Describes the mode of operation of the air conditioning system.",
            "rdfs:label": "acMode",
            "rdfs:isDefinedBy": {
                "@id": "iudx:"
            },
            "iudx:domainIncludes": [
                {
                    "@id": "iudx:AirConditioner"
                }
            ],
            "iudx:rangeIncludes": [
                {
                    "@id": "iudx:Text"
                },
                {
                    "@id": "iudx:ValueDescriptor"
                }
            ]
        },
        {
            "@id": "iudx:accessURL",
            "@type": [
                "iudx:TextProperty"
            ],
            "rdfs:comment": "The IRI pointing to the domain from which data can be accessed.",
            "rdfs:label": "accessURL",
            "iudx:domainIncludes": [
                {
                    "@id": "iudx:HTTPAccess"
                },
                {
                    "@id": "iudx:FileAccess"
                },
                {
                    "@id": "iudx:StreamingAccess"
                }
            ],
            "iudx:rangeIncludes": [
                {
                    "@id": "iudx:Text"
                },
                {
                    "@id": "iudx:ValueDescriptor"
                }
            ],
            "rdfs:isDefinedBy": {
                "@id": "iudx:"
            }
        },
        {
            "@id": "iudx:activePower",
            "@type": [
                "iudx:QuantitativeProperty"
            ],
            "rdfs:comment": "Active power consumed per phase. Ordered triple comprising of active power from three phases in the following order: [R Y B]",
            "rdfs:label": "activePower",
            "rdfs:isDefinedBy": {
                "@id": "iudx:"
            },
            "iudx:domainIncludes": [
                {
                    "@id": "iudx:StreetLightFeeder"
                },
                {
                    "@id": "iudx:SolarEnergy"
                }
            ],
            "iudx:rangeIncludes": [
                {
                    "@id": "iudx:NumericArray"
                },
                {
                    "@id": "iudx:ValueDescriptor"
                }
            ],
            "skos:exactMatch": {
                "@id": "Fiware:activePower"
            }
        },
        {
            "@id": "iudx:address",
            "@type": [
                "iudx:GeoProperty"
            ],
            "rdfs:comment": "Physical address of a place.",
            "rdfs:label": "address",
            "iudx:domainIncludes": [
                {
                    "@id": "iudx:Place"
                },
                {
                    "@id": "iudx:PointOfInterest"
                },
                {
                    "@id": "iudx:IssueReporting"
                },
                {
                    "@id": "iudx:Streetlight"
                },
                {
                    "@id": "iudx:BikeDockingStation"
                },
                {
                    "@id": "iudx:WaterDistributionNetwork"
                },
                {
                    "@id": "iudx:RevenueCollection"
                },
                {
                    "@id": "iudx:EmergencyVehicle"
                },
                {
                    "@id": "iudx:EVChargingStation"
                },
                {
                    "@id": "iudx:MosquitoDensity"
                },
                {
                    "@id": "iudx:TouristDestination"
                },
                {
                    "@id": "iudx:WmgmtVehicle"
                }
            ],
            "iudx:rangeIncludes": [
                {
                    "@id": "iudx:Text"
                },
                {
                    "@id": "iudx:ValueDescriptor"
                }
            ],
            "rdfs:isDefinedBy": {
                "@id": "iudx:"
            },
            "skos:exactMatch": {
                "@id": "schema:address"
            }
        },
        {
            "@id": "iudx:agency_email",
            "@type": [
                "iudx:TextProperty"
            ],
            "rdfs:comment": "Email address actively monitored by the agency\u2019s customer service department. SameAs: 'agency_email' field from GTFS Static Field Definition - agency.txt (https://developers.google.com/transit/gtfs/reference#agencytxt)",
            "rdfs:label": "agency_email",
            "rdfs:isDefinedBy": {
                "@id": "iudx:"
            },
            "iudx:domainIncludes": [
                {
                    "@id": "iudx:AgencyDesc"
                }
            ],
            "iudx:rangeIncludes": [
                {
                    "@id": "iudx:Text"
                },
                {
                    "@id": "iudx:ValueDescriptor"
                }
            ],
            "skos:exactMatch": {
                "@id": "GTFS: agency_email"
            }
        },
        {
            "@id": "iudx:agency_fare_url",
            "@type": [
                "iudx:TextProperty"
            ],
            "rdfs:comment": "URL of a web page that contains the details of the fares and also could allow to purchase tickets for that agency online. SameAs: 'agency_fare_url' field from GTFS Static Field Definition - agency.txt (https://developers.google.com/transit/gtfs/reference#agencytxt)",
            "rdfs:label": "agency_fare_url",
            "rdfs:isDefinedBy": {
                "@id": "iudx:"
            },
            "iudx:domainIncludes": [
                {
                    "@id": "iudx:AgencyDesc"
                }
            ],
            "iudx:rangeIncludes": [
                {
                    "@id": "iudx:Text"
                },
                {
                    "@id": "iudx:ValueDescriptor"
                }
            ],
            "skos:exactMatch": {
                "@id": "GTFS: agency_fare_url"
            }
        },
        {
            "@id": "iudx:agency_id",
            "@type": [
                "iudx:TextProperty"
            ],
            "rdfs:comment": "ID that uniquely identifies a transit agency. A transit feed may represent data from more than one agency. The agency_id is dataset unique. This field is optional for transit feeds that only contain data for a single agency. SameAs: 'agency_id' field from GTFS Static Field Definition - agency.txt (https://developers.google.com/transit/gtfs/reference#agencytxt)",
            "rdfs:label": "agency_id",
            "rdfs:isDefinedBy": {
                "@id": "iudx:"
            },
            "iudx:domainIncludes": [
                {
                    "@id": "iudx:AgencyDesc"
                }
            ],
            "iudx:rangeIncludes": [
                {
                    "@id": "iudx:Text"
                },
                {
                    "@id": "iudx:ValueDescriptor"
                }
            ],
            "skos:exactMatch": {
                "@id": "GTFS: agency_id"
            }
        },
        {
            "@id": "iudx:agency_lang",
            "@type": [
                "iudx:TextProperty"
            ],
            "rdfs:comment": "Contains a two-letter ISO 639-1 code for the primary language used by this transit agency. The language code is case-insensitive (both en and EN are accepted). SameAs: 'agency_lang' field from GTFS Static Field Definition - agency.txt (https://developers.google.com/transit/gtfs/reference#agencytxt)",
            "rdfs:label": "agency_lang",
            "rdfs:isDefinedBy": {
                "@id": "iudx:"
            },
            "iudx:domainIncludes": [
                {
                    "@id": "iudx:AgencyDesc"
                }
            ],
            "iudx:rangeIncludes": [
                {
                    "@id": "iudx:Text"
                },
                {
                    "@id": "iudx:ValueDescriptor"
                }
            ],
            "skos:exactMatch": {
                "@id": "GTFS: agency_lang"
            }
        },
        {
            "@id": "iudx:agency_name",
            "@type": [
                "iudx:TextProperty"
            ],
            "rdfs:comment": "The agency_name field contains the full name of the transit agency. SameAs: 'agency_name' field from GTFS Static Field Definition - agency.txt (https://developers.google.com/transit/gtfs/reference#agencytxt)",
            "rdfs:label": "agency_name",
            "rdfs:isDefinedBy": {
                "@id": "iudx:"
            },
            "iudx:domainIncludes": [
                {
                    "@id": "iudx:AgencyDesc"
                }
            ],
            "iudx:rangeIncludes": [
                {
                    "@id": "iudx:Text"
                },
                {
                    "@id": "iudx:ValueDescriptor"
                }
            ],
            "skos:exactMatch": {
                "@id": "GTFS: agency_name"
            }
        },
        {
            "@id": "iudx:agency_phone",
            "@type": [
                "iudx:TextProperty"
            ],
            "rdfs:comment": "A voice telephone number for the specified agency.SameAs: 'agency_phone' field from GTFS Static Field Definition - agency.txt (https://developers.google.com/transit/gtfs/reference#agencytxt)",
            "rdfs:label": "agency_phone",
            "rdfs:isDefinedBy": {
                "@id": "iudx:"
            },
            "iudx:domainIncludes": [
                {
                    "@id": "iudx:AgencyDesc"
                }
            ],
            "iudx:rangeIncludes": [
                {
                    "@id": "iudx:Text"
                },
                {
                    "@id": "iudx:ValueDescriptor"
                }
            ],
            "skos:exactMatch": {
                "@id": "GTFS: agency_phone"
            }
        },
        {
            "@id": "iudx:agency_timezone",
            "@type": [
                "iudx:TextProperty"
            ],
            "rdfs:comment": "Timezone field contains the timezone where the transit agency is located. SameAs: 'agency_timezone' field from GTFS Static Field Definition - agency.txt (https://developers.google.com/transit/gtfs/reference#agencytxt)",
            "rdfs:label": "agency_timezone",
            "rdfs:isDefinedBy": {
                "@id": "iudx:"
            },
            "iudx:domainIncludes": [
                {
                    "@id": "iudx:AgencyDesc"
                }
            ],
            "iudx:rangeIncludes": [
                {
                    "@id": "iudx:Text"
                },
                {
                    "@id": "iudx:ValueDescriptor"
                }
            ],
            "skos:exactMatch": {
                "@id": "GTFS:agency_timezone"
            }
        },
        {
            "@id": "iudx:agency_url",
            "@type": [
                "iudx:TextProperty"
            ],
            "rdfs:comment": "The agency_url field contains the URL of the transit agency. SameAs: 'agency_url' field from GTFS Static Field Definition - agency.txt (https://developers.google.com/transit/gtfs/reference#agencytxt)",
            "rdfs:label": "agency_url",
            "iudx:domainIncludes": [
                {
                    "@id": "iudx:AgencyDesc"
                },
                {
                    "@id": "iudx:TouristDestination"
                }
            ],
            "iudx:rangeIncludes": [
                {
                    "@id": "iudx:Text"
                },
                {
                    "@id": "iudx:ValueDescriptor"
                }
            ],
            "rdfs:isDefinedBy": {
                "@id": "iudx:"
            },
            "skos:exactMatch": {
                "@id": "GTFS: agency_url"
            }
        },
        {
            "@id": "iudx:aggregationDuration",
            "@type": [
                "iudx:QuantitativeProperty"
            ],
            "rdfs:comment": "Specifies the interval duration for computing statistical aggregations. Default duration interval unit is in Hours. Other units can be specified using ValueDescriptor Type.",
            "rdfs:label": "aggregationDuration",
            "iudx:domainIncludes": [
                {
                    "@id": "iudx:ValueDescriptor"
                }
            ],
            "iudx:rangeIncludes": [
                {
                    "@id": "iudx:Number"
                },
                {
                    "@id": "iudx:ValueDescriptor"
                }
            ],
            "rdfs:isDefinedBy": {
                "@id": "iudx:"
            }
        },
        {
            "@id": "iudx:airDirection",
            "@type": [
                "iudx:QuantitativeProperty"
            ],
            "rdfs:comment": "Represents the air direction status as an analog input.",
            "rdfs:label": "airDirection",
            "rdfs:isDefinedBy": {
                "@id": "iudx:"
            },
            "iudx:domainIncludes": [
                {
                    "@id": "iudx:AirConditioner"
                }
            ],
            "iudx:rangeIncludes": [
                {
                    "@id": "iudx:Number"
                },
                {
                    "@id": "iudx:ValueDescriptor"
                }
            ]
        },
        {
            "@id": "iudx:airFlowRate",
            "@type": [
                "iudx:TextProperty"
            ],
            "rdfs:comment": "Describes the rate of air flow corresponding to this observation.",
            "rdfs:label": "airFlowRate",
            "rdfs:isDefinedBy": {
                "@id": "iudx:"
            },
            "iudx:domainIncludes": [
                {
                    "@id": "iudx:AirConditioner"
                }
            ],
            "iudx:rangeIncludes": [
                {
                    "@id": "iudx:Text"
                },
                {
                    "@id": "iudx:ValueDescriptor"
                }
            ]
        },
        {
            "@id": "iudx:airQualityIndex",
            "@type": [
                "iudx:QuantitativeProperty"
            ],
            "rdfs:comment": "Overall Air Quality Index (AQI) for the observed air quality.",
            "rdfs:label": "airQualityIndex",
            "iudx:domainIncludes": [
                {
                    "@id": "iudx:EnvWeather"
                },
                {
                    "@id": "iudx:EnvAQM"
                },
                {
                    "@id": "iudx:AirQuality"
                }
            ],
            "iudx:rangeIncludes": [
                {
                    "@id": "iudx:Number"
                },
                {
                    "@id": "iudx:ValueDescriptor"
                }
            ],
            "rdfs:isDefinedBy": {
                "@id": "iudx:"
            }
        },
        {
            "@id": "iudx:airQualityIndexForecast",
            "@type": [
                "iudx:QuantitativeProperty"
            ],
            "rdfs:comment": "Forecasted overall Air Quality Index (AQI) over a certain duration in future.",
            "rdfs:label": "airQualityIndexForecast",
            "rdfs:isDefinedBy": {
                "@id": "iudx:"
            },
            "iudx:domainIncludes": [
                {
                    "@id": "iudx:EnvWeather"
                }
            ],
            "iudx:rangeIncludes": [
                {
                    "@id": "iudx:Number"
                },
                {
                    "@id": "iudx:ValueDescriptor"
                }
            ]
        },
        {
            "@id": "iudx:airQualityLevel",
            "@type": [
                "iudx:TextProperty"
            ],
            "rdfs:comment": "Air Quality Category Indication. Qualitative level defined according to the local health agencies. For example, 'GOOD', 'MODERATE', 'POOR', 'UNHEALTHY', 'SEVERE', 'HAZARDOUS' etc.",
            "rdfs:label": "airQualityLevel",
            "iudx:domainIncludes": [
                {
                    "@id": "iudx:EnvAQM"
                },
                {
                    "@id": "iudx:AirQuality"
                }
            ],
            "iudx:rangeIncludes": [
                {
                    "@id": "iudx:Text"
                },
                {
                    "@id": "iudx:ValueDescriptor"
                }
            ],
            "rdfs:isDefinedBy": {
                "@id": "iudx:"
            },
            "skos:exactMatch": {
                "@id": "Fiware:airQualityLevel"
            }
        },
        {
            "@id": "iudx:airTemperatureForecast",
            "@type": [
                "iudx:QuantitativeProperty"
            ],
            "rdfs:comment": "Forecasted value of air temperature over a certain duration in future.",
            "rdfs:label": "airTemperatureForecast",
            "rdfs:isDefinedBy": {
                "@id": "iudx:"
            },
            "iudx:domainIncludes": [
                {
                    "@id": "iudx:EnvWeather"
                }
            ],
            "iudx:rangeIncludes": [
                {
                    "@id": "iudx:Number"
                },
                {
                    "@id": "iudx:ValueDescriptor"
                }
            ]
        },
        {
            "@id": "iudx:alarmStatus",
            "@type": [
                "iudx:QuantitativeProperty"
            ],
            "rdfs:comment": "Describes the alarm status of the air conditioning system by a binary Input (0-Inactive, 1-Active)",
            "rdfs:label": "alarmStatus",
            "rdfs:isDefinedBy": {
                "@id": "iudx:"
            },
            "iudx:domainIncludes": [
                {
                    "@id": "iudx:AirConditioner"
                }
            ],
            "iudx:rangeIncludes": [
                {
                    "@id": "iudx:Number"
                },
                {
                    "@id": "iudx:ValueDescriptor"
                }
            ]
        },
        {
            "@id": "iudx:alertLevel",
            "@type": [
                "iudx:QuantitativeProperty"
            ],
            "rdfs:comment": "Reference alert level threshold value set for the sensing station corresponding to this observation. An Alert signal is generated if the current level crosses the alert level threshold value.",
            "rdfs:label": "alertLevel",
            "rdfs:isDefinedBy": {
                "@id": "iudx:"
            },
            "iudx:domainIncludes": [
                {
                    "@id": "iudx:EnvFlood"
                }
            ],
            "iudx:rangeIncludes": [
                {
                    "@id": "iudx:Number"
                },
                {
                    "@id": "iudx:ValueDescriptor"
                }
            ]
        },
        {
            "@id": "iudx:allowedVehicleType",
            "@type": [
                "iudx:TextProperty"
            ],
            "rdfs:comment": "Represents the vehicle type(s) allowed to ply on the road segment corresponding to this observation.",
            "rdfs:label": "allowedVehicleType",
            "rdfs:isDefinedBy": {
                "@id": "iudx:"
            },
            "iudx:domainIncludes": [
                {
                    "@id": "iudx:RoadSegment"
                }
            ],
            "iudx:rangeIncludes": [
                {
                    "@id": "iudx:Text"
                },
                {
                    "@id": "iudx:ValueDescriptor"
                }
            ],
            "skos:exactMatch": {
                "@id": "Fiware: allowedVehicleType"
            }
        },
        {
            "@id": "iudx:amountCollected",
            "@type": [
                "iudx:QuantitativeProperty"
            ],
            "rdfs:comment": "Amount collected towards the service corresponding to this observation.",
            "rdfs:label": "amountCollected",
            "rdfs:isDefinedBy": {
                "@id": "iudx:"
            },
            "iudx:domainIncludes": [
                {
                    "@id": "iudx:RevenueCollection"
                },
                {
                    "@id": "iudx:TrafficViolations"
                },
                {
                    "@id": "iudx:EVChargingStation"
                },
                {
                    "@id": "iudx:BikeDockingStation"
                }
            ],
            "iudx:rangeIncludes": [
                {
                    "@id": "iudx:Number"
                },
                {
                    "@id": "iudx:ValueDescriptor"
                }
            ]
        },
        {
            "@id": "iudx:annotatedMap",
            "@type": [
                "iudx:TextProperty"
            ],
            "rdfs:comment": "Annotated map view indicating the orientations for the camera corresponding to this observation",
            "rdfs:label": "annotatedMap",
            "rdfs:isDefinedBy": {
                "@id": "iudx:"
            },
            "iudx:domainIncludes": [
                {
                    "@id": "iudx:Orientation"
                }
            ],
            "iudx:rangeIncludes": [
                {
                    "@id": "iudx:Text"
                },
                {
                    "@id": "iudx:ValueDescriptor"
                }
            ]
        },
        {
            "@id": "iudx:apparentPower",
            "@type": [
                "iudx:QuantitativeProperty"
            ],
            "rdfs:comment": "Apparent power consumed per phase. Ordered triple comprising of active power from three phases in the following order: [R Y B]",
            "rdfs:label": "apparentPower",
            "rdfs:isDefinedBy": {
                "@id": "iudx:"
            },
            "iudx:domainIncludes": [
                {
                    "@id": "iudx:StreetLightFeeder"
                },
                {
                    "@id": "iudx:SolarEnergy"
                }
            ],
            "iudx:rangeIncludes": [
                {
                    "@id": "iudx:NumericArray"
                },
                {
                    "@id": "iudx:ValueDescriptor"
                }
            ],
            "skos:exactMatch": {
                "@id": "Fiware: apparentPower"
            }
        },
        {
            "@id": "iudx:aqiMajorPollutant",
            "@type": [
                "iudx:TextProperty"
            ],
            "rdfs:comment": "Major pollutant in the Air Quality Index (AQI).",
            "rdfs:label": "aqiMajorPollutant",
            "iudx:domainIncludes": [
                {
                    "@id": "iudx:EnvWeather"
                },
                {
                    "@id": "iudx:EnvAQM"
                },
                {
                    "@id": "iudx:AirQuality"
                }
            ],
            "iudx:rangeIncludes": [
                {
                    "@id": "iudx:Text"
                },
                {
                    "@id": "iudx:ValueDescriptor"
                }
            ],
            "rdfs:isDefinedBy": {
                "@id": "iudx:"
            }
        },
        {
            "@id": "iudx:aqiMajorPollutantForecast",
            "@type": [
                "iudx:TextProperty"
            ],
            "rdfs:comment": "Forecasted major air pollutant in the Air Quality Index (AQI) over a certain duration in future.",
            "rdfs:label": "aqiMajorPollutantForecast",
            "rdfs:isDefinedBy": {
                "@id": "iudx:"
            },
            "iudx:domainIncludes": [
                {
                    "@id": "iudx:EnvWeather"
                }
            ],
            "iudx:rangeIncludes": [
                {
                    "@id": "iudx:Text"
                },
                {
                    "@id": "iudx:ValueDescriptor"
                }
            ]
        },
        {
            "@id": "iudx:area",
            "@type": [
                "iudx:QuantitativeProperty"
            ],
            "rdfs:comment": "The total area of the entity corresponding to this observation.",
            "rdfs:label": "area",
            "rdfs:isDefinedBy": {
                "@id": "iudx:"
            },
            "iudx:domainIncludes": [
                {
                    "@id": "iudx:Headquarters"
                }
            ],
            "iudx:rangeIncludes": [
                {
                    "@id": "iudx:Number"
                },
                {
                    "@id": "iudx:ValueDescriptor"
                }
            ]
        },
        {
            "@id": "iudx:arrivalUncertainty",
            "@type": [
                "iudx:QuantitativeProperty"
            ],
            "rdfs:comment": "If schedule_relationship is empty or SCHEDULED, either arrival or departure must be provided within a StopTimeUpdate. SameAs: 'arrival' field from GTFS Realtime message-StopTimeUpdate (https://developers.google.com/transit/gtfs-realtime/reference#message-stoptimeupdate)",
            "rdfs:label": "arrivalUncertainty",
            "rdfs:isDefinedBy": {
                "@id": "iudx:"
            },
            "iudx:domainIncludes": [
                {
                    "@id": "iudx:TransitManagement"
                }
            ],
            "iudx:rangeIncludes": [
                {
                    "@id": "iudx:Number"
                },
                {
                    "@id": "iudx:ValueDescriptor"
                }
            ]
        },
        {
            "@id": "iudx:arrival_time",
            "@type": [
                "iudx:TimeProperty"
            ],
            "rdfs:comment": "Specifies the arrival time at a specific stop for a specific trip on a route. Times must be eight digits in HH:MM:SS format (HH:MM:SS is also accepted, if the hour begins with 0). Note: Trips that span multiple dates will have stop times greater than 24:00:00. For example, if a trip begins at 10:30:00 p.m. and ends at 2:15:00 a.m. on the following day, the stop times would be 22:30:00 and 26:15:00. Entering those stop times as 22:30:00 and 02:15:00 would not produce the desired results. SameAs: 'arrival_time' field from GTFS Static Field definitions-stop_times.txt (https://developers.google.com/transit/gtfs/reference#stop_timestxt)",
            "rdfs:label": "arrival_time",
            "rdfs:isDefinedBy": {
                "@id": "iudx:"
            },
            "iudx:domainIncludes": [
                {
                    "@id": "iudx:StopTimesDesc"
                }
            ],
            "iudx:rangeIncludes": [
                {
                    "@id": "iudx:Text"
                },
                {
                    "@id": "iudx:ValueDescriptor"
                }
            ],
            "skos:exactMatch": {
                "@id": "GTFS: arrival_time"
            }
        },
        {
            "@id": "iudx:atmosphericPressure",
            "@type": [
                "iudx:QuantitativeProperty"
            ],
            "rdfs:comment": "Observed air (atmospheric or barometric) pressure.",
            "rdfs:label": "atmosphericPressure",
            "iudx:domainIncludes": [
                {
                    "@id": "iudx:EnvWeather"
                },
                {
                    "@id": "iudx:EnvAQM"
                },
                {
                    "@id": "iudx:AirQuality"
                }
            ],
            "iudx:rangeIncludes": [
                {
                    "@id": "iudx:Number"
                },
                {
                    "@id": "iudx:ValueDescriptor"
                }
            ],
            "rdfs:isDefinedBy": {
                "@id": "iudx:"
            },
            "skos:exactMatch": {
                "@id": "Fiware:atmosphericPressure"
            }
        },
        {
            "@id": "iudx:availableBikeNumber",
            "@type": [
                "iudx:QuantitativeProperty"
            ],
            "rdfs:comment": "The number of bikes available in the bike hire docking station to be hired by users.",
            "rdfs:label": "availableBikeNumber",
            "rdfs:isDefinedBy": {
                "@id": "iudx:"
            },
            "iudx:domainIncludes": [
                {
                    "@id": "iudx:BikeDockingStation"
                }
            ],
            "iudx:rangeIncludes": [
                {
                    "@id": "iudx:Number"
                },
                {
                    "@id": "iudx:ValueDescriptor"
                }
            ],
            "skos:exactMatch": {
                "@id": "Fiware:availableBikeNumber"
            }
        },
        {
            "@id": "iudx:availableSpotNumber",
            "@type": [
                "iudx:QuantitativeProperty"
            ],
            "rdfs:comment": "Number of parking spots available for use in the smart parking site corresponding to this observation. This must a positve number lower than or equal to the totalSpotNumber.",
            "rdfs:label": "availableSpotNumber",
            "rdfs:isDefinedBy": {
                "@id": "iudx:"
            },
            "iudx:domainIncludes": [
                {
                    "@id": "iudx:ParkingSpotStatus"
                }
            ],
            "iudx:rangeIncludes": [
                {
                    "@id": "iudx:Number"
                },
                {
                    "@id": "iudx:ValueDescriptor"
                }
            ],
            "skos:exactMatch": {
                "@id": "Fiware: OffStreetParking.availableSpotNumber"
            }
        },
        {
            "@id": "iudx:averageSpotLength",
            "@type": [
                "iudx:QuantitativeProperty"
            ],
            "rdfs:comment": "The average length of parking spots in the parking site corresponding to this observation.",
            "rdfs:label": "averageSpotLength",
            "rdfs:isDefinedBy": {
                "@id": "iudx:"
            },
            "iudx:domainIncludes": [
                {
                    "@id": "iudx:SmartParking"
                }
            ],
            "iudx:rangeIncludes": [
                {
                    "@id": "iudx:Number"
                },
                {
                    "@id": "iudx:ValueDescriptor"
                }
            ],
            "skos:exactMatch": {
                "@id": "Fiware: OffStreetParking.averageSpotLength"
            }
        },
        {
            "@id": "iudx:averageSpotWidth",
            "@type": [
                "iudx:QuantitativeProperty"
            ],
            "rdfs:comment": "The average width of parking spots in the parking site corresponding to this observation.",
            "rdfs:label": "averageSpotWidth",
            "rdfs:isDefinedBy": {
                "@id": "iudx:"
            },
            "iudx:domainIncludes": [
                {
                    "@id": "iudx:SmartParking"
                }
            ],
            "iudx:rangeIncludes": [
                {
                    "@id": "iudx:Number"
                },
                {
                    "@id": "iudx:ValueDescriptor"
                }
            ],
            "skos:exactMatch": {
                "@id": "Fiware: OffStreetParking.averageSpotWidth"
            }
        },
        {
            "@id": "iudx:avgOverTime",
            "@type": [
                "iudx:QuantitativeProperty"
            ],
            "rdfs:comment": "Describes the average value of a time-series data over a specified duration in past. The duration is specified using another parameter in the value descriptor object related to this value",
            "rdfs:label": "avgOverTime",
            "iudx:domainIncludes": [
                {
                    "@id": "iudx:TimeSeriesAggregation"
                }
            ],
            "iudx:rangeIncludes": [
                {
                    "@id": "iudx:Number"
                },
                {
                    "@id": "iudx:ValueDescriptor"
                }
            ]
        },
        {
            "@id": "iudx:bearing",
            "@type": [
                "iudx:QuantitativeProperty"
            ],
            "rdfs:comment": "Gives the vehicle GPS angle measured in a clockwise direction from the True North. SameAs 'bearing' field from GTFS Realtime message-Position(https://developers.google.com/transit/gtfs-realtime/reference#message-position)",
            "rdfs:label": "bearing",
            "rdfs:isDefinedBy": {
                "@id": "iudx:"
            },
            "iudx:domainIncludes": [
                {
                    "@id": "iudx:Position"
                },
                {
                    "@id": "iudx:WmgmtVehicle"
                },
                {
                    "@id": "iudx:EmergencyVehicle"
                }
            ],
            "iudx:rangeIncludes": [
                {
                    "@id": "iudx:Number"
                },
                {
                    "@id": "iudx:ValueDescriptor"
                }
            ],
            "skos:exactMatch": {
                "@id": "GTFS: bearing"
            }
        },
        {
            "@id": "iudx:beneficiaryCount",
            "@type": [
                "iudx:QuantitativeProperty"
            ],
            "rdfs:comment": "Represents the count of people benifited under the scheme corresponding to this observation.",
            "rdfs:label": "beneficiaryCount",
            "rdfs:isDefinedBy": {
                "@id": "iudx:"
            },
            "iudx:domainIncludes": [
                {
                    "@id": "iudx:PublicSchemes"
                }
            ],
            "iudx:rangeIncludes": [
                {
                    "@id": "iudx:Number"
                },
                {
                    "@id": "iudx:ValueDescriptor"
                }
            ]
        },
        {
            "@id": "iudx:bikeType",
            "@type": [
                "iudx:TextProperty"
            ],
            "rdfs:comment": "Type of the bike corresponding to this observation. ENUM: [ELECTRIC BIKE, BICYCLE, STANDARD BIKE, GEARLESS BIKE, ELECTRIC BICYCLE, HYBRID BIKE, MOPED BIKE, MOPED BICYCLE, SPECIALITY BIKE].",
            "rdfs:label": "bikeType",
            "rdfs:isDefinedBy": {
                "@id": "iudx:"
            },
            "iudx:domainIncludes": [
                {
                    "@id": "iudx:BikeDockingStation"
                }
            ],
            "iudx:rangeIncludes": [
                {
                    "@id": "iudx:Text"
                },
                {
                    "@id": "iudx:ValueDescriptor"
                }
            ]
        },
        {
            "@id": "iudx:binCapacity",
            "@type": [
                "iudx:QuantitativeProperty"
            ],
            "rdfs:comment": "Total capacity in terms of the volume of waste the bin can hold.",
            "rdfs:label": "binCapacity",
            "rdfs:isDefinedBy": {
                "@id": "iudx:"
            },
            "iudx:domainIncludes": [
                {
                    "@id": "iudx:WmgmtBin"
                },
                {
                    "@id": "iudx:WasteBinModel"
                }
            ],
            "iudx:rangeIncludes": [
                {
                    "@id": "iudx:Number"
                },
                {
                    "@id": "iudx:ValueDescriptor"
                }
            ],
            "skos:exactMatch": {
                "@id": "fiware:cargoVolume"
            }
        },
        {
            "@id": "iudx:binCategory",
            "@type": [
                "iudx:TextProperty"
            ],
            "rdfs:comment": "Category/type of the waste container bin. It can be a household bin or a dumpster or any other pre-defined category/type.",
            "rdfs:label": "binCategory",
            "rdfs:isDefinedBy": {
                "@id": "iudx:"
            },
            "iudx:domainIncludes": [
                {
                    "@id": "iudx:WmgmtBin"
                },
                {
                    "@id": "iudx:WasteBinModel"
                }
            ],
            "iudx:rangeIncludes": [
                {
                    "@id": "iudx:Text"
                },
                {
                    "@id": "iudx:ValueDescriptor"
                }
            ]
        },
        {
            "@id": "iudx:binColor",
            "@type": [
                "iudx:TextProperty"
            ],
            "rdfs:comment": "Color of the bin. Could be used for indicating the type of waste. The color coding should follow the conventions applicable to the geographical area the bins are located.",
            "rdfs:label": "binColor",
            "rdfs:isDefinedBy": {
                "@id": "iudx:"
            },
            "iudx:domainIncludes": [
                {
                    "@id": "iudx:WmgmtBin"
                },
                {
                    "@id": "iudx:WasteBinModel"
                }
            ],
            "iudx:rangeIncludes": [
                {
                    "@id": "iudx:Text"
                },
                {
                    "@id": "iudx:ValueDescriptor"
                }
            ],
            "skos:exactMatch": {
                "@id": "fiware:color"
            }
        },
        {
            "@id": "iudx:binFillingLevel",
            "@type": [
                "iudx:QuantitativeProperty"
            ],
            "rdfs:comment": "Current level of waste in the bin. Typically, the level is specified in terms of percentage volume filled.",
            "rdfs:label": "binFillingLevel",
            "rdfs:isDefinedBy": {
                "@id": "iudx:"
            },
            "iudx:domainIncludes": [
                {
                    "@id": "iudx:WmgmtBin"
                }
            ],
            "iudx:rangeIncludes": [
                {
                    "@id": "iudx:Number"
                },
                {
                    "@id": "iudx:ValueDescriptor"
                }
            ],
            "skos:exactMatch": {
                "@id": "fiware:fillingLevel"
            }
        },
        {
            "@id": "iudx:binFullnessThreshold",
            "@type": [
                "iudx:QuantitativeProperty"
            ],
            "rdfs:comment": "The fullness threshold level of the bin defined as the level (in terms of percentage) when the bin full alert or notification will be generated.",
            "rdfs:label": "binFullnessThreshold",
            "rdfs:isDefinedBy": {
                "@id": "iudx:"
            },
            "iudx:domainIncludes": [
                {
                    "@id": "iudx:WmgmtBin"
                },
                {
                    "@id": "iudx:WasteBinModel"
                }
            ],
            "iudx:rangeIncludes": [
                {
                    "@id": "iudx:Number"
                },
                {
                    "@id": "iudx:ValueDescriptor"
                }
            ],
            "skos:exactMatch": {
                "@id": "fiware:fullnessThreshold"
            }
        },
        {
            "@id": "iudx:binID",
            "@type": [
                "iudx:TextProperty"
            ],
            "rdfs:comment": "ID of the waste carrying bin",
            "rdfs:label": "binID",
            "rdfs:isDefinedBy": {
                "@id": "iudx:"
            },
            "iudx:domainIncludes": [
                {
                    "@id": "iudx:WmgmtBin"
                }
            ],
            "iudx:rangeIncludes": [
                {
                    "@id": "iudx:Text"
                },
                {
                    "@id": "iudx:ValueDescriptor"
                }
            ]
        },
        {
            "@id": "iudx:binMaxLoad",
            "@type": [
                "iudx:QuantitativeProperty"
            ],
            "rdfs:comment": "Maximum load (weight) that the waste bin can hold.",
            "rdfs:label": "binMaxLoad",
            "rdfs:isDefinedBy": {
                "@id": "iudx:"
            },
            "iudx:domainIncludes": [
                {
                    "@id": "iudx:WmgmtBin"
                },
                {
                    "@id": "iudx:WasteBinModel"
                }
            ],
            "iudx:rangeIncludes": [
                {
                    "@id": "iudx:Number"
                },
                {
                    "@id": "iudx:ValueDescriptor"
                }
            ],
            "skos:exactMatch": {
                "@id": "fiware:maximumLoad"
            }
        },
        {
            "@id": "iudx:binRecommendedLoad",
            "@type": [
                "iudx:QuantitativeProperty"
            ],
            "rdfs:comment": "Recommended load (weight) that the waste bin corresponding to this observation can hold.",
            "rdfs:label": "binRecommendedLoad",
            "rdfs:isDefinedBy": {
                "@id": "iudx:"
            },
            "iudx:domainIncludes": [
                {
                    "@id": "iudx:WmgmtBin"
                },
                {
                    "@id": "iudx:WasteBinModel"
                }
            ],
            "iudx:rangeIncludes": [
                {
                    "@id": "iudx:Number"
                },
                {
                    "@id": "iudx:ValueDescriptor"
                }
            ],
            "skos:exactMatch": {
                "@id": "fiware:recommendedLoad"
            }
        },
        {
            "@id": "iudx:bod",
            "@type": [
                "iudx:QuantitativeProperty"
            ],
            "rdfs:comment": "Biological Oxygen Demand concentration measured in the waste-water treatment plant corresponding to this observation.",
            "rdfs:label": "bod",
            "rdfs:isDefinedBy": {
                "@id": "iudx:"
            },
            "iudx:domainIncludes": [
                {
                    "@id": "iudx:WasteWaterMgmt"
                }
            ],
            "iudx:rangeIncludes": [
                {
                    "@id": "iudx:Number"
                },
                {
                    "@id": "iudx:ValueDescriptor"
                }
            ],
            "skos:exactMatch": {
                "@id": "fiware:bod"
            }
        },
        {
            "@id": "iudx:bridgeCount",
            "@type": [
                "iudx:QuantitativeProperty"
            ],
            "rdfs:comment": "Number of bridges in the road segment corresponding to this observation. Takes 0 (zero) as the value when the road segment has no bridges.",
            "rdfs:label": "bridgeCount",
            "rdfs:isDefinedBy": {
                "@id": "iudx:"
            },
            "iudx:domainIncludes": [
                {
                    "@id": "iudx:RoadSegment"
                }
            ],
            "iudx:rangeIncludes": [
                {
                    "@id": "iudx:Number"
                },
                {
                    "@id": "iudx:ValueDescriptor"
                }
            ]
        },
        {
            "@id": "iudx:cameraName",
            "@type": [
                "iudx:TextProperty"
            ],
            "rdfs:comment": "Name of the camera corresponding to this observation",
            "rdfs:label": "cameraName",
            "rdfs:isDefinedBy": {
                "@id": "iudx:"
            },
            "iudx:domainIncludes": [
                {
                    "@id": "iudx:Camera"
                }
            ],
            "iudx:rangeIncludes": [
                {
                    "@id": "iudx:Text"
                },
                {
                    "@id": "iudx:ValueDescriptor"
                }
            ]
        },
        {
            "@id": "iudx:cameraNum",
            "@type": [
                "iudx:QuantitativeProperty"
            ],
            "rdfs:comment": "Camera number corresponding to this observation",
            "rdfs:label": "cameraNum",
            "rdfs:isDefinedBy": {
                "@id": "iudx:"
            },
            "iudx:domainIncludes": [
                {
                    "@id": "iudx:Camera"
                }
            ],
            "iudx:rangeIncludes": [
                {
                    "@id": "iudx:Number"
                },
                {
                    "@id": "iudx:ValueDescriptor"
                }
            ]
        },
        {
            "@id": "iudx:cameraType",
            "@type": [
                "iudx:TextProperty"
            ],
            "rdfs:comment": "Type of the camera corresponding to this observation. ENUM: [FIXED, PTZ, DOME, DAY/NIGHT, C-MOUNT, BULLET].",
            "rdfs:label": "cameraType",
            "rdfs:isDefinedBy": {
                "@id": "iudx:"
            },
            "iudx:domainIncludes": [
                {
                    "@id": "iudx:Camera"
                }
            ],
            "iudx:rangeIncludes": [
                {
                    "@id": "iudx:Text"
                },
                {
                    "@id": "iudx:ValueDescriptor"
                }
            ]
        },
        {
            "@id": "iudx:cameraUsage",
            "@type": [
                "iudx:TextProperty"
            ],
            "rdfs:comment": "Purpose of the camera corresponding to this observation. ENUM: [SURVEILLANCE, RLVD, ANPR/LPR].",
            "rdfs:label": "cameraUsage",
            "rdfs:isDefinedBy": {
                "@id": "iudx:"
            },
            "iudx:domainIncludes": [
                {
                    "@id": "iudx:Camera"
                }
            ],
            "iudx:rangeIncludes": [
                {
                    "@id": "iudx:Text"
                },
                {
                    "@id": "iudx:ValueDescriptor"
                }
            ]
        },
        {
            "@id": "iudx:carbonCreditValue",
            "@type": [
                "iudx:QuantitativeProperty"
            ],
            "rdfs:comment": "It represents a measurable decrease or elimination of greenhouse gas emissions, specifically carbon dioxide (CO2) or its equivalents, permitted or asserted during the reporting period corresponding to this observation.",
            "rdfs:label": "carbonCreditValue",
            "rdfs:isDefinedBy": {
                "@id": "iudx:"
            },
            "iudx:domainIncludes": [
                {
                    "@id": "iudx:BikeDockingStation"
                }
            ],
            "iudx:rangeIncludes": [
                {
                    "@id": "iudx:Number"
                },
                {
                    "@id": "iudx:ValueDescriptor"
                }
            ]
        },
        {
            "@id": "iudx:cardID",
            "@type": [
                "iudx:TextProperty"
            ],
            "rdfs:comment": "Unique ticket ID of the transaction or ID of the smart card used in the transaction.",
            "rdfs:label": "cardID",
            "rdfs:isDefinedBy": {
                "@id": "iudx:"
            },
            "iudx:domainIncludes": [
                {
                    "@id": "iudx:FareCollectionSystem"
                }
            ],
            "iudx:rangeIncludes": [
                {
                    "@id": "iudx:Text"
                },
                {
                    "@id": "iudx:ValueDescriptor"
                }
            ]
        },
        {
            "@id": "iudx:carriagewayLength",
            "@type": [
                "iudx:QuantitativeProperty"
            ],
            "rdfs:comment": "Total length of the carriage way of the road segment corresponding to this observation.",
            "rdfs:label": "carriagewayLength",
            "rdfs:isDefinedBy": {
                "@id": "iudx:"
            },
            "iudx:domainIncludes": [
                {
                    "@id": "iudx:RoadSegment"
                }
            ],
            "iudx:rangeIncludes": [
                {
                    "@id": "iudx:Number"
                },
                {
                    "@id": "iudx:ValueDescriptor"
                }
            ]
        },
        {
            "@id": "iudx:carriagewayWidth",
            "@type": [
                "iudx:QuantitativeProperty"
            ],
            "rdfs:comment": "Total width of the carriage way of the road segment corresponding to this observation.",
            "rdfs:label": "carriagewayWidth",
            "rdfs:isDefinedBy": {
                "@id": "iudx:"
            },
            "iudx:domainIncludes": [
                {
                    "@id": "iudx:RoadSegment"
                }
            ],
            "iudx:rangeIncludes": [
                {
                    "@id": "iudx:Number"
                },
                {
                    "@id": "iudx:ValueDescriptor"
                }
            ]
        },
        {
            "@id": "iudx:category",
            "@type": [
                "iudx:TextProperty"
            ],
            "rdfs:comment": "The category name corresponding to the issue that has been reported.",
            "rdfs:label": "category",
            "iudx:domainIncludes": [
                {
                    "@id": "iudx:IssueReporting"
                },
                {
                    "@id": "iudx:TouristDestination"
                }
            ],
            "iudx:rangeIncludes": [
                {
                    "@id": "iudx:Text"
                },
                {
                    "@id": "iudx:ValueDescriptor"
                }
            ],
            "rdfs:isDefinedBy": {
                "@id": "iudx:"
            },
            "skos:exactMatch": {
                "@id": "open311:group"
            }
        },
        {
            "@id": "iudx:categoryCode",
            "@type": [
                "iudx:TextProperty"
            ],
            "rdfs:comment": "Unique identifier for the category corresponding to the issue reported.",
            "rdfs:label": "categoryCode",
            "rdfs:isDefinedBy": {
                "@id": "iudx:"
            },
            "iudx:domainIncludes": [
                {
                    "@id": "iudx:IssueReporting"
                }
            ],
            "iudx:rangeIncludes": [
                {
                    "@id": "iudx:Text"
                },
                {
                    "@id": "iudx:ValueDescriptor"
                }
            ]
        },
        {
            "@id": "iudx:chargingUnitID",
            "@type": [
                "iudx:TextProperty"
            ],
            "rdfs:comment": "The ID of the charging point in the EV charging station corresponding to this observation.",
            "rdfs:label": "chargingUnitID",
            "rdfs:isDefinedBy": {
                "@id": "iudx:"
            },
            "iudx:domainIncludes": [
                {
                    "@id": "iudx:EVChargingStation"
                }
            ],
            "iudx:rangeIncludes": [
                {
                    "@id": "iudx:Text"
                },
                {
                    "@id": "iudx:ValueDescriptor"
                }
            ]
        },
        {
            "@id": "iudx:cityID",
            "@type": [
                "iudx:TextProperty"
            ],
            "rdfs:comment": "City ID corresponding to this observation.",
            "rdfs:label": "cityID",
            "rdfs:isDefinedBy": {
                "@id": "iudx:"
            },
            "iudx:domainIncludes": [
                {
                    "@id": "iudx:MunicipalityDesc"
                }
            ],
            "iudx:rangeIncludes": [
                {
                    "@id": "iudx:Text"
                },
                {
                    "@id": "iudx:ValueDescriptor"
                }
            ]
        },
        {
            "@id": "iudx:cityName",
            "@type": [
                "iudx:TextProperty"
            ],
            "rdfs:comment": "City name corresponding to this observation.",
            "rdfs:label": "cityName",
            "rdfs:isDefinedBy": {
                "@id": "iudx:"
            },
            "iudx:domainIncludes": [
                {
                    "@id": "iudx:MunicipalityDesc"
                }
            ],
            "iudx:rangeIncludes": [
                {
                    "@id": "iudx:Text"
                },
                {
                    "@id": "iudx:ValueDescriptor"
                }
            ]
        },
        {
            "@id": "iudx:cl",
            "@type": [
                "iudx:QuantitativeProperty"
            ],
            "rdfs:comment": "Concentration of chlorides in the water.",
            "rdfs:label": "cl",
            "rdfs:isDefinedBy": {
                "@id": "iudx:"
            },
            "iudx:domainIncludes": [
                {
                    "@id": "iudx:WaterDistributionNetwork"
                }
            ],
            "iudx:rangeIncludes": [
                {
                    "@id": "iudx:TimeSeriesAggregation"
                },
                {
                    "@id": "iudx:ValueDescriptor"
                }
            ],
            "skos:exactMatch": {
                "@id": "Fiware: WaterQualityObserved.Cl"
            }
        },
        {
            "@id": "iudx:cod",
            "@type": [
                "iudx:QuantitativeProperty"
            ],
            "rdfs:comment": "Chemical Oxygen Demand concentration measured in the waste-water treatment plant corresponding to this observation.",
            "rdfs:label": "cod",
            "rdfs:isDefinedBy": {
                "@id": "iudx:"
            },
            "iudx:domainIncludes": [
                {
                    "@id": "iudx:WasteWaterMgmt"
                }
            ],
            "iudx:rangeIncludes": [
                {
                    "@id": "iudx:Number"
                },
                {
                    "@id": "iudx:ValueDescriptor"
                }
            ],
            "skos:exactMatch": {
                "@id": "fiware:cod"
            }
        },
        {
            "@id": "iudx:collectedPOI",
            "@type": [
                "iudx:QuantitativeProperty"
            ],
            "rdfs:comment": "The count of points of interest (waste collection points) that the waste management vehicle corresponding to this observation has served or collected the waste from.",
            "rdfs:label": "collectedPOI",
            "iudx:domainIncludes": [
                {
                    "@id": "iudx:WmgmtVehicle"
                }
            ],
            "iudx:rangeIncludes": [
                {
                    "@id": "iudx:Number"
                },
                {
                    "@id": "iudx:ValueDescriptor"
                }
            ],
            "rdfs:isDefinedBy": {
                "@id": "iudx:"
            }
        },
        {
            "@id": "iudx:comments",
            "@type": [
                "iudx:TextProperty"
            ],
            "rdfs:comment": "User comments corresponding to this observation.",
            "rdfs:label": "comments",
            "rdfs:isDefinedBy": {
                "@id": "iudx:"
            },
            "iudx:domainIncludes": [
                {
                    "@id": "iudx:SafetiPin"
                },
                {
                    "@id": "iudx:IssueReporting"
                },
                {
                    "@id": "iudx:Version"
                },
                {
                    "@id": "iudx:Orientation"
                },
                {
                    "@id": "iudx:BikeDockingStation"
                }
            ],
            "iudx:rangeIncludes": [
                {
                    "@container": "@list",
                    "@id": "iudx:Text"
                },
                {
                    "@id": "iudx:Text"
                },
                {
                    "@id": "iudx:ValueDescriptor"
                }
            ]
        },
        {
            "@id": "iudx:commercialPOIs",
            "@type": [
                "iudx:QuantitativeProperty"
            ],
            "rdfs:comment": "The total count of commercial establishments which serve as point of interests corresponding to this observation.",
            "rdfs:label": "commercialPOIs",
            "iudx:domainIncludes": [
                {
                    "@id": "iudx:WmgmtVehicle"
                }
            ],
            "iudx:rangeIncludes": [
                {
                    "@id": "iudx:Number"
                },
                {
                    "@id": "iudx:ValueDescriptor"
                }
            ],
            "rdfs:isDefinedBy": {
                "@id": "iudx:"
            }
        },
        {
            "@id": "iudx:commercialUnitsCount",
            "@type": [
                "iudx:QuantitativeProperty"
            ],
            "rdfs:comment": "The total number of commercial or trade establishments present at the location corresponding to this observation.",
            "rdfs:label": "commercialUnitsCount",
            "rdfs:isDefinedBy": {
                "@id": "iudx:"
            },
            "iudx:domainIncludes": [
                {
                    "@id": "iudx:WmgmtVehicle"
                }
            ],
            "iudx:rangeIncludes": [
                {
                    "@id": "iudx:Number"
                },
                {
                    "@id": "iudx:ValueDescriptor"
                }
            ]
        },
        {
            "@id": "iudx:compensatedTDS",
            "@type": [
                "iudx:QuantitativeProperty"
            ],
            "rdfs:comment": "The value of TDS (Total Dissolved Solids) level in the water with temperature compensation.",
            "rdfs:label": "compensatedTDS",
            "rdfs:isDefinedBy": {
                "@id": "iudx:"
            },
            "iudx:domainIncludes": [
                {
                    "@id": "iudx:WasteWaterMgmt"
                },
                {
                    "@id": "iudx:WaterDistributionNetwork"
                }
            ],
            "iudx:rangeIncludes": [
                {
                    "@id": "iudx:Number"
                },
                {
                    "@id": "iudx:ValueDescriptor"
                }
            ]
        },
        {
            "@id": "iudx:compressorStatus",
            "@type": [
                "iudx:QuantitativeProperty"
            ],
            "rdfs:comment": "Describes the compressor status of the air conditioning system by a binary input (0-Inactive, 1-Active)",
            "rdfs:label": "compressorStatus",
            "rdfs:isDefinedBy": {
                "@id": "iudx:"
            },
            "iudx:domainIncludes": [
                {
                    "@id": "iudx:AirConditioner"
                }
            ],
            "iudx:rangeIncludes": [
                {
                    "@id": "iudx:Number"
                },
                {
                    "@id": "iudx:ValueDescriptor"
                }
            ]
        },
        {
            "@id": "iudx:congestion_level",
            "@type": [
                "iudx:TextProperty"
            ],
            "rdfs:comment": "Describes the congestion level that is affecting this vehicle. ENUM [UNKNOWN_CONGESTION_LEVEL, RUNNING_SMOOTHLY, STOP_AND_GO, CONGESTION, SEVERE_CONGESTION]",
            "rdfs:label": "congestion_level",
            "rdfs:isDefinedBy": {
                "@id": "iudx:"
            },
            "iudx:domainIncludes": [
                {
                    "@id": "iudx:VehiclePosition"
                }
            ],
            "iudx:rangeIncludes": [
                {
                    "@id": "iudx:Text"
                },
                {
                    "@id": "iudx:ValueDescriptor"
                }
            ],
            "skos:exactMatch": {
                "@id": "GTFS: congestion_level"
            }
        },
        {
            "@id": "iudx:continuous_drop_off",
            "@type": [
                "iudx:QuantitativeProperty"
            ],
            "rdfs:comment": "Indicates whether a rider can alight from the transit vehicle at any point along the vehicle\u2019s travel path.SameAs: 'continuous_drop_off' field from GTFS Static Field definitions-stop_times.txt (https://developers.google.com/transit/gtfs/reference#stop_timestxt)",
            "rdfs:label": "continuous_drop_off",
            "rdfs:isDefinedBy": {
                "@id": "iudx:"
            },
            "iudx:domainIncludes": [
                {
                    "@id": "iudx:StopTimesDesc"
                }
            ],
            "iudx:rangeIncludes": [
                {
                    "@id": "iudx:Number"
                },
                {
                    "@id": "iudx:ValueDescriptor"
                }
            ],
            "skos:exactMatch": {
                "@id": "GTFS: continuous_drop_off"
            }
        },
        {
            "@id": "iudx:continuous_pickup",
            "@type": [
                "iudx:QuantitativeProperty"
            ],
            "rdfs:comment": "Indicates whether a rider can board the transit vehicle at any point along the vehicle\u2019s travel path.SameAs: 'continuous_pickup' field from GTFS Static Field definitions-stop_times.txt (https://developers.google.com/transit/gtfs/reference#stop_timestxt)",
            "rdfs:label": "continuous_pickup",
            "rdfs:isDefinedBy": {
                "@id": "iudx:"
            },
            "iudx:domainIncludes": [
                {
                    "@id": "iudx:StopTimesDesc"
                }
            ],
            "iudx:rangeIncludes": [
                {
                    "@id": "iudx:Number"
                },
                {
                    "@id": "iudx:ValueDescriptor"
                }
            ],
            "skos:exactMatch": {
                "@id": "GTFS: continuous_pickup"
            }
        },
        {
            "@id": "iudx:culvertCount",
            "@type": [
                "iudx:QuantitativeProperty"
            ],
            "rdfs:comment": "Number of culverts prevalent in the trace of the road corresponding to this observation.",
            "rdfs:label": "culvertCount",
            "rdfs:isDefinedBy": {
                "@id": "iudx:"
            },
            "iudx:domainIncludes": [
                {
                    "@id": "iudx:RoadSegment"
                }
            ],
            "iudx:rangeIncludes": [
                {
                    "@id": "iudx:Number"
                },
                {
                    "@id": "iudx:ValueDescriptor"
                }
            ]
        },
        {
            "@id": "iudx:current",
            "@type": [
                "iudx:QuantitativeProperty"
            ],
            "rdfs:comment": "The value of Current in the entity corresponding to this observation.",
            "rdfs:label": "current",
            "rdfs:isDefinedBy": {
                "@id": "iudx:"
            },
            "iudx:domainIncludes": [
                {
                    "@id": "iudx:Streetlight"
                },
                {
                    "@id": "iudx:SolarEnergy"
                },
                {
                    "@id": "iudx:EnergyMeter"
                }
            ],
            "iudx:rangeIncludes": [
                {
                    "@id": "iudx:Number"
                },
                {
                    "@id": "iudx:ValueDescriptor"
                }
            ]
        },
        {
            "@id": "iudx:currentLevel",
            "@type": [
                "iudx:QuantitativeProperty"
            ],
            "rdfs:comment": "Current flooding level indicated by the sensing station corresponding to this observation.",
            "rdfs:label": "currentLevel",
            "rdfs:isDefinedBy": {
                "@id": "iudx:"
            },
            "iudx:domainIncludes": [
                {
                    "@id": "iudx:EnvFlood"
                }
            ],
            "iudx:rangeIncludes": [
                {
                    "@id": "iudx:Number"
                },
                {
                    "@id": "iudx:ValueDescriptor"
                }
            ]
        },
        {
            "@id": "iudx:currentTripCount",
            "@type": [
                "iudx:QuantitativeProperty"
            ],
            "rdfs:comment": "The current count of trips made by the vehicle(s) corresponding to this observation.",
            "rdfs:label": "currentTripCount",
            "rdfs:isDefinedBy": {
                "@id": "iudx:"
            },
            "iudx:domainIncludes": [
                {
                    "@id": "iudx:FareCollectionSystem"
                },
                {
                    "@id": "iudx:WmgmtVehicle"
                },
                {
                    "@id": "iudx:BikeDockingStation"
                }
            ],
            "iudx:rangeIncludes": [
                {
                    "@id": "iudx:Number"
                },
                {
                    "@id": "iudx:ValueDescriptor"
                }
            ]
        },
        {
            "@id": "iudx:current_status",
            "@type": [
                "iudx:TextProperty"
            ],
            "rdfs:comment": "Describes the status of the vehicle w.r.t the stop corresponding to this observation ENUM: [INCOMING_AT, STOPPED_AT, IN_TRANSIT_TO]. SameAs:'current_status' field from GTFS Realtime message-VehiclePosition(https://developers.google.com/transit/gtfs-realtime/reference#message-vehicleposition)",
            "rdfs:label": "current_status",
            "rdfs:isDefinedBy": {
                "@id": "iudx:"
            },
            "iudx:domainIncludes": [
                {
                    "@id": "iudx:VehiclePosition"
                }
            ],
            "iudx:rangeIncludes": [
                {
                    "@id": "iudx:Text"
                },
                {
                    "@id": "iudx:ValueDescriptor"
                }
            ],
            "skos:exactMatch": {
                "@id": "GTFS: current_status"
            }
        },
        {
            "@id": "iudx:current_stop_sequence",
            "@type": [
                "iudx:QuantitativeProperty"
            ],
            "rdfs:comment": "Gives the stop sequence index of the current stop. This is determined by considering current_status, if current_status is missing IN_TRANSIT_TO is assumed. SameAs:'current_stop_sequence' field from GTFS Realtime message-VehiclePosition(https://developers.google.com/transit/gtfs-realtime/reference#message-vehicleposition)",
            "rdfs:label": "current_stop_sequence",
            "rdfs:isDefinedBy": {
                "@id": "iudx:"
            },
            "iudx:domainIncludes": [
                {
                    "@id": "iudx:VehiclePosition"
                }
            ],
            "iudx:rangeIncludes": [
                {
                    "@id": "iudx:Number"
                },
                {
                    "@id": "iudx:ValueDescriptor"
                }
            ],
            "skos:exactMatch": {
                "@id": "GTFS: current_stop_sequence"
            }
        },
        {
            "@id": "iudx:cyclePathLeftHeight",
            "@type": [
                "iudx:QuantitativeProperty"
            ],
            "rdfs:comment": "Height of the cycle track on the left edge of the road corresponding to this observation",
            "rdfs:label": "cyclePathLeftHeight",
            "rdfs:isDefinedBy": {
                "@id": "iudx:"
            },
            "iudx:domainIncludes": [
                {
                    "@id": "iudx:RoadSegment"
                }
            ],
            "iudx:rangeIncludes": [
                {
                    "@id": "iudx:Number"
                },
                {
                    "@id": "iudx:ValueDescriptor"
                }
            ]
        },
        {
            "@id": "iudx:cyclePathLeftWidth",
            "@type": [
                "iudx:QuantitativeProperty"
            ],
            "rdfs:comment": "Width of the cycle track on the left edge of the road corresponding to this observation.",
            "rdfs:label": "cyclePathLeftWidth",
            "rdfs:isDefinedBy": {
                "@id": "iudx:"
            },
            "iudx:domainIncludes": [
                {
                    "@id": "iudx:RoadSegment"
                }
            ],
            "iudx:rangeIncludes": [
                {
                    "@id": "iudx:Number"
                },
                {
                    "@id": "iudx:ValueDescriptor"
                }
            ]
        },
        {
            "@id": "iudx:cyclePathMaterial",
            "@type": [
                "iudx:TextProperty"
            ],
            "rdfs:comment": "Construction material used for laying the cycle path on the sides of the road corresponding to this observation.",
            "rdfs:label": "cyclePathMaterial",
            "rdfs:isDefinedBy": {
                "@id": "iudx:"
            },
            "iudx:domainIncludes": [
                {
                    "@id": "iudx:RoadSegment"
                }
            ],
            "iudx:rangeIncludes": [
                {
                    "@id": "iudx:Text"
                },
                {
                    "@id": "iudx:ValueDescriptor"
                }
            ]
        },
        {
            "@id": "iudx:cyclePathPlacement",
            "@type": [
                "iudx:TextProperty"
            ],
            "rdfs:comment": "Describes the placement of cycle track along the road segment corresponding to this observation. ENUM: [RIGHT, LEFT, BOTH, NOT_AVAILABLE]",
            "rdfs:label": "cyclePathPlacement",
            "rdfs:isDefinedBy": {
                "@id": "iudx:"
            },
            "iudx:domainIncludes": [
                {
                    "@id": "iudx:RoadSegment"
                }
            ],
            "iudx:rangeIncludes": [
                {
                    "@id": "iudx:Text"
                },
                {
                    "@id": "iudx:ValueDescriptor"
                }
            ]
        },
        {
            "@id": "iudx:cyclePathRightHeight",
            "@type": [
                "iudx:QuantitativeProperty"
            ],
            "rdfs:comment": "Height of the cycle track on the right edge of the road corresponding to this observation",
            "rdfs:label": "cyclePathRightHeight",
            "rdfs:isDefinedBy": {
                "@id": "iudx:"
            },
            "iudx:domainIncludes": [
                {
                    "@id": "iudx:RoadSegment"
                }
            ],
            "iudx:rangeIncludes": [
                {
                    "@id": "iudx:Number"
                },
                {
                    "@id": "iudx:ValueDescriptor"
                }
            ]
        },
        {
            "@id": "iudx:cyclePathRightWidth",
            "@type": [
                "iudx:QuantitativeProperty"
            ],
            "rdfs:comment": "Width of the cycle track on the right edge of the road corresponding to this observation.",
            "rdfs:label": "cyclePathRightWidth",
            "rdfs:isDefinedBy": {
                "@id": "iudx:"
            },
            "iudx:domainIncludes": [
                {
                    "@id": "iudx:RoadSegment"
                }
            ],
            "iudx:rangeIncludes": [
                {
                    "@id": "iudx:Number"
                },
                {
                    "@id": "iudx:ValueDescriptor"
                }
            ]
        },
        {
            "@id": "iudx:dangerLevel",
            "@type": [
                "iudx:QuantitativeProperty"
            ],
            "rdfs:comment": "Reference danger level threshold value set for the sensing station corresponding to this observation. Flood level status is marked danger if the current level crosses the danger level threshold value.",
            "rdfs:label": "dangerLevel",
            "rdfs:isDefinedBy": {
                "@id": "iudx:"
            },
            "iudx:domainIncludes": [
                {
                    "@id": "iudx:EnvFlood"
                }
            ],
            "iudx:rangeIncludes": [
                {
                    "@id": "iudx:Number"
                },
                {
                    "@id": "iudx:ValueDescriptor"
                }
            ]
        },
        {
            "@id": "iudx:dataRate",
            "@type": [
                "iudx:QuantitativeProperty"
            ],
            "rdfs:comment": "The number of bits transmitted from one device to another or over a network per second",
            "rdfs:label": "dataRate",
            "rdfs:isDefinedBy": {
                "@id": "iudx:"
            },
            "iudx:domainIncludes": [
                {
                    "@id": "iudx:WirelessNetwork"
                }
            ],
            "iudx:rangeIncludes": [
                {
                    "@id": "iudx:Number"
                },
                {
                    "@id": "iudx:ValueDescriptor"
                }
            ]
        },
        {
            "@id": "iudx:dataSchema",
            "@type": [
                "iudx:TextProperty"
            ],
            "rdfs:comment": "Associated data schema. Specified as an URI (linking it to one of the known data type vocabulary, e.g., xsd)",
            "rdfs:label": "dataSchema",
            "iudx:domainIncludes": [
                {
                    "@id": "iudx:ValueDescriptor"
                }
            ],
            "iudx:rangeIncludes": [
                {
                    "@id": "iudx:Text",
                    "@type": "@id"
                }
            ],
            "rdfs:isDefinedBy": {
                "@id": "iudx:"
            }
        },
        {
            "@id": "iudx:date",
            "@type": [
                "iudx:TextProperty"
            ],
            "rdfs:comment": "Date corresponding to this observation and is described in YYYY-MM-DD format, for eg. '2020-11-01'.",
            "rdfs:label": "date",
            "iudx:domainIncludes": [
                {
                    "@id": "iudx:RevenueCollection"
                },
                {
                    "@id": "iudx:EmployeeDetails"
                }
            ],
            "iudx:rangeIncludes": [
                {
                    "@id": "iudx:Text"
                },
                {
                    "@id": "iudx:ValueDescriptor"
                }
            ],
            "rdfs:isDefinedBy": {
                "@id": "iudx:"
            }
        },
        {
            "@id": "iudx:daysOff",
            "@type": [
                "iudx:TextProperty"
            ],
            "rdfs:comment": "The days on which the public site or tourist destination is closed.",
            "rdfs:label": "daysOff",
            "rdfs:isDefinedBy": {
                "@id": "iudx:"
            },
            "iudx:domainIncludes": [
                {
                    "@id": "iudx:TouristDestination"
                }
            ],
            "iudx:rangeIncludes": [
                {
                    "@id": "iudx:Text"
                },
                {
                    "@id": "iudx:ValueDescriptor"
                }
            ]
        },
        {
            "@id": "iudx:department",
            "@type": [
                "iudx:TextProperty"
            ],
            "rdfs:comment": "Division or section of the organization corresponding to this observation. Eg. Health, Transport.",
            "rdfs:label": "department",
            "iudx:domainIncludes": [
                {
                    "@id": "iudx:EmployeeDetails"
                },
                {
                    "@id": "iudx:IssueReporting"
                },
                {
                    "@id": "iudx:EnergyMeter"
                },
                {
                    "@id": "iudx:PublicSchemes"
                }
            ],
            "iudx:rangeIncludes": [
                {
                    "@id": "iudx:Text"
                },
                {
                    "@id": "iudx:ValueDescriptor"
                }
            ],
            "rdfs:isDefinedBy": {
                "@id": "iudx:"
            },
            "skos:exactMatch": {
                "@id": "schema:department"
            }
        },
        {
            "@id": "iudx:departmentID",
            "@type": [
                "iudx:TextProperty"
            ],
            "rdfs:comment": "Unique ID or code associated with the department which is associated with the service or the issue corresponding to this observation.",
            "rdfs:label": "departmentID",
            "iudx:domainIncludes": [
                {
                    "@id": "iudx:IssueReporting"
                },
                {
                    "@id": "iudx:EmployeeDetails"
                },
                {
                    "@id": "iudx:PublicSchemes"
                }
            ],
            "iudx:rangeIncludes": [
                {
                    "@id": "iudx:Text"
                },
                {
                    "@id": "iudx:ValueDescriptor"
                }
            ],
            "rdfs:isDefinedBy": {
                "@id": "iudx:"
            }
        },
        {
            "@id": "iudx:departureUncertainty",
            "@type": [
                "iudx:QuantitativeProperty"
            ],
            "rdfs:comment": "If schedule_relationship is empty or SCHEDULED, either arrival or departure must be provided within a StopTimeUpdate. SameAs: 'departure' field from GTFS Realtime message-StopTimeUpdate (https://developers.google.com/transit/gtfs-realtime/reference#message-stoptimeupdate)",
            "rdfs:label": "departureUncertainty",
            "rdfs:isDefinedBy": {
                "@id": "iudx:"
            },
            "iudx:domainIncludes": [
                {
                    "@id": "iudx:TransitManagement"
                }
            ],
            "iudx:rangeIncludes": [
                {
                    "@id": "iudx:Number"
                },
                {
                    "@id": "iudx:ValueDescriptor"
                }
            ]
        },
        {
            "@id": "iudx:departure_time",
            "@type": [
                "iudx:TimeProperty"
            ],
            "rdfs:comment": "Specifies the departure time from a specific stop for a specific trip on a route. Times must be eight digits in HH:MM:SS format (HH:MM:SS is also accepted, if the hour begins with 0). Note: Trips that span multiple dates will have stop times greater than 24:00:00. For example, if a trip begins at 10:30:00 p.m. and ends at 2:15:00 a.m. on the following day, the stop times would be 22:30:00 and 26:15:00. Entering those stop times as 22:30:00 and 02:15:00 would not produce the desired results. SameAs: 'departure_time' field from GTFS Static Field definitions-stop_times.txt (https://developers.google.com/transit/gtfs/reference#stop_timestxt)",
            "rdfs:label": "departure_time",
            "rdfs:isDefinedBy": {
                "@id": "iudx:"
            },
            "iudx:domainIncludes": [
                {
                    "@id": "iudx:StopTimesDesc"
                }
            ],
            "iudx:rangeIncludes": [
                {
                    "@id": "iudx:Text"
                },
                {
                    "@id": "iudx:ValueDescriptor"
                }
            ],
            "skos:exactMatch": {
                "@id": "GTFS: departure_time"
            }
        },
        {
            "@id": "iudx:depotID",
            "@type": [
                "iudx:TextProperty"
            ],
            "rdfs:comment": "Describes the unique id of the bus depot corresponding to this observation.",
            "rdfs:label": "depotID",
            "rdfs:isDefinedBy": {
                "@id": "iudx:"
            },
            "iudx:domainIncludes": [
                {
                    "@id": "iudx:TransitManagement"
                }
            ],
            "iudx:rangeIncludes": [
                {
                    "@id": "iudx:Text"
                },
                {
                    "@id": "iudx:ValueDescriptor"
                }
            ]
        },
        {
            "@id": "iudx:depotName",
            "@type": [
                "iudx:TextProperty"
            ],
            "rdfs:comment": "Describes the depot name of the bus depot corresponding to this observation.",
            "rdfs:label": "depotName",
            "rdfs:isDefinedBy": {
                "@id": "iudx:"
            },
            "iudx:domainIncludes": [
                {
                    "@id": "iudx:TransitManagement"
                }
            ],
            "iudx:rangeIncludes": [
                {
                    "@id": "iudx:Text"
                },
                {
                    "@id": "iudx:ValueDescriptor"
                }
            ]
        },
        {
            "@id": "iudx:description",
            "@type": [
                "iudx:TextProperty"
            ],
            "rdfs:comment": "Description for an IUDX thing.",
            "rdfs:label": "description",
            "iudx:domainIncludes": [
                {
                    "@id": "iudx:Thing"
                }
            ],
            "iudx:rangeIncludes": [
                {
                    "@id": "iudx:Text"
                }
            ],
            "rdfs:isDefinedBy": {
                "@id": "iudx:"
            }
        },
        {
            "@id": "iudx:destinationLocation",
            "@type": [
                "iudx:GeoProperty"
            ],
            "rdfs:comment": "The destination location of the ride corresponding to the observation.",
            "rdfs:label": "destinationLocation",
            "rdfs:isDefinedBy": {
                "@id": "iudx:"
            },
            "iudx:domainIncludes": [
                {
                    "@id": "iudx:BikeDockingStation"
                }
            ],
            "iudx:rangeIncludes": [
                {
                    "@id": "iudx:Place"
                },
                {
                    "@id": "iudx:ValueDescriptor"
                }
            ]
        },
        {
            "@id": "iudx:destinationStopCategory",
            "@type": [
                "iudx:TextProperty"
            ],
            "rdfs:comment": "Type of the destination bus stop corresponding to this observation.",
            "rdfs:label": "destinationStopCategory",
            "rdfs:isDefinedBy": {
                "@id": "iudx:"
            },
            "iudx:domainIncludes": [
                {
                    "@id": "iudx:FareCollectionSystem"
                }
            ],
            "iudx:rangeIncludes": [
                {
                    "@id": "iudx:Text"
                },
                {
                    "@id": "iudx:ValueDescriptor"
                }
            ]
        },
        {
            "@id": "iudx:destinationStopID",
            "@type": [
                "iudx:TextProperty"
            ],
            "rdfs:comment": "Unique ID of the bus stop at which the passenger deboards from the bus corresponding to this observation.",
            "rdfs:label": "destinationStopID",
            "rdfs:isDefinedBy": {
                "@id": "iudx:"
            },
            "iudx:domainIncludes": [
                {
                    "@id": "iudx:FareCollectionSystem"
                }
            ],
            "iudx:rangeIncludes": [
                {
                    "@id": "iudx:Text"
                },
                {
                    "@id": "iudx:ValueDescriptor"
                }
            ]
        },
        {
            "@id": "iudx:destinationStopName",
            "@type": [
                "iudx:TextProperty"
            ],
            "rdfs:comment": "The name of the destination bus stop corresponding to this observation.",
            "rdfs:label": "destinationStopName",
            "rdfs:isDefinedBy": {
                "@id": "iudx:"
            },
            "iudx:domainIncludes": [
                {
                    "@id": "iudx:FareCollectionSystem"
                }
            ],
            "iudx:rangeIncludes": [
                {
                    "@id": "iudx:Text"
                },
                {
                    "@id": "iudx:ValueDescriptor"
                }
            ]
        },
        {
            "@id": "iudx:destinationType",
            "@type": [
                "iudx:TextProperty"
            ],
            "rdfs:comment": "The type of public site or tourist destination corresponding to this observation. Example Historic Monuments, Religious sites, etc.",
            "rdfs:label": "destinationType",
            "rdfs:isDefinedBy": {
                "@id": "iudx:"
            },
            "iudx:domainIncludes": [
                {
                    "@id": "iudx:TouristDestination"
                }
            ],
            "iudx:rangeIncludes": [
                {
                    "@id": "iudx:Text"
                },
                {
                    "@id": "iudx:ValueDescriptor"
                }
            ]
        },
        {
            "@id": "iudx:deviceBatteryStatus",
            "@type": [
                "iudx:TextProperty"
            ],
            "rdfs:comment": "Gives the Battery charging status of the reporting device. ENUM: [Connected, Disconnected].",
            "rdfs:label": "deviceBatteryStatus",
            "rdfs:isDefinedBy": {
                "@id": "iudx:"
            },
            "iudx:domainIncludes": [
                {
                    "@id": "iudx:Device"
                }
            ],
            "iudx:rangeIncludes": [
                {
                    "@id": "iudx:Text"
                },
                {
                    "@id": "iudx:ValueDescriptor"
                }
            ]
        },
        {
            "@id": "iudx:deviceCount",
            "@type": [
                "iudx:QuantitativeProperty"
            ],
            "rdfs:comment": "The number of devices that have been installed at a location corresponding to this observation.",
            "rdfs:label": "deviceCount",
            "rdfs:isDefinedBy": {
                "@id": "iudx:"
            },
            "iudx:domainIncludes": [
                {
                    "@id": "iudx:Device"
                }
            ],
            "iudx:rangeIncludes": [
                {
                    "@id": "iudx:Number"
                },
                {
                    "@id": "iudx:ValueDescriptor"
                }
            ]
        },
        {
            "@id": "iudx:deviceID",
            "@type": [
                "iudx:TextProperty"
            ],
            "rdfs:comment": "Device ID of the physical sensor/ measurement station corresponding to this observation.",
            "rdfs:label": "deviceID",
            "rdfs:isDefinedBy": {
                "@id": "iudx:"
            },
            "iudx:domainIncludes": [
                {
                    "@id": "iudx:Device"
                }
            ],
            "iudx:rangeIncludes": [
                {
                    "@id": "iudx:Text"
                },
                {
                    "@id": "iudx:ValueDescriptor"
                }
            ]
        },
        {
            "@id": "iudx:deviceName",
            "@type": [
                "iudx:TextProperty"
            ],
            "rdfs:comment": "Device Name or Station name of the sensor device/station corresponding to this observation.",
            "rdfs:label": "deviceName",
            "rdfs:isDefinedBy": {
                "@id": "iudx:"
            },
            "iudx:domainIncludes": [
                {
                    "@id": "iudx:Device"
                }
            ],
            "iudx:rangeIncludes": [
                {
                    "@id": "iudx:Text"
                },
                {
                    "@id": "iudx:ValueDescriptor"
                }
            ]
        },
        {
            "@id": "iudx:deviceSimNumber",
            "@type": [
                "iudx:TextProperty"
            ],
            "rdfs:comment": "Gives the sim number of the tracker device in the vehicle.",
            "rdfs:label": "deviceSimNumber",
            "rdfs:isDefinedBy": {
                "@id": "iudx:"
            },
            "iudx:domainIncludes": [
                {
                    "@id": "iudx:Device"
                }
            ],
            "iudx:rangeIncludes": [
                {
                    "@id": "iudx:Text"
                },
                {
                    "@id": "iudx:ValueDescriptor"
                }
            ]
        },
        {
            "@id": "iudx:deviceStatus",
            "@type": [
                "iudx:TextProperty"
            ],
            "rdfs:comment": "Indicates the status of physical device or devices.",
            "rdfs:label": "deviceStatus",
            "iudx:domainIncludes": [
                {
                    "@id": "iudx:EnvAQM"
                },
                {
                    "@id": "iudx:EnvFlood"
                },
                {
                    "@id": "iudx:Streetlight"
                },
                {
                    "@id": "iudx:AirQuality"
                }
            ],
            "iudx:rangeIncludes": [
                {
                    "@id": "iudx:Text"
                },
                {
                    "@id": "iudx:ValueDescriptor"
                }
            ],
            "rdfs:isDefinedBy": {
                "@id": "iudx:"
            }
        },
        {
            "@id": "iudx:dewPoint",
            "@type": [
                "iudx:QuantitativeProperty"
            ],
            "rdfs:comment": "Observed  temperature to which air must be cooled to become saturated with water vapor.",
            "rdfs:label": "dewPoint",
            "rdfs:isDefinedBy": {
                "@id": "iudx:"
            },
            "iudx:domainIncludes": [
                {
                    "@id": "iudx:EnvWeather"
                }
            ],
            "iudx:rangeIncludes": [
                {
                    "@id": "iudx:Number"
                },
                {
                    "@id": "iudx:ValueDescriptor"
                }
            ],
            "skos:exactMatch": {
                "@id": "Fiware:dewPoint"
            }
        },
        {
            "@id": "iudx:direction_id",
            "@type": [
                "iudx:QuantitativeProperty"
            ],
            "rdfs:comment": "Indicates the direction of travel of the vehicle corresponding to this observation, can be referenced from the GTFS static feed trips.txt. SameAs: 'direction_id' field from GTFS Realtime message-TripDescriptor (https://developers.google.com/transit/gtfs-realtime/reference#message-tripdescriptor)",
            "rdfs:label": "direction_id",
            "rdfs:isDefinedBy": {
                "@id": "iudx:"
            },
            "iudx:domainIncludes": [
                {
                    "@id": "iudx:TripDescriptor"
                },
                {
                    "@id": "iudx:FareCollectionSystem"
                }
            ],
            "iudx:rangeIncludes": [
                {
                    "@id": "iudx:Number"
                },
                {
                    "@id": "iudx:ValueDescriptor"
                }
            ]
        },
        {
            "@id": "iudx:district",
            "@type": [
                "iudx:TextProperty"
            ],
            "rdfs:comment": "District name corresponding to this observation.",
            "rdfs:label": "district",
            "iudx:domainIncludes": [
                {
                    "@id": "iudx:Headquarters"
                },
                {
                    "@id": "iudx:District"
                },
                {
                    "@id": "iudx:Headquarters"
                }
            ],
            "iudx:rangeIncludes": [
                {
                    "@id": "iudx:Text"
                },
                {
                    "@id": "iudx:ValueDescriptor"
                }
            ],
            "rdfs:isDefinedBy": {
                "@id": "iudx:"
            }
        },
        {
            "@id": "iudx:district_l",
            "@type": [
                "iudx:TextProperty"
            ],
            "rdfs:comment": "Name of district I corresponding to this observation",
            "rdfs:label": "district_l",
            "rdfs:isDefinedBy": {
                "@id": "iudx:"
            },
            "iudx:domainIncludes": [
                {
                    "@id": "iudx:District"
                }
            ],
            "iudx:rangeIncludes": [
                {
                    "@id": "iudx:Text"
                },
                {
                    "@id": "iudx:ValueDescriptor"
                }
            ]
        },
        {
            "@id": "iudx:do",
            "@type": [
                "iudx:QuantitativeProperty"
            ],
            "rdfs:comment": "Dissolved oxygen measured in the waste-water treatment plant corresponding to this observation.",
            "rdfs:label": "do",
            "rdfs:isDefinedBy": {
                "@id": "iudx:"
            },
            "iudx:domainIncludes": [
                {
                    "@id": "iudx:WasteWaterMgmt"
                }
            ],
            "iudx:rangeIncludes": [
                {
                    "@id": "iudx:Number"
                },
                {
                    "@id": "iudx:ValueDescriptor"
                }
            ],
            "skos:exactMatch": {
                "@id": "fiware:do"
            }
        },
        {
            "@id": "iudx:drop_off_type",
            "@type": [
                "iudx:TextProperty"
            ],
            "rdfs:comment": "Indicates drop off method. SameAs: 'drop_off_type' field from GTFS Static Field definitions-stop_times.txt (https://developers.google.com/transit/gtfs/reference#stop_timestxt)",
            "rdfs:label": "drop_off_type",
            "rdfs:isDefinedBy": {
                "@id": "iudx:"
            },
            "iudx:domainIncludes": [
                {
                    "@id": "iudx:StopTimesDesc"
                }
            ],
            "iudx:rangeIncludes": [
                {
                    "@id": "iudx:Text"
                },
                {
                    "@id": "iudx:ValueDescriptor"
                }
            ],
            "skos:exactMatch": {
                "@id": "GTFS: drop_off_type"
            }
        },
        {
            "@id": "iudx:durationInHours",
            "@type": [
                "iudx:QuantitativeProperty"
            ],
            "rdfs:comment": "Specifies an interval duration in hours for computing statistical aggregations.",
            "rdfs:label": "durationInHours",
            "iudx:domainIncludes": [
                {
                    "@id": "iudx:ValueDescriptor"
                }
            ],
            "iudx:rangeIncludes": [
                {
                    "@id": "iudx:Number"
                }
            ],
            "rdfs:isDefinedBy": {
                "@id": "iudx:"
            }
        },
        {
            "@id": "iudx:durationInMinutes",
            "@type": [
                "iudx:QuantitativeProperty"
            ],
            "rdfs:comment": "Specifies an interval duration in minutes for computing statistical aggregations.",
            "rdfs:label": "durationInMinutes",
            "iudx:domainIncludes": [
                {
                    "@id": "iudx:ValueDescriptor"
                }
            ],
            "iudx:rangeIncludes": [
                {
                    "@id": "iudx:Number"
                }
            ],
            "rdfs:isDefinedBy": {
                "@id": "iudx:"
            }
        },
        {
            "@id": "iudx:ecRecoveryAmount",
            "@type": [
                "iudx:QuantitativeProperty"
            ],
            "rdfs:comment": "Amount collected towards Enrollment Certificate from the establishment on annual basis.",
            "rdfs:label": "ecRecoveryAmount",
            "rdfs:isDefinedBy": {
                "@id": "iudx:"
            },
            "iudx:domainIncludes": [
                {
                    "@id": "iudx:RevenueCollection"
                }
            ],
            "iudx:rangeIncludes": [
                {
                    "@id": "iudx:Number"
                },
                {
                    "@id": "iudx:ValueDescriptor"
                }
            ]
        },
        {
            "@id": "iudx:elevation",
            "@type": [
                "iudx:QuantitativeProperty"
            ],
            "rdfs:comment": "The elevation of the entity corresponding to this observation. It is the distance above the sea level/ the height to which the entity is raised.",
            "rdfs:label": "elevation",
            "rdfs:isDefinedBy": {
                "@id": "iudx:"
            },
            "iudx:domainIncludes": [
                {
                    "@id": "iudx:MajorTowns"
                }
            ],
            "iudx:rangeIncludes": [
                {
                    "@id": "iudx:Number"
                },
                {
                    "@id": "iudx:ValueDescriptor"
                }
            ]
        },
        {
            "@id": "iudx:eligibleBeneficiaries",
            "@type": [
                "iudx:TextProperty"
            ],
            "rdfs:comment": "Represents the group(s) or category(ies) of people who can avail the benefits of the scheme corresponding to this observation.",
            "rdfs:label": "eligibleBeneficiaries",
            "rdfs:isDefinedBy": {
                "@id": "iudx:"
            },
            "iudx:domainIncludes": [
                {
                    "@id": "iudx:PublicSchemes"
                }
            ],
            "iudx:rangeIncludes": [
                {
                    "@container": "@list",
                    "@id": "iudx:Text"
                },
                {
                    "@id": "iudx:ValueDescriptor"
                }
            ]
        },
        {
            "@id": "iudx:emergencyVehicleType",
            "@type": [
                "iudx:TextProperty"
            ],
            "rdfs:comment": "Type of emergency vehicle corresponding to this observation. ENUM: [POLICE CAR, POLICE MOTORCYCLE, POLICE VAN, POLICE S.W.A.T, FIRE ENGINE, WATER TENDER, AIR AMBULANCE, AMBULANCE, MOTORCYCLE AMBULANCE, RESCUE VEHICLE, HAZARDOUS MATERIALS APPARATUS, TOW TRUCK]",
            "rdfs:label": "emergencyVehicleType",
            "rdfs:isDefinedBy": {
                "@id": "iudx:"
            },
            "iudx:domainIncludes": [
                {
                    "@id": "iudx:EmergencyVehicle"
                }
            ],
            "iudx:rangeIncludes": [
                {
                    "@id": "iudx:Text"
                },
                {
                    "@id": "iudx:ValueDescriptor"
                }
            ]
        },
        {
            "@id": "iudx:employeeDesignation",
            "@type": [
                "iudx:TextProperty"
            ],
            "rdfs:comment": "Title assigned to the employee corresponding to this observation. Eg. Sweeper, Driver, Helper, Supervisor, Safai Meth, Cleaner, Bhisti. etc.",
            "rdfs:label": "employeeDesignation",
            "rdfs:isDefinedBy": {
                "@id": "iudx:"
            },
            "iudx:domainIncludes": [
                {
                    "@id": "iudx:EmployeeDetails"
                }
            ],
            "iudx:rangeIncludes": [
                {
                    "@id": "iudx:Text"
                },
                {
                    "@id": "iudx:ValueDescriptor"
                }
            ],
            "skos:exactMatch": {
                "@id": "schema:jobTitle"
            }
        },
        {
            "@id": "iudx:employeeID",
            "@type": [
                "iudx:TextProperty"
            ],
            "rdfs:comment": "Unique ID of the employee corresponding to this observation",
            "rdfs:label": "employeeID",
            "rdfs:isDefinedBy": {
                "@id": "iudx:"
            },
            "iudx:domainIncludes": [
                {
                    "@id": "iudx:EmployeeDetails"
                }
            ],
            "iudx:rangeIncludes": [
                {
                    "@id": "iudx:Text"
                },
                {
                    "@id": "iudx:ValueDescriptor"
                }
            ]
        },
        {
            "@id": "iudx:employmentType",
            "@type": [
                "iudx:TextProperty"
            ],
            "rdfs:comment": "Type of employment. ENUM: [Contractual New, Contractual Old, Regular, Outsourcing]",
            "rdfs:label": "employmentType",
            "rdfs:isDefinedBy": {
                "@id": "iudx:"
            },
            "iudx:domainIncludes": [
                {
                    "@id": "iudx:EmployeeDetails"
                }
            ],
            "iudx:rangeIncludes": [
                {
                    "@id": "iudx:Text"
                },
                {
                    "@id": "iudx:ValueDescriptor"
                }
            ],
            "skos:exactMatch": {
                "@id": "schema:employmentType"
            }
        },
        {
            "@id": "iudx:employmentUnit",
            "@type": [
                "iudx:TextProperty"
            ],
            "rdfs:comment": "Unit and/or facility where the employee reports and/or in which the job is to be performed.\nENUM: [Sweeping, Drainage, Vehicle Driver, Vehicle Helper, Workshop, Door to Door, Supervisor, Office Work]",
            "rdfs:label": "employmentUnit",
            "rdfs:isDefinedBy": {
                "@id": "iudx:"
            },
            "iudx:domainIncludes": [
                {
                    "@id": "iudx:EmployeeDetails"
                }
            ],
            "iudx:rangeIncludes": [
                {
                    "@id": "iudx:Text"
                },
                {
                    "@id": "iudx:ValueDescriptor"
                }
            ],
            "skos:exactMatch": {
                "@id": "schema:employmentUnit"
            }
        },
        {
            "@id": "iudx:endDateTime",
            "@type": [
                "iudx:TimeProperty"
            ],
            "rdfs:comment": "Reported end time corresponding to this observation.",
            "rdfs:label": "endDateTime",
            "rdfs:isDefinedBy": {
                "@id": "iudx:"
            },
            "iudx:domainIncludes": [
                {
                    "@id": "iudx:Version"
                },
                {
                    "@id": "iudx:Camera"
                },
                {
                    "@id": "iudx:EVChargingStation"
                },
                {
                    "@id": "iudx:BikeDockingStation"
                }
            ],
            "iudx:rangeIncludes": [
                {
                    "@id": "iudx:DateTime"
                },
                {
                    "@id": "iudx:ValueDescriptor"
                }
            ]
        },
        {
            "@id": "iudx:energyConsumed",
            "@type": [
                "iudx:QuantitativeProperty"
            ],
            "rdfs:comment": "Energy consumed over a specific time corresponding to this observation.",
            "rdfs:label": "energyConsumed",
            "rdfs:isDefinedBy": {
                "@id": "iudx:"
            },
            "iudx:domainIncludes": [
                {
                    "@id": "iudx:Streetlight"
                },
                {
                    "@id": "iudx:EnergyMeter"
                }
            ],
            "iudx:rangeIncludes": [
                {
                    "@id": "iudx:Number"
                },
                {
                    "@id": "iudx:ValueDescriptor"
                }
            ],
            "skos:exactMatch": {
                "@id": "Fiware:energyConsumed"
            }
        },
        {
            "@id": "iudx:energyEfficiencyStatus",
            "@type": [
                "iudx:QuantitativeProperty"
            ],
            "rdfs:comment": "Describes the energy efficiency status of the air conditioning system by a binary input (0-Inactive, 1-Active)",
            "rdfs:label": "energyEfficiencyStatus",
            "rdfs:isDefinedBy": {
                "@id": "iudx:"
            },
            "iudx:domainIncludes": [
                {
                    "@id": "iudx:AirConditioner"
                }
            ],
            "iudx:rangeIncludes": [
                {
                    "@id": "iudx:Number"
                },
                {
                    "@id": "iudx:ValueDescriptor"
                }
            ]
        },
        {
            "@id": "iudx:energyGenerated",
            "@type": [
                "iudx:QuantitativeProperty"
            ],
            "rdfs:comment": "Energy generated over a specific time range from the energy resource corresponding to this observation.",
            "rdfs:label": "energyGenerated",
            "rdfs:isDefinedBy": {
                "@id": "iudx:"
            },
            "iudx:domainIncludes": [
                {
                    "@id": "iudx:SolarEnergy"
                }
            ],
            "iudx:rangeIncludes": [
                {
                    "@id": "iudx:Number"
                },
                {
                    "@id": "iudx:ValueDescriptor"
                }
            ]
        },
        {
            "@id": "iudx:entity_id",
            "@type": [
                "iudx:TextProperty"
            ],
            "rdfs:comment": "Feed unique ID for the entity corresponding to this observation.SameAs:'entity_id' field from GTFS Realtime message-FeedEntity(https://developers.google.com/transit/gtfs-realtime/reference#message-feedentity)",
            "rdfs:label": "entity_id",
            "rdfs:isDefinedBy": {
                "@id": "iudx:"
            },
            "iudx:domainIncludes": [
                {
                    "@id": "iudx:TransitManagement"
                }
            ],
            "iudx:rangeIncludes": [
                {
                    "@id": "iudx:Text"
                },
                {
                    "@id": "iudx:ValueDescriptor"
                }
            ]
        },
        {
            "@id": "iudx:entryAreaCode",
            "@type": [
                "iudx:TextProperty"
            ],
            "rdfs:comment": "Area code of the passenger boarding stop (used by the fare collection agency). For example, whether the stop is city-bus-service stop or brts stop or other service type stop etc.",
            "rdfs:label": "entryAreaCode",
            "rdfs:isDefinedBy": {
                "@id": "iudx:"
            },
            "iudx:domainIncludes": [
                {
                    "@id": "iudx:FareCollectionSystem"
                }
            ],
            "iudx:rangeIncludes": [
                {
                    "@id": "iudx:Text"
                },
                {
                    "@id": "iudx:ValueDescriptor"
                }
            ]
        },
        {
            "@id": "iudx:entryFee",
            "@type": [
                "iudx:TextProperty"
            ],
            "rdfs:comment": "The amount to be paid to enter the  public site or tourist destination.",
            "rdfs:label": "entryFee",
            "rdfs:isDefinedBy": {
                "@id": "iudx:"
            },
            "iudx:domainIncludes": [
                {
                    "@id": "iudx:TouristDestination"
                }
            ],
            "iudx:rangeIncludes": [
                {
                    "@id": "iudx:Text"
                },
                {
                    "@id": "iudx:ValueDescriptor"
                }
            ]
        },
        {
            "@id": "iudx:equipmentCompanyCode",
            "@type": [
                "iudx:TextProperty"
            ],
            "rdfs:comment": "Company/Agency code for the transaction equipment (used by fare collection agency). For example, 103 - CBS (city bus service),102 -  BRTS etc.",
            "rdfs:label": "equipmentCompanyCode",
            "rdfs:isDefinedBy": {
                "@id": "iudx:"
            },
            "iudx:domainIncludes": [
                {
                    "@id": "iudx:FareCollectionSystem"
                }
            ],
            "iudx:rangeIncludes": [
                {
                    "@id": "iudx:Text"
                },
                {
                    "@id": "iudx:ValueDescriptor"
                }
            ]
        },
        {
            "@id": "iudx:equipmentID",
            "@type": [
                "iudx:TextProperty"
            ],
            "rdfs:comment": "Unique ID of the equipment corresponding to this observation.",
            "rdfs:label": "equipmentID",
            "rdfs:isDefinedBy": {
                "@id": "iudx:"
            },
            "iudx:domainIncludes": [
                {
                    "@id": "iudx:FareCollectionSystem"
                },
                {
                    "@id": "iudx:TrafficViolations"
                }
            ],
            "iudx:rangeIncludes": [
                {
                    "@id": "iudx:Text"
                },
                {
                    "@id": "iudx:ValueDescriptor"
                }
            ]
        },
        {
            "@id": "iudx:equipmentSequenceNumber",
            "@type": [
                "iudx:QuantitativeProperty"
            ],
            "rdfs:comment": "Sequence number for the given equipment.",
            "rdfs:label": "equipmentSequenceNumber",
            "rdfs:isDefinedBy": {
                "@id": "iudx:"
            },
            "iudx:domainIncludes": [
                {
                    "@id": "iudx:FareCollectionSystem"
                }
            ],
            "iudx:rangeIncludes": [
                {
                    "@id": "iudx:Number"
                },
                {
                    "@id": "iudx:ValueDescriptor"
                }
            ]
        },
        {
            "@id": "iudx:equipmentStopID",
            "@type": [
                "iudx:TextProperty"
            ],
            "rdfs:comment": "Stop ID (BRTS) at which the equipment corresponding to this transaction is installed.",
            "rdfs:label": "equipmentStopID",
            "rdfs:isDefinedBy": {
                "@id": "iudx:"
            },
            "iudx:domainIncludes": [
                {
                    "@id": "iudx:FareCollectionSystem"
                }
            ],
            "iudx:rangeIncludes": [
                {
                    "@id": "iudx:Text"
                },
                {
                    "@id": "iudx:ValueDescriptor"
                }
            ]
        },
        {
            "@id": "iudx:equipmentType",
            "@type": [
                "iudx:TextProperty"
            ],
            "rdfs:comment": "Type of equipment or the name of the equipment corresponding to this observation.",
            "rdfs:label": "equipmentType",
            "rdfs:isDefinedBy": {
                "@id": "iudx:"
            },
            "iudx:domainIncludes": [
                {
                    "@id": "iudx:FareCollectionSystem"
                },
                {
                    "@id": "iudx:TrafficViolations"
                }
            ],
            "iudx:rangeIncludes": [
                {
                    "@id": "iudx:Text"
                },
                {
                    "@id": "iudx:ValueDescriptor"
                }
            ]
        },
        {
            "@id": "iudx:equipmentTypeCode",
            "@type": [
                "iudx:TextProperty"
            ],
            "rdfs:comment": "Unique code indicating the type of equipment used in the transaction (used by fare collection agency).ENUM [1B, 42, 02, 08, 41]\n1B - POS, 42 - HTT, 02- Mobile, 08- Fare Gate, 41- Pole Validator",
            "rdfs:label": "equipmentTypeCode",
            "rdfs:isDefinedBy": {
                "@id": "iudx:"
            },
            "iudx:domainIncludes": [
                {
                    "@id": "iudx:FareCollectionSystem"
                }
            ],
            "iudx:rangeIncludes": [
                {
                    "@id": "iudx:Text"
                },
                {
                    "@id": "iudx:ValueDescriptor"
                }
            ]
        },
        {
            "@id": "iudx:establishmentType",
            "@type": [
                "iudx:TextProperty"
            ],
            "rdfs:comment": "Type of public service or business or facility set up for public welfare or governance. For eg., the establishment can be a business under an individual as a sole proprietor(or a company) or smart public installments such as lavatories etc.",
            "rdfs:label": "establishmentType",
            "rdfs:isDefinedBy": {
                "@id": "iudx:"
            },
            "iudx:domainIncludes": [
                {
                    "@id": "iudx:RevenueCollection"
                }
            ],
            "iudx:rangeIncludes": [
                {
                    "@id": "iudx:Text"
                },
                {
                    "@id": "iudx:ValueDescriptor"
                }
            ]
        },
        {
            "@id": "iudx:etx",
            "@type": [
                "iudx:QuantitativeProperty"
            ],
            "rdfs:comment": "Expected Transmission Count is an Exponentially Weighted Moving Average of the number of expected packet transmissions required for error-free reception at destination.",
            "rdfs:label": "etx",
            "rdfs:isDefinedBy": {
                "@id": "iudx:"
            },
            "iudx:domainIncludes": [
                {
                    "@id": "iudx:WirelessNetwork"
                }
            ],
            "iudx:rangeIncludes": [
                {
                    "@id": "iudx:Number"
                },
                {
                    "@id": "iudx:ValueDescriptor"
                }
            ]
        },
        {
            "@id": "iudx:exitAreaCode",
            "@type": [
                "iudx:TextProperty"
            ],
            "rdfs:comment": "Area code of the passenger alighting stop (used by the fare collection agency). For example, whether the stop is city-bus-service stop or brts stop or other service type stop etc.",
            "rdfs:label": "exitAreaCode",
            "rdfs:isDefinedBy": {
                "@id": "iudx:"
            },
            "iudx:domainIncludes": [
                {
                    "@id": "iudx:FareCollectionSystem"
                }
            ],
            "iudx:rangeIncludes": [
                {
                    "@id": "iudx:Text"
                },
                {
                    "@id": "iudx:ValueDescriptor"
                }
            ]
        },
        {
            "@id": "iudx:f_name",
            "@type": [
                "iudx:TextProperty"
            ],
            "rdfs:comment": "Name of the feature corresponding this observation",
            "rdfs:label": "f_name",
            "rdfs:isDefinedBy": {
                "@id": "iudx:"
            },
            "iudx:domainIncludes": [
                {
                    "@id": "iudx:FeaturesOfInterest"
                }
            ],
            "iudx:rangeIncludes": [
                {
                    "@id": "iudx:Text"
                },
                {
                    "@id": "iudx:ValueDescriptor"
                }
            ]
        },
        {
            "@id": "iudx:fareForAdult",
            "@type": [
                "iudx:QuantitativeProperty"
            ],
            "rdfs:comment": "The fare for an adult in the journey corresponding to this observation.",
            "rdfs:label": "fareForAdult",
            "rdfs:isDefinedBy": {
                "@id": "iudx:"
            },
            "iudx:domainIncludes": [
                {
                    "@id": "iudx:FareCollectionSystem"
                }
            ],
            "iudx:rangeIncludes": [
                {
                    "@id": "iudx:Number"
                },
                {
                    "@id": "iudx:ValueDescriptor"
                }
            ]
        },
        {
            "@id": "iudx:fareForChild",
            "@type": [
                "iudx:QuantitativeProperty"
            ],
            "rdfs:comment": "The fare for a child in the journey corresponding to this observation.",
            "rdfs:label": "fareForChild",
            "rdfs:isDefinedBy": {
                "@id": "iudx:"
            },
            "iudx:domainIncludes": [
                {
                    "@id": "iudx:FareCollectionSystem"
                }
            ],
            "iudx:rangeIncludes": [
                {
                    "@id": "iudx:Number"
                },
                {
                    "@id": "iudx:ValueDescriptor"
                }
            ]
        },
        {
            "@id": "iudx:faultTitle",
            "@type": [
                "iudx:TextProperty"
            ],
            "rdfs:comment": "The brief discription of the fault or issues of the product based on the experience of user.",
            "rdfs:label": "faultTitle",
            "rdfs:isDefinedBy": {
                "@id": "iudx:"
            },
            "iudx:domainIncludes": [
                {
                    "@id": "iudx:BikeDockingStation"
                }
            ],
            "iudx:rangeIncludes": [
                {
                    "@id": "iudx:Text"
                },
                {
                    "@id": "iudx:ValueDescriptor"
                }
            ],
            "skos:exactMatch": {
                "@id": "Fiware:faultLog"
            }
        },
        {
            "@id": "iudx:feederConnectivity",
            "@type": [
                "iudx:TextProperty"
            ],
            "rdfs:comment": "Describes the connectivity status of the streetlight feeder panel associated with the streetlight corresponding to this observation. ENUM: [connected, disconnected]",
            "rdfs:label": "feederConnectivity",
            "rdfs:isDefinedBy": {
                "@id": "iudx:"
            },
            "iudx:domainIncludes": [
                {
                    "@id": "iudx:Streetlight"
                }
            ],
            "iudx:rangeIncludes": [
                {
                    "@id": "iudx:Text"
                },
                {
                    "@id": "iudx:ValueDescriptor"
                }
            ]
        },
        {
            "@id": "iudx:feederPillarNum",
            "@type": [
                "iudx:TextProperty"
            ],
            "rdfs:comment": "Streetlight feeder pillar information associated with the streetlight corresponding to this observation.",
            "rdfs:label": "feederPillarNum",
            "rdfs:isDefinedBy": {
                "@id": "iudx:"
            },
            "iudx:domainIncludes": [
                {
                    "@id": "iudx:Streetlight"
                }
            ],
            "iudx:rangeIncludes": [
                {
                    "@id": "iudx:Text"
                },
                {
                    "@id": "iudx:ValueDescriptor"
                }
            ]
        },
        {
            "@id": "iudx:femaleTotal",
            "@type": [
                "iudx:QuantitativeProperty"
            ],
            "rdfs:comment": "The total count of females of a particular species, as identified by the device.",
            "rdfs:label": "femaleTotal",
            "rdfs:isDefinedBy": {
                "@id": "iudx:"
            },
            "iudx:domainIncludes": [
                {
                    "@id": "iudx:MosquitoDensity"
                }
            ],
            "iudx:rangeIncludes": [
                {
                    "@id": "iudx:Number"
                },
                {
                    "@id": "iudx:ValueDescriptor"
                }
            ]
        },
        {
            "@id": "iudx:fid",
            "@type": [
                "iudx:QuantitativeProperty"
            ],
            "rdfs:comment": "The fid corresponding to this observation.",
            "rdfs:label": "fid",
            "iudx:domainIncludes": [
                {
                    "@id": "iudx:Headquarters"
                },
                {
                    "@id": "iudx:District"
                },
                {
                    "@id": "iudx:States"
                },
                {
                    "@id": "iudx:FeaturesOfInterest"
                }
            ],
            "iudx:rangeIncludes": [
                {
                    "@id": "iudx:Number"
                },
                {
                    "@id": "iudx:ValueDescriptor"
                }
            ],
            "rdfs:isDefinedBy": {
                "@id": "iudx:"
            }
        },
        {
            "@id": "iudx:filterSign",
            "@type": [
                "iudx:QuantitativeProperty"
            ],
            "rdfs:comment": "Binary Input (0-Inactive, 1-Active), [bool], [n/a], [n/a], [n/a]",
            "rdfs:label": "filterSign",
            "rdfs:isDefinedBy": {
                "@id": "iudx:"
            },
            "iudx:domainIncludes": [
                {
                    "@id": "iudx:AirConditioner"
                }
            ],
            "iudx:rangeIncludes": [
                {
                    "@id": "iudx:Number"
                },
                {
                    "@id": "iudx:ValueDescriptor"
                }
            ]
        },
        {
            "@id": "iudx:floodLevelStatus",
            "@type": [
                "iudx:TextProperty"
            ],
            "rdfs:comment": "Flood level status indication given by the flood sensing device. The status is marked Danger if the current level is higher than the danger level threshold value.",
            "rdfs:label": "floodLevelStatus",
            "rdfs:isDefinedBy": {
                "@id": "iudx:"
            },
            "iudx:domainIncludes": [
                {
                    "@id": "iudx:EnvFlood"
                }
            ],
            "iudx:rangeIncludes": [
                {
                    "@id": "iudx:Text"
                },
                {
                    "@id": "iudx:ValueDescriptor"
                }
            ]
        },
        {
            "@id": "iudx:flowrate",
            "@type": [
                "iudx:QuantitativeProperty"
            ],
            "rdfs:comment": "Volume of water flowing in/out of the water storage tank corresponding to this observation.",
            "rdfs:label": "flowrate",
            "rdfs:isDefinedBy": {
                "@id": "iudx:"
            },
            "iudx:domainIncludes": [
                {
                    "@id": "iudx:WaterDistributionNetwork"
                }
            ],
            "iudx:rangeIncludes": [
                {
                    "@id": "iudx:Number"
                },
                {
                    "@id": "iudx:ValueDescriptor"
                }
            ],
            "skos:exactMatch": {
                "@id": "Fiware: WasteWaterJunction.flowrate"
            }
        },
        {
            "@id": "iudx:forcedThermoOffStatus",
            "@type": [
                "iudx:QuantitativeProperty"
            ],
            "rdfs:comment": "Describes the status by a binary Input (0-Inactive, 1-Active)",
            "rdfs:label": "forcedThermoOffStatus",
            "rdfs:isDefinedBy": {
                "@id": "iudx:"
            },
            "iudx:domainIncludes": [
                {
                    "@id": "iudx:AirConditioner"
                }
            ],
            "iudx:rangeIncludes": [
                {
                    "@id": "iudx:Number"
                },
                {
                    "@id": "iudx:ValueDescriptor"
                }
            ]
        },
        {
            "@id": "iudx:freeSlotNumber",
            "@type": [
                "iudx:QuantitativeProperty"
            ],
            "rdfs:comment": "The number of bike racks or docking slots available for returning and parking bikes in the bike docking station corresponding to this observation.",
            "rdfs:label": "freeSlotNumber",
            "rdfs:isDefinedBy": {
                "@id": "iudx:"
            },
            "iudx:domainIncludes": [
                {
                    "@id": "iudx:BikeDockingStation"
                }
            ],
            "iudx:rangeIncludes": [
                {
                    "@id": "iudx:Number"
                },
                {
                    "@id": "iudx:ValueDescriptor"
                }
            ],
            "skos:exactMatch": {
                "@id": "Fiware:freeSlotNumber"
            }
        },
        {
            "@id": "iudx:frequency",
            "@type": [
                "iudx:QuantitativeProperty"
            ],
            "rdfs:comment": "Frequency observed from the entity corresponding to this observation.",
            "rdfs:label": "frequency",
            "rdfs:isDefinedBy": {
                "@id": "iudx:"
            },
            "iudx:domainIncludes": [
                {
                    "@id": "iudx:SolarEnergy"
                },
                {
                    "@id": "iudx:EnergyMeter"
                }
            ],
            "iudx:rangeIncludes": [
                {
                    "@id": "iudx:Number"
                },
                {
                    "@id": "iudx:ValueDescriptor"
                }
            ],
            "skos:exactMatch": {
                "@id": "Fiware:frequency"
            }
        },
        {
            "@id": "iudx:fuelEfficiency",
            "@type": [
                "iudx:QuantitativeProperty"
            ],
            "rdfs:comment": "The distance traveled per unit of fuel used.",
            "rdfs:label": "fuelEfficiency",
            "iudx:domainIncludes": [
                {
                    "@id": "iudx:WmgmtVehicle"
                },
                {
                    "@id": "iudx:EmergencyVehicle"
                }
            ],
            "iudx:rangeIncludes": [
                {
                    "@id": "iudx:Number"
                },
                {
                    "@id": "iudx:ValueDescriptor"
                }
            ],
            "rdfs:isDefinedBy": {
                "@id": "iudx:"
            },
            "skos:exactMatch": {
                "@id": "schema:fuelEfficiency"
            }
        },
        {
            "@id": "iudx:fuelFilled",
            "@type": [
                "iudx:QuantitativeProperty"
            ],
            "rdfs:comment": "Amount of fuel filled to the vehicle corresponding to this observation.",
            "rdfs:label": "fuelFilled",
            "rdfs:isDefinedBy": {
                "@id": "iudx:"
            },
            "iudx:domainIncludes": [
                {
                    "@id": "iudx:WmgmtVehicle"
                },
                {
                    "@id": "iudx:EmergencyVehicle"
                }
            ],
            "iudx:rangeIncludes": [
                {
                    "@id": "iudx:Number"
                },
                {
                    "@id": "iudx:ValueDescriptor"
                }
            ]
        },
        {
            "@id": "iudx:fuelType",
            "@type": [
                "iudx:TextProperty"
            ],
            "rdfs:comment": "The type of fuel suitable for the engine or engines of the vehicle corresponding to this observation.",
            "rdfs:label": "fuelType",
            "rdfs:isDefinedBy": {
                "@id": "iudx:"
            },
            "iudx:domainIncludes": [
                {
                    "@id": "iudx:WmgmtVehicle"
                },
                {
                    "@id": "iudx:EmergencyVehicle"
                }
            ],
            "iudx:rangeIncludes": [
                {
                    "@id": "iudx:Text"
                },
                {
                    "@id": "iudx:ValueDescriptor"
                }
            ],
            "skos:exactMatch": {
                "@id": "schema:fuelType"
            }
        },
        {
            "@id": "iudx:gender",
            "@type": [
                "iudx:TextProperty"
            ],
            "rdfs:comment": "Gender of the employee or person corresponding to this observation.",
            "rdfs:label": "gender",
            "rdfs:isDefinedBy": {
                "@id": "iudx:"
            },
            "iudx:domainIncludes": [
                {
                    "@id": "iudx:EmployeeDetails"
                }
            ],
            "iudx:rangeIncludes": [
                {
                    "@id": "iudx:Text"
                },
                {
                    "@id": "iudx:ValueDescriptor"
                }
            ],
            "skos:exactMatch": {
                "@id": "schema:gender"
            }
        },
        {
            "@id": "iudx:geometry",
            "@type": [
                "iudx:GeoProperty"
            ],
            "rdfs:comment": "The location coordinates of the corresponding issue reported.",
            "rdfs:label": "geometry",
            "rdfs:isDefinedBy": {
                "@id": "iudx:"
            },
            "iudx:domainIncludes": [
                {
                    "@id": "iudx:Headquarters"
                },
                {
                    "@id": "iudx:Headquarters"
                }
            ],
            "iudx:rangeIncludes": [
                {
                    "@id": "iudx:Place"
                },
                {
                    "@id": "iudx:ValueDescriptor"
                }
            ]
        },
        {
            "@id": "iudx:gisAccessToken",
            "@type": [
                "iudx:TextProperty"
            ],
            "rdfs:comment": "A string of encrypted information that contains the user's name, the token expiration time, and some proprietary information, which is used to access the secured GIS services from the GIS Server.",
            "rdfs:label": "gisAccessToken",
            "rdfs:isDefinedBy": {
                "@id": "iudx:"
            },
            "iudx:domainIncludes": [
                {
                    "@id": "iudx:GISData"
                }
            ],
            "iudx:rangeIncludes": [
                {
                    "@id": "iudx:Text"
                },
                {
                    "@id": "iudx:ValueDescriptor"
                }
            ]
        },
        {
            "@id": "iudx:gisServerURL",
            "@type": [
                "iudx:TextProperty"
            ],
            "rdfs:comment": "The Geographic Information System (GIS) Server's URL, used\u00a0for capturing, storing, and displaying data on positions on the earth's surface.",
            "rdfs:label": "gisServerURL",
            "rdfs:isDefinedBy": {
                "@id": "iudx:"
            },
            "iudx:domainIncludes": [
                {
                    "@id": "iudx:GISData"
                }
            ],
            "iudx:rangeIncludes": [
                {
                    "@id": "iudx:Text"
                },
                {
                    "@id": "iudx:ValueDescriptor"
                }
            ]
        },
        {
            "@id": "iudx:grantAmount",
            "@type": [
                "iudx:QuantitativeProperty"
            ],
            "rdfs:comment": "The amount released for the public welfare under the scheme from the total budget corresponding to this observation.",
            "rdfs:label": "grantAmount",
            "rdfs:isDefinedBy": {
                "@id": "iudx:"
            },
            "iudx:domainIncludes": [
                {
                    "@id": "iudx:PublicSchemes"
                }
            ],
            "iudx:rangeIncludes": [
                {
                    "@id": "iudx:Number"
                },
                {
                    "@id": "iudx:ValueDescriptor"
                }
            ],
            "skos:exactMatch": {
                "@id": "schema: funding"
            }
        },
        {
            "@id": "iudx:gustSpeed",
            "@type": [
                "iudx:QuantitativeProperty"
            ],
            "rdfs:comment": "A sudden burst of high-speed wind over the observed average wind speed lasting  only for a few seconds.",
            "rdfs:label": "gustSpeed",
            "rdfs:isDefinedBy": {
                "@id": "iudx:"
            },
            "iudx:domainIncludes": [
                {
                    "@id": "iudx:EnvWeather"
                }
            ],
            "iudx:rangeIncludes": [
                {
                    "@id": "iudx:Number"
                },
                {
                    "@id": "iudx:ValueDescriptor"
                }
            ]
        },
        {
            "@id": "iudx:hasObject",
            "@type": [
                "iudx:TextProperty"
            ],
            "rdfs:comment": "Value associated with RelationshipValue class. Contains IRI(s) that specify the relationship object(s).",
            "rdfs:label": "hasObject",
            "iudx:domainIncludes": [
                {
                    "@id": "iudx:RelationshipValue"
                }
            ],
            "iudx:rangeIncludes": [
                {
                    "@id": "iudx:Text",
                    "@type": "@id"
                },
                {
                    "@id": "iudx:Text",
                    "@type": "@id",
                    "@container": "@set"
                },
                {
                    "@id": "iudx:ValueDescriptor"
                }
            ]
        },
        {
            "@id": "iudx:heaterStatus",
            "@type": [
                "iudx:QuantitativeProperty"
            ],
            "rdfs:comment": "Describes the heater status of the air conditioning system by a binary input (0-Inactive, 1-Active)",
            "rdfs:label": "heaterStatus",
            "rdfs:isDefinedBy": {
                "@id": "iudx:"
            },
            "iudx:domainIncludes": [
                {
                    "@id": "iudx:AirConditioner"
                }
            ],
            "iudx:rangeIncludes": [
                {
                    "@id": "iudx:Number"
                },
                {
                    "@id": "iudx:ValueDescriptor"
                }
            ]
        },
        {
            "@id": "iudx:hq",
            "@type": [
                "iudx:TextProperty"
            ],
            "rdfs:comment": "Name of the headquarters corresponding to this observation.",
            "rdfs:label": "hq",
            "rdfs:isDefinedBy": {
                "@id": "iudx:"
            },
            "iudx:domainIncludes": [
                {
                    "@id": "iudx:Headquarters"
                }
            ],
            "iudx:rangeIncludes": [
                {
                    "@id": "iudx:Text"
                },
                {
                    "@id": "iudx:ValueDescriptor"
                }
            ]
        },
        {
            "@id": "iudx:ignitionStatus",
            "@type": [
                "iudx:TextProperty"
            ],
            "rdfs:comment": "Gives the ignition status of the vehicle.ENUM: [Y, N]",
            "rdfs:label": "ignitionStatus",
            "rdfs:isDefinedBy": {
                "@id": "iudx:"
            },
            "iudx:domainIncludes": [
                {
                    "@id": "iudx:WmgmtVehicle"
                },
                {
                    "@id": "iudx:EmergencyVehicle"
                }
            ],
            "iudx:rangeIncludes": [
                {
                    "@id": "iudx:Text"
                },
                {
                    "@id": "iudx:ValueDescriptor"
                }
            ]
        },
        {
            "@id": "iudx:illuminance",
            "@type": [
                "iudx:QuantitativeProperty"
            ],
            "rdfs:comment": "Observed instantaneous ambient light intensity.",
            "rdfs:label": "illuminance",
            "iudx:domainIncludes": [
                {
                    "@id": "iudx:EnvWeather"
                },
                {
                    "@id": "iudx:EnvAQM"
                },
                {
                    "@id": "iudx:AirQuality"
                }
            ],
            "iudx:rangeIncludes": [
                {
                    "@id": "iudx:Number"
                },
                {
                    "@id": "iudx:ValueDescriptor"
                },
                {
                    "@id": "iudx:TimeSeriesAggregation"
                }
            ],
            "rdfs:isDefinedBy": {
                "@id": "iudx:"
            },
            "skos:exactMatch": {
                "@id": "Fiware:illuminance"
            }
        },
        {
            "@id": "iudx:imageBounds",
            "@type": [
                "iudx:GeoProperty"
            ],
            "rdfs:comment": "A bbox in the form [lowerlon, lowerlat, upperlon, upperlat].",
            "rdfs:label": "imageBounds",
            "rdfs:isDefinedBy": {
                "@id": "iudx:"
            },
            "iudx:domainIncludes": [
                {
                    "@id": "iudx:MapTiles"
                }
            ],
            "iudx:rangeIncludes": [
                {
                    "@id": "iudx:GeoJSONGeometry"
                },
                {
                    "@id": "iudx:Place"
                },
                {
                    "@id": "iudx:ValueDescriptor"
                }
            ]
        },
        {
            "@id": "iudx:imageFormat",
            "@type": [
                "iudx:TextProperty"
            ],
            "rdfs:comment": "The format of the image corresponding this observation. It can take up values like png, jpg, etc",
            "rdfs:label": "imageFormat",
            "rdfs:isDefinedBy": {
                "@id": "iudx:"
            },
            "iudx:domainIncludes": [
                {
                    "@id": "iudx:MapTiles"
                }
            ],
            "iudx:rangeIncludes": [
                {
                    "@id": "iudx:Text"
                },
                {
                    "@id": "iudx:ValueDescriptor"
                }
            ]
        },
        {
            "@id": "iudx:imageSnapshot",
            "@type": [
                "iudx:TextProperty"
            ],
            "rdfs:comment": "Camera feed snapshot download link for the camera corresponding to this observation",
            "rdfs:label": "imageSnapshot",
            "rdfs:isDefinedBy": {
                "@id": "iudx:"
            },
            "iudx:domainIncludes": [
                {
                    "@id": "iudx:Camera"
                }
            ],
            "iudx:rangeIncludes": [
                {
                    "@id": "iudx:Text"
                },
                {
                    "@id": "iudx:ValueDescriptor"
                }
            ]
        },
        {
            "@id": "iudx:inFlow",
            "@type": [
                "iudx:QuantitativeProperty"
            ],
            "rdfs:comment": "In-flow amount into the treatment plant/reservoir corresponding to this observation.",
            "rdfs:label": "inFlow",
            "rdfs:isDefinedBy": {
                "@id": "iudx:"
            },
            "iudx:domainIncludes": [
                {
                    "@id": "iudx:WasteWaterMgmt"
                }
            ],
            "iudx:rangeIncludes": [
                {
                    "@id": "iudx:Number"
                },
                {
                    "@id": "iudx:ValueDescriptor"
                }
            ]
        },
        {
            "@id": "iudx:indiadpt",
            "@type": [
                "iudx:QuantitativeProperty"
            ],
            "rdfs:comment": "Department/Division or section of the organization corresponding to this observation. Eg. Health, Transport.",
            "rdfs:label": "indiadpt",
            "rdfs:isDefinedBy": {
                "@id": "iudx:"
            },
            "iudx:domainIncludes": [
                {
                    "@id": "iudx:Headquarters"
                }
            ],
            "iudx:rangeIncludes": [
                {
                    "@id": "iudx:Number"
                },
                {
                    "@id": "iudx:ValueDescriptor"
                }
            ]
        },
        {
            "@id": "iudx:indiadpt_i",
            "@type": [
                "iudx:QuantitativeProperty"
            ],
            "rdfs:comment": "The name of Indian department I corresponding to this observation.",
            "rdfs:label": "indiadpt_i",
            "rdfs:isDefinedBy": {
                "@id": "iudx:"
            },
            "iudx:domainIncludes": [
                {
                    "@id": "iudx:Headquarters"
                }
            ],
            "iudx:rangeIncludes": [
                {
                    "@id": "iudx:Number"
                },
                {
                    "@id": "iudx:ValueDescriptor"
                }
            ]
        },
        {
            "@id": "iudx:indoorFanStatus",
            "@type": [
                "iudx:QuantitativeProperty"
            ],
            "rdfs:comment": "Describes the indoor fan status of the air conditioning system by a binary input (0-Inactive, 1-Active)",
            "rdfs:label": "indoorFanStatus",
            "rdfs:isDefinedBy": {
                "@id": "iudx:"
            },
            "iudx:domainIncludes": [
                {
                    "@id": "iudx:AirConditioner"
                }
            ],
            "iudx:rangeIncludes": [
                {
                    "@id": "iudx:Number"
                },
                {
                    "@id": "iudx:ValueDescriptor"
                }
            ]
        },
        {
            "@id": "iudx:instValue",
            "@type": [
                "iudx:QuantitativeProperty"
            ],
            "rdfs:comment": "Describes the instantaneous value (associated with the current timestamp) of a time varying quantity.",
            "rdfs:label": "instValue",
            "iudx:domainIncludes": [
                {
                    "@id": "iudx:TimeSeriesAggregation"
                }
            ],
            "iudx:rangeIncludes": [
                {
                    "@id": "iudx:Number"
                },
                {
                    "@id": "iudx:ValueDescriptor"
                }
            ]
        },
        {
            "@id": "iudx:irradiation",
            "@type": [
                "iudx:QuantitativeProperty"
            ],
            "rdfs:comment": "The measure of radiation falling per unit area of a surface exposed to it.",
            "rdfs:label": "irradiation",
            "rdfs:isDefinedBy": {
                "@id": "iudx:"
            },
            "iudx:domainIncludes": [
                {
                    "@id": "iudx:SolarEnergy"
                }
            ],
            "iudx:rangeIncludes": [
                {
                    "@id": "iudx:Number"
                },
                {
                    "@id": "iudx:ValueDescriptor"
                }
            ]
        },
        {
            "@id": "iudx:isOccupied",
            "@type": [
                "iudx:QuantitativeProperty"
            ],
            "rdfs:comment": "A flag that denotes if the entity corresponding to this observation is occupied or not (0 - Occupied, 1 - Not Occupied).",
            "rdfs:label": "isOccupied",
            "rdfs:isDefinedBy": {
                "@id": "iudx:"
            },
            "iudx:domainIncludes": [
                {
                    "@id": "iudx:RoomOccupancy"
                }
            ],
            "iudx:rangeIncludes": [
                {
                    "@id": "iudx:Number"
                },
                {
                    "@id": "iudx:ValueDescriptor"
                }
            ]
        },
        {
            "@id": "iudx:isRelatedTo",
            "@type": [
                "iudx:TextProperty"
            ],
            "rdfs:comment": "Value associated with RelationshipValue class. Contains IRI(s) that specify the relationship object(s).",
            "rdfs:label": "isRelatedTo",
            "iudx:domainIncludes": [
                {
                    "@id": "iudx:RelationshipValue"
                }
            ],
            "iudx:rangeIncludes": [
                {
                    "@id": "iudx:Text",
                    "@type": "@id"
                },
                {
                    "@id": "iudx:Text",
                    "@type": "@id",
                    "@container": "@set"
                },
                {
                    "@id": "iudx:ValueDescriptor"
                }
            ]
        },
        {
            "@id": "iudx:junctionID",
            "@type": [
                "iudx:TextProperty"
            ],
            "rdfs:comment": "Unique representation of the junction corresponding to this observation.",
            "rdfs:label": "junctionID",
            "rdfs:isDefinedBy": {
                "@id": "iudx:"
            },
            "iudx:domainIncludes": [
                {
                    "@id": "iudx:RoadSegment"
                }
            ],
            "iudx:rangeIncludes": [
                {
                    "@id": "iudx:Text"
                },
                {
                    "@id": "iudx:ValueDescriptor"
                }
            ]
        },
        {
            "@id": "iudx:junctionLocation",
            "@type": [
                "iudx:GeoProperty"
            ],
            "rdfs:comment": "The physical coordinates of the location of junction corresponding to this observation.",
            "rdfs:label": "junctionLocation",
            "rdfs:isDefinedBy": {
                "@id": "iudx:"
            },
            "iudx:domainIncludes": [
                {
                    "@id": "iudx:RoadSegment"
                }
            ],
            "iudx:rangeIncludes": [
                {
                    "@id": "iudx:Place"
                },
                {
                    "@id": "iudx:ValueDescriptor"
                }
            ]
        },
        {
            "@id": "iudx:junctionMode",
            "@type": [
                "iudx:TextProperty"
            ],
            "rdfs:comment": "The mode of operation of the traffic junction corresponding to this observation. For eg, Blinker, Flash, ATCS, etc.",
            "rdfs:label": "junctionMode",
            "rdfs:isDefinedBy": {
                "@id": "iudx:"
            },
            "iudx:domainIncludes": [
                {
                    "@id": "iudx:RoadSegment"
                }
            ],
            "iudx:rangeIncludes": [
                {
                    "@id": "iudx:Text"
                },
                {
                    "@id": "iudx:ValueDescriptor"
                }
            ]
        },
        {
            "@id": "iudx:junctionName",
            "@type": [
                "iudx:TextProperty"
            ],
            "rdfs:comment": "The name of the road junction corresponding to this observation",
            "rdfs:label": "junctionName",
            "rdfs:isDefinedBy": {
                "@id": "iudx:"
            },
            "iudx:domainIncludes": [
                {
                    "@id": "iudx:RoadSegment"
                }
            ],
            "iudx:rangeIncludes": [
                {
                    "@id": "iudx:Text"
                },
                {
                    "@id": "iudx:ValueDescriptor"
                }
            ]
        },
        {
            "@id": "iudx:landfillSite",
            "@type": [
                "iudx:TextProperty"
            ],
            "rdfs:comment": "The name of the landfill site or dump yard or dumping station corresponding this observation.",
            "rdfs:label": "landfillSite",
            "rdfs:isDefinedBy": {
                "@id": "iudx:"
            },
            "iudx:domainIncludes": [
                {
                    "@id": "iudx:WmgmtVehicle"
                }
            ],
            "iudx:rangeIncludes": [
                {
                    "@id": "iudx:Text"
                },
                {
                    "@id": "iudx:ValueDescriptor"
                }
            ]
        },
        {
            "@id": "iudx:landmark",
            "@type": [
                "iudx:GeoProperty"
            ],
            "rdfs:comment": "A physical distinguishing feature on land that marks a locality or a place.",
            "rdfs:label": "landmark",
            "iudx:domainIncludes": [
                {
                    "@id": "iudx:IssueReporting"
                }
            ],
            "iudx:rangeIncludes": [
                {
                    "@id": "iudx:Text"
                },
                {
                    "@id": "iudx:ValueDescriptor"
                }
            ],
            "rdfs:isDefinedBy": {
                "@id": "iudx:"
            }
        },
        {
            "@id": "iudx:laneDirection",
            "@type": [
                "iudx:TextProperty"
            ],
            "rdfs:comment": "Describes the direction in which vehicles are plying on the lane corresponding to this observation. ENUM [FORWARD, BACKWARD, INBOUND, OUTBOUND, RIGHT, LEFT]",
            "rdfs:label": "laneDirection",
            "rdfs:isDefinedBy": {
                "@id": "iudx:"
            },
            "iudx:domainIncludes": [
                {
                    "@id": "iudx:LaneDesc"
                }
            ],
            "iudx:rangeIncludes": [
                {
                    "@id": "iudx:Text"
                },
                {
                    "@id": "iudx:ValueDescriptor"
                }
            ],
            "skos:exactMatch": {
                "@id": "Fiware:laneDirection"
            }
        },
        {
            "@id": "iudx:laneId",
            "@type": [
                "iudx:QuantitativeProperty"
            ],
            "rdfs:comment": "Unique identification number of the lane corresponding to this observation.",
            "rdfs:label": "laneId",
            "rdfs:isDefinedBy": {
                "@id": "iudx:"
            },
            "iudx:domainIncludes": [
                {
                    "@id": "iudx:LaneDesc"
                }
            ],
            "iudx:rangeIncludes": [
                {
                    "@id": "iudx:Number"
                },
                {
                    "@id": "iudx:ValueDescriptor"
                }
            ],
            "skos:exactMatch": {
                "@id": "Fiware: laneId"
            }
        },
        {
            "@id": "iudx:laneLength",
            "@type": [
                "iudx:QuantitativeProperty"
            ],
            "rdfs:comment": "Length of the lane corresponding to this observation",
            "rdfs:label": "laneLength",
            "rdfs:isDefinedBy": {
                "@id": "iudx:"
            },
            "iudx:domainIncludes": [
                {
                    "@id": "iudx:LaneDesc"
                }
            ],
            "iudx:rangeIncludes": [
                {
                    "@id": "iudx:Number"
                },
                {
                    "@id": "iudx:ValueDescriptor"
                }
            ],
            "skos:exactMatch": {
                "@id": "Fiware:laneLength"
            }
        },
        {
            "@id": "iudx:laneWidth",
            "@type": [
                "iudx:QuantitativeProperty"
            ],
            "rdfs:comment": "Width of the lane corresponding to this observation",
            "rdfs:label": "laneWidth",
            "rdfs:isDefinedBy": {
                "@id": "iudx:"
            },
            "iudx:domainIncludes": [
                {
                    "@id": "iudx:LaneDesc"
                }
            ],
            "iudx:rangeIncludes": [
                {
                    "@id": "iudx:Number"
                },
                {
                    "@id": "iudx:ValueDescriptor"
                }
            ],
            "skos:exactMatch": {
                "@id": "Fiware:laneWidth"
            }
        },
        {
            "@id": "iudx:last_stop_arrival_time",
            "@type": [
                "iudx:TimeProperty"
            ],
            "rdfs:comment": "Specifies the arrival time at the previous stop for a specific trip on a route. Times must be eight digits in HH:MM:SS format (H:MM:SS is also accepted, if the hour begins with 0). \nNote: Trips that span multiple dates will have stop times greater than 24:00:00. For example, if a trip begins at 10:30:00 p.m. and ends at 2:15:00 a.m. on the following day, the stop times would be 22:30:00 and 26:15:00. Entering those stop times as 22:30:00 and 02:15:00 would not produce the desired results. This is SameAs: absolute 'time'(StopTimeEvent) in the 'arrival' field of the stop_time_update (StopTimeUpdate) message of the GTFS Realtime message-TripUpdate (https://developers.google.com/transit/gtfs-realtime/reference#message-tripupdate)",
            "rdfs:label": "last_stop_arrival_time",
            "rdfs:isDefinedBy": {
                "@id": "iudx:"
            },
            "iudx:domainIncludes": [
                {
                    "@id": "iudx:TransitManagement"
                }
            ],
            "iudx:rangeIncludes": [
                {
                    "@id": "iudx:Text"
                },
                {
                    "@id": "iudx:ValueDescriptor"
                }
            ]
        },
        {
            "@id": "iudx:last_stop_departure_time",
            "@type": [
                "iudx:TimeProperty"
            ],
            "rdfs:comment": "Specifies the departure time from the previous stop for a specific trip on a route. Times must be eight digits in HH:MM:SS format (H:MM:SS is also accepted, if the hour begins with 0). \nNote: Trips that span multiple dates will have stop times greater than 24:00:00. For example, if a trip begins at 10:30:00 p.m. and ends at 2:15:00 a.m. on the following day, the stop times would be 22:30:00 and 26:15:00. Entering those stop times as 22:30:00 and 02:15:00 would not produce the desired results. This is SameAs: absolute 'time'(StopTimeEvent) in the 'departure' field of the stop_time_update (StopTimeUpdate) message of the GTFS Realtime message-TripUpdate (https://developers.google.com/transit/gtfs-realtime/reference#message-tripupdate)",
            "rdfs:label": "last_stop_departure_time",
            "rdfs:isDefinedBy": {
                "@id": "iudx:"
            },
            "iudx:domainIncludes": [
                {
                    "@id": "iudx:TransitManagement"
                }
            ],
            "iudx:rangeIncludes": [
                {
                    "@id": "iudx:Text"
                },
                {
                    "@id": "iudx:ValueDescriptor"
                }
            ]
        },
        {
            "@id": "iudx:last_stop_id",
            "@type": [
                "iudx:TextProperty"
            ],
            "rdfs:comment": "Stop ID/Stop name of the previous bus stop corresponding to the bus in this observation. SameAs: 'stop_id' field from GTFS Realtime message-VehiclePosition (https://developers.google.com/transit/gtfs-realtime/reference#message-vehicleposition)",
            "rdfs:label": "last_stop_id",
            "rdfs:isDefinedBy": {
                "@id": "iudx:"
            },
            "iudx:domainIncludes": [
                {
                    "@id": "iudx:TransitManagement"
                }
            ],
            "iudx:rangeIncludes": [
                {
                    "@id": "iudx:Text"
                },
                {
                    "@id": "iudx:ValueDescriptor"
                }
            ]
        },
        {
            "@id": "iudx:latency",
            "@type": [
                "iudx:QuantitativeProperty"
            ],
            "rdfs:comment": "The value of latency in packet transmission.",
            "rdfs:label": "latency",
            "rdfs:isDefinedBy": {
                "@id": "iudx:"
            },
            "iudx:domainIncludes": [
                {
                    "@id": "iudx:WirelessNetwork"
                }
            ],
            "iudx:rangeIncludes": [
                {
                    "@id": "iudx:Number"
                },
                {
                    "@id": "iudx:ValueDescriptor"
                }
            ]
        },
        {
            "@id": "iudx:licenseExpiryDate",
            "@type": [
                "iudx:TimeProperty"
            ],
            "rdfs:comment": "License number expiry date for the business establishment corresponding to this observation.",
            "rdfs:label": "licenseExpiryDate",
            "rdfs:isDefinedBy": {
                "@id": "iudx:"
            },
            "iudx:domainIncludes": [
                {
                    "@id": "iudx:RevenueCollection"
                }
            ],
            "iudx:rangeIncludes": [
                {
                    "@id": "iudx:Text"
                },
                {
                    "@id": "iudx:ValueDescriptor"
                }
            ]
        },
        {
            "@id": "iudx:licenseIssualDate",
            "@type": [
                "iudx:TimeProperty"
            ],
            "rdfs:comment": "Date of issual of license for the entity or service corresponding to this observation.",
            "rdfs:label": "licenseIssualDate",
            "rdfs:isDefinedBy": {
                "@id": "iudx:"
            },
            "iudx:domainIncludes": [
                {
                    "@id": "iudx:RevenueCollection"
                }
            ],
            "iudx:rangeIncludes": [
                {
                    "@id": "iudx:Text"
                },
                {
                    "@id": "iudx:ValueDescriptor"
                }
            ]
        },
        {
            "@id": "iudx:license_plate",
            "@type": [
                "iudx:TextProperty"
            ],
            "rdfs:comment": "Gives the License Plate number of the vehice. SameAs: 'license_plate' field from GTFS Realtime message-VehicleDescriptor (https://developers.google.com/transit/gtfs-realtime/reference#message-vehicledescriptor)",
            "rdfs:label": "license_plate",
            "rdfs:isDefinedBy": {
                "@id": "iudx:"
            },
            "iudx:domainIncludes": [
                {
                    "@id": "iudx:WmgmtBin"
                },
                {
                    "@id": "iudx:WmgmtVehicle"
                },
                {
                    "@id": "iudx:VehicleDescriptor"
                },
                {
                    "@id": "iudx:EmergencyVehicle"
                }
            ],
            "iudx:rangeIncludes": [
                {
                    "@id": "iudx:Text"
                },
                {
                    "@id": "iudx:ValueDescriptor"
                }
            ],
            "skos:exactMatch": {
                "@id": "GTFS: license_plate"
            }
        },
        {
            "@id": "iudx:location",
            "@type": [
                "iudx:GeoProperty"
            ],
            "rdfs:comment": "Location associated with a resource Item (a spatial point), a group of resource items (a spatial region) or even an observation in case of a mobile sensor.",
            "rdfs:label": "location",
            "iudx:domainIncludes": [
                {
                    "@id": "iudx:Resource"
                },
                {
                    "@id": "iudx:ResourceGroup"
                },
                {
                    "@id": "iudx:Provider"
                },
                {
                    "@id": "iudx:ResourceServer"
                },
                {
                    "@id": "iudx:Organization"
                },
                {
                    "@id": "iudx:EnvAQM"
                },
                {
                    "@id": "iudx:EnvFlood"
                },
                {
                    "@id": "iudx:StreetLightFeeder"
                },
                {
                    "@id": "iudx:WmgmtBin"
                },
                {
                    "@id": "iudx:TransitManagement"
                },
                {
                    "@id": "iudx:PointOfInterest"
                },
                {
                    "@id": "iudx:SafetiPin"
                },
                {
                    "@id": "iudx:IssueReporting"
                },
                {
                    "@id": "iudx:TrafficViolations"
                },
                {
                    "@id": "iudx:Streetlight"
                },
                {
                    "@id": "iudx:BikeDockingStation"
                },
                {
                    "@id": "iudx:WaterDistributionNetwork"
                },
                {
                    "@id": "iudx:Camera"
                },
                {
                    "@id": "iudx:WasteWaterMgmt"
                },
                {
                    "@id": "iudx:SmartParking"
                },
                {
                    "@id": "iudx:EmergencyVehicle"
                },
                {
                    "@id": "iudx:SolarEnergy"
                },
                {
                    "@id": "iudx:LaneDesc"
                },
                {
                    "@id": "iudx:EVChargingStation"
                },
                {
                    "@id": "iudx:MosquitoDensity"
                },
                {
                    "@id": "iudx:WmgmtVehicle"
                },
                {
                    "@id": "iudx:TouristDestination"
                },
                {
                    "@id": "iudx:AirQuality"
                }
            ],
            "iudx:rangeIncludes": [
                {
                    "@id": "iudx:Point"
                },
                {
                    "@id": "iudx:GeoJSONGeometry"
                },
                {
                    "@id": "iudx:Place"
                },
                {
                    "@id": "iudx:Text"
                },
                {
                    "@id": "iudx:ValueDescriptor"
                },
                {
                    "@id": "iudx:Geojsongeometry"
                }
            ],
            "rdfs:isDefinedBy": {
                "@id": "iudx:"
            },
            "skos:exactMatch": {
                "@id": "schema:location"
            }
        },
        {
            "@id": "iudx:macAddress",
            "@type": [
                "iudx:TextProperty"
            ],
            "rdfs:comment": "The Media Access Control address which is a 12-digit hexadecimal number assigned to each device connected to the network",
            "rdfs:label": "macAddress",
            "rdfs:isDefinedBy": {
                "@id": "iudx:"
            },
            "iudx:domainIncludes": [
                {
                    "@id": "iudx:WirelessNetwork"
                }
            ],
            "iudx:rangeIncludes": [
                {
                    "@id": "iudx:Text"
                },
                {
                    "@id": "iudx:ValueDescriptor"
                }
            ]
        },
        {
            "@id": "iudx:mac_tx_count",
            "@type": [
                "iudx:QuantitativeProperty"
            ],
            "rdfs:comment": "MAC transmission count represents the number of packets transmitted over the air.",
            "rdfs:label": "mac_tx_count",
            "rdfs:isDefinedBy": {
                "@id": "iudx:"
            },
            "iudx:domainIncludes": [
                {
                    "@id": "iudx:WirelessNetwork"
                }
            ],
            "iudx:rangeIncludes": [
                {
                    "@id": "iudx:Number"
                },
                {
                    "@id": "iudx:ValueDescriptor"
                }
            ]
        },
        {
            "@id": "iudx:mac_tx_failed_count",
            "@type": [
                "iudx:QuantitativeProperty"
            ],
            "rdfs:comment": "MAC transmit failed represents the number of unsuccessful transmission attempts.",
            "rdfs:label": "mac_tx_failed_count",
            "rdfs:isDefinedBy": {
                "@id": "iudx:"
            },
            "iudx:domainIncludes": [
                {
                    "@id": "iudx:WirelessNetwork"
                }
            ],
            "iudx:rangeIncludes": [
                {
                    "@id": "iudx:Number"
                },
                {
                    "@id": "iudx:ValueDescriptor"
                }
            ]
        },
        {
            "@id": "iudx:maleTotal",
            "@type": [
                "iudx:QuantitativeProperty"
            ],
            "rdfs:comment": "The total count of males of a particular species, as identified by the device.",
            "rdfs:label": "maleTotal",
            "rdfs:isDefinedBy": {
                "@id": "iudx:"
            },
            "iudx:domainIncludes": [
                {
                    "@id": "iudx:MosquitoDensity"
                }
            ],
            "iudx:rangeIncludes": [
                {
                    "@id": "iudx:Number"
                },
                {
                    "@id": "iudx:ValueDescriptor"
                }
            ]
        },
        {
            "@id": "iudx:malfunctionCode",
            "@type": [
                "iudx:TextProperty"
            ],
            "rdfs:comment": "Describes the error code/ malfunction code of the air conditioning system.",
            "rdfs:label": "malfunctionCode",
            "rdfs:isDefinedBy": {
                "@id": "iudx:"
            },
            "iudx:domainIncludes": [
                {
                    "@id": "iudx:AirConditioner"
                }
            ],
            "iudx:rangeIncludes": [
                {
                    "@id": "iudx:Text"
                },
                {
                    "@id": "iudx:ValueDescriptor"
                }
            ]
        },
        {
            "@id": "iudx:maxOverTime",
            "@type": [
                "iudx:QuantitativeProperty"
            ],
            "rdfs:comment": "Describes the maximum value of a time-series data over a specified duration in past. The duration is specified using another parameter in the value descriptor object related to this value",
            "rdfs:label": "maxOverTime",
            "iudx:domainIncludes": [
                {
                    "@id": "iudx:TimeSeriesAggregation"
                }
            ],
            "iudx:rangeIncludes": [
                {
                    "@id": "iudx:Number"
                },
                {
                    "@id": "iudx:ValueDescriptor"
                }
            ]
        },
        {
            "@id": "iudx:maxSolarPowerMeasure",
            "@type": [
                "iudx:QuantitativeProperty"
            ],
            "rdfs:comment": "A measure of maximum solar energy that can be generated.",
            "rdfs:label": "maxSolarPowerMeasure",
            "rdfs:isDefinedBy": {
                "@id": "iudx:"
            },
            "iudx:domainIncludes": [
                {
                    "@id": "iudx:SolarEnergy"
                }
            ],
            "iudx:rangeIncludes": [
                {
                    "@id": "iudx:Number"
                },
                {
                    "@id": "iudx:ValueDescriptor"
                }
            ]
        },
        {
            "@id": "iudx:maxValue",
            "@type": [
                "iudx:QuantitativeProperty"
            ],
            "rdfs:comment": "The upper value of a quantity/property.",
            "rdfs:label": "maxValue",
            "iudx:domainIncludes": [
                {
                    "@id": "iudx:ValueDescriptor"
                }
            ],
            "iudx:rangeIncludes": [
                {
                    "@id": "iudx:Number"
                }
            ],
            "skos:exactMatch": {
                "@id": "schema:maxValue"
            },
            "rdfs:isDefinedBy": {
                "@id": "iudx:"
            }
        },
        {
            "@id": "iudx:maxZoom",
            "@type": [
                "iudx:QuantitativeProperty"
            ],
            "rdfs:comment": "A number between 0 to 18 denoting maximum zoom.",
            "rdfs:label": "maxZoom",
            "rdfs:isDefinedBy": {
                "@id": "iudx:"
            },
            "iudx:domainIncludes": [
                {
                    "@id": "iudx:MapTiles"
                }
            ],
            "iudx:rangeIncludes": [
                {
                    "@id": "iudx:Number"
                },
                {
                    "@id": "iudx:ValueDescriptor"
                }
            ]
        },
        {
            "@id": "iudx:maximumAllowedHeight",
            "@type": [
                "iudx:QuantitativeProperty"
            ],
            "rdfs:comment": "Maximum allowed height for vehicles using the entity corresponding to this observation.",
            "rdfs:label": "maximumAllowedHeight",
            "rdfs:isDefinedBy": {
                "@id": "iudx:"
            },
            "iudx:domainIncludes": [
                {
                    "@id": "iudx:SmartParking"
                },
                {
                    "@id": "iudx:RoadSegment"
                }
            ],
            "iudx:rangeIncludes": [
                {
                    "@id": "iudx:Number"
                },
                {
                    "@id": "iudx:ValueDescriptor"
                }
            ],
            "skos:exactMatch": {
                "@id": "Fiware: OffStreetParking.maximumAllowedHeight"
            }
        },
        {
            "@id": "iudx:maximumAllowedSpeed",
            "@type": [
                "iudx:QuantitativeProperty"
            ],
            "rdfs:comment": "The maximum speed allowed for vehicles plying the road segment corresponding to this observation.",
            "rdfs:label": "maximumAllowedSpeed",
            "rdfs:isDefinedBy": {
                "@id": "iudx:"
            },
            "iudx:domainIncludes": [
                {
                    "@id": "iudx:RoadSegment"
                }
            ],
            "iudx:rangeIncludes": [
                {
                    "@id": "iudx:Number"
                },
                {
                    "@id": "iudx:ValueDescriptor"
                }
            ],
            "skos:exactMatch": {
                "@id": "Fiware: maximumAllowedSpeed"
            }
        },
        {
            "@id": "iudx:maximumAllowedWidth",
            "@type": [
                "iudx:QuantitativeProperty"
            ],
            "rdfs:comment": "Maximum allowed width for vehicles using the entity corresponding to this observation.",
            "rdfs:label": "maximumAllowedWidth",
            "rdfs:isDefinedBy": {
                "@id": "iudx:"
            },
            "iudx:domainIncludes": [
                {
                    "@id": "iudx:SmartParking"
                },
                {
                    "@id": "iudx:RoadSegment"
                }
            ],
            "iudx:rangeIncludes": [
                {
                    "@id": "iudx:Number"
                },
                {
                    "@id": "iudx:ValueDescriptor"
                }
            ],
            "skos:exactMatch": {
                "@id": "Fiware: OffStreetParking.maximumAllowedWidth"
            }
        },
        {
            "@id": "iudx:maximumParkingDuration",
            "@type": [
                "iudx:QuantitativeProperty"
            ],
            "rdfs:comment": "The maximum amount of time for which a vehicle can be parked in the parking site corresponding to this observation.",
            "rdfs:label": "maximumParkingDuration",
            "rdfs:isDefinedBy": {
                "@id": "iudx:"
            },
            "iudx:domainIncludes": [
                {
                    "@id": "iudx:SmartParking"
                }
            ],
            "iudx:rangeIncludes": [
                {
                    "@id": "iudx:Number"
                },
                {
                    "@id": "iudx:ValueDescriptor"
                }
            ],
            "skos:exactMatch": {
                "@id": "Fiware:OffStreetParking.maximumParkingDuration"
            }
        },
        {
            "@id": "iudx:measAccuracy",
            "@type": [
                "iudx:TextProperty"
            ],
            "rdfs:comment": "Accuracy of a measurement. Maximum difference that can exist between the actual value and the measured value. It can be specified in relative as well as absolute terms.",
            "rdfs:label": "measAccuracy",
            "iudx:domainIncludes": [
                {
                    "@id": "iudx:ValueDescriptor"
                }
            ],
            "iudx:rangeIncludes": [
                {
                    "@id": "iudx:Text"
                },
                {
                    "@id": "iudx:ValueDescriptor"
                }
            ],
            "rdfs:isDefinedBy": {
                "@id": "iudx:"
            }
        },
        {
            "@id": "iudx:measuredDistance",
            "@type": [
                "iudx:QuantitativeProperty"
            ],
            "rdfs:comment": "Describes the distance measured by the sensor, from the sensor tip to the upper surface of water.",
            "rdfs:label": "measuredDistance",
            "rdfs:isDefinedBy": {
                "@id": "iudx:"
            },
            "iudx:domainIncludes": [
                {
                    "@id": "iudx:EnvFlood"
                }
            ],
            "iudx:rangeIncludes": [
                {
                    "@id": "iudx:Number"
                },
                {
                    "@id": "iudx:ValueDescriptor"
                }
            ]
        },
        {
            "@id": "iudx:mediaURL",
            "@type": [
                "iudx:TextProperty"
            ],
            "rdfs:comment": "URL providing further information of any image(s) or media of the complaint or place.",
            "rdfs:label": "mediaURL",
            "iudx:domainIncludes": [
                {
                    "@id": "iudx:SafetiPin"
                },
                {
                    "@id": "iudx:IssueReporting"
                },
                {
                    "@id": "iudx:TrafficViolations"
                },
                {
                    "@id": "iudx:BikeDockingStation"
                },
                {
                    "@id": "iudx:Camera"
                },
                {
                    "@id": "iudx:TouristDestination"
                }
            ],
            "iudx:rangeIncludes": [
                {
                    "@container": "@list",
                    "@id": "iudx:Text"
                },
                {
                    "@id": "iudx:ValueDescriptor"
                }
            ],
            "rdfs:isDefinedBy": {
                "@id": "iudx:"
            },
            "skos:exactMatch": {
                "@id": "open311:media_url"
            }
        },
        {
            "@id": "iudx:medianHeight",
            "@type": [
                "iudx:QuantitativeProperty"
            ],
            "rdfs:comment": "Height of the median or central reservation in the road corresponding to this observation.",
            "rdfs:label": "medianHeight",
            "rdfs:isDefinedBy": {
                "@id": "iudx:"
            },
            "iudx:domainIncludes": [
                {
                    "@id": "iudx:RoadSegment"
                }
            ],
            "iudx:rangeIncludes": [
                {
                    "@id": "iudx:Number"
                },
                {
                    "@id": "iudx:ValueDescriptor"
                }
            ]
        },
        {
            "@id": "iudx:medianLength",
            "@type": [
                "iudx:QuantitativeProperty"
            ],
            "rdfs:comment": "Length of the median or central reservation in the road corresponding to this observation.",
            "rdfs:label": "medianLength",
            "rdfs:isDefinedBy": {
                "@id": "iudx:"
            },
            "iudx:domainIncludes": [
                {
                    "@id": "iudx:RoadSegment"
                }
            ],
            "iudx:rangeIncludes": [
                {
                    "@id": "iudx:Number"
                },
                {
                    "@id": "iudx:ValueDescriptor"
                }
            ]
        },
        {
            "@id": "iudx:medianWidth",
            "@type": [
                "iudx:QuantitativeProperty"
            ],
            "rdfs:comment": "Width of the median or central reservation in the road corresponding to this observation.",
            "rdfs:label": "medianWidth",
            "rdfs:isDefinedBy": {
                "@id": "iudx:"
            },
            "iudx:domainIncludes": [
                {
                    "@id": "iudx:RoadSegment"
                }
            ],
            "iudx:rangeIncludes": [
                {
                    "@id": "iudx:Number"
                },
                {
                    "@id": "iudx:ValueDescriptor"
                }
            ]
        },
        {
            "@id": "iudx:minOverTime",
            "@type": [
                "iudx:QuantitativeProperty"
            ],
            "rdfs:comment": "Describes the minimum value of a time-series data over a specified duration in past. The duration is specified using another parameter in the value descriptor object related to this value",
            "rdfs:label": "minOverTime",
            "iudx:domainIncludes": [
                {
                    "@id": "iudx:TimeSeriesAggregation"
                }
            ],
            "iudx:rangeIncludes": [
                {
                    "@id": "iudx:Number"
                },
                {
                    "@id": "iudx:ValueDescriptor"
                }
            ]
        },
        {
            "@id": "iudx:minValue",
            "@type": [
                "iudx:QuantitativeProperty"
            ],
            "rdfs:comment": "The lower value of a quantity/property.",
            "rdfs:label": "minValue",
            "iudx:domainIncludes": [
                {
                    "@id": "iudx:ValueDescriptor"
                }
            ],
            "iudx:rangeIncludes": [
                {
                    "@id": "iudx:Number"
                }
            ],
            "skos:exactMatch": {
                "@id": "schema:minValue"
            },
            "rdfs:isDefinedBy": {
                "@id": "iudx:"
            }
        },
        {
            "@id": "iudx:minZoom",
            "@type": [
                "iudx:QuantitativeProperty"
            ],
            "rdfs:comment": "A number between 0 to 18 denoting minimum zoom.",
            "rdfs:label": "minZoom",
            "rdfs:isDefinedBy": {
                "@id": "iudx:"
            },
            "iudx:domainIncludes": [
                {
                    "@id": "iudx:MapTiles"
                }
            ],
            "iudx:rangeIncludes": [
                {
                    "@id": "iudx:Number"
                },
                {
                    "@id": "iudx:ValueDescriptor"
                }
            ]
        },
        {
            "@id": "iudx:minimumAllowedSpeed",
            "@type": [
                "iudx:QuantitativeProperty"
            ],
            "rdfs:comment": "The minimum speed allowed for vehicles plying the road segment corresponding to this observation.",
            "rdfs:label": "minimumAllowedSpeed",
            "rdfs:isDefinedBy": {
                "@id": "iudx:"
            },
            "iudx:domainIncludes": [
                {
                    "@id": "iudx:RoadSegment"
                }
            ],
            "iudx:rangeIncludes": [
                {
                    "@id": "iudx:Number"
                },
                {
                    "@id": "iudx:ValueDescriptor"
                }
            ],
            "skos:exactMatch": {
                "@id": "Fiware: minimumAllowedSpeed"
            }
        },
        {
            "@id": "iudx:month",
            "@type": [
                "iudx:QuantitativeProperty"
            ],
            "rdfs:comment": "Month corresponding to this observation and is described in MM format, for eg. 11 for the month of November.",
            "rdfs:label": "month",
            "rdfs:isDefinedBy": {
                "@id": "iudx:"
            },
            "iudx:domainIncludes": [
                {
                    "@id": "iudx:RevenueCollection"
                }
            ],
            "iudx:rangeIncludes": [
                {
                    "@id": "iudx:Number"
                },
                {
                    "@id": "iudx:ValueDescriptor"
                }
            ]
        },
        {
            "@id": "iudx:name",
            "@type": [
                "iudx:TextProperty"
            ],
            "rdfs:comment": "Name of the entity.",
            "rdfs:label": "name",
            "iudx:domainIncludes": [
                {
                    "@id": "iudx:Place"
                },
                {
                    "@id": "iudx:Organization"
                },
                {
                    "@id": "iudx:RelationshipValue"
                },
                {
                    "@id": "iudx:IUDXEntity",
                    "iudx:requiredProperty": true
                },
                {
                    "@id": "iudx:PointOfInterest"
                },
                {
                    "@id": "iudx:BikeDockingStation"
                },
                {
                    "@id": "iudx:TouristDestination"
                }
            ],
            "iudx:rangeIncludes": [
                {
                    "@id": "iudx:Text"
                },
                {
                    "@id": "iudx:ValueDescriptor"
                }
            ],
            "skos:exactMatch": {
                "@id": "schema:name"
            },
            "rdfs:isDefinedBy": {
                "@id": "iudx:"
            }
        },
        {
            "@id": "iudx:name_of_town",
            "@type": [
                "iudx:TextProperty"
            ],
            "rdfs:comment": "Name of the town corresponding to this observation.",
            "rdfs:label": "name_of_town",
            "rdfs:isDefinedBy": {
                "@id": "iudx:"
            },
            "iudx:domainIncludes": [
                {
                    "@id": "iudx:MajorTowns"
                }
            ],
            "iudx:rangeIncludes": [
                {
                    "@id": "iudx:Text"
                },
                {
                    "@id": "iudx:ValueDescriptor"
                }
            ]
        },
        {
            "@id": "iudx:newAssessmentCount",
            "@type": [
                "iudx:QuantitativeProperty"
            ],
            "rdfs:comment": "Number of fresh assessments conducted to assess the value of property.",
            "rdfs:label": "newAssessmentCount",
            "rdfs:isDefinedBy": {
                "@id": "iudx:"
            },
            "iudx:domainIncludes": [
                {
                    "@id": "iudx:RevenueCollection"
                }
            ],
            "iudx:rangeIncludes": [
                {
                    "@id": "iudx:Number"
                },
                {
                    "@id": "iudx:ValueDescriptor"
                }
            ]
        },
        {
            "@id": "iudx:nh4",
            "@type": [
                "iudx:QuantitativeProperty"
            ],
            "rdfs:comment": "Ammonium concentration measured in the waste-water treatment plant corresponding to this observation.",
            "rdfs:label": "nh4",
            "rdfs:isDefinedBy": {
                "@id": "iudx:"
            },
            "iudx:domainIncludes": [
                {
                    "@id": "iudx:WasteWaterMgmt"
                }
            ],
            "iudx:rangeIncludes": [
                {
                    "@id": "iudx:Number"
                },
                {
                    "@id": "iudx:ValueDescriptor"
                }
            ],
            "skos:exactMatch": {
                "@id": "fiware:nh4"
            }
        },
        {
            "@id": "iudx:no3",
            "@type": [
                "iudx:QuantitativeProperty"
            ],
            "rdfs:comment": "Nitrate concentration measured in waste-water treatment plant corresponding to this observation.",
            "rdfs:label": "no3",
            "rdfs:isDefinedBy": {
                "@id": "iudx:"
            },
            "iudx:domainIncludes": [
                {
                    "@id": "iudx:WasteWaterMgmt"
                }
            ],
            "iudx:rangeIncludes": [
                {
                    "@id": "iudx:Number"
                },
                {
                    "@id": "iudx:ValueDescriptor"
                }
            ],
            "skos:exactMatch": {
                "@id": "fiware:no3"
            }
        },
        {
            "@id": "iudx:numStreetlight",
            "@type": [
                "iudx:QuantitativeProperty"
            ],
            "rdfs:comment": "Describes the total number of streetlights connected to the feeder panel corresponding to this observation.",
            "rdfs:label": "numStreetlight",
            "rdfs:isDefinedBy": {
                "@id": "iudx:"
            },
            "iudx:domainIncludes": [
                {
                    "@id": "iudx:StreetLightFeeder"
                }
            ],
            "iudx:rangeIncludes": [
                {
                    "@id": "iudx:Number"
                },
                {
                    "@id": "iudx:ValueDescriptor"
                }
            ]
        },
        {
            "@id": "iudx:objectid",
            "@type": [
                "iudx:QuantitativeProperty"
            ],
            "rdfs:comment": "The object ID corresponding to this observation.",
            "rdfs:label": "objectid",
            "rdfs:isDefinedBy": {
                "@id": "iudx:"
            },
            "iudx:domainIncludes": [
                {
                    "@id": "iudx:Headquarters"
                }
            ],
            "iudx:rangeIncludes": [
                {
                    "@id": "iudx:Number"
                },
                {
                    "@id": "iudx:ValueDescriptor"
                }
            ]
        },
        {
            "@id": "iudx:observationDateTime",
            "@type": [
                "iudx:TimeProperty"
            ],
            "rdfs:comment": "Last reported time of observation.",
            "rdfs:label": "observationDateTime",
            "iudx:domainIncludes": [
                {
                    "@id": "iudx:EnvAQM"
                },
                {
                    "@id": "iudx:EnvFlood"
                },
                {
                    "@id": "iudx:EnvWeather"
                },
                {
                    "@id": "iudx:TransitManagement"
                },
                {
                    "@id": "iudx:StreetLightFeeder"
                },
                {
                    "@id": "iudx:WmgmtVehicle"
                },
                {
                    "@id": "iudx:SafetiPin"
                },
                {
                    "@id": "iudx:IssueReporting"
                },
                {
                    "@id": "iudx:FareCollectionSystem"
                },
                {
                    "@id": "iudx:EmployeeDetails"
                },
                {
                    "@id": "iudx:TrafficViolations"
                },
                {
                    "@id": "iudx:Streetlight"
                },
                {
                    "@id": "iudx:BikeDockingStation"
                },
                {
                    "@id": "iudx:WaterDistributionNetwork"
                },
                {
                    "@id": "iudx:WasteWaterMgmt"
                },
                {
                    "@id": "iudx:SmartParking"
                },
                {
                    "@id": "iudx:EmergencyVehicle"
                },
                {
                    "@id": "iudx:GISData"
                },
                {
                    "@id": "iudx:SolarEnergy"
                },
                {
                    "@id": "iudx:EnergyMeter"
                },
                {
                    "@id": "iudx:EVChargingStation"
                },
                {
                    "@id": "iudx:MosquitoDensity"
                },
                {
                    "@id": "iudx:RoomOccupancy"
                },
                {
                    "@id": "iudx:TouristDestination"
                },
                {
                    "@id": "iudx:RoadSegment"
                },
                {
                    "@id": "iudx:AirQuality"
                }
            ],
            "iudx:rangeIncludes": [
                {
                    "@id": "iudx:DateTime"
                },
                {
                    "@id": "iudx:ValueDescriptor"
                },
                {
                    "@id": "iudx:Datetime"
                }
            ],
            "rdfs:isDefinedBy": {
                "@id": "iudx:"
            }
        },
        {
            "@id": "iudx:occupancyLevel",
            "@type": [
                "iudx:TextProperty"
            ],
            "rdfs:comment": "Occupancy level in the public transit bus corresponding to this observation. 'Red' indicates the congestion level in the bus is HIGH, 'Yellow' indicates the congestion level in the bus is MODERATE and 'Green' indicates the congestion level in the bus is LOW.",
            "rdfs:label": "occupancyLevel",
            "rdfs:isDefinedBy": {
                "@id": "iudx:"
            },
            "iudx:domainIncludes": [
                {
                    "@id": "iudx:FareCollectionSystem"
                }
            ],
            "iudx:rangeIncludes": [
                {
                    "@id": "iudx:Text"
                },
                {
                    "@id": "iudx:ValueDescriptor"
                }
            ]
        },
        {
            "@id": "iudx:occupancy_status",
            "@type": [
                "iudx:TextProperty"
            ],
            "rdfs:comment": "The degree of passenger occupancy for the vehicle. ENUM [EMPTY,  MANY_SEATS_AVAILABLE, FEW_SEATS_AVAILABLE, STANDING_ROOM_ONLY, CRUSHED_STANDING_ROOM_ONLY, FULL,  NOT_ACCEPTING_PASSENGERS, NO_DATA_AVAILABLE, NOT_BOARDABLE]",
            "rdfs:label": "occupancy_status",
            "rdfs:isDefinedBy": {
                "@id": "iudx:"
            },
            "iudx:domainIncludes": [
                {
                    "@id": "iudx:VehiclePosition"
                }
            ],
            "iudx:rangeIncludes": [
                {
                    "@id": "iudx:Text"
                },
                {
                    "@id": "iudx:ValueDescriptor"
                }
            ],
            "skos:exactMatch": {
                "@id": "GTFS: occupancy_status"
            }
        },
        {
            "@id": "iudx:occupiedSpotNumber",
            "@type": [
                "iudx:QuantitativeProperty"
            ],
            "rdfs:comment": "Number of parking spots occupied in the smart parking site corresponding to this observation. This must a positve number lower than or equal to the totalSpotNumber.",
            "rdfs:label": "occupiedSpotNumber",
            "rdfs:isDefinedBy": {
                "@id": "iudx:"
            },
            "iudx:domainIncludes": [
                {
                    "@id": "iudx:ParkingSpotStatus"
                }
            ],
            "iudx:rangeIncludes": [
                {
                    "@id": "iudx:Number"
                },
                {
                    "@id": "iudx:ValueDescriptor"
                }
            ],
            "skos:exactMatch": {
                "@id": "Fiware: OffStreetParking.occupiedSpotNumber"
            }
        },
        {
            "@id": "iudx:odometer",
            "@type": [
                "iudx:QuantitativeProperty"
            ],
            "rdfs:comment": "Odometer value.",
            "rdfs:label": "odometer",
            "rdfs:isDefinedBy": {
                "@id": "iudx:"
            },
            "iudx:domainIncludes": [
                {
                    "@id": "iudx:Position"
                }
            ],
            "iudx:rangeIncludes": [
                {
                    "@id": "iudx:Number"
                },
                {
                    "@id": "iudx:ValueDescriptor"
                }
            ],
            "skos:exactMatch": {
                "@id": "GTFS: odometer"
            }
        },
        {
            "@id": "iudx:openHours",
            "@type": [
                "iudx:TextProperty"
            ],
            "rdfs:comment": "The time period or hours between which the entity or service is open or operational.",
            "rdfs:label": "openHours",
            "iudx:domainIncludes": [
                {
                    "@id": "iudx:PointOfInterest"
                },
                {
                    "@id": "iudx:TouristDestination"
                }
            ],
            "iudx:rangeIncludes": [
                {
                    "@id": "iudx:Text"
                },
                {
                    "@id": "iudx:ValueDescriptor"
                }
            ],
            "skos:exactMatch": {
                "@id": "Fiware:Building.openingHours"
            },
            "rdfs:isDefinedBy": {
                "@id": "iudx:"
            }
        },
        {
            "@id": "iudx:originDestinationCode",
            "@type": [
                "iudx:TextProperty"
            ],
            "rdfs:comment": "The code for the origin and destination stops corresponding to this observation.",
            "rdfs:label": "originDestinationCode",
            "rdfs:isDefinedBy": {
                "@id": "iudx:"
            },
            "iudx:domainIncludes": [
                {
                    "@id": "iudx:FareCollectionSystem"
                }
            ],
            "iudx:rangeIncludes": [
                {
                    "@id": "iudx:Text"
                },
                {
                    "@id": "iudx:ValueDescriptor"
                }
            ]
        },
        {
            "@id": "iudx:originLocation",
            "@type": [
                "iudx:GeoProperty"
            ],
            "rdfs:comment": "The source location of the ride corresponding to the observation.",
            "rdfs:label": "originLocation",
            "rdfs:isDefinedBy": {
                "@id": "iudx:"
            },
            "iudx:domainIncludes": [
                {
                    "@id": "iudx:BikeDockingStation"
                }
            ],
            "iudx:rangeIncludes": [
                {
                    "@id": "iudx:Place"
                },
                {
                    "@id": "iudx:ValueDescriptor"
                }
            ]
        },
        {
            "@id": "iudx:originStopCategory",
            "@type": [
                "iudx:TextProperty"
            ],
            "rdfs:comment": "Type of the origin bus stop corresponding to this observation.",
            "rdfs:label": "originStopCategory",
            "rdfs:isDefinedBy": {
                "@id": "iudx:"
            },
            "iudx:domainIncludes": [
                {
                    "@id": "iudx:FareCollectionSystem"
                }
            ],
            "iudx:rangeIncludes": [
                {
                    "@id": "iudx:Text"
                },
                {
                    "@id": "iudx:ValueDescriptor"
                }
            ]
        },
        {
            "@id": "iudx:originStopID",
            "@type": [
                "iudx:TextProperty"
            ],
            "rdfs:comment": "Unique ID of the bus stop at which the passenger boards into the bus corresponding to this observation.",
            "rdfs:label": "originStopID",
            "rdfs:isDefinedBy": {
                "@id": "iudx:"
            },
            "iudx:domainIncludes": [
                {
                    "@id": "iudx:FareCollectionSystem"
                }
            ],
            "iudx:rangeIncludes": [
                {
                    "@id": "iudx:Text"
                },
                {
                    "@id": "iudx:ValueDescriptor"
                }
            ]
        },
        {
            "@id": "iudx:originStopName",
            "@type": [
                "iudx:TextProperty"
            ],
            "rdfs:comment": "The name of the origin bus stop corresponding to this observation.",
            "rdfs:label": "originStopName",
            "rdfs:isDefinedBy": {
                "@id": "iudx:"
            },
            "iudx:domainIncludes": [
                {
                    "@id": "iudx:FareCollectionSystem"
                }
            ],
            "iudx:rangeIncludes": [
                {
                    "@id": "iudx:Text"
                },
                {
                    "@id": "iudx:ValueDescriptor"
                }
            ]
        },
        {
            "@id": "iudx:outFlow",
            "@type": [
                "iudx:QuantitativeProperty"
            ],
            "rdfs:comment": "Out-flow amount into the treatment plant/reservoir corresponding to this observation.",
            "rdfs:label": "outFlow",
            "rdfs:isDefinedBy": {
                "@id": "iudx:"
            },
            "iudx:domainIncludes": [
                {
                    "@id": "iudx:WasteWaterMgmt"
                }
            ],
            "iudx:rangeIncludes": [
                {
                    "@id": "iudx:Number"
                },
                {
                    "@id": "iudx:ValueDescriptor"
                }
            ]
        },
        {
            "@id": "iudx:outOfServiceSlotNumber",
            "@type": [
                "iudx:QuantitativeProperty"
            ],
            "rdfs:comment": "The number of bike racks/bike-docking slots or parking slots that are out of order and cannot be used to hire or park a bike in the bike docking station or parking site corresponding to this observation.",
            "rdfs:label": "outOfServiceSlotNumber",
            "rdfs:isDefinedBy": {
                "@id": "iudx:"
            },
            "iudx:domainIncludes": [
                {
                    "@id": "iudx:BikeDockingStation"
                },
                {
                    "@id": "iudx:SmartParking"
                }
            ],
            "iudx:rangeIncludes": [
                {
                    "@id": "iudx:Number"
                },
                {
                    "@id": "iudx:ValueDescriptor"
                }
            ],
            "skos:exactMatch": {
                "@id": "Fiware:outOfServiceSlotNumber"
            }
        },
        {
            "@id": "iudx:pH",
            "@type": [
                "iudx:QuantitativeProperty"
            ],
            "rdfs:comment": "Acidity level or basicity level obsevered in the water.",
            "rdfs:label": "pH",
            "rdfs:isDefinedBy": {
                "@id": "iudx:"
            },
            "iudx:domainIncludes": [
                {
                    "@id": "iudx:WaterDistributionNetwork"
                },
                {
                    "@id": "iudx:WasteWaterMgmt"
                }
            ],
            "iudx:rangeIncludes": [
                {
                    "@id": "iudx:TimeSeriesAggregation"
                },
                {
                    "@id": "iudx:ValueDescriptor"
                }
            ],
            "skos:exactMatch": {
                "@id": "Fiware: WaterQualityObserved.pH"
            }
        },
        {
            "@id": "iudx:packetSize",
            "@type": [
                "iudx:QuantitativeProperty"
            ],
            "rdfs:comment": "The size of a data packet.",
            "rdfs:label": "packetSize",
            "rdfs:isDefinedBy": {
                "@id": "iudx:"
            },
            "iudx:domainIncludes": [
                {
                    "@id": "iudx:WirelessNetwork"
                }
            ],
            "iudx:rangeIncludes": [
                {
                    "@id": "iudx:Number"
                },
                {
                    "@id": "iudx:ValueDescriptor"
                }
            ]
        },
        {
            "@id": "iudx:panelHumidity",
            "@type": [
                "iudx:QuantitativeProperty"
            ],
            "rdfs:comment": "The humidity of the solar panel corresponding to this observation.",
            "rdfs:label": "panelHumidity",
            "rdfs:isDefinedBy": {
                "@id": "iudx:"
            },
            "iudx:domainIncludes": [
                {
                    "@id": "iudx:SolarEnergy"
                }
            ],
            "iudx:rangeIncludes": [
                {
                    "@id": "iudx:Number"
                },
                {
                    "@id": "iudx:ValueDescriptor"
                }
            ]
        },
        {
            "@id": "iudx:panelTemperature",
            "@type": [
                "iudx:QuantitativeProperty"
            ],
            "rdfs:comment": "The temperature of the solar panel corresponding to this observation.",
            "rdfs:label": "panelTemperature",
            "rdfs:isDefinedBy": {
                "@id": "iudx:"
            },
            "iudx:domainIncludes": [
                {
                    "@id": "iudx:SolarEnergy"
                }
            ],
            "iudx:rangeIncludes": [
                {
                    "@id": "iudx:Number"
                },
                {
                    "@id": "iudx:ValueDescriptor"
                }
            ]
        },
        {
            "@id": "iudx:parkingMode",
            "@type": [
                "iudx:TextProperty"
            ],
            "rdfs:comment": "Parking mode followed in the parking site corresponding to this observation.  ENUM [PARALLEL_PARKING, PERPENDICULAR_PARKING, ANGLE_PARKING].",
            "rdfs:label": "parkingMode",
            "rdfs:isDefinedBy": {
                "@id": "iudx:"
            },
            "iudx:domainIncludes": [
                {
                    "@id": "iudx:SmartParking"
                }
            ],
            "iudx:rangeIncludes": [
                {
                    "@id": "iudx:Text"
                },
                {
                    "@id": "iudx:ValueDescriptor"
                }
            ],
            "skos:exactMatch": {
                "@id": "Fiware: OffStreetParking.parkingMode"
            }
        },
        {
            "@id": "iudx:parkingSiteID",
            "@type": [
                "iudx:TextProperty"
            ],
            "rdfs:comment": "The unique ID of the parking site or parking lot corresponding to this observation.",
            "rdfs:label": "parkingSiteID",
            "rdfs:isDefinedBy": {
                "@id": "iudx:"
            },
            "iudx:domainIncludes": [
                {
                    "@id": "iudx:SmartParking"
                }
            ],
            "iudx:rangeIncludes": [
                {
                    "@id": "iudx:Text"
                },
                {
                    "@id": "iudx:ValueDescriptor"
                }
            ]
        },
        {
            "@id": "iudx:parkingSiteName",
            "@type": [
                "iudx:TextProperty"
            ],
            "rdfs:comment": "Name of the parking site or parking lot corresponding to this observation.",
            "rdfs:label": "parkingSiteName",
            "rdfs:isDefinedBy": {
                "@id": "iudx:"
            },
            "iudx:domainIncludes": [
                {
                    "@id": "iudx:SmartParking"
                }
            ],
            "iudx:rangeIncludes": [
                {
                    "@id": "iudx:Text"
                },
                {
                    "@id": "iudx:ValueDescriptor"
                }
            ]
        },
        {
            "@id": "iudx:passengerCount",
            "@type": [
                "iudx:QuantitativeProperty"
            ],
            "rdfs:comment": "Number of passengers travelling in the public transit bus corresponding to this observation. This count is computed based on the realtime ticketing transactions in the public transit bus.",
            "rdfs:label": "passengerCount",
            "rdfs:isDefinedBy": {
                "@id": "iudx:"
            },
            "iudx:domainIncludes": [
                {
                    "@id": "iudx:FareCollectionSystem"
                }
            ],
            "iudx:rangeIncludes": [
                {
                    "@id": "iudx:Number"
                },
                {
                    "@id": "iudx:ValueDescriptor"
                }
            ]
        },
        {
            "@id": "iudx:paymentStatus",
            "@type": [
                "iudx:TextProperty"
            ],
            "rdfs:comment": "The payment status of the fine or violation or challan corresponding to this observation. ENUM[\"Paid\", \"Unpaid\"].",
            "rdfs:label": "paymentStatus",
            "rdfs:isDefinedBy": {
                "@id": "iudx:"
            },
            "iudx:domainIncludes": [
                {
                    "@id": "iudx:TrafficViolations"
                }
            ],
            "iudx:rangeIncludes": [
                {
                    "@id": "iudx:Text"
                },
                {
                    "@id": "iudx:ValueDescriptor"
                }
            ]
        },
        {
            "@id": "iudx:pcu",
            "@type": [
                "iudx:QuantitativeProperty"
            ],
            "rdfs:comment": "The PCU(Passenger Car Unit) value based on vehicle types as defined by the Indo-HCM(Indian Highway Capacity Manual) and IRC(Indian Road Congress). Indo-HCM: https://crridom.gov.in/sites/default/files/files/Indo-HCM%20Snippets.pdf, IRC: https://law.resource.org/pub/in/bis/irc/irc.gov.in.106.1990.pdf",
            "rdfs:label": "pcu",
            "rdfs:isDefinedBy": {
                "@id": "iudx:"
            },
            "iudx:domainIncludes": [
                {
                    "@id": "iudx:RoadSegment"
                }
            ],
            "iudx:rangeIncludes": [
                {
                    "@id": "iudx:Number"
                },
                {
                    "@id": "iudx:ValueDescriptor"
                }
            ]
        },
        {
            "@id": "iudx:pedestrianPathLeftHeight",
            "@type": [
                "iudx:QuantitativeProperty"
            ],
            "rdfs:comment": "Height of the walkway placed on the left edge of the road corresponding to this observation",
            "rdfs:label": "pedestrianPathLeftHeight",
            "rdfs:isDefinedBy": {
                "@id": "iudx:"
            },
            "iudx:domainIncludes": [
                {
                    "@id": "iudx:RoadSegment"
                }
            ],
            "iudx:rangeIncludes": [
                {
                    "@id": "iudx:Number"
                },
                {
                    "@id": "iudx:ValueDescriptor"
                }
            ]
        },
        {
            "@id": "iudx:pedestrianPathLeftWidth",
            "@type": [
                "iudx:QuantitativeProperty"
            ],
            "rdfs:comment": "Width of the walkway placed on the left edge of the road corresponding to this observation.",
            "rdfs:label": "pedestrianPathLeftWidth",
            "rdfs:isDefinedBy": {
                "@id": "iudx:"
            },
            "iudx:domainIncludes": [
                {
                    "@id": "iudx:RoadSegment"
                }
            ],
            "iudx:rangeIncludes": [
                {
                    "@id": "iudx:Number"
                },
                {
                    "@id": "iudx:ValueDescriptor"
                }
            ]
        },
        {
            "@id": "iudx:pedestrianPathMaterial",
            "@type": [
                "iudx:TextProperty"
            ],
            "rdfs:comment": "Construction material used for laying the walkway / footpath on the sides of the road corresponding to this observation.",
            "rdfs:label": "pedestrianPathMaterial",
            "rdfs:isDefinedBy": {
                "@id": "iudx:"
            },
            "iudx:domainIncludes": [
                {
                    "@id": "iudx:RoadSegment"
                }
            ],
            "iudx:rangeIncludes": [
                {
                    "@id": "iudx:Text"
                },
                {
                    "@id": "iudx:ValueDescriptor"
                }
            ]
        },
        {
            "@id": "iudx:pedestrianPathPlacement",
            "@type": [
                "iudx:TextProperty"
            ],
            "rdfs:comment": "Describes the presence and placement of pedestrian along the road segment corresponding to this observation. ENUM: [RIGHT, LEFT, BOTH, NOT_AVAILABLE]",
            "rdfs:label": "pedestrianPathPlacement",
            "rdfs:isDefinedBy": {
                "@id": "iudx:"
            },
            "iudx:domainIncludes": [
                {
                    "@id": "iudx:RoadSegment"
                }
            ],
            "iudx:rangeIncludes": [
                {
                    "@id": "iudx:Text"
                },
                {
                    "@id": "iudx:ValueDescriptor"
                }
            ]
        },
        {
            "@id": "iudx:pedestrianPathRightHeight",
            "@type": [
                "iudx:QuantitativeProperty"
            ],
            "rdfs:comment": "Height of the walkway placed on the right edge of the road corresponding to this observation",
            "rdfs:label": "pedestrianPathRightHeight",
            "rdfs:isDefinedBy": {
                "@id": "iudx:"
            },
            "iudx:domainIncludes": [
                {
                    "@id": "iudx:RoadSegment"
                }
            ],
            "iudx:rangeIncludes": [
                {
                    "@id": "iudx:Number"
                },
                {
                    "@id": "iudx:ValueDescriptor"
                }
            ]
        },
        {
            "@id": "iudx:pedestrianPathRightWidth",
            "@type": [
                "iudx:QuantitativeProperty"
            ],
            "rdfs:comment": "Width of the walkway placed on the right edge of the road corresponding to this observation.",
            "rdfs:label": "pedestrianPathRightWidth",
            "rdfs:isDefinedBy": {
                "@id": "iudx:"
            },
            "iudx:domainIncludes": [
                {
                    "@id": "iudx:RoadSegment"
                }
            ],
            "iudx:rangeIncludes": [
                {
                    "@id": "iudx:Number"
                },
                {
                    "@id": "iudx:ValueDescriptor"
                }
            ]
        },
        {
            "@id": "iudx:performanceRatio",
            "@type": [
                "iudx:QuantitativeProperty"
            ],
            "rdfs:comment": "The ratio of the measured output to the expected( or calculated) output.",
            "rdfs:label": "performanceRatio",
            "rdfs:isDefinedBy": {
                "@id": "iudx:"
            },
            "iudx:domainIncludes": [
                {
                    "@id": "iudx:SolarEnergy"
                }
            ],
            "iudx:rangeIncludes": [
                {
                    "@id": "iudx:Number"
                },
                {
                    "@id": "iudx:ValueDescriptor"
                }
            ]
        },
        {
            "@id": "iudx:perimeter",
            "@type": [
                "iudx:QuantitativeProperty"
            ],
            "rdfs:comment": "The length of the boundary lining the entity corresponding to this observation.",
            "rdfs:label": "perimeter",
            "rdfs:isDefinedBy": {
                "@id": "iudx:"
            },
            "iudx:domainIncludes": [
                {
                    "@id": "iudx:Headquarters"
                }
            ],
            "iudx:rangeIncludes": [
                {
                    "@id": "iudx:Number"
                },
                {
                    "@id": "iudx:ValueDescriptor"
                }
            ]
        },
        {
            "@id": "iudx:phaseCurrent",
            "@type": [
                "iudx:QuantitativeProperty"
            ],
            "rdfs:comment": "Current per phase. Ordered triple comprising of active current from three phases in the following order: [R Y B]",
            "rdfs:label": "phaseCurrent",
            "rdfs:isDefinedBy": {
                "@id": "iudx:"
            },
            "iudx:domainIncludes": [
                {
                    "@id": "iudx:StreetLightFeeder"
                },
                {
                    "@id": "iudx:SolarEnergy"
                },
                {
                    "@id": "iudx:EnergyMeter"
                }
            ],
            "iudx:rangeIncludes": [
                {
                    "@id": "iudx:NumericArray"
                },
                {
                    "@id": "iudx:ValueDescriptor"
                }
            ]
        },
        {
            "@id": "iudx:phaseVoltage",
            "@type": [
                "iudx:QuantitativeProperty"
            ],
            "rdfs:comment": "Voltage per phase. Ordered triple comprising of active voltage from three phases in the following order: [R Y B]",
            "rdfs:label": "phaseVoltage",
            "rdfs:isDefinedBy": {
                "@id": "iudx:"
            },
            "iudx:domainIncludes": [
                {
                    "@id": "iudx:StreetLightFeeder"
                },
                {
                    "@id": "iudx:SolarEnergy"
                },
                {
                    "@id": "iudx:EnergyMeter"
                }
            ],
            "iudx:rangeIncludes": [
                {
                    "@id": "iudx:NumericArray"
                },
                {
                    "@id": "iudx:ValueDescriptor"
                }
            ],
            "skos:exactMatch": {
                "@id": "Fiware:voltage"
            }
        },
        {
            "@id": "iudx:pickup_type",
            "@type": [
                "iudx:TextProperty"
            ],
            "rdfs:comment": "Indicates pickup method.SameAs: 'pickup_type' field from GTFS Static Field definitions-stop_times.txt (https://developers.google.com/transit/gtfs/reference#stop_timestxt)",
            "rdfs:label": "pickup_type",
            "rdfs:isDefinedBy": {
                "@id": "iudx:"
            },
            "iudx:domainIncludes": [
                {
                    "@id": "iudx:StopTimesDesc"
                }
            ],
            "iudx:rangeIncludes": [
                {
                    "@id": "iudx:Text"
                },
                {
                    "@id": "iudx:ValueDescriptor"
                }
            ],
            "skos:exactMatch": {
                "@id": "GTFS: pickup_type"
            }
        },
        {
            "@id": "iudx:po4",
            "@type": [
                "iudx:QuantitativeProperty"
            ],
            "rdfs:comment": "Ortho-phosphate concentration measured in the waste-water treatment plant corresponding to this observation.",
            "rdfs:label": "po4",
            "rdfs:isDefinedBy": {
                "@id": "iudx:"
            },
            "iudx:domainIncludes": [
                {
                    "@id": "iudx:WasteWaterMgmt"
                }
            ],
            "iudx:rangeIncludes": [
                {
                    "@id": "iudx:Number"
                },
                {
                    "@id": "iudx:ValueDescriptor"
                }
            ],
            "skos:exactMatch": {
                "@id": "fiware:po4"
            }
        },
        {
            "@id": "iudx:poiID",
            "@type": [
                "iudx:TextProperty"
            ],
            "rdfs:comment": "The ID of the waste collection region, which can be an aisle comprising of waste bin(s) or a larger dump yard.",
            "rdfs:label": "poiID",
            "rdfs:isDefinedBy": {
                "@id": "iudx:"
            },
            "iudx:domainIncludes": [
                {
                    "@id": "iudx:WmgmtVehicle"
                }
            ],
            "iudx:rangeIncludes": [
                {
                    "@id": "iudx:Text"
                },
                {
                    "@id": "iudx:ValueDescriptor"
                }
            ]
        },
        {
            "@id": "iudx:poiName",
            "@type": [
                "iudx:TextProperty"
            ],
            "rdfs:comment": "The name identifying the waste collection region, which can be an aisle comprising of waste bin(s) or a larger dump yard.",
            "rdfs:label": "poiName",
            "rdfs:isDefinedBy": {
                "@id": "iudx:"
            },
            "iudx:domainIncludes": [
                {
                    "@id": "iudx:WmgmtVehicle"
                }
            ],
            "iudx:rangeIncludes": [
                {
                    "@id": "iudx:Text"
                },
                {
                    "@id": "iudx:ValueDescriptor"
                }
            ]
        },
        {
            "@id": "iudx:poiType",
            "@type": [
                "iudx:TextProperty"
            ],
            "rdfs:comment": "The type of the waste collection point of interest corresponding to this observation. For eg., landfill, dumpyard, household etc.",
            "rdfs:label": "poiType",
            "rdfs:isDefinedBy": {
                "@id": "iudx:"
            },
            "iudx:domainIncludes": [
                {
                    "@id": "iudx:WmgmtVehicle"
                }
            ],
            "iudx:rangeIncludes": [
                {
                    "@id": "iudx:Text"
                },
                {
                    "@id": "iudx:ValueDescriptor"
                }
            ]
        },
        {
            "@id": "iudx:powerConsumption",
            "@type": [
                "iudx:QuantitativeProperty"
            ],
            "rdfs:comment": "Power consumed by the entity corresponding to this observation.",
            "rdfs:label": "powerConsumption",
            "rdfs:isDefinedBy": {
                "@id": "iudx:"
            },
            "iudx:domainIncludes": [
                {
                    "@id": "iudx:Streetlight"
                },
                {
                    "@id": "iudx:EnergyMeter"
                },
                {
                    "@id": "iudx:EVChargingStation"
                }
            ],
            "iudx:rangeIncludes": [
                {
                    "@id": "iudx:Number"
                },
                {
                    "@id": "iudx:ValueDescriptor"
                }
            ],
            "skos:exactMatch": {
                "@id": "Fiware:powerConsumption"
            }
        },
        {
            "@id": "iudx:powerFactor",
            "@type": [
                "iudx:QuantitativeProperty"
            ],
            "rdfs:comment": "Power factor or the ratio of working power of the entity corresponding to this observation.",
            "rdfs:label": "powerFactor",
            "rdfs:isDefinedBy": {
                "@id": "iudx:"
            },
            "iudx:domainIncludes": [
                {
                    "@id": "iudx:Streetlight"
                },
                {
                    "@id": "iudx:SolarEnergy"
                },
                {
                    "@id": "iudx:EnergyMeter"
                }
            ],
            "iudx:rangeIncludes": [
                {
                    "@id": "iudx:Number"
                },
                {
                    "@id": "iudx:ValueDescriptor"
                }
            ],
            "skos:exactMatch": {
                "@id": "Fiware:powerFactor"
            }
        },
        {
            "@id": "iudx:powerRating",
            "@type": [
                "iudx:QuantitativeProperty"
            ],
            "rdfs:comment": "Power rating of the LED or the streetlight bulb corresponding to this observation.",
            "rdfs:label": "powerRating",
            "rdfs:isDefinedBy": {
                "@id": "iudx:"
            },
            "iudx:domainIncludes": [
                {
                    "@id": "iudx:Streetlight"
                }
            ],
            "iudx:rangeIncludes": [
                {
                    "@id": "iudx:Number"
                },
                {
                    "@id": "iudx:ValueDescriptor"
                }
            ]
        },
        {
            "@id": "iudx:powerState",
            "@type": [
                "iudx:TextProperty"
            ],
            "rdfs:comment": "Indicates the current power status of the entity corresponding to this observation.",
            "rdfs:label": "powerState",
            "rdfs:isDefinedBy": {
                "@id": "iudx:"
            },
            "iudx:domainIncludes": [
                {
                    "@id": "iudx:StreetLightFeeder"
                },
                {
                    "@id": "iudx:Streetlight"
                }
            ],
            "iudx:rangeIncludes": [
                {
                    "@id": "iudx:Text"
                },
                {
                    "@id": "iudx:ValueDescriptor"
                }
            ],
            "skos:exactMatch": {
                "@id": "Fiware:powerState"
            }
        },
        {
            "@id": "iudx:precipitation",
            "@type": [
                "iudx:QuantitativeProperty"
            ],
            "rdfs:comment": "Observed precipitation/rainfall level over a given duration.",
            "rdfs:label": "precipitation",
            "iudx:domainIncludes": [
                {
                    "@id": "iudx:EnvWeather"
                },
                {
                    "@id": "iudx:EnvAQM"
                },
                {
                    "@id": "iudx:MosquitoDensity"
                },
                {
                    "@id": "iudx:AirQuality"
                }
            ],
            "iudx:rangeIncludes": [
                {
                    "@id": "iudx:Number"
                },
                {
                    "@id": "iudx:ValueDescriptor"
                }
            ],
            "rdfs:isDefinedBy": {
                "@id": "iudx:"
            },
            "skos:exactMatch": {
                "@id": "Fiware:precipitation"
            }
        },
        {
            "@id": "iudx:precipitationForecast",
            "@type": [
                "iudx:QuantitativeProperty"
            ],
            "rdfs:comment": "Forecasted rainfall over a certain duration in future.",
            "rdfs:label": "precipitationForecast",
            "rdfs:isDefinedBy": {
                "@id": "iudx:"
            },
            "iudx:domainIncludes": [
                {
                    "@id": "iudx:EnvWeather"
                }
            ],
            "iudx:rangeIncludes": [
                {
                    "@id": "iudx:Number"
                },
                {
                    "@id": "iudx:ValueDescriptor"
                }
            ]
        },
        {
            "@id": "iudx:protocol",
            "@type": [
                "iudx:TextProperty"
            ],
            "rdfs:comment": "The name of the network protocol used for data communication.",
            "rdfs:label": "protocol",
            "iudx:domainIncludes": [
                {
                    "@id": "iudx:HTTPAccess"
                },
                {
                    "@id": "iudx:FileAccess"
                },
                {
                    "@id": "iudx:StreamingAccess"
                }
            ],
            "iudx:rangeIncludes": [
                {
                    "@id": "iudx:Text"
                },
                {
                    "@id": "iudx:ValueDescriptor"
                }
            ],
            "rdfs:isDefinedBy": {
                "@id": "iudx:"
            }
        },
        {
            "@id": "iudx:rcRecoveryAmount",
            "@type": [
                "iudx:QuantitativeProperty"
            ],
            "rdfs:comment": "Amount collected towards Registration Certificate on monthly basis from the establishment per emplyoee.",
            "rdfs:label": "rcRecoveryAmount",
            "rdfs:isDefinedBy": {
                "@id": "iudx:"
            },
            "iudx:domainIncludes": [
                {
                    "@id": "iudx:RevenueCollection"
                }
            ],
            "iudx:rangeIncludes": [
                {
                    "@id": "iudx:Number"
                },
                {
                    "@id": "iudx:ValueDescriptor"
                }
            ]
        },
        {
            "@id": "iudx:reAssessmentCount",
            "@type": [
                "iudx:QuantitativeProperty"
            ],
            "rdfs:comment": "Number of re-assessments conducted to assess the value of property.",
            "rdfs:label": "reAssessmentCount",
            "rdfs:isDefinedBy": {
                "@id": "iudx:"
            },
            "iudx:domainIncludes": [
                {
                    "@id": "iudx:RevenueCollection"
                }
            ],
            "iudx:rangeIncludes": [
                {
                    "@id": "iudx:Number"
                },
                {
                    "@id": "iudx:ValueDescriptor"
                }
            ]
        },
        {
            "@id": "iudx:reactiveEnergyLag",
            "@type": [
                "iudx:QuantitativeProperty"
            ],
            "rdfs:comment": "The value of Lag Reactive Energy consumed by the device corresponding to this observation.",
            "rdfs:label": "reactiveEnergyLag",
            "rdfs:isDefinedBy": {
                "@id": "iudx:"
            },
            "iudx:domainIncludes": [
                {
                    "@id": "iudx:EnergyMeter"
                }
            ],
            "iudx:rangeIncludes": [
                {
                    "@id": "iudx:Number"
                },
                {
                    "@id": "iudx:ValueDescriptor"
                }
            ]
        },
        {
            "@id": "iudx:reactiveEnergyLead",
            "@type": [
                "iudx:QuantitativeProperty"
            ],
            "rdfs:comment": "The value of Lead Reactive Energy consumed by the device corresponding to this observation.",
            "rdfs:label": "reactiveEnergyLead",
            "rdfs:isDefinedBy": {
                "@id": "iudx:"
            },
            "iudx:domainIncludes": [
                {
                    "@id": "iudx:EnergyMeter"
                }
            ],
            "iudx:rangeIncludes": [
                {
                    "@id": "iudx:Number"
                },
                {
                    "@id": "iudx:ValueDescriptor"
                }
            ]
        },
        {
            "@id": "iudx:reactivePower",
            "@type": [
                "iudx:QuantitativeProperty"
            ],
            "rdfs:comment": "Reactive power consumed per phase. Ordered triple comprising of active power from three phases in the following order: [R Y B]",
            "rdfs:label": "reactivePower",
            "rdfs:isDefinedBy": {
                "@id": "iudx:"
            },
            "iudx:domainIncludes": [
                {
                    "@id": "iudx:StreetLightFeeder"
                },
                {
                    "@id": "iudx:SolarEnergy"
                }
            ],
            "iudx:rangeIncludes": [
                {
                    "@id": "iudx:NumericArray"
                },
                {
                    "@id": "iudx:ValueDescriptor"
                }
            ],
            "skos:exactMatch": {
                "@id": "Fiware:reactivePower"
            }
        },
        {
            "@id": "iudx:redox",
            "@type": [
                "iudx:QuantitativeProperty"
            ],
            "rdfs:comment": "Reduction potential or oxidation measured in waste-water treatment plant corresponding to this observation.",
            "rdfs:label": "redox",
            "rdfs:isDefinedBy": {
                "@id": "iudx:"
            },
            "iudx:domainIncludes": [
                {
                    "@id": "iudx:WasteWaterMgmt"
                }
            ],
            "iudx:rangeIncludes": [
                {
                    "@id": "iudx:Number"
                },
                {
                    "@id": "iudx:ValueDescriptor"
                }
            ],
            "skos:exactMatch": {
                "@id": "fiware:redox"
            }
        },
        {
            "@id": "iudx:referenceLevel",
            "@type": [
                "iudx:QuantitativeProperty"
            ],
            "rdfs:comment": "Reference setting used to compute the currentLevel.",
            "rdfs:label": "referenceLevel",
            "rdfs:isDefinedBy": {
                "@id": "iudx:"
            },
            "iudx:domainIncludes": [
                {
                    "@id": "iudx:EnvFlood"
                }
            ],
            "iudx:rangeIncludes": [
                {
                    "@id": "iudx:Number"
                },
                {
                    "@id": "iudx:ValueDescriptor"
                }
            ]
        },
        {
            "@id": "iudx:relationType",
            "@type": [
                "iudx:TextProperty"
            ],
            "rdfs:comment": "Type of relation. ENUM: [REL_MESSAGESTREAM, REL_FILE, REL_DATASET, REL_THING].",
            "rdfs:label": "relationType",
            "iudx:domainIncludes": [
                {
                    "@id": "iudx:RelationshipValue",
                    "iudx:requiredProperty": true
                }
            ],
            "iudx:rangeIncludes": [
                {
                    "@id": "iudx:Text"
                },
                {
                    "@id": "iudx:ValueDescriptor"
                }
            ],
            "rdfs:isDefinedBy": {
                "@id": "iudx:"
            }
        },
        {
            "@id": "iudx:relativeHumidityForecast",
            "@type": [
                "iudx:QuantitativeProperty"
            ],
            "rdfs:comment": "Forecasted relative humidity (water vapour in air) over a certain duration in future.",
            "rdfs:label": "relativeHumidityForecast",
            "rdfs:isDefinedBy": {
                "@id": "iudx:"
            },
            "iudx:domainIncludes": [
                {
                    "@id": "iudx:EnvWeather"
                }
            ],
            "iudx:rangeIncludes": [
                {
                    "@id": "iudx:Number"
                },
                {
                    "@id": "iudx:ValueDescriptor"
                }
            ]
        },
        {
            "@id": "iudx:remarks",
            "@type": [
                "iudx:TextProperty"
            ],
            "rdfs:comment": "Remarks or additional information of the entity corresponding to this observation",
            "rdfs:label": "remarks",
            "rdfs:isDefinedBy": {
                "@id": "iudx:"
            },
            "iudx:domainIncludes": [
                {
                    "@id": "iudx:District"
                }
            ],
            "iudx:rangeIncludes": [
                {
                    "@id": "iudx:Text"
                },
                {
                    "@id": "iudx:ValueDescriptor"
                }
            ]
        },
        {
            "@id": "iudx:reportID",
            "@type": [
                "iudx:TextProperty"
            ],
            "rdfs:comment": "Unique ID assigned for the issue or report or feedback or transaction corresponding to this observation.",
            "rdfs:label": "reportID",
            "rdfs:isDefinedBy": {
                "@id": "iudx:"
            },
            "iudx:domainIncludes": [
                {
                    "@id": "iudx:IssueReporting"
                },
                {
                    "@id": "iudx:SafetiPin"
                },
                {
                    "@id": "iudx:TrafficViolations"
                },
                {
                    "@id": "iudx:WmgmtVehicle"
                }
            ],
            "iudx:rangeIncludes": [
                {
                    "@id": "iudx:Text"
                },
                {
                    "@id": "iudx:ValueDescriptor"
                }
            ],
            "skos:exactMatch": {
                "@id": "open311:servicecode"
            }
        },
        {
            "@id": "iudx:reportingMode",
            "@type": [
                "iudx:TextProperty"
            ],
            "rdfs:comment": "The communication channel or medium used to convey the issue or report or feedback or transaction corresponding to this observation. For eg., Email, SMS, Telephone etc.",
            "rdfs:label": "reportingMode",
            "rdfs:isDefinedBy": {
                "@id": "iudx:"
            },
            "iudx:domainIncludes": [
                {
                    "@id": "iudx:IssueReporting"
                }
            ],
            "iudx:rangeIncludes": [
                {
                    "@id": "iudx:Text"
                },
                {
                    "@id": "iudx:ValueDescriptor"
                }
            ]
        },
        {
            "@id": "iudx:residentialPOIs",
            "@type": [
                "iudx:QuantitativeProperty"
            ],
            "rdfs:comment": "The total count of households which serve as point of interests corresponding to this observation.",
            "rdfs:label": "residentialPOIs",
            "iudx:domainIncludes": [
                {
                    "@id": "iudx:WmgmtVehicle"
                }
            ],
            "iudx:rangeIncludes": [
                {
                    "@id": "iudx:Number"
                },
                {
                    "@id": "iudx:ValueDescriptor"
                }
            ],
            "rdfs:isDefinedBy": {
                "@id": "iudx:"
            }
        },
        {
            "@id": "iudx:residentialUnitsCount",
            "@type": [
                "iudx:QuantitativeProperty"
            ],
            "rdfs:comment": "The total number of households or residential properties present at the location corresponding to this observation.",
            "rdfs:label": "residentialUnitsCount",
            "rdfs:isDefinedBy": {
                "@id": "iudx:"
            },
            "iudx:domainIncludes": [
                {
                    "@id": "iudx:WmgmtVehicle"
                }
            ],
            "iudx:rangeIncludes": [
                {
                    "@id": "iudx:Number"
                },
                {
                    "@id": "iudx:ValueDescriptor"
                }
            ]
        },
        {
            "@id": "iudx:resolution",
            "@type": [
                "iudx:QuantitativeProperty"
            ],
            "rdfs:comment": "Resolution of a measurement. That is, the smallest change in a quantity being measured that causes a perceptible change in the corresponding observation under specified conditions.",
            "rdfs:label": "resolution",
            "iudx:domainIncludes": [
                {
                    "@id": "iudx:ValueDescriptor"
                }
            ],
            "iudx:rangeIncludes": [
                {
                    "@id": "iudx:Number"
                },
                {
                    "@id": "iudx:ValueDescriptor"
                }
            ],
            "rdfs:isDefinedBy": {
                "@id": "iudx:"
            }
        },
        {
            "@id": "iudx:resolutionStatus",
            "@type": [
                "iudx:TextProperty"
            ],
            "rdfs:comment": "Status of the issue that was reported in terms of resolution or the actions taken on it. Could be Open, Assigned, InProgress, Unassigned, Resolved, Closed, Reopened.",
            "rdfs:label": "resolutionStatus",
            "rdfs:isDefinedBy": {
                "@id": "iudx:"
            },
            "iudx:domainIncludes": [
                {
                    "@id": "iudx:IssueReporting"
                }
            ],
            "iudx:rangeIncludes": [
                {
                    "@id": "iudx:Text"
                },
                {
                    "@id": "iudx:ValueDescriptor"
                }
            ]
        },
        {
            "@id": "iudx:revenueCollectionType",
            "@type": [
                "iudx:TextProperty"
            ],
            "rdfs:comment": "Type of source from which the city administration collects the revenue, could be property tax, vehicle registration, party hall booking, community hall booking, auditorium booking etc.",
            "rdfs:label": "revenueCollectionType",
            "rdfs:isDefinedBy": {
                "@id": "iudx:"
            },
            "iudx:domainIncludes": [
                {
                    "@id": "iudx:RevenueCollection"
                }
            ],
            "iudx:rangeIncludes": [
                {
                    "@id": "iudx:Text"
                },
                {
                    "@id": "iudx:ValueDescriptor"
                }
            ]
        },
        {
            "@id": "iudx:revenueLicense",
            "@type": [
                "iudx:TextProperty"
            ],
            "rdfs:comment": "License number of the business establishment under which an individual as a sole proprietor or a company chooses to do business.",
            "rdfs:label": "revenueLicense",
            "rdfs:isDefinedBy": {
                "@id": "iudx:"
            },
            "iudx:domainIncludes": [
                {
                    "@id": "iudx:RevenueCollection"
                }
            ],
            "iudx:rangeIncludes": [
                {
                    "@id": "iudx:Text"
                },
                {
                    "@id": "iudx:ValueDescriptor"
                }
            ]
        },
        {
            "@id": "iudx:revenueLicenseStatus",
            "@type": [
                "iudx:TextProperty"
            ],
            "rdfs:comment": "Status of the license number of the business establishment under which an individual as a sole proprietor or a company chooses to do business.",
            "rdfs:label": "revenueLicenseStatus",
            "rdfs:isDefinedBy": {
                "@id": "iudx:"
            },
            "iudx:domainIncludes": [
                {
                    "@id": "iudx:RevenueCollection"
                }
            ],
            "iudx:rangeIncludes": [
                {
                    "@id": "iudx:Text"
                },
                {
                    "@id": "iudx:ValueDescriptor"
                }
            ]
        },
        {
            "@id": "iudx:rfID",
            "@type": [
                "iudx:TextProperty"
            ],
            "rdfs:comment": "Gives the ID of the RFID reader.",
            "rdfs:label": "rfID",
            "rdfs:isDefinedBy": {
                "@id": "iudx:"
            },
            "iudx:domainIncludes": [
                {
                    "@id": "iudx:Device"
                },
                {
                    "@id": "iudx:WmgmtBin"
                }
            ],
            "iudx:rangeIncludes": [
                {
                    "@id": "iudx:Text"
                },
                {
                    "@id": "iudx:ValueDescriptor"
                }
            ]
        },
        {
            "@id": "iudx:rightOfWayWidth",
            "@type": [
                "iudx:QuantitativeProperty"
            ],
            "rdfs:comment": "Right of Way (RoW) is the total land area available for the roadway. Its width accommodates for carriages way + other necessities + future extension, along the road's alignment.",
            "rdfs:label": "rightOfWayWidth",
            "rdfs:isDefinedBy": {
                "@id": "iudx:"
            },
            "iudx:domainIncludes": [
                {
                    "@id": "iudx:RoadSegment"
                }
            ],
            "iudx:rangeIncludes": [
                {
                    "@id": "iudx:Number"
                },
                {
                    "@id": "iudx:ValueDescriptor"
                }
            ]
        },
        {
            "@id": "iudx:roadClass",
            "@type": [
                "iudx:TextProperty"
            ],
            "rdfs:comment": "The type of road corresponding to this observation. ENUM: [OTHER_PUBLIC_ROAD, PRIVATE_ROAD, MINOR_CITY_ROAD, MAJOR_DISTRICT_ROAD, MAJOR_CITY_ROAD, NATIONAL_HIGHWAY, SERVICE_ROAD, STATE_HIGHWAY, OTHER_DISTRICT_ROAD, PORT_ROAD].",
            "rdfs:label": "roadClass",
            "rdfs:isDefinedBy": {
                "@id": "iudx:"
            },
            "iudx:domainIncludes": [
                {
                    "@id": "iudx:RoadSegment"
                }
            ],
            "iudx:rangeIncludes": [
                {
                    "@id": "iudx:Text"
                },
                {
                    "@id": "iudx:ValueDescriptor"
                }
            ],
            "skos:exactMatch": {
                "@id": "Fiware: roadClass"
            }
        },
        {
            "@id": "iudx:roadDirection",
            "@type": [
                "iudx:TextProperty"
            ],
            "rdfs:comment": "Represents the direction the road is heading to. ENUM: [N, S, E, W]. The values N,S,E,W represent North,South,East,West respectively.",
            "rdfs:label": "roadDirection",
            "rdfs:isDefinedBy": {
                "@id": "iudx:"
            },
            "iudx:domainIncludes": [
                {
                    "@id": "iudx:RoadSegment"
                }
            ],
            "iudx:rangeIncludes": [
                {
                    "@id": "iudx:Text"
                },
                {
                    "@id": "iudx:ValueDescriptor"
                }
            ]
        },
        {
            "@id": "iudx:roadEndPoint",
            "@type": [
                "iudx:GeoProperty"
            ],
            "rdfs:comment": "Describes the point where the road segment corresponding to this observation ends.",
            "rdfs:label": "roadEndPoint",
            "rdfs:isDefinedBy": {
                "@id": "iudx:"
            },
            "iudx:domainIncludes": [
                {
                    "@id": "iudx:RoadSegment"
                }
            ],
            "iudx:rangeIncludes": [
                {
                    "@id": "iudx:Place"
                },
                {
                    "@id": "iudx:ValueDescriptor"
                }
            ],
            "skos:exactMatch": {
                "@id": "Fiware: endPoint"
            }
        },
        {
            "@id": "iudx:roadID",
            "@type": [
                "iudx:TextProperty"
            ],
            "rdfs:comment": "Unique representation of the road corresponding to this observation",
            "rdfs:label": "roadID",
            "rdfs:isDefinedBy": {
                "@id": "iudx:"
            },
            "iudx:domainIncludes": [
                {
                    "@id": "iudx:RoadSegment"
                }
            ],
            "iudx:rangeIncludes": [
                {
                    "@id": "iudx:Text"
                },
                {
                    "@id": "iudx:ValueDescriptor"
                }
            ]
        },
        {
            "@id": "iudx:roadMaterial",
            "@type": [
                "iudx:TextProperty"
            ],
            "rdfs:comment": "The construction material used for laying the carriageway corresponding to this observation. For eg. concrete, earthen, tar etc.",
            "rdfs:label": "roadMaterial",
            "rdfs:isDefinedBy": {
                "@id": "iudx:"
            },
            "iudx:domainIncludes": [
                {
                    "@id": "iudx:RoadSegment"
                }
            ],
            "iudx:rangeIncludes": [
                {
                    "@id": "iudx:Text"
                },
                {
                    "@id": "iudx:ValueDescriptor"
                }
            ]
        },
        {
            "@id": "iudx:roadName",
            "@type": [
                "iudx:TextProperty"
            ],
            "rdfs:comment": "The name of the road corresponding to this observation",
            "rdfs:label": "roadName",
            "rdfs:isDefinedBy": {
                "@id": "iudx:"
            },
            "iudx:domainIncludes": [
                {
                    "@id": "iudx:RoadSegment"
                }
            ],
            "iudx:rangeIncludes": [
                {
                    "@id": "iudx:Text"
                },
                {
                    "@id": "iudx:ValueDescriptor"
                }
            ]
        },
        {
            "@id": "iudx:roadOccupancy",
            "@type": [
                "iudx:QuantitativeProperty"
            ],
            "rdfs:comment": "The percentage of carriage way length that is occupied by vehicles corresponding to this observation.",
            "rdfs:label": "roadOccupancy",
            "rdfs:isDefinedBy": {
                "@id": "iudx:"
            },
            "iudx:domainIncludes": [
                {
                    "@id": "iudx:RoadSegment"
                }
            ],
            "iudx:rangeIncludes": [
                {
                    "@id": "iudx:Number"
                },
                {
                    "@id": "iudx:ValueDescriptor"
                }
            ]
        },
        {
            "@id": "iudx:roadStartPoint",
            "@type": [
                "iudx:GeoProperty"
            ],
            "rdfs:comment": "Describes the point where the road segment corresponding to this observation starts.",
            "rdfs:label": "roadStartPoint",
            "rdfs:isDefinedBy": {
                "@id": "iudx:"
            },
            "iudx:domainIncludes": [
                {
                    "@id": "iudx:RoadSegment"
                }
            ],
            "iudx:rangeIncludes": [
                {
                    "@id": "iudx:Place"
                },
                {
                    "@id": "iudx:ValueDescriptor"
                }
            ],
            "skos:exactMatch": {
                "@id": "Fiware: startPoint"
            }
        },
        {
            "@id": "iudx:roadWork",
            "@type": [
                "iudx:TextProperty"
            ],
            "rdfs:comment": "Reasons for the road work in case of urgent intervention. A combination of these values. ENUM: [COLLAPSE, DERAILMENT, FIRE, FLOOD, GASLEAK, LANDSLIDE, OTHER, POWERCUT, ROCKFALL, SAGGING, WATERLEAK]",
            "rdfs:label": "roadWork",
            "rdfs:isDefinedBy": {
                "@id": "iudx:"
            },
            "iudx:domainIncludes": [
                {
                    "@id": "iudx:RoadSegment"
                }
            ],
            "iudx:rangeIncludes": [
                {
                    "@id": "iudx:Text"
                },
                {
                    "@id": "iudx:ValueDescriptor"
                }
            ]
        },
        {
            "@id": "iudx:rotation",
            "@type": [
                "iudx:QuantitativeProperty"
            ],
            "rdfs:comment": "The angle of rotational transformation of the polygon enclosing the entity corresponding to this observation.",
            "rdfs:label": "rotation",
            "rdfs:isDefinedBy": {
                "@id": "iudx:"
            },
            "iudx:domainIncludes": [
                {
                    "@id": "iudx:MajorTowns"
                }
            ],
            "iudx:rangeIncludes": [
                {
                    "@id": "iudx:Number"
                },
                {
                    "@id": "iudx:ValueDescriptor"
                }
            ]
        },
        {
            "@id": "iudx:routeStopSequence",
            "@type": [
                "iudx:TextProperty"
            ],
            "rdfs:comment": "Gives the stop ids/stop codes or station ids/station codes in the right sequence for the route/line/trip corresponding to this observation.",
            "rdfs:label": "routeStopSequence",
            "rdfs:isDefinedBy": {
                "@id": "iudx:"
            },
            "iudx:domainIncludes": [
                {
                    "@id": "iudx:TransitManagement"
                },
                {
                    "@id": "iudx:WmgmtVehicle"
                }
            ],
            "iudx:rangeIncludes": [
                {
                    "@id": "iudx:Text",
                    "@container": "@list"
                },
                {
                    "@id": "iudx:ValueDescriptor"
                }
            ]
        },
        {
            "@id": "iudx:route_color",
            "@type": [
                "iudx:TextProperty"
            ],
            "rdfs:comment": "If assigned, this field defines a color that corresponds to a route. The color must be provided as a six-character hexadecimal number, for example, 00FFFF. If no color is specified, the default route color is white (FFFFFF). SameAs: 'route_color' field from GTFS Static Field definitions-routes.txt (https://developers.google.com/transit/gtfs/reference#routestxt)",
            "rdfs:label": "route_color",
            "rdfs:isDefinedBy": {
                "@id": "iudx:"
            },
            "iudx:domainIncludes": [
                {
                    "@id": "iudx:RoutesDesc"
                }
            ],
            "iudx:rangeIncludes": [
                {
                    "@id": "iudx:Text"
                },
                {
                    "@id": "iudx:ValueDescriptor"
                }
            ],
            "skos:exactMatch": {
                "@id": "GTFS: route_color"
            }
        },
        {
            "@id": "iudx:route_desc",
            "@type": [
                "iudx:TextProperty"
            ],
            "rdfs:comment": "Description of the route. This can include the entire route details including to and from destination and timing information in a text description form. SameAs: 'route_desc' field from GTFS Static Field definitions-routes.txt (https://developers.google.com/transit/gtfs/reference#routestxt)",
            "rdfs:label": "route_desc",
            "rdfs:isDefinedBy": {
                "@id": "iudx:"
            },
            "iudx:domainIncludes": [
                {
                    "@id": "iudx:RoutesDesc"
                }
            ],
            "iudx:rangeIncludes": [
                {
                    "@id": "iudx:Text"
                },
                {
                    "@id": "iudx:ValueDescriptor"
                }
            ],
            "skos:exactMatch": {
                "@id": "GTFS: route_desc"
            }
        },
        {
            "@id": "iudx:route_id",
            "@type": [
                "iudx:TextProperty"
            ],
            "rdfs:comment": "Route ID assigned to the route on which the bus/vehicle corresponding to the bus in this observation is currently plying on.",
            "rdfs:label": "route_id",
            "iudx:domainIncludes": [
                {
                    "@id": "iudx:GtfsCommons"
                },
                {
                    "@id": "iudx:TripDescriptor"
                },
                {
                    "@id": "iudx:FareCollectionSystem"
                },
                {
                    "@id": "iudx:RoutesDesc"
                },
                {
                    "@id": "iudx:TransitManagement"
                }
            ],
            "iudx:rangeIncludes": [
                {
                    "@id": "iudx:Text"
                },
                {
                    "@id": "iudx:ValueDescriptor"
                }
            ],
            "rdfs:isDefinedBy": {
                "@id": "iudx:"
            },
            "skos:exactMatch": {
                "@id": "GTFS: route_id"
            }
        },
        {
            "@id": "iudx:route_long_name",
            "@type": [
                "iudx:TextProperty"
            ],
            "rdfs:comment": "Full name of a route. This name is more descriptive than the routeShortName and often includes the route's destination or stop. This mostly includes the to and from destination names of the route. SameAs: 'route_long_name' field from GTFS Static Field definitions-routes.txt (https://developers.google.com/transit/gtfs/reference#routestxt)",
            "rdfs:label": "route_long_name",
            "rdfs:isDefinedBy": {
                "@id": "iudx:"
            },
            "iudx:domainIncludes": [
                {
                    "@id": "iudx:RoutesDesc"
                }
            ],
            "iudx:rangeIncludes": [
                {
                    "@id": "iudx:Text"
                },
                {
                    "@id": "iudx:ValueDescriptor"
                }
            ],
            "skos:exactMatch": {
                "@id": "GTFS: route_long_name"
            }
        },
        {
            "@id": "iudx:route_short_name",
            "@type": [
                "iudx:TextProperty"
            ],
            "rdfs:comment": "Short name of a route. This will often be the transit vehicle's board name like \"402D\",  or \"Green\" that riders use to identify a route. SameAs: 'route_short_name' field from GTFS Static Field definitions-routes.txt (https://developers.google.com/transit/gtfs/reference#routestxt)",
            "rdfs:label": "route_short_name",
            "rdfs:isDefinedBy": {
                "@id": "iudx:"
            },
            "iudx:domainIncludes": [
                {
                    "@id": "iudx:RoutesDesc"
                }
            ],
            "iudx:rangeIncludes": [
                {
                    "@id": "iudx:Text"
                },
                {
                    "@id": "iudx:ValueDescriptor"
                }
            ],
            "skos:exactMatch": {
                "@id": "GTFS: route_short_name"
            }
        },
        {
            "@id": "iudx:route_text_color",
            "@type": [
                "iudx:TextProperty"
            ],
            "rdfs:comment": "This field can be used to specify a legible color to use for text drawn against a background of route_color. The color must be provided as a six-character hexadecimal number, for example, FFD700. If no color is specified, the default text color is black (000000). SameAs: 'route_text_color' field from GTFS Static Field definitions-routes.txt (https://developers.google.com/transit/gtfs/reference#routestxt)",
            "rdfs:label": "route_text_color",
            "rdfs:isDefinedBy": {
                "@id": "iudx:"
            },
            "iudx:domainIncludes": [
                {
                    "@id": "iudx:RoutesDesc"
                }
            ],
            "iudx:rangeIncludes": [
                {
                    "@id": "iudx:Text"
                },
                {
                    "@id": "iudx:ValueDescriptor"
                }
            ],
            "skos:exactMatch": {
                "@id": "GTFS: route_text_color"
            }
        },
        {
            "@id": "iudx:route_type",
            "@type": [
                "iudx:QuantitativeProperty"
            ],
            "rdfs:comment": "Number indicating the type of transport-\n1 - Subway, Metro. Any underground rail system within a metropolitan area.\n2 - Rail. Used for intercity or long-distance travel.\n3 - Bus. Used for short- and long-distance bus routes. \nSameAs: 'route_type' field from GTFS Static Field definitions-routes.txt <a href=\"https://developers.google.com/transit/gtfs/reference#routestxt\">https://developers.google.com/transit/gtfs/reference#routestxt</a>",
            "rdfs:label": "route_type",
            "rdfs:isDefinedBy": {
                "@id": "iudx:"
            },
            "iudx:domainIncludes": [
                {
                    "@id": "iudx:RoutesDesc"
                }
            ],
            "iudx:rangeIncludes": [
                {
                    "@id": "iudx:Number"
                },
                {
                    "@id": "iudx:ValueDescriptor"
                }
            ],
            "skos:exactMatch": {
                "@id": "GTFS: route_type"
            }
        },
        {
            "@id": "iudx:route_url",
            "@type": [
                "iudx:TextProperty"
            ],
            "rdfs:comment": "Contains the URL of a web page about that particular route and is different from the agency_url. SameAs: 'route_url' field from GTFS Static Field definitions-routes.txt (https://developers.google.com/transit/gtfs/reference#routestxt)",
            "rdfs:label": "route_url",
            "rdfs:isDefinedBy": {
                "@id": "iudx:"
            },
            "iudx:domainIncludes": [
                {
                    "@id": "iudx:RoutesDesc"
                }
            ],
            "iudx:rangeIncludes": [
                {
                    "@id": "iudx:Text"
                },
                {
                    "@id": "iudx:ValueDescriptor"
                }
            ],
            "skos:exactMatch": {
                "@id": "GTFS: route_url"
            }
        },
        {
            "@id": "iudx:rplRank",
            "@type": [
                "iudx:QuantitativeProperty"
            ],
            "rdfs:comment": "RPL rank represents the rank or hop distance from the tree root.",
            "rdfs:label": "rplRank",
            "rdfs:isDefinedBy": {
                "@id": "iudx:"
            },
            "iudx:domainIncludes": [
                {
                    "@id": "iudx:WirelessNetwork"
                }
            ],
            "iudx:rangeIncludes": [
                {
                    "@id": "iudx:Number"
                },
                {
                    "@id": "iudx:ValueDescriptor"
                }
            ]
        },
        {
            "@id": "iudx:rslIn",
            "@type": [
                "iudx:QuantitativeProperty"
            ],
            "rdfs:comment": "The Received Signal Level in is an EWMA of the received signal level for the neighbor-to-node direction.",
            "rdfs:label": "rslIn",
            "rdfs:isDefinedBy": {
                "@id": "iudx:"
            },
            "iudx:domainIncludes": [
                {
                    "@id": "iudx:WirelessNetwork"
                }
            ],
            "iudx:rangeIncludes": [
                {
                    "@id": "iudx:Number"
                },
                {
                    "@id": "iudx:ValueDescriptor"
                }
            ]
        },
        {
            "@id": "iudx:rslOut",
            "@type": [
                "iudx:QuantitativeProperty"
            ],
            "rdfs:comment": "The Received Signal Level out is an EWMA of the received signal level for the node-to-neighbor direction.",
            "rdfs:label": "rslOut",
            "rdfs:isDefinedBy": {
                "@id": "iudx:"
            },
            "iudx:domainIncludes": [
                {
                    "@id": "iudx:WirelessNetwork"
                }
            ],
            "iudx:rangeIncludes": [
                {
                    "@id": "iudx:Number"
                },
                {
                    "@id": "iudx:ValueDescriptor"
                }
            ]
        },
        {
            "@id": "iudx:rssi",
            "@type": [
                "iudx:QuantitativeProperty"
            ],
            "rdfs:comment": "The RSSI (Received Signal Strength Indicator) value of the entity corresponding to this observation.",
            "rdfs:label": "rssi",
            "rdfs:isDefinedBy": {
                "@id": "iudx:"
            },
            "iudx:domainIncludes": [
                {
                    "@id": "iudx:Device"
                }
            ],
            "iudx:rangeIncludes": [
                {
                    "@id": "iudx:Number"
                },
                {
                    "@id": "iudx:ValueDescriptor"
                }
            ],
            "skos:exactMatch": {
                "@id": "Fiware: Device.rssi"
            }
        },
        {
            "@id": "iudx:safetiPinScore",
            "@type": [
                "iudx:QuantitativeProperty"
            ],
            "rdfs:comment": "Score given to the location corresponding to this observation. The score is on a scale of 5 if the SafetiPinType is 'Feeling' and on a scale of 10 if the SafetiPinType is 'Audit'",
            "rdfs:label": "safetiPinScore",
            "rdfs:isDefinedBy": {
                "@id": "iudx:"
            },
            "iudx:domainIncludes": [
                {
                    "@id": "iudx:SafetiPin"
                }
            ],
            "iudx:rangeIncludes": [
                {
                    "@id": "iudx:Number"
                },
                {
                    "@id": "iudx:ValueDescriptor"
                }
            ]
        },
        {
            "@id": "iudx:sameAs",
            "@type": [
                "iudx:TextProperty"
            ],
            "rdfs:comment": "URL reference to another thing/entity that identifies the given thing/entity. This may be used to provide references to another data models where a property is described or say a reference to Wiki pages for a given thing etc.",
            "rdfs:label": "sameAs",
            "iudx:domainIncludes": [
                {
                    "@id": "iudx:ValueDescriptor"
                }
            ],
            "iudx:rangeIncludes": [
                {
                    "@id": "iudx:Text",
                    "@type": "@id"
                }
            ],
            "skos:exactMatch": {
                "@id": "schema:sameAs"
            },
            "rdfs:isDefinedBy": {
                "@id": "iudx:"
            }
        },
        {
            "@id": "iudx:sanctionedAmount",
            "@type": [
                "iudx:QuantitativeProperty"
            ],
            "rdfs:comment": "The actual amount spent from the grant/allocated amount for the scheme.",
            "rdfs:label": "sanctionedAmount",
            "rdfs:isDefinedBy": {
                "@id": "iudx:"
            },
            "iudx:domainIncludes": [
                {
                    "@id": "iudx:PublicSchemes"
                }
            ],
            "iudx:rangeIncludes": [
                {
                    "@id": "iudx:Number"
                },
                {
                    "@id": "iudx:ValueDescriptor"
                }
            ]
        },
        {
            "@id": "iudx:scale",
            "@type": [
                "iudx:QuantitativeProperty"
            ],
            "rdfs:comment": "The amount of translation invloved in representing a point/place graphically.",
            "rdfs:label": "scale",
            "rdfs:isDefinedBy": {
                "@id": "iudx:"
            },
            "iudx:domainIncludes": [
                {
                    "@id": "iudx:MajorTowns"
                }
            ],
            "iudx:rangeIncludes": [
                {
                    "@id": "iudx:Number"
                },
                {
                    "@id": "iudx:ValueDescriptor"
                }
            ]
        },
        {
            "@id": "iudx:schedule_relationship",
            "@type": [
                "iudx:TextProperty"
            ],
            "rdfs:comment": "Describes if the Route/Trip has been scheduled. SameAs: 'schedule_relationship' field from GTFS Realtime message-TripDescriptor ENUM[SCHEDULED, ADDED, UNSCHEDULED, CANCELED] (https://developers.google.com/transit/gtfs-realtime/reference#message-tripdescriptor)",
            "rdfs:label": "schedule_relationship",
            "rdfs:isDefinedBy": {
                "@id": "iudx:"
            },
            "iudx:domainIncludes": [
                {
                    "@id": "iudx:TripDescriptor"
                }
            ],
            "iudx:rangeIncludes": [
                {
                    "@id": "iudx:Text"
                },
                {
                    "@id": "iudx:ValueDescriptor"
                }
            ],
            "skos:exactMatch": {
                "@id": "GTFS: schedule_relationship"
            }
        },
        {
            "@id": "iudx:schemeID",
            "@type": [
                "iudx:TextProperty"
            ],
            "rdfs:comment": "The unique ID representing the scheme corresponding to this observation.",
            "rdfs:label": "schemeID",
            "rdfs:isDefinedBy": {
                "@id": "iudx:"
            },
            "iudx:domainIncludes": [
                {
                    "@id": "iudx:PublicSchemes"
                }
            ],
            "iudx:rangeIncludes": [
                {
                    "@id": "iudx:Text"
                },
                {
                    "@id": "iudx:ValueDescriptor"
                }
            ]
        },
        {
            "@id": "iudx:schemeName",
            "@type": [
                "iudx:TextProperty"
            ],
            "rdfs:comment": "The name of the scheme or programme introduced by the government for public welfare and development.",
            "rdfs:label": "schemeName",
            "rdfs:isDefinedBy": {
                "@id": "iudx:"
            },
            "iudx:domainIncludes": [
                {
                    "@id": "iudx:PublicSchemes"
                }
            ],
            "iudx:rangeIncludes": [
                {
                    "@id": "iudx:Text"
                },
                {
                    "@id": "iudx:ValueDescriptor"
                }
            ]
        },
        {
            "@id": "iudx:seatingCapacity",
            "@type": [
                "iudx:QuantitativeProperty"
            ],
            "rdfs:comment": "Describes the passenger seating capacity of the vehicle corresponding to this observation.",
            "rdfs:label": "seatingCapacity",
            "rdfs:isDefinedBy": {
                "@id": "iudx:"
            },
            "iudx:domainIncludes": [
                {
                    "@id": "iudx:TransitManagement"
                }
            ],
            "iudx:rangeIncludes": [
                {
                    "@id": "iudx:Number"
                },
                {
                    "@id": "iudx:ValueDescriptor"
                }
            ]
        },
        {
            "@id": "iudx:serviceCompany",
            "@type": [
                "iudx:TextProperty"
            ],
            "rdfs:comment": "Service agency or company corresponding to this observation",
            "rdfs:label": "serviceCompany",
            "rdfs:isDefinedBy": {
                "@id": "iudx:"
            },
            "iudx:domainIncludes": [
                {
                    "@id": "iudx:EmployeeDetails"
                }
            ],
            "iudx:rangeIncludes": [
                {
                    "@id": "iudx:Text"
                },
                {
                    "@id": "iudx:ValueDescriptor"
                }
            ]
        },
        {
            "@id": "iudx:serviceOnDuty",
            "@type": [
                "iudx:TextProperty"
            ],
            "rdfs:comment": "Nature of service provided by emergency vehicle corresponding to this observation. ENUM: [YES, NO]. YES indicates the emergency vehicle corresponding to this observation is attending to/ servicing to an emergency call of duty and is NO otherwise.",
            "rdfs:label": "serviceOnDuty",
            "rdfs:isDefinedBy": {
                "@id": "iudx:"
            },
            "iudx:domainIncludes": [
                {
                    "@id": "iudx:EmergencyVehicle"
                }
            ],
            "iudx:rangeIncludes": [
                {
                    "@id": "iudx:Text"
                },
                {
                    "@id": "iudx:ValueDescriptor"
                }
            ]
        },
        {
            "@id": "iudx:setPointTemperature",
            "@type": [
                "iudx:QuantitativeProperty"
            ],
            "rdfs:comment": "The setpoint temperature of the air conditioning system.",
            "rdfs:label": "setPointTemperature",
            "rdfs:isDefinedBy": {
                "@id": "iudx:"
            },
            "iudx:domainIncludes": [
                {
                    "@id": "iudx:AirConditioner"
                }
            ],
            "iudx:rangeIncludes": [
                {
                    "@id": "iudx:Number"
                },
                {
                    "@id": "iudx:ValueDescriptor"
                }
            ]
        },
        {
            "@id": "iudx:shape_area",
            "@type": [
                "iudx:QuantitativeProperty"
            ],
            "rdfs:comment": "The total area enclosed within the polygon or by the boundary lining the shape of entity corresponding to this observation.",
            "rdfs:label": "shape_area",
            "iudx:domainIncludes": [
                {
                    "@id": "iudx:District"
                },
                {
                    "@id": "iudx:States"
                },
                {
                    "@id": "iudx:FeaturesOfInterest"
                }
            ],
            "iudx:rangeIncludes": [
                {
                    "@id": "iudx:Number"
                },
                {
                    "@id": "iudx:ValueDescriptor"
                }
            ],
            "rdfs:isDefinedBy": {
                "@id": "iudx:"
            }
        },
        {
            "@id": "iudx:shape_dist_traveled",
            "@type": [
                "iudx:QuantitativeProperty"
            ],
            "rdfs:comment": "Actual distance traveled along the shape from the first shape point to the point specified in this record. Used by trip planners to show the correct portion of the shape on a map. Values must increase along with shape_pt_sequence; they cannot be used to show reverse travel along a route. Distance units must be consistent with those used in stop_times.txt.\n\nExample: If a bus travels along the three points defined above for A_shp, the additional shape_dist_traveled values (shown here in kilometers) would look like this:\nshape_id,shape_pt_lat,shape_pt_lon,shape_pt_sequence,shape_dist_traveled\nA_shp,37.61956,-122.48161,0,0\nA_shp,37.64430,-122.41070,6,6.8310\nA_shp,37.65863,-122.30839,11,15.8765",
            "rdfs:label": "shape_dist_traveled",
            "rdfs:isDefinedBy": {
                "@id": "iudx:"
            },
            "iudx:domainIncludes": [
                {
                    "@id": "iudx:ShapesDesc"
                }
            ],
            "iudx:rangeIncludes": [
                {
                    "@id": "iudx:Number"
                },
                {
                    "@id": "iudx:ValueDescriptor"
                }
            ],
            "skos:exactMatch": {
                "@id": "GTFS: shape_dist_traveled"
            }
        },
        {
            "@id": "iudx:shape_id",
            "@type": [
                "iudx:TextProperty"
            ],
            "rdfs:comment": "Identifies a shape.",
            "rdfs:label": "shape_id",
            "rdfs:isDefinedBy": {
                "@id": "iudx:"
            },
            "iudx:domainIncludes": [
                {
                    "@id": "iudx:ShapesDesc"
                }
            ],
            "iudx:rangeIncludes": [
                {
                    "@id": "iudx:Text"
                },
                {
                    "@id": "iudx:ValueDescriptor"
                }
            ],
            "skos:exactMatch": {
                "@id": "GTFS: shape_id"
            }
        },
        {
            "@id": "iudx:shape_length",
            "@type": [
                "iudx:QuantitativeProperty"
            ],
            "rdfs:comment": "The total length of the boundary lining the shape of entity corresponding to this observation.",
            "rdfs:label": "shape_length",
            "iudx:domainIncludes": [
                {
                    "@id": "iudx:District"
                },
                {
                    "@id": "iudx:States"
                },
                {
                    "@id": "iudx:FeaturesOfInterest"
                }
            ],
            "iudx:rangeIncludes": [
                {
                    "@id": "iudx:Number"
                },
                {
                    "@id": "iudx:ValueDescriptor"
                }
            ],
            "rdfs:isDefinedBy": {
                "@id": "iudx:"
            }
        },
        {
            "@id": "iudx:shape_pt_sequence",
            "@type": [
                "iudx:QuantitativeProperty"
            ],
            "rdfs:comment": "Sequence in which the shape points connect to form the shape. Values must increase along the trip but do not need to be consecutive.\n\nExample: If the shape \"A_shp\" has three points in its definition, the shapes.txt file might contain these records to define the shape:\nshape_id,shape_pt_lat,shape_pt_lon,shape_pt_sequence\nA_shp,37.61956,-122.48161,0\nA_shp,37.64430,-122.41070,6\nA_shp,37.65863,-122.30839,11",
            "rdfs:label": "shape_pt_sequence",
            "rdfs:isDefinedBy": {
                "@id": "iudx:"
            },
            "iudx:domainIncludes": [
                {
                    "@id": "iudx:ShapesDesc"
                }
            ],
            "iudx:rangeIncludes": [
                {
                    "@id": "iudx:Number"
                },
                {
                    "@id": "iudx:ValueDescriptor"
                }
            ],
            "skos:exactMatch": {
                "@id": "GTFS: shape_pt_sequence"
            }
        },
        {
            "@id": "iudx:shiftOfOperation",
            "@type": [
                "iudx:TextProperty"
            ],
            "rdfs:comment": "Shift of operation of the public transit vehicle operated by the fare collection agency/ public transit agency or the employee corresponding to this observation. Indiacted as '1' when the vehicle operates in the first shift, '2' when the vehicle operates in the second shift and '3' when the vehilce operates in the third shift.",
            "rdfs:label": "shiftOfOperation",
            "rdfs:isDefinedBy": {
                "@id": "iudx:"
            },
            "iudx:domainIncludes": [
                {
                    "@id": "iudx:FareCollectionSystem"
                },
                {
                    "@id": "iudx:EmployeeDetails"
                }
            ],
            "iudx:rangeIncludes": [
                {
                    "@id": "iudx:Text"
                },
                {
                    "@id": "iudx:ValueDescriptor"
                }
            ]
        },
        {
            "@id": "iudx:siteCode",
            "@type": [
                "iudx:TextProperty"
            ],
            "rdfs:comment": "Unique ID of the public site or tourist destination.",
            "rdfs:label": "siteCode",
            "rdfs:isDefinedBy": {
                "@id": "iudx:"
            },
            "iudx:domainIncludes": [
                {
                    "@id": "iudx:TouristDestination"
                }
            ],
            "iudx:rangeIncludes": [
                {
                    "@id": "iudx:Text"
                },
                {
                    "@id": "iudx:ValueDescriptor"
                }
            ]
        },
        {
            "@id": "iudx:siteDescription",
            "@type": [
                "iudx:TextProperty"
            ],
            "rdfs:comment": "The detailed description about a public site or tourist destination corresponding to this observation.",
            "rdfs:label": "siteDescription",
            "rdfs:isDefinedBy": {
                "@id": "iudx:"
            },
            "iudx:domainIncludes": [
                {
                    "@id": "iudx:TouristDestination"
                }
            ],
            "iudx:rangeIncludes": [
                {
                    "@id": "iudx:Text"
                },
                {
                    "@id": "iudx:ValueDescriptor"
                }
            ]
        },
        {
            "@id": "iudx:siteName",
            "@type": [
                "iudx:TextProperty"
            ],
            "rdfs:comment": "Name of the public site or tourist destination.",
            "rdfs:label": "siteName",
            "rdfs:isDefinedBy": {
                "@id": "iudx:"
            },
            "iudx:domainIncludes": [
                {
                    "@id": "iudx:TouristDestination"
                }
            ],
            "iudx:rangeIncludes": [
                {
                    "@id": "iudx:Text"
                },
                {
                    "@id": "iudx:ValueDescriptor"
                }
            ]
        },
        {
            "@id": "iudx:slogan",
            "@type": [
                "iudx:TextProperty"
            ],
            "rdfs:comment": "A slogan or motto associated with the public site or tourist destination.",
            "rdfs:label": "slogan",
            "rdfs:isDefinedBy": {
                "@id": "iudx:"
            },
            "iudx:domainIncludes": [
                {
                    "@id": "iudx:TouristDestination"
                }
            ],
            "iudx:rangeIncludes": [
                {
                    "@id": "iudx:Text"
                },
                {
                    "@id": "iudx:ValueDescriptor"
                }
            ],
            "skos:exactMatch": {
                "@id": "schema:slogan"
            }
        },
        {
            "@id": "iudx:sludgeLevel",
            "@type": [
                "iudx:QuantitativeProperty"
            ],
            "rdfs:comment": "Level of Sludge measured in the waste-water treatment plant's tank or the manhole sensor corresponding to this observation.",
            "rdfs:label": "sludgeLevel",
            "rdfs:isDefinedBy": {
                "@id": "iudx:"
            },
            "iudx:domainIncludes": [
                {
                    "@id": "iudx:WasteWaterMgmt"
                }
            ],
            "iudx:rangeIncludes": [
                {
                    "@id": "iudx:Number"
                },
                {
                    "@id": "iudx:Text"
                },
                {
                    "@id": "iudx:ValueDescriptor"
                }
            ],
            "skos:exactMatch": {
                "@id": "fiware:sludgeLevel"
            }
        },
        {
            "@id": "iudx:socketType",
            "@type": [
                "iudx:TextProperty"
            ],
            "rdfs:comment": "The type of charging socket offered by the EV charging station.",
            "rdfs:label": "socketType",
            "rdfs:isDefinedBy": {
                "@id": "iudx:"
            },
            "iudx:domainIncludes": [
                {
                    "@id": "iudx:EVChargingStation"
                }
            ],
            "iudx:rangeIncludes": [
                {
                    "@id": "iudx:Text"
                },
                {
                    "@id": "iudx:ValueDescriptor"
                }
            ]
        },
        {
            "@id": "iudx:solarRadiation",
            "@type": [
                "iudx:QuantitativeProperty"
            ],
            "rdfs:comment": "The number of photons that are being emitted by the sun.",
            "rdfs:label": "solarRadiation",
            "iudx:domainIncludes": [
                {
                    "@id": "iudx:EnvWeather"
                },
                {
                    "@id": "iudx:EnvAQM"
                },
                {
                    "@id": "iudx:SolarEnergy"
                },
                {
                    "@id": "iudx:AirQuality"
                }
            ],
            "iudx:rangeIncludes": [
                {
                    "@id": "iudx:Number"
                },
                {
                    "@id": "iudx:ValueDescriptor"
                }
            ],
            "rdfs:isDefinedBy": {
                "@id": "iudx:"
            },
            "skos:exactMatch": {
                "@id": "Fiware:solarRadiation"
            }
        },
        {
            "@id": "iudx:sourceWeightCollected",
            "@type": [
                "iudx:QuantitativeProperty"
            ],
            "rdfs:comment": "The weight of the entity at source location.",
            "rdfs:label": "sourceWeightCollected",
            "rdfs:isDefinedBy": {
                "@id": "iudx:"
            },
            "iudx:domainIncludes": [
                {
                    "@id": "iudx:WmgmtVehicle"
                }
            ],
            "iudx:rangeIncludes": [
                {
                    "@id": "iudx:Number"
                },
                {
                    "@id": "iudx:ValueDescriptor"
                }
            ]
        },
        {
            "@id": "iudx:specialRestrictions",
            "@type": [
                "iudx:TextProperty"
            ],
            "rdfs:comment": "The restrictions or considerations at the premises to maintain the sanctity and tradition.",
            "rdfs:label": "specialRestrictions",
            "rdfs:isDefinedBy": {
                "@id": "iudx:"
            },
            "iudx:domainIncludes": [
                {
                    "@id": "iudx:TouristDestination"
                }
            ],
            "iudx:rangeIncludes": [
                {
                    "@id": "iudx:Text"
                },
                {
                    "@id": "iudx:ValueDescriptor"
                }
            ],
            "skos:exactMatch": {
                "@id": "Fiware:specialRestrictions"
            }
        },
        {
            "@id": "iudx:speciesName",
            "@type": [
                "iudx:TextProperty"
            ],
            "rdfs:comment": "The binomial/ zoological nomenclature of the species as identified by the device.",
            "rdfs:label": "speciesName",
            "rdfs:isDefinedBy": {
                "@id": "iudx:"
            },
            "iudx:domainIncludes": [
                {
                    "@id": "iudx:MosquitoDensity"
                }
            ],
            "iudx:rangeIncludes": [
                {
                    "@id": "iudx:Text"
                },
                {
                    "@id": "iudx:ValueDescriptor"
                }
            ]
        },
        {
            "@id": "iudx:speciesTotal",
            "@type": [
                "iudx:QuantitativeProperty"
            ],
            "rdfs:comment": "The total count of a particular species detected by the device.",
            "rdfs:label": "speciesTotal",
            "rdfs:isDefinedBy": {
                "@id": "iudx:"
            },
            "iudx:domainIncludes": [
                {
                    "@id": "iudx:MosquitoDensity"
                }
            ],
            "iudx:rangeIncludes": [
                {
                    "@id": "iudx:Number"
                },
                {
                    "@id": "iudx:ValueDescriptor"
                }
            ]
        },
        {
            "@id": "iudx:speed",
            "@type": [
                "iudx:QuantitativeProperty"
            ],
            "rdfs:comment": "Momentary speed measured by the vehicle.",
            "rdfs:label": "speed",
            "rdfs:isDefinedBy": {
                "@id": "iudx:"
            },
            "iudx:domainIncludes": [
                {
                    "@id": "iudx:Position"
                },
                {
                    "@id": "iudx:WmgmtVehicle"
                },
                {
                    "@id": "iudx:EmergencyVehicle"
                }
            ],
            "iudx:rangeIncludes": [
                {
                    "@id": "iudx:Number"
                },
                {
                    "@id": "iudx:ValueDescriptor"
                }
            ],
            "skos:exactMatch": {
                "@id": "GTFS: speed"
            }
        },
        {
            "@id": "iudx:stage",
            "@type": [
                "iudx:QuantitativeProperty"
            ],
            "rdfs:comment": "Total number of stages from the origin bus stop to the destination bus stop.",
            "rdfs:label": "stage",
            "rdfs:isDefinedBy": {
                "@id": "iudx:"
            },
            "iudx:domainIncludes": [
                {
                    "@id": "iudx:FareCollectionSystem"
                }
            ],
            "iudx:rangeIncludes": [
                {
                    "@id": "iudx:Number"
                },
                {
                    "@id": "iudx:ValueDescriptor"
                }
            ]
        },
        {
            "@id": "iudx:standingCapacity",
            "@type": [
                "iudx:QuantitativeProperty"
            ],
            "rdfs:comment": "Describes the passenger standing capacity of the vehicle corresponding to this observation.",
            "rdfs:label": "standingCapacity",
            "rdfs:isDefinedBy": {
                "@id": "iudx:"
            },
            "iudx:domainIncludes": [
                {
                    "@id": "iudx:TransitManagement"
                }
            ],
            "iudx:rangeIncludes": [
                {
                    "@id": "iudx:Number"
                },
                {
                    "@id": "iudx:ValueDescriptor"
                }
            ]
        },
        {
            "@id": "iudx:startDateTime",
            "@type": [
                "iudx:TimeProperty"
            ],
            "rdfs:comment": "Reported start time corresponding to this observation.",
            "rdfs:label": "startDateTime",
            "rdfs:isDefinedBy": {
                "@id": "iudx:"
            },
            "iudx:domainIncludes": [
                {
                    "@id": "iudx:Version"
                },
                {
                    "@id": "iudx:Camera"
                },
                {
                    "@id": "iudx:EVChargingStation"
                },
                {
                    "@id": "iudx:BikeDockingStation"
                }
            ],
            "iudx:rangeIncludes": [
                {
                    "@id": "iudx:DateTime"
                },
                {
                    "@id": "iudx:ValueDescriptor"
                }
            ]
        },
        {
            "@id": "iudx:startStopStatus",
            "@type": [
                "iudx:QuantitativeProperty"
            ],
            "rdfs:comment": "Describes the start and stop status of the air conditioning system by a binary Input (0-Inactive, 1-Active)",
            "rdfs:label": "startStopStatus",
            "rdfs:isDefinedBy": {
                "@id": "iudx:"
            },
            "iudx:domainIncludes": [
                {
                    "@id": "iudx:AirConditioner"
                }
            ],
            "iudx:rangeIncludes": [
                {
                    "@id": "iudx:Number"
                },
                {
                    "@id": "iudx:ValueDescriptor"
                }
            ]
        },
        {
            "@id": "iudx:start_date",
            "@type": [
                "iudx:TextProperty"
            ],
            "rdfs:comment": "Describes the initial scheduled date of the trip corresponding to the vehicle this observation. An example format for this field - YYYYMMDD. SameAs: 'start_date' field from GTFS Realtime message-TripDescriptor (https://developers.google.com/transit/gtfs-realtime/reference#message-tripdescriptor)",
            "rdfs:label": "start_date",
            "rdfs:isDefinedBy": {
                "@id": "iudx:"
            },
            "iudx:domainIncludes": [
                {
                    "@id": "iudx:TripDescriptor"
                }
            ],
            "iudx:rangeIncludes": [
                {
                    "@id": "iudx:Text"
                },
                {
                    "@id": "iudx:ValueDescriptor"
                }
            ],
            "skos:exactMatch": {
                "@id": "GTFS: start_date"
            }
        },
        {
            "@id": "iudx:start_time",
            "@type": [
                "iudx:TimeProperty"
            ],
            "rdfs:comment": "Describes the initial scheduled start time of the trip corresponding to the vehicle this observation. An example format for this field - 11:15:35 or 25:15:35. SameAs: 'start_time' field from GTFS Realtime message-TripDescriptor (https://developers.google.com/transit/gtfs-realtime/reference#message-tripdescriptor)",
            "rdfs:label": "start_time",
            "rdfs:isDefinedBy": {
                "@id": "iudx:"
            },
            "iudx:domainIncludes": [
                {
                    "@id": "iudx:TripDescriptor"
                }
            ],
            "iudx:rangeIncludes": [
                {
                    "@id": "iudx:Text"
                },
                {
                    "@id": "iudx:ValueDescriptor"
                }
            ],
            "skos:exactMatch": {
                "@id": "GTFS: start_time"
            }
        },
        {
            "@id": "iudx:state",
            "@type": [
                "iudx:TextProperty"
            ],
            "rdfs:comment": "Name of the state corresponding to this observation.",
            "rdfs:label": "state",
            "iudx:domainIncludes": [
                {
                    "@id": "iudx:Headquarters"
                },
                {
                    "@id": "iudx:District"
                },
                {
                    "@id": "iudx:States"
                }
            ],
            "iudx:rangeIncludes": [
                {
                    "@id": "iudx:Text"
                },
                {
                    "@id": "iudx:ValueDescriptor"
                }
            ],
            "rdfs:isDefinedBy": {
                "@id": "iudx:"
            }
        },
        {
            "@id": "iudx:stateName",
            "@type": [
                "iudx:TextProperty"
            ],
            "rdfs:comment": "Name of the state corresponding to this observation.",
            "rdfs:label": "stateName",
            "rdfs:isDefinedBy": {
                "@id": "iudx:"
            },
            "iudx:domainIncludes": [
                {
                    "@id": "iudx:MunicipalityDesc"
                }
            ],
            "iudx:rangeIncludes": [
                {
                    "@id": "iudx:Text"
                },
                {
                    "@id": "iudx:ValueDescriptor"
                }
            ]
        },
        {
            "@id": "iudx:state_lgd",
            "@type": [
                "iudx:QuantitativeProperty"
            ],
            "rdfs:comment": "The state legend corresponding to this observation",
            "rdfs:label": "state_lgd",
            "iudx:domainIncludes": [
                {
                    "@id": "iudx:District"
                },
                {
                    "@id": "iudx:States"
                }
            ],
            "iudx:rangeIncludes": [
                {
                    "@id": "iudx:Number"
                },
                {
                    "@id": "iudx:ValueDescriptor"
                }
            ],
            "rdfs:isDefinedBy": {
                "@id": "iudx:"
            }
        },
        {
            "@id": "iudx:stationCode",
            "@type": [
                "iudx:TextProperty"
            ],
            "rdfs:comment": "The station number or station code of the bike hire docking station corresponding to the observation.",
            "rdfs:label": "stationCode",
            "rdfs:isDefinedBy": {
                "@id": "iudx:"
            },
            "iudx:domainIncludes": [
                {
                    "@id": "iudx:BikeDockingStation"
                }
            ],
            "iudx:rangeIncludes": [
                {
                    "@id": "iudx:Text"
                },
                {
                    "@id": "iudx:ValueDescriptor"
                }
            ]
        },
        {
            "@id": "iudx:stationName",
            "@type": [
                "iudx:TextProperty"
            ],
            "rdfs:comment": "The name station corresponding to this observation. It can be the name of bike docking station, charging station, etc.",
            "rdfs:label": "stationName",
            "rdfs:isDefinedBy": {
                "@id": "iudx:"
            },
            "iudx:domainIncludes": [
                {
                    "@id": "iudx:BikeDockingStation"
                },
                {
                    "@id": "iudx:EVChargingStation"
                }
            ],
            "iudx:rangeIncludes": [
                {
                    "@id": "iudx:Text"
                },
                {
                    "@id": "iudx:ValueDescriptor"
                }
            ]
        },
        {
            "@id": "iudx:stopScheduleRelationship",
            "@type": [
                "iudx:TextProperty"
            ],
            "rdfs:comment": "Describes the relationship between the static schedule and the stop. SameAs: 'schedule_relationship' field from GTFS Realtime message-StopTimeUpdate ENUM[SCHEDULED, SKIPPED, NO_DATA] (https://developers.google.com/transit/gtfs-realtime/reference#message-stoptimeupdate)",
            "rdfs:label": "stopScheduleRelationship",
            "rdfs:isDefinedBy": {
                "@id": "iudx:"
            },
            "iudx:domainIncludes": [
                {
                    "@id": "iudx:StopTimeUpdate"
                }
            ],
            "iudx:rangeIncludes": [
                {
                    "@id": "iudx:Text"
                },
                {
                    "@id": "iudx:ValueDescriptor"
                }
            ],
            "skos:exactMatch": {
                "@id": "GTFS: schedule_relationship"
            }
        },
        {
            "@id": "iudx:stop_code",
            "@type": [
                "iudx:TextProperty"
            ],
            "rdfs:comment": "This field contains short text or a number that uniquely identifies the stop for passengers. Can be same as stop_id if it is for public. SameAs: 'stop_code' field from GTFS Static Field definitions-stops.txt (https://developers.google.com/transit/gtfs/reference#stopstxt)",
            "rdfs:label": "stop_code",
            "rdfs:isDefinedBy": {
                "@id": "iudx:"
            },
            "iudx:domainIncludes": [
                {
                    "@id": "iudx:StopsDesc"
                }
            ],
            "iudx:rangeIncludes": [
                {
                    "@id": "iudx:Text"
                },
                {
                    "@id": "iudx:ValueDescriptor"
                }
            ],
            "skos:exactMatch": {
                "@id": "GTFS: stop_code"
            }
        },
        {
            "@id": "iudx:stop_desc",
            "@type": [
                "iudx:TextProperty"
            ],
            "rdfs:comment": "This field contains a description of a stop. SameAs: 'stop_desc' field from GTFS Static Field definitions-stops.txt (https://developers.google.com/transit/gtfs/reference#stopstxt)",
            "rdfs:label": "stop_desc",
            "rdfs:isDefinedBy": {
                "@id": "iudx:"
            },
            "iudx:domainIncludes": [
                {
                    "@id": "iudx:StopsDesc"
                }
            ],
            "iudx:rangeIncludes": [
                {
                    "@id": "iudx:Text"
                },
                {
                    "@id": "iudx:ValueDescriptor"
                }
            ],
            "skos:exactMatch": {
                "@id": "GTFS: stop_desc"
            }
        },
        {
            "@id": "iudx:stop_headsign",
            "@type": [
                "iudx:TextProperty"
            ],
            "rdfs:comment": "This field contains the text that appears on a sign that identifies the trip\u2019s destination to passengers. SameAs: 'stop_headsign' field from GTFS Static Field definitions-stop_times.txt (https://developers.google.com/transit/gtfs/reference#stop_timestxt)",
            "rdfs:label": "stop_headsign",
            "rdfs:isDefinedBy": {
                "@id": "iudx:"
            },
            "iudx:domainIncludes": [
                {
                    "@id": "iudx:StopTimesDesc"
                }
            ],
            "iudx:rangeIncludes": [
                {
                    "@id": "iudx:Text"
                },
                {
                    "@id": "iudx:ValueDescriptor"
                }
            ],
            "skos:exactMatch": {
                "@id": "GTFS: stop_headsign"
            }
        },
        {
            "@id": "iudx:stop_id",
            "@type": [
                "iudx:TextProperty"
            ],
            "rdfs:comment": "Unique ID assigned to the stop corresponding to this observation.",
            "rdfs:label": "stop_id",
            "rdfs:isDefinedBy": {
                "@id": "iudx:"
            },
            "iudx:domainIncludes": [
                {
                    "@id": "iudx:GtfsCommons"
                },
                {
                    "@id": "iudx:VehiclePosition"
                },
                {
                    "@id": "iudx:StopTimeUpdate"
                },
                {
                    "@id": "iudx:StopsDesc"
                },
                {
                    "@id": "iudx:StopTimesDesc"
                }
            ],
            "iudx:rangeIncludes": [
                {
                    "@id": "iudx:Text"
                },
                {
                    "@id": "iudx:ValueDescriptor"
                }
            ],
            "skos:exactMatch": {
                "@id": "GTFS: stop_id"
            }
        },
        {
            "@id": "iudx:stop_name",
            "@type": [
                "iudx:TextProperty"
            ],
            "rdfs:comment": "Describes the name of a stop or station. SameAs: 'stop_name' field from GTFS Static Field definitions-stops.txt (https://developers.google.com/transit/gtfs/reference#stopstxt)",
            "rdfs:label": "stop_name",
            "rdfs:isDefinedBy": {
                "@id": "iudx:"
            },
            "iudx:domainIncludes": [
                {
                    "@id": "iudx:StopsDesc"
                }
            ],
            "iudx:rangeIncludes": [
                {
                    "@id": "iudx:Text"
                },
                {
                    "@id": "iudx:ValueDescriptor"
                }
            ],
            "skos:exactMatch": {
                "@id": "GTFS: stop_name"
            }
        },
        {
            "@id": "iudx:stop_sequence",
            "@type": [
                "iudx:QuantitativeProperty"
            ],
            "rdfs:comment": "This field identifies the order of the stops for a particular trip. The values for stop_sequence must be non-negative integers, and they must increase along the trip. For example, the first stop on the trip could have a stop_sequence of 1, the second stop on the trip could have a stop_sequence of 23, the third stop could have a stop_sequence of 40, and so on.",
            "rdfs:label": "stop_sequence",
            "rdfs:isDefinedBy": {
                "@id": "iudx:"
            },
            "iudx:domainIncludes": [
                {
                    "@id": "iudx:GtfsCommons"
                },
                {
                    "@id": "iudx:StopTimeUpdate"
                },
                {
                    "@id": "iudx:StopTimesDesc"
                }
            ],
            "iudx:rangeIncludes": [
                {
                    "@id": "iudx:Number"
                },
                {
                    "@id": "iudx:ValueDescriptor"
                }
            ],
            "skos:exactMatch": {
                "@id": "GTFS: stop_sequence"
            }
        },
        {
            "@id": "iudx:stop_url",
            "@type": [
                "iudx:TextProperty"
            ],
            "rdfs:comment": "This field contains the URL of a web page about a particular stop and is different from the agency_url and the route_url fields. SameAs: 'stop_url' field from GTFS Static Field definitions-stops.txt (https://developers.google.com/transit/gtfs/reference#stopstxt)",
            "rdfs:label": "stop_url",
            "rdfs:isDefinedBy": {
                "@id": "iudx:"
            },
            "iudx:domainIncludes": [
                {
                    "@id": "iudx:StopsDesc"
                }
            ],
            "iudx:rangeIncludes": [
                {
                    "@id": "iudx:Text"
                },
                {
                    "@id": "iudx:ValueDescriptor"
                }
            ],
            "skos:exactMatch": {
                "@id": "GTFS: stop_url"
            }
        },
        {
            "@id": "iudx:streamName",
            "@type": [
                "iudx:TextProperty"
            ],
            "rdfs:comment": "Name of the video stream from the camera corresponding to this observation",
            "rdfs:label": "streamName",
            "rdfs:isDefinedBy": {
                "@id": "iudx:"
            },
            "iudx:domainIncludes": [
                {
                    "@id": "iudx:Camera"
                }
            ],
            "iudx:rangeIncludes": [
                {
                    "@id": "iudx:Text"
                },
                {
                    "@id": "iudx:ValueDescriptor"
                }
            ]
        },
        {
            "@id": "iudx:streamURL",
            "@type": [
                "iudx:TextProperty"
            ],
            "rdfs:comment": "URL providing video streaming information for the camera corresponding to this observation",
            "rdfs:label": "streamURL",
            "rdfs:isDefinedBy": {
                "@id": "iudx:"
            },
            "iudx:domainIncludes": [
                {
                    "@id": "iudx:Camera"
                }
            ],
            "iudx:rangeIncludes": [
                {
                    "@id": "iudx:Text"
                },
                {
                    "@id": "iudx:ValueDescriptor"
                }
            ]
        },
        {
            "@id": "iudx:streetPoleNum",
            "@type": [
                "iudx:TextProperty"
            ],
            "rdfs:comment": "Street pole information associated with the streetlight corresponding to this observation.",
            "rdfs:label": "streetPoleNum",
            "rdfs:isDefinedBy": {
                "@id": "iudx:"
            },
            "iudx:domainIncludes": [
                {
                    "@id": "iudx:Streetlight"
                }
            ],
            "iudx:rangeIncludes": [
                {
                    "@id": "iudx:Text"
                },
                {
                    "@id": "iudx:ValueDescriptor"
                }
            ]
        },
        {
            "@id": "iudx:subCategory",
            "@type": [
                "iudx:TextProperty"
            ],
            "rdfs:comment": "The sub-category name corresponding to the issue that has been reported.",
            "rdfs:label": "subCategory",
            "rdfs:isDefinedBy": {
                "@id": "iudx:"
            },
            "iudx:domainIncludes": [
                {
                    "@id": "iudx:IssueReporting"
                }
            ],
            "iudx:rangeIncludes": [
                {
                    "@id": "iudx:Text"
                },
                {
                    "@id": "iudx:ValueDescriptor"
                }
            ]
        },
        {
            "@id": "iudx:subCategoryCode",
            "@type": [
                "iudx:TextProperty"
            ],
            "rdfs:comment": "Unique identifier for the sub-category corresponding to the issue reported.",
            "rdfs:label": "subCategoryCode",
            "rdfs:isDefinedBy": {
                "@id": "iudx:"
            },
            "iudx:domainIncludes": [
                {
                    "@id": "iudx:IssueReporting"
                }
            ],
            "iudx:rangeIncludes": [
                {
                    "@id": "iudx:Text"
                },
                {
                    "@id": "iudx:ValueDescriptor"
                }
            ]
        },
        {
            "@id": "iudx:subdistrict",
            "@type": [
                "iudx:TextProperty"
            ],
            "rdfs:comment": "Name of the subdistrict corresponding to this observation.",
            "rdfs:label": "subdistrict",
            "rdfs:isDefinedBy": {
                "@id": "iudx:"
            },
            "iudx:domainIncludes": [
                {
                    "@id": "iudx:District"
                }
            ],
            "iudx:rangeIncludes": [
                {
                    "@id": "iudx:Text"
                },
                {
                    "@id": "iudx:ValueDescriptor"
                }
            ]
        },
        {
            "@id": "iudx:taluk",
            "@type": [
                "iudx:TextProperty"
            ],
            "rdfs:comment": "Name of the taluk corresponding to this observation.",
            "rdfs:label": "taluk",
            "rdfs:isDefinedBy": {
                "@id": "iudx:"
            },
            "iudx:domainIncludes": [
                {
                    "@id": "iudx:Headquarters"
                }
            ],
            "iudx:rangeIncludes": [
                {
                    "@id": "iudx:Text"
                },
                {
                    "@id": "iudx:ValueDescriptor"
                }
            ]
        },
        {
            "@id": "iudx:tankBreadth",
            "@type": [
                "iudx:QuantitativeProperty"
            ],
            "rdfs:comment": "Breadth of the Cuboid shaped water storage tank.",
            "rdfs:label": "tankBreadth",
            "rdfs:isDefinedBy": {
                "@id": "iudx:"
            },
            "iudx:domainIncludes": [
                {
                    "@id": "iudx:WaterDistributionNetwork"
                }
            ],
            "iudx:rangeIncludes": [
                {
                    "@id": "iudx:Number"
                },
                {
                    "@id": "iudx:ValueDescriptor"
                }
            ]
        },
        {
            "@id": "iudx:tankCapacity",
            "@type": [
                "iudx:QuantitativeProperty"
            ],
            "rdfs:comment": "Maximum amount of water the water storage tank corresponding to this observation can hold.",
            "rdfs:label": "tankCapacity",
            "rdfs:isDefinedBy": {
                "@id": "iudx:"
            },
            "iudx:domainIncludes": [
                {
                    "@id": "iudx:WaterDistributionNetwork"
                }
            ],
            "iudx:rangeIncludes": [
                {
                    "@id": "iudx:Number"
                },
                {
                    "@id": "iudx:ValueDescriptor"
                }
            ]
        },
        {
            "@id": "iudx:tankDepth",
            "@type": [
                "iudx:QuantitativeProperty"
            ],
            "rdfs:comment": "Depth of the water storage tank corresponding to this observation.",
            "rdfs:label": "tankDepth",
            "rdfs:isDefinedBy": {
                "@id": "iudx:"
            },
            "iudx:domainIncludes": [
                {
                    "@id": "iudx:WaterDistributionNetwork"
                }
            ],
            "iudx:rangeIncludes": [
                {
                    "@id": "iudx:Number"
                },
                {
                    "@id": "iudx:ValueDescriptor"
                }
            ]
        },
        {
            "@id": "iudx:tankDiameter",
            "@type": [
                "iudx:QuantitativeProperty"
            ],
            "rdfs:comment": "Diameter of Cylindrical or Spherical water storage tanks.",
            "rdfs:label": "tankDiameter",
            "rdfs:isDefinedBy": {
                "@id": "iudx:"
            },
            "iudx:domainIncludes": [
                {
                    "@id": "iudx:WaterDistributionNetwork"
                }
            ],
            "iudx:rangeIncludes": [
                {
                    "@id": "iudx:Number"
                },
                {
                    "@id": "iudx:ValueDescriptor"
                }
            ]
        },
        {
            "@id": "iudx:tankLength",
            "@type": [
                "iudx:QuantitativeProperty"
            ],
            "rdfs:comment": "Length of the Cuboid shaped water storage tank.",
            "rdfs:label": "tankLength",
            "rdfs:isDefinedBy": {
                "@id": "iudx:"
            },
            "iudx:domainIncludes": [
                {
                    "@id": "iudx:WaterDistributionNetwork"
                }
            ],
            "iudx:rangeIncludes": [
                {
                    "@id": "iudx:Number"
                },
                {
                    "@id": "iudx:ValueDescriptor"
                }
            ]
        },
        {
            "@id": "iudx:tankName",
            "@type": [
                "iudx:TextProperty"
            ],
            "rdfs:comment": "Name of the water storage tank corresponding to this observation.",
            "rdfs:label": "tankName",
            "rdfs:isDefinedBy": {
                "@id": "iudx:"
            },
            "iudx:domainIncludes": [
                {
                    "@id": "iudx:WaterDistributionNetwork"
                }
            ],
            "iudx:rangeIncludes": [
                {
                    "@id": "iudx:Text"
                },
                {
                    "@id": "iudx:ValueDescriptor"
                }
            ]
        },
        {
            "@id": "iudx:tankShape",
            "@type": [
                "iudx:TextProperty"
            ],
            "rdfs:comment": "Physical shape of the water storage tank corresponding to this observation. ENUM: [Cylindrical, Conical, Cuboid, Spherical]",
            "rdfs:label": "tankShape",
            "rdfs:isDefinedBy": {
                "@id": "iudx:"
            },
            "iudx:domainIncludes": [
                {
                    "@id": "iudx:WaterDistributionNetwork"
                }
            ],
            "iudx:rangeIncludes": [
                {
                    "@id": "iudx:Text"
                },
                {
                    "@id": "iudx:ValueDescriptor"
                }
            ]
        },
        {
            "@id": "iudx:taxAmountCollected",
            "@type": [
                "iudx:QuantitativeProperty"
            ],
            "rdfs:comment": "The amount of tax levied on the products, things and services which includes sales tax, value-added tax, service tax, Good and Service tax, customs duty, etc.",
            "rdfs:label": "taxAmountCollected",
            "rdfs:isDefinedBy": {
                "@id": "iudx:"
            },
            "iudx:domainIncludes": [
                {
                    "@id": "iudx:RevenueCollection"
                },
                {
                    "@id": "iudx:EVChargingStation"
                }
            ],
            "iudx:rangeIncludes": [
                {
                    "@id": "iudx:Number"
                },
                {
                    "@id": "iudx:ValueDescriptor"
                }
            ]
        },
        {
            "@id": "iudx:tee",
            "@type": [
                "iudx:QuantitativeProperty"
            ],
            "rdfs:comment": "Total Energy Exported, it is the total energy consumed by the load connected to the device corresponding to this observation.",
            "rdfs:label": "tee",
            "rdfs:isDefinedBy": {
                "@id": "iudx:"
            },
            "iudx:domainIncludes": [
                {
                    "@id": "iudx:SolarEnergy"
                }
            ],
            "iudx:rangeIncludes": [
                {
                    "@id": "iudx:Number"
                },
                {
                    "@id": "iudx:ValueDescriptor"
                }
            ]
        },
        {
            "@id": "iudx:tehsil",
            "@type": [
                "iudx:TextProperty"
            ],
            "rdfs:comment": "Name of the tehsil corresponding to this observation.",
            "rdfs:label": "tehsil",
            "rdfs:isDefinedBy": {
                "@id": "iudx:"
            },
            "iudx:domainIncludes": [
                {
                    "@id": "iudx:District"
                }
            ],
            "iudx:rangeIncludes": [
                {
                    "@id": "iudx:Text"
                },
                {
                    "@id": "iudx:ValueDescriptor"
                }
            ]
        },
        {
            "@id": "iudx:tei",
            "@type": [
                "iudx:QuantitativeProperty"
            ],
            "rdfs:comment": "Total Energy Imported, it is the total energy received by the device corresponding to this observation.",
            "rdfs:label": "tei",
            "rdfs:isDefinedBy": {
                "@id": "iudx:"
            },
            "iudx:domainIncludes": [
                {
                    "@id": "iudx:SolarEnergy"
                }
            ],
            "iudx:rangeIncludes": [
                {
                    "@id": "iudx:Number"
                },
                {
                    "@id": "iudx:ValueDescriptor"
                }
            ]
        },
        {
            "@id": "iudx:thermoStatus",
            "@type": [
                "iudx:QuantitativeProperty"
            ],
            "rdfs:comment": "Describes the thermo status of the air conditioning system by a binary input (0-Inactive, 1-Active)",
            "rdfs:label": "thermoStatus",
            "rdfs:isDefinedBy": {
                "@id": "iudx:"
            },
            "iudx:domainIncludes": [
                {
                    "@id": "iudx:AirConditioner"
                }
            ],
            "iudx:rangeIncludes": [
                {
                    "@id": "iudx:Number"
                },
                {
                    "@id": "iudx:ValueDescriptor"
                }
            ]
        },
        {
            "@id": "iudx:tic",
            "@type": [
                "iudx:QuantitativeProperty"
            ],
            "rdfs:comment": "Total Inorganic Carbon concentration measured in the waste-water treatment plant corresponding to this observation.",
            "rdfs:label": "tic",
            "rdfs:isDefinedBy": {
                "@id": "iudx:"
            },
            "iudx:domainIncludes": [
                {
                    "@id": "iudx:WasteWaterMgmt"
                }
            ],
            "iudx:rangeIncludes": [
                {
                    "@id": "iudx:Number"
                },
                {
                    "@id": "iudx:ValueDescriptor"
                }
            ],
            "skos:exactMatch": {
                "@id": "fiware:tic"
            }
        },
        {
            "@id": "iudx:ticketTypeCode",
            "@type": [
                "iudx:TextProperty"
            ],
            "rdfs:comment": "Unique ticket type code of the corresponding trip.",
            "rdfs:label": "ticketTypeCode",
            "rdfs:isDefinedBy": {
                "@id": "iudx:"
            },
            "iudx:domainIncludes": [
                {
                    "@id": "iudx:FareCollectionSystem"
                }
            ],
            "iudx:rangeIncludes": [
                {
                    "@id": "iudx:Text"
                },
                {
                    "@id": "iudx:ValueDescriptor"
                }
            ]
        },
        {
            "@id": "iudx:title",
            "@type": [
                "iudx:TextProperty"
            ],
            "rdfs:comment": "The title assigned to the issue, report or feedback corresponding to this observation.",
            "rdfs:label": "title",
            "rdfs:isDefinedBy": {
                "@id": "iudx:"
            },
            "iudx:domainIncludes": [
                {
                    "@id": "iudx:IssueReporting"
                }
            ],
            "iudx:rangeIncludes": [
                {
                    "@id": "iudx:Text"
                },
                {
                    "@id": "iudx:ValueDescriptor"
                }
            ],
            "skos:exactMatch": {
                "@id": "open311:description"
            }
        },
        {
            "@id": "iudx:titleCode",
            "@type": [
                "iudx:TextProperty"
            ],
            "rdfs:comment": "The code assigned to the title corresponding to this observation.",
            "rdfs:label": "titleCode",
            "rdfs:isDefinedBy": {
                "@id": "iudx:"
            },
            "iudx:domainIncludes": [
                {
                    "@id": "iudx:IssueReporting"
                },
                {
                    "@id": "iudx:TrafficViolations"
                }
            ],
            "iudx:rangeIncludes": [
                {
                    "@id": "iudx:Text"
                },
                {
                    "@id": "iudx:ValueDescriptor"
                }
            ]
        },
        {
            "@id": "iudx:tn",
            "@type": [
                "iudx:QuantitativeProperty"
            ],
            "rdfs:comment": "Total Nitrogen concentration measured in waste-water treatment plant corresponding to this observation.",
            "rdfs:label": "tn",
            "rdfs:isDefinedBy": {
                "@id": "iudx:"
            },
            "iudx:domainIncludes": [
                {
                    "@id": "iudx:WasteWaterMgmt"
                }
            ],
            "iudx:rangeIncludes": [
                {
                    "@id": "iudx:Number"
                },
                {
                    "@id": "iudx:ValueDescriptor"
                }
            ],
            "skos:exactMatch": {
                "@id": "fiware:tn"
            }
        },
        {
            "@id": "iudx:toc",
            "@type": [
                "iudx:QuantitativeProperty"
            ],
            "rdfs:comment": "Total Organic Carbon concentration measured in the waste-water treatment plant corresponding to this observation.",
            "rdfs:label": "toc",
            "rdfs:isDefinedBy": {
                "@id": "iudx:"
            },
            "iudx:domainIncludes": [
                {
                    "@id": "iudx:WasteWaterMgmt"
                }
            ],
            "iudx:rangeIncludes": [
                {
                    "@id": "iudx:Number"
                },
                {
                    "@id": "iudx:ValueDescriptor"
                }
            ],
            "skos:exactMatch": {
                "@id": "fiware:toc"
            }
        },
        {
            "@id": "iudx:topoSheetNo",
            "@type": [
                "iudx:TextProperty"
            ],
            "rdfs:comment": "The unique number assigned to the toposheet corresponding to this observation.",
            "rdfs:label": "topoSheetNo",
            "rdfs:isDefinedBy": {
                "@id": "iudx:"
            },
            "iudx:domainIncludes": [
                {
                    "@id": "iudx:DigitalElevationModel"
                }
            ],
            "iudx:rangeIncludes": [
                {
                    "@id": "iudx:Text"
                },
                {
                    "@id": "iudx:ValueDescriptor"
                }
            ]
        },
        {
            "@id": "iudx:totalAbsent",
            "@type": [
                "iudx:QuantitativeProperty"
            ],
            "rdfs:comment": "Number of employees failed to report to work",
            "rdfs:label": "totalAbsent",
            "rdfs:isDefinedBy": {
                "@id": "iudx:"
            },
            "iudx:domainIncludes": [
                {
                    "@id": "iudx:EmployeeDetails"
                }
            ],
            "iudx:rangeIncludes": [
                {
                    "@id": "iudx:Number"
                },
                {
                    "@id": "iudx:ValueDescriptor"
                }
            ]
        },
        {
            "@id": "iudx:totalActivePower",
            "@type": [
                "iudx:QuantitativeProperty"
            ],
            "rdfs:comment": "Total active power consumed by all phases.",
            "rdfs:label": "totalActivePower",
            "iudx:domainIncludes": [
                {
                    "@id": "iudx:StreetLightFeeder"
                },
                {
                    "@id": "iudx:SolarEnergy"
                },
                {
                    "@id": "iudx:EnergyMeter"
                },
                {
                    "@id": "iudx:AirConditioner"
                }
            ],
            "iudx:rangeIncludes": [
                {
                    "@id": "iudx:Number"
                },
                {
                    "@id": "iudx:ValueDescriptor"
                }
            ],
            "rdfs:isDefinedBy": {
                "@id": "iudx:"
            },
            "skos:exactMatch": {
                "@id": "Fiware:totalActivePower"
            }
        },
        {
            "@id": "iudx:totalApparentPower",
            "@type": [
                "iudx:QuantitativeProperty"
            ],
            "rdfs:comment": "Total apparent power consumed by all the phases",
            "rdfs:label": "totalApparentPower",
            "rdfs:isDefinedBy": {
                "@id": "iudx:"
            },
            "iudx:domainIncludes": [
                {
                    "@id": "iudx:StreetLightFeeder"
                },
                {
                    "@id": "iudx:SolarEnergy"
                },
                {
                    "@id": "iudx:EnergyMeter"
                }
            ],
            "iudx:rangeIncludes": [
                {
                    "@id": "iudx:Number"
                },
                {
                    "@id": "iudx:ValueDescriptor"
                }
            ],
            "skos:exactMatch": {
                "@id": "Fiware: totalApparentPower"
            }
        },
        {
            "@id": "iudx:totalCount",
            "@type": [
                "iudx:QuantitativeProperty"
            ],
            "rdfs:comment": "The total count of the entity or service corresponding to this observation.",
            "rdfs:label": "totalCount",
            "rdfs:isDefinedBy": {
                "@id": "iudx:"
            },
            "iudx:domainIncludes": [
                {
                    "@id": "iudx:RevenueCollection"
                },
                {
                    "@id": "iudx:RoadSegment"
                }
            ],
            "iudx:rangeIncludes": [
                {
                    "@id": "iudx:Number"
                },
                {
                    "@id": "iudx:ValueDescriptor"
                }
            ]
        },
        {
            "@id": "iudx:totalCyclePathWidth",
            "@type": [
                "iudx:QuantitativeProperty"
            ],
            "rdfs:comment": "Total width of the cycle track present in the road corresponding to this observation.",
            "rdfs:label": "totalCyclePathWidth",
            "rdfs:isDefinedBy": {
                "@id": "iudx:"
            },
            "iudx:domainIncludes": [
                {
                    "@id": "iudx:RoadSegment"
                }
            ],
            "iudx:rangeIncludes": [
                {
                    "@id": "iudx:Number"
                },
                {
                    "@id": "iudx:ValueDescriptor"
                }
            ]
        },
        {
            "@id": "iudx:totalEmployee",
            "@type": [
                "iudx:QuantitativeProperty"
            ],
            "rdfs:comment": "Number of the employees in the organization",
            "rdfs:label": "totalEmployee",
            "rdfs:isDefinedBy": {
                "@id": "iudx:"
            },
            "iudx:domainIncludes": [
                {
                    "@id": "iudx:EmployeeDetails"
                }
            ],
            "iudx:rangeIncludes": [
                {
                    "@id": "iudx:Number"
                },
                {
                    "@id": "iudx:ValueDescriptor"
                }
            ],
            "skos:exactMatch": {
                "@id": "schema:numberOfEmployees"
            }
        },
        {
            "@id": "iudx:totalEnergyGenerated",
            "@type": [
                "iudx:QuantitativeProperty"
            ],
            "rdfs:comment": "Total energy generated by the energy resource corresponding to this observation.",
            "rdfs:label": "totalEnergyGenerated",
            "rdfs:isDefinedBy": {
                "@id": "iudx:"
            },
            "iudx:domainIncludes": [
                {
                    "@id": "iudx:SolarEnergy"
                }
            ],
            "iudx:rangeIncludes": [
                {
                    "@id": "iudx:Number"
                },
                {
                    "@id": "iudx:ValueDescriptor"
                }
            ]
        },
        {
            "@id": "iudx:totalGasPower",
            "@type": [
                "iudx:QuantitativeProperty"
            ],
            "rdfs:comment": "Total amount of gas consumed by the AC accumulator corresponding to this observation.",
            "rdfs:label": "totalGasPower",
            "rdfs:isDefinedBy": {
                "@id": "iudx:"
            },
            "iudx:domainIncludes": [
                {
                    "@id": "iudx:AirConditioner"
                }
            ],
            "iudx:rangeIncludes": [
                {
                    "@id": "iudx:Number"
                },
                {
                    "@id": "iudx:ValueDescriptor"
                }
            ]
        },
        {
            "@id": "iudx:totalLaneNumber",
            "@type": [
                "iudx:QuantitativeProperty"
            ],
            "rdfs:comment": "The total number of lanes the road corresponding to this observation possesses.",
            "rdfs:label": "totalLaneNumber",
            "rdfs:isDefinedBy": {
                "@id": "iudx:"
            },
            "iudx:domainIncludes": [
                {
                    "@id": "iudx:RoadSegment"
                }
            ],
            "iudx:rangeIncludes": [
                {
                    "@id": "iudx:Number"
                },
                {
                    "@id": "iudx:ValueDescriptor"
                }
            ],
            "skos:exactMatch": {
                "@id": "Fiware: totalLaneNumber"
            }
        },
        {
            "@id": "iudx:totalML",
            "@type": [
                "iudx:QuantitativeProperty"
            ],
            "rdfs:comment": "Total MLDs of water discharged from the water storage tank corresponding to this observation.",
            "rdfs:label": "totalML",
            "rdfs:isDefinedBy": {
                "@id": "iudx:"
            },
            "iudx:domainIncludes": [
                {
                    "@id": "iudx:WaterDistributionNetwork"
                }
            ],
            "iudx:rangeIncludes": [
                {
                    "@id": "iudx:Number"
                },
                {
                    "@id": "iudx:ValueDescriptor"
                }
            ]
        },
        {
            "@id": "iudx:totalPOI",
            "@type": [
                "iudx:QuantitativeProperty"
            ],
            "rdfs:comment": "The total count of point of interests (waste collection points) along a route corresponding to this observation .",
            "rdfs:label": "totalPOI",
            "iudx:domainIncludes": [
                {
                    "@id": "iudx:WmgmtVehicle"
                }
            ],
            "iudx:rangeIncludes": [
                {
                    "@id": "iudx:Number"
                },
                {
                    "@id": "iudx:ValueDescriptor"
                }
            ],
            "rdfs:isDefinedBy": {
                "@id": "iudx:"
            }
        },
        {
            "@id": "iudx:totalPedestrianPathLength",
            "@type": [
                "iudx:QuantitativeProperty"
            ],
            "rdfs:comment": "Total length of the walkway present in the road corresponding to this observation.",
            "rdfs:label": "totalPedestrianPathLength",
            "rdfs:isDefinedBy": {
                "@id": "iudx:"
            },
            "iudx:domainIncludes": [
                {
                    "@id": "iudx:RoadSegment"
                }
            ],
            "iudx:rangeIncludes": [
                {
                    "@id": "iudx:Number"
                },
                {
                    "@id": "iudx:ValueDescriptor"
                }
            ]
        },
        {
            "@id": "iudx:totalPedestrianPathWidth",
            "@type": [
                "iudx:QuantitativeProperty"
            ],
            "rdfs:comment": "Total width of the walkway present in the road corresponding to this observation.",
            "rdfs:label": "totalPedestrianPathWidth",
            "rdfs:isDefinedBy": {
                "@id": "iudx:"
            },
            "iudx:domainIncludes": [
                {
                    "@id": "iudx:RoadSegment"
                }
            ],
            "iudx:rangeIncludes": [
                {
                    "@id": "iudx:Number"
                },
                {
                    "@id": "iudx:ValueDescriptor"
                }
            ]
        },
        {
            "@id": "iudx:totalPresent",
            "@type": [
                "iudx:QuantitativeProperty"
            ],
            "rdfs:comment": "Number of employees reported to work",
            "rdfs:label": "totalPresent",
            "rdfs:isDefinedBy": {
                "@id": "iudx:"
            },
            "iudx:domainIncludes": [
                {
                    "@id": "iudx:EmployeeDetails"
                }
            ],
            "iudx:rangeIncludes": [
                {
                    "@id": "iudx:Number"
                },
                {
                    "@id": "iudx:ValueDescriptor"
                }
            ]
        },
        {
            "@id": "iudx:totalReactivePower",
            "@type": [
                "iudx:QuantitativeProperty"
            ],
            "rdfs:comment": "Total reactive power for all phases.",
            "rdfs:label": "totalReactivePower",
            "rdfs:isDefinedBy": {
                "@id": "iudx:"
            },
            "iudx:domainIncludes": [
                {
                    "@id": "iudx:StreetLightFeeder"
                },
                {
                    "@id": "iudx:SolarEnergy"
                }
            ],
            "iudx:rangeIncludes": [
                {
                    "@id": "iudx:Number"
                },
                {
                    "@id": "iudx:ValueDescriptor"
                }
            ],
            "skos:exactMatch": {
                "@id": "Fiware:totalReactivePower"
            }
        },
        {
            "@id": "iudx:totalSlotNumber",
            "@type": [
                "iudx:QuantitativeProperty"
            ],
            "rdfs:comment": "The total number of bike racks/bike-docking slots or parking slots in the bike docking station or the parking site corresponding to this observation.",
            "rdfs:label": "totalSlotNumber",
            "rdfs:isDefinedBy": {
                "@id": "iudx:"
            },
            "iudx:domainIncludes": [
                {
                    "@id": "iudx:BikeDockingStation"
                },
                {
                    "@id": "iudx:SmartParking"
                }
            ],
            "iudx:rangeIncludes": [
                {
                    "@id": "iudx:Number"
                },
                {
                    "@id": "iudx:ValueDescriptor"
                }
            ],
            "skos:exactMatch": {
                "@id": "Fiware:totalSlotNumber"
            }
        },
        {
            "@id": "iudx:totalSpotNumber",
            "@type": [
                "iudx:QuantitativeProperty"
            ],
            "rdfs:comment": "The total number of spots offered by the parking site corresponding to this observation.",
            "rdfs:label": "totalSpotNumber",
            "rdfs:isDefinedBy": {
                "@id": "iudx:"
            },
            "iudx:domainIncludes": [
                {
                    "@id": "iudx:ParkingSpotStatus"
                }
            ],
            "iudx:rangeIncludes": [
                {
                    "@id": "iudx:Number"
                },
                {
                    "@id": "iudx:ValueDescriptor"
                }
            ],
            "skos:exactMatch": {
                "@id": "Fiware: OffStreetParking.totalSpotNumber"
            }
        },
        {
            "@id": "iudx:totalTripCount",
            "@type": [
                "iudx:QuantitativeProperty"
            ],
            "rdfs:comment": "The total count of trips made by the vehicle(s) corresponding to this observation on the given day of operation.",
            "rdfs:label": "totalTripCount",
            "rdfs:isDefinedBy": {
                "@id": "iudx:"
            },
            "iudx:domainIncludes": [
                {
                    "@id": "iudx:BikeDockingStation"
                }
            ],
            "iudx:rangeIncludes": [
                {
                    "@id": "iudx:Number"
                },
                {
                    "@id": "iudx:ValueDescriptor"
                }
            ]
        },
        {
            "@id": "iudx:town",
            "@type": [
                "iudx:TextProperty"
            ],
            "rdfs:comment": "Name of the town corresponding to this observation.",
            "rdfs:label": "town",
            "rdfs:isDefinedBy": {
                "@id": "iudx:"
            },
            "iudx:domainIncludes": [
                {
                    "@id": "iudx:Headquarters"
                }
            ],
            "iudx:rangeIncludes": [
                {
                    "@id": "iudx:Text"
                },
                {
                    "@id": "iudx:ValueDescriptor"
                }
            ]
        },
        {
            "@id": "iudx:tradeName",
            "@type": [
                "iudx:TextProperty"
            ],
            "rdfs:comment": "The official name under which an individual as a sole proprietor or a company chooses to do business.",
            "rdfs:label": "tradeName",
            "rdfs:isDefinedBy": {
                "@id": "iudx:"
            },
            "iudx:domainIncludes": [
                {
                    "@id": "iudx:RevenueCollection"
                }
            ],
            "iudx:rangeIncludes": [
                {
                    "@id": "iudx:Text"
                },
                {
                    "@id": "iudx:ValueDescriptor"
                }
            ]
        },
        {
            "@id": "iudx:transactionDateTime",
            "@type": [
                "iudx:TimeProperty"
            ],
            "rdfs:comment": "Date-time of the transaction corresponding to this observation.",
            "rdfs:label": "transactionDateTime",
            "rdfs:isDefinedBy": {
                "@id": "iudx:"
            },
            "iudx:domainIncludes": [
                {
                    "@id": "iudx:FareCollectionSystem"
                }
            ],
            "iudx:rangeIncludes": [
                {
                    "@id": "iudx:DateTime"
                },
                {
                    "@id": "iudx:ValueDescriptor"
                }
            ]
        },
        {
            "@id": "iudx:transactionID",
            "@type": [
                "iudx:TextProperty"
            ],
            "rdfs:comment": "Unique transaction ID of the entity corresponding to this observation.",
            "rdfs:label": "transactionID",
            "rdfs:isDefinedBy": {
                "@id": "iudx:"
            },
            "iudx:domainIncludes": [
                {
                    "@id": "iudx:FareCollectionSystem"
                },
                {
                    "@id": "iudx:EVChargingStation"
                }
            ],
            "iudx:rangeIncludes": [
                {
                    "@id": "iudx:Text"
                },
                {
                    "@id": "iudx:ValueDescriptor"
                }
            ]
        },
        {
            "@id": "iudx:transactionType",
            "@type": [
                "iudx:TextProperty"
            ],
            "rdfs:comment": "Type of the transaction based on the mode of payment (For eg. mobile/UPI, card, etc) or mode of service (For eg. Issue, ReIssue, Entry, Exit etc.) corresponding to this observation.",
            "rdfs:label": "transactionType",
            "rdfs:isDefinedBy": {
                "@id": "iudx:"
            },
            "iudx:domainIncludes": [
                {
                    "@id": "iudx:FareCollectionSystem"
                },
                {
                    "@id": "iudx:EVChargingStation"
                }
            ],
            "iudx:rangeIncludes": [
                {
                    "@id": "iudx:Text"
                },
                {
                    "@id": "iudx:ValueDescriptor"
                }
            ]
        },
        {
            "@id": "iudx:transactionTypeDescription",
            "@type": [
                "iudx:TextProperty"
            ],
            "rdfs:comment": "Description of the transaction type. Explanation of various transanctionTypeID codes used in the data.",
            "rdfs:label": "transactionTypeDescription",
            "rdfs:isDefinedBy": {
                "@id": "iudx:"
            },
            "iudx:domainIncludes": [
                {
                    "@id": "iudx:FareCollectionSystem"
                }
            ],
            "iudx:rangeIncludes": [
                {
                    "@id": "iudx:Text"
                },
                {
                    "@id": "iudx:ValueDescriptor"
                }
            ]
        },
        {
            "@id": "iudx:transactionTypeID",
            "@type": [
                "iudx:TextProperty"
            ],
            "rdfs:comment": "ID for the transactionType corresponding to this observation. 2401 - QR sale, C201- smart card entry , C202 - smart card exit etc.",
            "rdfs:label": "transactionTypeID",
            "rdfs:isDefinedBy": {
                "@id": "iudx:"
            },
            "iudx:domainIncludes": [
                {
                    "@id": "iudx:FareCollectionSystem"
                }
            ],
            "iudx:rangeIncludes": [
                {
                    "@id": "iudx:Text"
                },
                {
                    "@id": "iudx:ValueDescriptor"
                }
            ]
        },
        {
            "@id": "iudx:transactionVehicleNum",
            "@type": [
                "iudx:QuantitativeProperty"
            ],
            "rdfs:comment": "Code used by fare collection agency for the vehicle number corresponding to the transaction.",
            "rdfs:label": "transactionVehicleNum",
            "rdfs:isDefinedBy": {
                "@id": "iudx:"
            },
            "iudx:domainIncludes": [
                {
                    "@id": "iudx:FareCollectionSystem"
                }
            ],
            "iudx:rangeIncludes": [
                {
                    "@id": "iudx:Number"
                },
                {
                    "@id": "iudx:ValueDescriptor"
                }
            ]
        },
        {
            "@id": "iudx:travelDistance",
            "@type": [
                "iudx:QuantitativeProperty"
            ],
            "rdfs:comment": "The distance between the origin location and the destination location or the total distance travelled corresponding to this observation.",
            "rdfs:label": "travelDistance",
            "rdfs:isDefinedBy": {
                "@id": "iudx:"
            },
            "iudx:domainIncludes": [
                {
                    "@id": "iudx:TransitManagement"
                },
                {
                    "@id": "iudx:FareCollectionSystem"
                },
                {
                    "@id": "iudx:WmgmtVehicle"
                },
                {
                    "@id": "iudx:EmergencyVehicle"
                },
                {
                    "@id": "iudx:BikeDockingStation"
                }
            ],
            "iudx:rangeIncludes": [
                {
                    "@id": "iudx:Number"
                },
                {
                    "@id": "iudx:ValueDescriptor"
                }
            ]
        },
        {
            "@id": "iudx:travelTime",
            "@type": [
                "iudx:TimeProperty"
            ],
            "rdfs:comment": "The time taken to travel between the origin location and the destination location corresponding to this observation in HH:MM:SS format(HH:MM:SS is also accepted, if the hour begins with 0).",
            "rdfs:label": "travelTime",
            "rdfs:isDefinedBy": {
                "@id": "iudx:"
            },
            "iudx:domainIncludes": [
                {
                    "@id": "iudx:TransitManagement"
                }
            ],
            "iudx:rangeIncludes": [
                {
                    "@id": "iudx:Text"
                },
                {
                    "@id": "iudx:ValueDescriptor"
                }
            ]
        },
        {
            "@id": "iudx:treatmentPlantCapacity",
            "@type": [
                "iudx:QuantitativeProperty"
            ],
            "rdfs:comment": "Handling capacity of the waste-water treatment plant corresponding to this observation.",
            "rdfs:label": "treatmentPlantCapacity",
            "rdfs:isDefinedBy": {
                "@id": "iudx:"
            },
            "iudx:domainIncludes": [
                {
                    "@id": "iudx:WasteWaterMgmt"
                }
            ],
            "iudx:rangeIncludes": [
                {
                    "@id": "iudx:Number"
                },
                {
                    "@id": "iudx:ValueDescriptor"
                }
            ]
        },
        {
            "@id": "iudx:treatmentPlantID",
            "@type": [
                "iudx:QuantitativeProperty"
            ],
            "rdfs:comment": "Unique identification number for the waste-water treatment plant corresponding to this observation.",
            "rdfs:label": "treatmentPlantID",
            "rdfs:isDefinedBy": {
                "@id": "iudx:"
            },
            "iudx:domainIncludes": [
                {
                    "@id": "iudx:WasteWaterMgmt"
                }
            ],
            "iudx:rangeIncludes": [
                {
                    "@id": "iudx:Number"
                },
                {
                    "@id": "iudx:ValueDescriptor"
                }
            ]
        },
        {
            "@id": "iudx:treatmentPlantName",
            "@type": [
                "iudx:TextProperty"
            ],
            "rdfs:comment": "Name of the waste-water treatment plant corresponding to this observation.",
            "rdfs:label": "treatmentPlantName",
            "rdfs:isDefinedBy": {
                "@id": "iudx:"
            },
            "iudx:domainIncludes": [
                {
                    "@id": "iudx:WasteWaterMgmt"
                }
            ],
            "iudx:rangeIncludes": [
                {
                    "@id": "iudx:Text"
                },
                {
                    "@id": "iudx:ValueDescriptor"
                }
            ]
        },
        {
            "@id": "iudx:tripNetWeightCollected",
            "@type": [
                "iudx:QuantitativeProperty"
            ],
            "rdfs:comment": "The net weight of garbage collected by the SWM vehicle corresponding to this observation at the end of the trip.",
            "rdfs:label": "tripNetWeightCollected",
            "rdfs:isDefinedBy": {
                "@id": "iudx:"
            },
            "iudx:domainIncludes": [
                {
                    "@id": "iudx:WmgmtVehicle"
                }
            ],
            "iudx:rangeIncludes": [
                {
                    "@id": "iudx:Number"
                },
                {
                    "@id": "iudx:ValueDescriptor"
                }
            ]
        },
        {
            "@id": "iudx:tripStatus",
            "@type": [
                "iudx:TextProperty"
            ],
            "rdfs:comment": "Current status of the ride corresponding to this observation. ENUM: [ACCEPTED, ONGOING, COMPLETED, CANCELLED, TERMINATED]",
            "rdfs:label": "tripStatus",
            "rdfs:isDefinedBy": {
                "@id": "iudx:"
            },
            "iudx:domainIncludes": [
                {
                    "@id": "iudx:BikeDockingStation"
                },
                {
                    "@id": "iudx:WmgmtVehicle"
                }
            ],
            "iudx:rangeIncludes": [
                {
                    "@id": "iudx:Text"
                },
                {
                    "@id": "iudx:ValueDescriptor"
                }
            ]
        },
        {
            "@id": "iudx:trip_delay",
            "@type": [
                "iudx:QuantitativeProperty"
            ],
            "rdfs:comment": "This can be positive and negative in seconds and shows how much the vehicle deviates from the planned one. SameAs: 'delay' field from GTFS Realtime message-StopTimeEvent (https://developers.google.com/transit/gtfs-realtime/reference#message-stoptimeevent)",
            "rdfs:label": "trip_delay",
            "rdfs:isDefinedBy": {
                "@id": "iudx:"
            },
            "iudx:domainIncludes": [
                {
                    "@id": "iudx:TransitManagement"
                }
            ],
            "iudx:rangeIncludes": [
                {
                    "@id": "iudx:Number"
                },
                {
                    "@id": "iudx:ValueDescriptor"
                }
            ],
            "skos:exactMatch": {
                "@id": "GTFS: delay"
            }
        },
        {
            "@id": "iudx:trip_direction",
            "@type": [
                "iudx:TextProperty"
            ],
            "rdfs:comment": "Indicates the direction of travel of the vehicle corresponding to this observation, can be referenced from the GTFS static feed trips.txt. SameAs: 'direction_id' field from GTFS Realtime message-TripDescriptor (https://developers.google.com/transit/gtfs-realtime/reference#message-tripdescriptor)",
            "rdfs:label": "trip_direction",
            "rdfs:isDefinedBy": {
                "@id": "iudx:"
            },
            "iudx:domainIncludes": [
                {
                    "@id": "iudx:TransitManagement"
                },
                {
                    "@id": "iudx:FareCollectionSystem"
                }
            ],
            "iudx:rangeIncludes": [
                {
                    "@id": "iudx:Text"
                },
                {
                    "@id": "iudx:ValueDescriptor"
                }
            ],
            "skos:exactMatch": {
                "@id": "GTFS: direction_id"
            }
        },
        {
            "@id": "iudx:trip_id",
            "@type": [
                "iudx:TextProperty"
            ],
            "rdfs:comment": "Trip ID/Trip name allotted to the bus corresponding to this observation, in consideration to the time of the day and the direction of the trip on the given routeId.",
            "rdfs:label": "trip_id",
            "rdfs:isDefinedBy": {
                "@id": "iudx:"
            },
            "iudx:domainIncludes": [
                {
                    "@id": "iudx:GtfsCommons"
                },
                {
                    "@id": "iudx:TripDescriptor"
                },
                {
                    "@id": "iudx:FareCollectionSystem"
                },
                {
                    "@id": "iudx:StopTimesDesc"
                },
                {
                    "@id": "iudx:WmgmtVehicle"
                }
            ],
            "iudx:rangeIncludes": [
                {
                    "@id": "iudx:Text"
                },
                {
                    "@id": "iudx:ValueDescriptor"
                }
            ],
            "skos:exactMatch": {
                "@id": "GTFS: trip_id"
            }
        },
        {
            "@id": "iudx:tss",
            "@type": [
                "iudx:QuantitativeProperty"
            ],
            "rdfs:comment": "Total suspended solids concentration measured in a waste-water treatment plant corresponding to this observation.",
            "rdfs:label": "tss",
            "rdfs:isDefinedBy": {
                "@id": "iudx:"
            },
            "iudx:domainIncludes": [
                {
                    "@id": "iudx:WasteWaterMgmt"
                }
            ],
            "iudx:rangeIncludes": [
                {
                    "@id": "iudx:Number"
                },
                {
                    "@id": "iudx:ValueDescriptor"
                }
            ],
            "skos:exactMatch": {
                "@id": "fiware:tss"
            }
        },
        {
            "@id": "iudx:turbidity",
            "@type": [
                "iudx:QuantitativeProperty"
            ],
            "rdfs:comment": "Measurement of the amount of light that is scattered by material in the water when a light is shined through the water.",
            "rdfs:label": "turbidity",
            "rdfs:isDefinedBy": {
                "@id": "iudx:"
            },
            "iudx:domainIncludes": [
                {
                    "@id": "iudx:WaterDistributionNetwork"
                }
            ],
            "iudx:rangeIncludes": [
                {
                    "@id": "iudx:TimeSeriesAggregation"
                },
                {
                    "@id": "iudx:ValueDescriptor"
                }
            ],
            "skos:exactMatch": {
                "@id": "Fiware: WaterQualityObserved.turbidity"
            }
        },
        {
            "@id": "iudx:ulbName",
            "@type": [
                "iudx:TextProperty"
            ],
            "rdfs:comment": "Name of the Urban Local Body corresponding to this observation.",
            "rdfs:label": "ulbName",
            "rdfs:isDefinedBy": {
                "@id": "iudx:"
            },
            "iudx:domainIncludes": [
                {
                    "@id": "iudx:MunicipalityDesc"
                }
            ],
            "iudx:rangeIncludes": [
                {
                    "@id": "iudx:Text"
                },
                {
                    "@id": "iudx:ValueDescriptor"
                }
            ]
        },
        {
            "@id": "iudx:uncompensatedTDS",
            "@type": [
                "iudx:QuantitativeProperty"
            ],
            "rdfs:comment": "The value of TDS (Total Dissolved Solids) level in the water without temperature compensation.",
            "rdfs:label": "uncompensatedTDS",
            "rdfs:isDefinedBy": {
                "@id": "iudx:"
            },
            "iudx:domainIncludes": [
                {
                    "@id": "iudx:WasteWaterMgmt"
                },
                {
                    "@id": "iudx:WaterDistributionNetwork"
                }
            ],
            "iudx:rangeIncludes": [
                {
                    "@id": "iudx:Number"
                },
                {
                    "@id": "iudx:ValueDescriptor"
                }
            ]
        },
        {
            "@id": "iudx:unitCode",
            "@type": [
                "iudx:TextProperty"
            ],
            "rdfs:comment": "The unit of measurement given using the UN/CEFACT Common Code (3 characters) or a URL. Other codes/unit vocabularies may be used with a prefix",
            "rdfs:label": "unitCode",
            "iudx:domainIncludes": [
                {
                    "@id": "iudx:ValueDescriptor"
                }
            ],
            "iudx:rangeIncludes": [
                {
                    "@id": "iudx:Text"
                },
                {
                    "@id": "iudx:Text",
                    "@type": "@id"
                }
            ],
            "skos:exactMatch": {
                "@id": "schema:unitCode"
            },
            "rdfs:isDefinedBy": {
                "@id": "iudx:"
            }
        },
        {
            "@id": "iudx:unitText",
            "@type": [
                "iudx:TextProperty"
            ],
            "rdfs:comment": "Describes the unit of measurement. Useful if unitCode is not available.",
            "rdfs:label": "unitText",
            "iudx:domainIncludes": [
                {
                    "@id": "iudx:ValueDescriptor"
                }
            ],
            "iudx:rangeIncludes": [
                {
                    "@id": "iudx:Text"
                }
            ],
            "skos:exactMatch": {
                "@id": "schema:unitText"
            },
            "rdfs:isDefinedBy": {
                "@id": "iudx:"
            }
        },
        {
            "@id": "iudx:userScore",
            "@type": [
                "iudx:QuantitativeProperty"
            ],
            "rdfs:comment": "The feedback rating given by the user based on his personal experience with the products or things or services.",
            "rdfs:label": "userScore",
            "rdfs:isDefinedBy": {
                "@id": "iudx:"
            },
            "iudx:domainIncludes": [
                {
                    "@id": "iudx:BikeDockingStation"
                }
            ],
            "iudx:rangeIncludes": [
                {
                    "@id": "iudx:Number"
                },
                {
                    "@id": "iudx:ValueDescriptor"
                }
            ]
        },
        {
            "@id": "iudx:value",
            "@type": [
                "iudx:QuantitativeProperty"
            ],
            "rdfs:comment": "Value of the quantity being described in the ValueDescriptor object.",
            "rdfs:label": "value",
            "iudx:domainIncludes": [
                {
                    "@id": "iudx:ValueDescriptor"
                }
            ],
            "iudx:rangeIncludes": [
                {
                    "@id": "iudx:Number"
                },
                {
                    "@id": "iudx:Text"
                },
                {
                    "@id": "iudx:Boolean"
                },
                {
                    "@id": "iudx:NumericArray"
                },
                {
                    "@id": "iudx:StructuredValue"
                }
            ],
            "rdfs:isDefinedBy": {
                "@id": "iudx:"
            }
        },
        {
            "@id": "iudx:vehicleAltitude",
            "@type": [
                "iudx:QuantitativeProperty"
            ],
            "rdfs:comment": "Gives the current altitude of the vehicle using GPS",
            "rdfs:label": "vehicleAltitude",
            "rdfs:isDefinedBy": {
                "@id": "iudx:"
            },
            "iudx:domainIncludes": [
                {
                    "@id": "iudx:WmgmtVehicle"
                },
                {
                    "@id": "iudx:EmergencyVehicle"
                }
            ],
            "iudx:rangeIncludes": [
                {
                    "@id": "iudx:Number"
                },
                {
                    "@id": "iudx:ValueDescriptor"
                }
            ]
        },
        {
            "@id": "iudx:vehicleCapacity",
            "@type": [
                "iudx:QuantitativeProperty"
            ],
            "rdfs:comment": "Describes the total capacity (including the seating and standing capacity) of the vehicle corresponding to this observation.",
            "rdfs:label": "vehicleCapacity",
            "rdfs:isDefinedBy": {
                "@id": "iudx:"
            },
            "iudx:domainIncludes": [
                {
                    "@id": "iudx:TransitManagement"
                }
            ],
            "iudx:rangeIncludes": [
                {
                    "@id": "iudx:Number"
                },
                {
                    "@id": "iudx:ValueDescriptor"
                }
            ]
        },
        {
            "@id": "iudx:vehicleCount",
            "@type": [
                "iudx:QuantitativeProperty"
            ],
            "rdfs:comment": "The total count of vehicles corresponding to this observation.",
            "rdfs:label": "vehicleCount",
            "rdfs:isDefinedBy": {
                "@id": "iudx:"
            },
            "iudx:domainIncludes": [
                {
                    "@id": "iudx:RoadSegment"
                }
            ],
            "iudx:rangeIncludes": [
                {
                    "@id": "iudx:Number"
                },
                {
                    "@id": "iudx:ValueDescriptor"
                }
            ]
        },
        {
            "@id": "iudx:vehicleID",
            "@type": [
                "iudx:TextProperty"
            ],
            "rdfs:comment": "Unique ID(s) assigned to the vehicle(s) corresponding to this observation, used in internal system identification. SameAs: 'id' field from GTFS Realtime message-VehicleDescriptor (https://developers.google.com/transit/gtfs-realtime/reference#message-vehicledescriptor)",
            "rdfs:label": "vehicleID",
            "rdfs:isDefinedBy": {
                "@id": "iudx:"
            },
            "iudx:domainIncludes": [
                {
                    "@id": "iudx:VehicleDescriptor"
                },
                {
                    "@id": "iudx:BikeDockingStation"
                }
            ],
            "iudx:rangeIncludes": [
                {
                    "@container": "@list",
                    "@id": "iudx:Text"
                },
                {
                    "@id": "iudx:ValueDescriptor"
                }
            ],
            "skos:exactMatch": {
                "@id": "GTFS: id"
            }
        },
        {
            "@id": "iudx:vehicleRunningStatus",
            "@type": [
                "iudx:TextProperty"
            ],
            "rdfs:comment": "Moving status of the vehicle. For eg., running, idle, etc.",
            "rdfs:label": "vehicleRunningStatus",
            "rdfs:isDefinedBy": {
                "@id": "iudx:"
            },
            "iudx:domainIncludes": [
                {
                    "@id": "iudx:WmgmtVehicle"
                },
                {
                    "@id": "iudx:EmergencyVehicle"
                }
            ],
            "iudx:rangeIncludes": [
                {
                    "@id": "iudx:Text"
                },
                {
                    "@id": "iudx:ValueDescriptor"
                }
            ]
        },
        {
            "@id": "iudx:vehicleSupportType",
            "@type": [
                "iudx:TextProperty"
            ],
            "rdfs:comment": "Support capability being provided by the vehicle corresponding to this observation. ENUM[ALS,BLS]. \nALS refers to Advance Life Support and BLS refers to Basic life support",
            "rdfs:label": "vehicleSupportType",
            "rdfs:isDefinedBy": {
                "@id": "iudx:"
            },
            "iudx:domainIncludes": [
                {
                    "@id": "iudx:EmergencyVehicle"
                }
            ],
            "iudx:rangeIncludes": [
                {
                    "@id": "iudx:Text"
                },
                {
                    "@id": "iudx:ValueDescriptor"
                }
            ]
        },
        {
            "@id": "iudx:vehicleTrackerDevice",
            "@type": [
                "iudx:TextProperty"
            ],
            "rdfs:comment": "Installation status of the GPS device or the tracking device fitted to the vehicle corresponding to this observation.",
            "rdfs:label": "vehicleTrackerDevice",
            "rdfs:isDefinedBy": {
                "@id": "iudx:"
            },
            "iudx:domainIncludes": [
                {
                    "@id": "iudx:WmgmtVehicle"
                },
                {
                    "@id": "iudx:EmergencyVehicle"
                }
            ],
            "iudx:rangeIncludes": [
                {
                    "@id": "iudx:Text"
                },
                {
                    "@id": "iudx:ValueDescriptor"
                }
            ]
        },
        {
            "@id": "iudx:vehicleType",
            "@type": [
                "iudx:TextProperty"
            ],
            "rdfs:comment": "Describes the type of vehicle corresponding to this observation, could be hopper, compactor, tipper, dumper in case of solid waste management vehicles, BRT mini bus, BRT bus, city bus in case of ITMS vehicles, Ambulance, Fire tender, Police van etc, in case of emergency vehicles and Moped/Scooter, Motor Cycle,  Autorickshaw, Private car/ Jeep car, Tempo, Bus, E-Moped/E-Scooter/E-Motor Cycle, Public motor in case of vehicle registration.",
            "rdfs:label": "vehicleType",
            "iudx:domainIncludes": [
                {
                    "@id": "iudx:WmgmtVehicle"
                },
                {
                    "@id": "iudx:TransitManagement"
                },
                {
                    "@id": "iudx:RevenueCollection"
                },
                {
                    "@id": "iudx:EmergencyVehicle"
                },
                {
                    "@id": "iudx:EVChargingStation"
                }
            ],
            "iudx:rangeIncludes": [
                {
                    "@id": "iudx:Text"
                },
                {
                    "@id": "iudx:ValueDescriptor"
                }
            ],
            "rdfs:isDefinedBy": {
                "@id": "iudx:"
            }
        },
        {
            "@id": "iudx:vehicleTypeCode",
            "@type": [
                "iudx:TextProperty"
            ],
            "rdfs:comment": "The code for vehicleType corresponding to this observation. For eg.- '1' - MOPED/SCOOTER, '2' - MOTOR CYCLE, '4' - PRIVATE MOTOR CAR/JEEP CAR, '21' - TEMPO, '26' - BUS, etc.",
            "rdfs:label": "vehicleTypeCode",
            "rdfs:isDefinedBy": {
                "@id": "iudx:"
            },
            "iudx:domainIncludes": [
                {
                    "@id": "iudx:RevenueCollection"
                }
            ],
            "iudx:rangeIncludes": [
                {
                    "@id": "iudx:Text"
                },
                {
                    "@id": "iudx:ValueDescriptor"
                }
            ]
        },
        {
            "@id": "iudx:vehicleTypeCount",
            "@type": [
                "iudx:StructuredProperty"
            ],
            "rdfs:comment": "Provides the count of vehicles for each vehicle type corresponding to this observation.",
            "rdfs:label": "vehicleTypeCount",
            "rdfs:isDefinedBy": {
                "@id": "iudx:"
            },
            "iudx:domainIncludes": [
                {
                    "@id": "iudx:RoadSegment"
                }
            ],
            "iudx:rangeIncludes": [
                {
                    "@id": "iudx:Object"
                },
                {
                    "@id": "iudx:ValueDescriptor"
                }
            ]
        },
        {
            "@id": "iudx:vehicle_label",
            "@type": [
                "iudx:TextProperty"
            ],
            "rdfs:comment": "User visible label, i.e., something that must be shown to the passenger to help identify the correct vehicle. SameAs: 'label' field from GTFS Realtime message-VehicleDescriptor (https://developers.google.com/transit/gtfs-realtime/reference#message-vehicledescriptor)",
            "rdfs:label": "vehicle_label",
            "rdfs:isDefinedBy": {
                "@id": "iudx:"
            },
            "iudx:domainIncludes": [
                {
                    "@id": "iudx:VehicleDescriptor"
                },
                {
                    "@id": "iudx:FareCollectionSystem"
                }
            ],
            "iudx:rangeIncludes": [
                {
                    "@id": "iudx:Text"
                },
                {
                    "@id": "iudx:ValueDescriptor"
                }
            ],
            "skos:exactMatch": {
                "@id": "GTFS: label"
            }
        },
        {
            "@id": "iudx:versionName",
            "@type": [
                "iudx:TextProperty"
            ],
            "rdfs:comment": "Version name corresponding to this observation",
            "rdfs:label": "versionName",
            "rdfs:isDefinedBy": {
                "@id": "iudx:"
            },
            "iudx:domainIncludes": [
                {
                    "@id": "iudx:Version"
                }
            ],
            "iudx:rangeIncludes": [
                {
                    "@id": "iudx:Text"
                },
                {
                    "@id": "iudx:ValueDescriptor"
                }
            ]
        },
        {
            "@id": "iudx:versionSpec",
            "@type": [
                "iudx:StructuredProperty"
            ],
            "rdfs:comment": "Version specifications or information corresponding to the version in this observation.",
            "rdfs:label": "versionSpec",
            "iudx:domainIncludes": [
                {
                    "@id": "iudx:Version"
                }
            ],
            "iudx:rangeIncludes": [
                {
                    "@id": "iudx:Text"
                },
                {
                    "@id": "iudx:Object"
                },
                {
                    "@id": "iudx:ValueDescriptor"
                }
            ]
        },
        {
            "@id": "iudx:visitDuration",
            "@type": [
                "iudx:TextProperty"
            ],
            "rdfs:comment": "The approximate amount of time required to explore the tourist site corresponding to this observation.",
            "rdfs:label": "visitDuration",
            "rdfs:isDefinedBy": {
                "@id": "iudx:"
            },
            "iudx:domainIncludes": [
                {
                    "@id": "iudx:TouristDestination"
                }
            ],
            "iudx:rangeIncludes": [
                {
                    "@id": "iudx:Text"
                },
                {
                    "@id": "iudx:ValueDescriptor"
                }
            ]
        },
        {
            "@id": "iudx:visitorCount",
            "@type": [
                "iudx:QuantitativeProperty"
            ],
            "rdfs:comment": "The total number of visitors corresponding to this observation.",
            "rdfs:label": "visitorCount",
            "rdfs:isDefinedBy": {
                "@id": "iudx:"
            },
            "iudx:domainIncludes": [
                {
                    "@id": "iudx:TouristDestination"
                }
            ],
            "iudx:rangeIncludes": [
                {
                    "@id": "iudx:Number"
                },
                {
                    "@id": "iudx:ValueDescriptor"
                }
            ]
        },
        {
            "@id": "iudx:vocRaw",
            "@type": [
                "iudx:QuantitativeProperty"
            ],
            "rdfs:comment": "Observed value of the natural form of volatile organic compounds in the environment corresponding to this observation.",
            "rdfs:label": "vocRaw",
            "iudx:domainIncludes": [
                {
                    "@id": "iudx:EnvAQM"
                },
                {
                    "@id": "iudx:AirQuality"
                }
            ],
            "iudx:rangeIncludes": [
                {
                    "@id": "iudx:Number"
                },
                {
                    "@id": "iudx:ValueDescriptor"
                }
            ],
            "rdfs:isDefinedBy": {
                "@id": "iudx:"
            },
            "skos:exactMatch": {
                "@id": "Fiware:volatileOrganicCompoundsTotal"
            }
        },
        {
            "@id": "iudx:vocTotal",
            "@type": [
                "iudx:QuantitativeProperty"
            ],
            "rdfs:comment": "Observed value of volatile organic compounds present in the environment corresponding to this observation. It could be industrial solvents, chemical by-products etc.",
            "rdfs:label": "vocTotal",
            "iudx:domainIncludes": [
                {
                    "@id": "iudx:EnvAQM"
                },
                {
                    "@id": "iudx:AirQuality"
                }
            ],
            "iudx:rangeIncludes": [
                {
                    "@id": "iudx:Number"
                },
                {
                    "@id": "iudx:ValueDescriptor"
                }
            ],
            "rdfs:isDefinedBy": {
                "@id": "iudx:"
            }
        },
        {
            "@id": "iudx:voltage",
            "@type": [
                "iudx:QuantitativeProperty"
            ],
            "rdfs:comment": "The value of Voltage in the entity corresponding to this observation.",
            "rdfs:label": "voltage",
            "rdfs:isDefinedBy": {
                "@id": "iudx:"
            },
            "iudx:domainIncludes": [
                {
                    "@id": "iudx:Streetlight"
                },
                {
                    "@id": "iudx:SolarEnergy"
                },
                {
                    "@id": "iudx:EnergyMeter"
                }
            ],
            "iudx:rangeIncludes": [
                {
                    "@id": "iudx:Number"
                },
                {
                    "@id": "iudx:ValueDescriptor"
                }
            ]
        },
        {
            "@id": "iudx:wardID",
            "@type": [
                "iudx:TextProperty"
            ],
            "rdfs:comment": "Ward ID corresponding to this observation.",
            "rdfs:label": "wardID",
            "rdfs:isDefinedBy": {
                "@id": "iudx:"
            },
            "iudx:domainIncludes": [
                {
                    "@id": "iudx:MunicipalityDesc"
                }
            ],
            "iudx:rangeIncludes": [
                {
                    "@id": "iudx:Text"
                },
                {
                    "@id": "iudx:ValueDescriptor"
                }
            ]
        },
        {
            "@id": "iudx:wardName",
            "@type": [
                "iudx:TextProperty"
            ],
            "rdfs:comment": "Ward name corresponding to this observation.",
            "rdfs:label": "wardName",
            "rdfs:isDefinedBy": {
                "@id": "iudx:"
            },
            "iudx:domainIncludes": [
                {
                    "@id": "iudx:MunicipalityDesc"
                }
            ],
            "iudx:rangeIncludes": [
                {
                    "@id": "iudx:Text"
                },
                {
                    "@id": "iudx:ValueDescriptor"
                }
            ]
        },
        {
            "@id": "iudx:wardNum",
            "@type": [
                "iudx:QuantitativeProperty"
            ],
            "rdfs:comment": "Ward number corresponding to this observation.",
            "rdfs:label": "wardNum",
            "rdfs:isDefinedBy": {
                "@id": "iudx:"
            },
            "iudx:domainIncludes": [
                {
                    "@id": "iudx:MunicipalityDesc"
                }
            ],
            "iudx:rangeIncludes": [
                {
                    "@id": "iudx:Number"
                },
                {
                    "@id": "iudx:ValueDescriptor"
                }
            ]
        },
        {
            "@id": "iudx:wasteCollectionStatus",
            "@type": [
                "iudx:TextProperty"
            ],
            "rdfs:comment": "The status of the waste collection corresponding to this observation",
            "rdfs:label": "wasteCollectionStatus",
            "rdfs:isDefinedBy": {
                "@id": "iudx:"
            },
            "iudx:domainIncludes": [
                {
                    "@id": "iudx:WmgmtVehicle"
                }
            ],
            "iudx:rangeIncludes": [
                {
                    "@id": "iudx:Text"
                },
                {
                    "@id": "iudx:ValueDescriptor"
                }
            ]
        },
        {
            "@id": "iudx:wasteType",
            "@type": [
                "iudx:TextProperty"
            ],
            "rdfs:comment": "The type of waste corresponding this observation.",
            "rdfs:label": "wasteType",
            "rdfs:isDefinedBy": {
                "@id": "iudx:"
            },
            "iudx:domainIncludes": [
                {
                    "@id": "iudx:WmgmtVehicle"
                }
            ],
            "iudx:rangeIncludes": [
                {
                    "@id": "iudx:Text"
                },
                {
                    "@id": "iudx:ValueDescriptor"
                }
            ]
        },
        {
            "@id": "iudx:waterFlow",
            "@type": [
                "iudx:QuantitativeProperty"
            ],
            "rdfs:comment": "Flow or current of water flowing from the water storage tank corresponding to this observation.",
            "rdfs:label": "waterFlow",
            "rdfs:isDefinedBy": {
                "@id": "iudx:"
            },
            "iudx:domainIncludes": [
                {
                    "@id": "iudx:WaterDistributionNetwork"
                }
            ],
            "iudx:rangeIncludes": [
                {
                    "@id": "iudx:Number"
                },
                {
                    "@id": "iudx:ValueDescriptor"
                }
            ]
        },
        {
            "@id": "iudx:waterLevel",
            "@type": [
                "iudx:QuantitativeProperty"
            ],
            "rdfs:comment": "Current water level in the water storage tank corresponding to this observation.",
            "rdfs:label": "waterLevel",
            "rdfs:isDefinedBy": {
                "@id": "iudx:"
            },
            "iudx:domainIncludes": [
                {
                    "@id": "iudx:WaterDistributionNetwork"
                }
            ],
            "iudx:rangeIncludes": [
                {
                    "@id": "iudx:Number"
                },
                {
                    "@id": "iudx:ValueDescriptor"
                }
            ]
        },
        {
            "@id": "iudx:waterPressure",
            "@type": [
                "iudx:QuantitativeProperty"
            ],
            "rdfs:comment": "Pressure of water flowing from the water storage tank corresponding to this observation.",
            "rdfs:label": "waterPressure",
            "rdfs:isDefinedBy": {
                "@id": "iudx:"
            },
            "iudx:domainIncludes": [
                {
                    "@id": "iudx:WaterDistributionNetwork"
                }
            ],
            "iudx:rangeIncludes": [
                {
                    "@id": "iudx:Number"
                },
                {
                    "@id": "iudx:ValueDescriptor"
                }
            ]
        },
        {
            "@id": "iudx:waterTemperature",
            "@type": [
                "iudx:QuantitativeProperty"
            ],
            "rdfs:comment": "Water temperature in the water storage tank corresponding to this observation.",
            "rdfs:label": "waterTemperature",
            "rdfs:isDefinedBy": {
                "@id": "iudx:"
            },
            "iudx:domainIncludes": [
                {
                    "@id": "iudx:WaterDistributionNetwork"
                }
            ],
            "iudx:rangeIncludes": [
                {
                    "@id": "iudx:Number"
                },
                {
                    "@id": "iudx:ValueDescriptor"
                }
            ]
        },
        {
            "@id": "iudx:weatherType",
            "@type": [
                "iudx:TextProperty"
            ],
            "rdfs:comment": "Observed weather type or status. Represented by a comma separated list of weather types, e.g., cloudy, sunny etc.",
            "rdfs:label": "weatherType",
            "iudx:domainIncludes": [
                {
                    "@id": "iudx:EnvWeather"
                },
                {
                    "@id": "iudx:EnvAQM"
                },
                {
                    "@id": "iudx:AirQuality"
                }
            ],
            "iudx:rangeIncludes": [
                {
                    "@id": "iudx:Text"
                },
                {
                    "@id": "iudx:ValueDescriptor"
                }
            ],
            "rdfs:isDefinedBy": {
                "@id": "iudx:"
            },
            "skos:exactMatch": {
                "@id": "Fiware:weatherType"
            }
        },
        {
            "@id": "iudx:windDirection",
            "@type": [
                "iudx:QuantitativeProperty"
            ],
            "rdfs:comment": "Observed wind directiont. Measured in degrees clockwise from due north.",
            "rdfs:label": "windDirection",
            "rdfs:isDefinedBy": {
                "@id": "iudx:"
            },
            "iudx:domainIncludes": [
                {
                    "@id": "iudx:EnvWeather"
                }
            ],
            "iudx:rangeIncludes": [
                {
                    "@id": "iudx:Number"
                },
                {
                    "@id": "iudx:ValueDescriptor"
                }
            ],
            "skos:exactMatch": {
                "@id": "Fiware:windDirection"
            }
        },
        {
            "@id": "iudx:windSpeed",
            "@type": [
                "iudx:QuantitativeProperty"
            ],
            "rdfs:comment": "Observed wind speed.",
            "rdfs:label": "windSpeed",
            "rdfs:isDefinedBy": {
                "@id": "iudx:"
            },
            "iudx:domainIncludes": [
                {
                    "@id": "iudx:EnvWeather"
                }
            ],
            "iudx:rangeIncludes": [
                {
                    "@id": "iudx:Number"
                },
                {
                    "@id": "iudx:ValueDescriptor"
                }
            ],
            "skos:exactMatch": {
                "@id": "Fiware:windSpeed"
            }
        },
        {
            "@id": "iudx:xField",
            "@type": [
                "iudx:QuantitativeProperty"
            ],
            "rdfs:comment": "The longitude corresponding to this observation.",
            "rdfs:label": "xField",
            "rdfs:isDefinedBy": {
                "@id": "iudx:"
            },
            "iudx:domainIncludes": [
                {
                    "@id": "iudx:DigitalElevationModel"
                }
            ],
            "iudx:rangeIncludes": [
                {
                    "@id": "iudx:Number"
                },
                {
                    "@id": "iudx:ValueDescriptor"
                }
            ]
        },
        {
            "@id": "iudx:yField",
            "@type": [
                "iudx:QuantitativeProperty"
            ],
            "rdfs:comment": "The latitude corresponding to this observation.",
            "rdfs:label": "yField",
            "rdfs:isDefinedBy": {
                "@id": "iudx:"
            },
            "iudx:domainIncludes": [
                {
                    "@id": "iudx:DigitalElevationModel"
                }
            ],
            "iudx:rangeIncludes": [
                {
                    "@id": "iudx:Number"
                },
                {
                    "@id": "iudx:ValueDescriptor"
                }
            ]
        },
        {
            "@id": "iudx:year",
            "@type": [
                "iudx:QuantitativeProperty"
            ],
            "rdfs:comment": "Year corresponding to this observation and is described in YYYY format, for eg. 2020.",
            "rdfs:label": "year",
            "iudx:domainIncludes": [
                {
                    "@id": "iudx:RevenueCollection"
                },
                {
                    "@id": "iudx:PublicSchemes"
                }
            ],
            "iudx:rangeIncludes": [
                {
                    "@id": "iudx:Number"
                },
                {
                    "@id": "iudx:ValueDescriptor"
                }
            ],
            "rdfs:isDefinedBy": {
                "@id": "iudx:"
            }
        },
        {
            "@id": "iudx:zField",
            "@type": [
                "iudx:QuantitativeProperty"
            ],
            "rdfs:comment": "The elevation of the point from the mean sea level corresponding to this observation",
            "rdfs:label": "zField",
            "rdfs:isDefinedBy": {
                "@id": "iudx:"
            },
            "iudx:domainIncludes": [
                {
                    "@id": "iudx:DigitalElevationModel"
                }
            ],
            "iudx:rangeIncludes": [
                {
                    "@id": "iudx:Number"
                },
                {
                    "@id": "iudx:ValueDescriptor"
                }
            ]
        },
        {
            "@id": "iudx:zoneID",
            "@type": [
                "iudx:TextProperty"
            ],
            "rdfs:comment": "Zone ID corresponding to this observation.",
            "rdfs:label": "zoneID",
            "rdfs:isDefinedBy": {
                "@id": "iudx:"
            },
            "iudx:domainIncludes": [
                {
                    "@id": "iudx:MunicipalityDesc"
                },
                {
                    "@id": "iudx:RoadSegment"
                }
            ],
            "iudx:rangeIncludes": [
                {
                    "@id": "iudx:Text"
                },
                {
                    "@id": "iudx:ValueDescriptor"
                }
            ]
        },
        {
            "@id": "iudx:zoneName",
            "@type": [
                "iudx:TextProperty"
            ],
            "rdfs:comment": "Zone name corresponding to this observation.",
            "rdfs:label": "zoneName",
            "rdfs:isDefinedBy": {
                "@id": "iudx:"
            },
            "iudx:domainIncludes": [
                {
                    "@id": "iudx:MunicipalityDesc"
                }
            ],
            "iudx:rangeIncludes": [
                {
                    "@id": "iudx:Text"
                },
                {
                    "@id": "iudx:ValueDescriptor"
                }
            ]
        }
    ],
    "@context": {
        "rdfs": "http://www.w3.org/2000/01/rdf-schema#",
        "iudx": "https://voc.iudx.org.in/",
        "owl": "http://www.w3.org/2002/07/owl#",
        "rdf": "http://www.w3.org/1999/02/22-rdf-syntax-ns#",
        "skos": "http://www.w3.org/2004/02/skos/core#",
        "xsd": "http://www.w3.org/2001/XMLSchema#",
        "schema": "http://schema.org/",
        "geojson": "https://purl.org/geojson/vocab#",
        "qudt": "http://qudt.org/vocab/unit/"
    }
}